# baseURI: https://data.naa.gov.au/def/agift
# prefix: agift

@prefix agift: <https://data.naa.gov.au/def/agift/> .
@prefix dcterms: <http://purl.org/dc/terms/> .
@prefix owl: <http://www.w3.org/2002/07/owl#> .
@prefix sdo: <https://schema.org/> .
@prefix skos: <http://www.w3.org/2004/02/skos/core#> .
@prefix vann: <http://purl.org/vocab/vann/> .
@prefix xsd: <http://www.w3.org/2001/XMLSchema#> .

agift:AGIFT
  a skos:ConceptScheme , owl:Ontology ;
  dcterms:contributor "KOdea" , "Nicholas J Car";
  dcterms:created "2016-07-06T02:43:29+00:00"^^xsd:dateTime ;
  dcterms:creator <https://linked.data.gov.au/org/naa> ;
  dcterms:modified "2021-01-18"^^xsd:date ;
  dcterms:provenance "Minor URI & label tidy-ups made by Nicholas J. Car in 2019, further tweaks of property types etc. for SOP in Jan 2021" ;
  dcterms:publisher <https://linked.data.gov.au/org/naa> ;
  dcterms:subject "The Australian Governments' Interactive Functions Thesaurus (AGIFT) is a three-level hierarchical thesaurus that describes the business functions carried out across Commonwealth, state and local governments in Australia."@en ;
  skos:prefLabel "Australian Governments' Interactive Functions Thesaurus"@en ;
  skos:altLabel "AGIFT"@en ;
  skos:hasTopConcept 
    agift:BUSINESS-SUPPORT-AND-REGULATION ,
    agift:CIVIC-INFRASTRUCTURE ,
    agift:COMMUNICATIONS ,
    agift:COMMUNITY-SERVICES ,
    agift:CULTURAL-AFFAIRS ,
    agift:DEFENCE ,
    agift:EDUCATION-AND-TRAINING ,
    agift:EMPLOYMENT ,
    agift:ENVIRONMENT ,
    agift:FINANCE-MANAGEMENT ,
    agift:GOVERNANCE ,
    agift:HEALTH-CARE ,
    agift:IMMIGRATION ,
    agift:INDIGENOUS-AFFAIRS ,
    agift:INTERNATIONAL-RELATIONS ,
    agift:JUSTICE-ADMINISTRATION ,
    agift:MARITIME-SERVICES ,
    agift:NATURAL-RESOURCES ,
    agift:PRIMARY-INDUSTRIES ,
    agift:SCIENCE ,
    agift:SECURITY ,
    agift:SPORT-AND-RECREATION ,
    agift:STATISTICAL-SERVICES ,
    agift:TOURISM ,
    agift:TRADE ,
    agift:TRANSPORT ;
    vann:preferredNamespacePrefix "agift"@en ;
    vann:preferredNamespaceUri "https://data.naa.gov.au/def/agift/" ;
.
<https://linked.data.gov.au/org/naa>
  a sdo:Organization ;
  sdo:name "National Archives of Australia" ;
  sdo:url <https://www.naa.gov.au> ;
.
agift:Accommodation-services
  a skos:Concept ;
  dcterms:contributor "KOdea" ;
  dcterms:created "2016-07-06T02:55:24+00:00"^^xsd:dateTime ;
  dcterms:creator "superadmin" ;
  dcterms:modified "2016-09-09T06:27:48+00:00"^^xsd:dateTime ;
  skos:altLabel "Homelessness support"@en ;
  skos:altLabel "Housing services"@en ;
  skos:altLabel "Indigenous housing"@en ;
  skos:altLabel "Public housing services"@en ;
  skos:broader agift:COMMUNITY-SERVICES ;
  skos:definition "Developing policy to support the provision of housing to those in need. Establishing eligibility criteria for services. Developing strategies to assist specific community groups at risk of homelessness. Includes liaison with areas responsible for public housing construction, to determine short-term and long-term community housing needs."@en ;
  skos:narrower agift:Defence-housing ;
  skos:narrower agift:Emergency-accommodation ;
  skos:narrower agift:Public-housing-entitlements ;
  skos:narrower agift:Refuge-support ;
  skos:prefLabel "Accommodation services"@en ;
  skos:related agift:Migrant-accommodation-services ;
  skos:related agift:Public-housing ;
  skos:related agift:Residential-services ;
.
agift:Accreditation-criteria
  skos:prefLabel "Accreditation criteria"@en ;
  owl:deprecated true ;
.
agift:Administrative-decision-appeal
  a skos:Concept ;
  dcterms:contributor "KOdea" ;
  dcterms:created "2016-07-06T04:54:25+00:00"^^xsd:dateTime ;
  dcterms:creator "superadmin" ;
  dcterms:modified "2016-09-09T07:20:08+00:00"^^xsd:dateTime ;
  skos:altLabel "Administrative appeals"@en ;
  skos:altLabel "Appeals"@en ;
  skos:broader agift:Administrative-law ;
  skos:definition "Developing processes to support applications to an independent authority to have a determination or judgement reviewed. Includes activities associated with receiving and managing appeals"@en ;
  skos:prefLabel "Administrative decision appeal"@en ;
  skos:related agift:Administrative-decision-review ;
  skos:related agift:Dispute-mediation-programs ;
.
agift:Administrative-decision-review
  a skos:Concept ;
  dcterms:contributor "KOdea" ;
  dcterms:created "2016-07-06T04:54:33+00:00"^^xsd:dateTime ;
  dcterms:creator "superadmin" ;
  dcterms:modified "2016-09-09T07:12:12+00:00"^^xsd:dateTime ;
  skos:altLabel "Independent review"@en ;
  skos:altLabel "Ombudsman"@en ;
  skos:broader agift:Administrative-law ;
  skos:definition "Examining and reconsidering a determination or judgement made by a public authority. Responding to the advice of an independent body which may reverse or uphold an earlier decision."@en ;
  skos:prefLabel "Administrative decision review"@en ;
  skos:related agift:Administrative-decision-appeal ;
.
agift:Administrative-law
  a skos:Concept ;
  dcterms:contributor "KOdea" ;
  dcterms:created "2016-07-06T03:36:59+00:00"^^xsd:dateTime ;
  dcterms:creator "superadmin" ;
  dcterms:modified "2016-09-09T06:31:22+00:00"^^xsd:dateTime ;
  skos:altLabel "Executive government"@en ;
  skos:altLabel "Public authorities"@en ;
  skos:altLabel "Tribunals"@en ;
  skos:broader agift:JUSTICE-ADMINISTRATION ;
  skos:definition "Administering the body of law that relates to the executive functions of government. Establishing the relationship between the government and the citizens of its jurisdiction. Regulating the powers, duties and organisation of public administration authorities."@en ;
  skos:narrower agift:Administrative-decision-appeal ;
  skos:narrower agift:Administrative-decision-review ;
  skos:narrower agift:Censorship-standards ;
  skos:narrower agift:Copyright-regulation ;
  skos:narrower agift:Freedom-of-information ;
  skos:narrower agift:Recordkeeping-standards ;
  skos:prefLabel "Administrative law"@en ;
  skos:related agift:Deportation ;
  skos:related agift:Public-administration ;
.
agift:Adoption-services
  a skos:Concept ;
  dcterms:contributor "KOdea" ;
  dcterms:created "2016-07-06T04:02:10+00:00"^^xsd:dateTime ;
  dcterms:creator "superadmin" ;
  dcterms:modified "2016-09-06T07:15:27+00:00"^^xsd:dateTime ;
  skos:altLabel "Child adoption services"@en ;
  skos:altLabel "Overseas adoption services"@en ;
  skos:broader agift:Community-support ;
  skos:definition "Assisting parents seeking to legally take responsibility for a child, or birth parents wishing to have their child adopted. Includes advice on the legal aspects of adoption and monitoring the adoption of overseas children."@en ;
  skos:prefLabel "Adoption services"@en ;
  skos:related agift:Child-care-services ;
  skos:related agift:Family-reunion-programs ;
.
agift:Adult-education-programs
  a skos:Concept ;
  dcterms:contributor "KOdea" ;
  dcterms:created "2016-07-06T04:13:22+00:00"^^xsd:dateTime ;
  dcterms:creator "superadmin" ;
  dcterms:modified "2016-09-09T06:08:02+00:00"^^xsd:dateTime ;
  skos:altLabel "Adult literacy"@en ;
  skos:altLabel "Bridging courses"@en ;
  skos:altLabel "Health education"@en ;
  skos:altLabel "Learning English"@en ;
  skos:altLabel "Sex education"@en ;
  skos:altLabel "Third age learning"@en ;
  skos:broader agift:Community-education ;
  skos:definition "Administering training designed to meet the needs of specific groups of adult learners. Includes life skills, literacy programs and bridging courses to assist adults moving into school, tertiary or vocational education."@en ;
  skos:prefLabel "Adult education programs"@en ;
  skos:related agift:Child-and-youth-support ;
  skos:related agift:Health-promotion ;
  skos:related agift:Primary-health-care ;
.
agift:Adult-migrant-education
  a skos:Concept ;
  dcterms:contributor "KOdea" ;
  dcterms:created "2016-07-06T04:13:29+00:00"^^xsd:dateTime ;
  dcterms:creator "superadmin" ;
  dcterms:modified "2016-09-09T06:38:08+00:00"^^xsd:dateTime ;
  skos:altLabel "English-as-a-second-language courses"@en ;
  skos:altLabel "Immigrant education"@en ;
  skos:altLabel "Migrant education"@en ;
  skos:broader agift:Community-education ;
  skos:definition "Administering training designed to assist adults from various ethnic backgrounds to live and work in Australia. Includes English language programs, courses on Australian society and laws, learning to deal with government or health facilities."@en ;
  skos:prefLabel "Adult migrant education"@en ;
  skos:related agift:Interpreter-services ;
  skos:related agift:Migrant-services ;
  skos:related agift:Migrant-settlement-programs ;
  skos:related agift:Special-needs-programs ;
.
agift:Advertising-campaigns
  skos:prefLabel "Advertising campaigns"@en ;
  owl:deprecated true ;
.
agift:Advertising-campaigns
  a skos:Concept ;
  dcterms:contributor "KOdea" ;
  dcterms:created "2016-07-06T05:12:05+00:00"^^xsd:dateTime ;
  dcterms:creator "superadmin" ;
  dcterms:modified "2016-09-13T06:54:14+00:00"^^xsd:dateTime ;
  skos:altLabel "Tourist advertising"@en ;
  skos:broader agift:Tourist-event-promotion ;
  skos:definition "Delivering television, printed and electronic marketing, public relations and information programs to promote Australia or a particular region as a travel and tourism destination. Includes advertising campaigns to promote tourist events and local products."@en ;
  skos:prefLabel "Advertising campaigns"@en ;
  skos:related agift:Government-media ;
  skos:related agift:Publishing ;
.
agift:Advertising-standards
  a skos:Concept ;
  dcterms:contributor "KOdea" ;
  dcterms:created "2016-07-06T02:53:20+00:00"^^xsd:dateTime ;
  dcterms:creator "superadmin" ;
  dcterms:modified "2016-09-09T07:14:42+00:00"^^xsd:dateTime ;
  skos:altLabel "Commercial standards"@en ;
  skos:altLabel "Media advertising standards"@en ;
  skos:altLabel "Radio advertising standards"@en ;
  skos:altLabel "Television advertising standards"@en ;
  skos:broader agift:COMMUNICATIONS ;
  skos:definition "Regulating the content and presentation of marketing material disseminated via any medium. Developing guidelines to guard against misleading or offensive advertising. Providing advice on the implementation of standards and monitoring compliance."@en ;
  skos:prefLabel "Advertising standards"@en ;
  skos:related agift:Broadcasting-standards ;
  skos:related agift:Business-sponsorship ;
  skos:related agift:Censorship-standards ;
  skos:related agift:Consumer-protection ;
  skos:related agift:Election-campaigning ;
.
agift:Aged-care-services
  a skos:Concept ;
  dcterms:contributor "KOdea" ;
  dcterms:created "2016-07-06T04:02:16+00:00"^^xsd:dateTime ;
  dcterms:creator "superadmin" ;
  dcterms:modified "2016-09-06T07:17:45+00:00"^^xsd:dateTime ;
  skos:altLabel "Aged care standards"@en ;
  skos:altLabel "Aged persons services"@en ;
  skos:altLabel "Geriatric services"@en ;
  skos:broader agift:Community-support ;
  skos:definition "Managing social support and services for elderly persons and their families. Providing advice on rights to financial or other assistance such as residential care or medical services. Includes funding and support for community-based or volunteer programs providing aged care services."@en ;
  skos:prefLabel "Aged care services"@en ;
  skos:related agift:Financial-assistance ;
  skos:related agift:Independent-living-services ;
  skos:related agift:Residential-services ;
  skos:related agift:Special-needs-services ;
  skos:related agift:Veterans-entitlements ;
.
agift:Agreement-bargaining-processes
  a skos:Concept ;
  dcterms:contributor "KOdea" ;
  dcterms:created "2016-07-06T04:22:39+00:00"^^xsd:dateTime ;
  dcterms:creator "superadmin" ;
  dcterms:modified "2016-08-19T07:23:14+00:00"^^xsd:dateTime ;
  skos:altLabel "Certified agreement negotiation"@en ;
  skos:altLabel "Enterprise bargaining processes"@en ;
  skos:broader agift:Workplace-agreement-processes ;
  skos:definition "Negotiating agreements to regulate the conduct of employer and employees across an organisation, or between an employer and an individual employee. Includes consultation between parties, drafting of agreements and liaison with bargaining agents or advisors."@en ;
  skos:prefLabel "Agreement bargaining processes"@en ;
.
agift:Agreement-dispute-mediation
  a skos:Concept ;
  dcterms:contributor "KOdea" ;
  dcterms:created "2016-07-06T04:22:47+00:00"^^xsd:dateTime ;
  dcterms:creator "superadmin" ;
  dcterms:modified "2016-09-09T07:19:48+00:00"^^xsd:dateTime ;
  skos:broader agift:Workplace-agreement-processes ;
  skos:prefLabel "Agreement dispute mediation"@en ;
  skos:related agift:Dispute-mediation-programs ;
  skos:related agift:Industrial-awards-and-conditions ;
  skos:related agift:Workplace-equity-and-justice-programs ;
.
agift:Agricultural-industry
  a skos:Concept ;
  dcterms:contributor "KOdea" ;
  dcterms:created "2016-07-06T05:01:46+00:00"^^xsd:dateTime ;
  dcterms:creator "superadmin" ;
  dcterms:modified "2016-09-12T06:10:19+00:00"^^xsd:dateTime ;
  skos:altLabel "Animal food supplements"@en ;
  skos:altLabel "Crop farming regulation"@en ;
  skos:altLabel "Farming industries regulation"@en ;
  skos:altLabel "Livestock industries regulation"@en ;
  skos:altLabel "Pastoral lease registration"@en ;
  skos:altLabel "Sustainable agriculture"@en ;
  skos:broader agift:Marine-and-rural-regulation ;
  skos:definition "Regulating crop and livestock farming industries. Administering quotas and issuing licenses for controlled activities. Certifying products and production methods. Conducting assessments and inspections to ensure compliance with standards and policy. Applying penalties for breaches of regulations."@en ;
  skos:prefLabel "Agricultural industry"@en ;
  skos:related agift:Agricultural-sciences ;
  skos:related agift:Horticultural-industry ;
  skos:related agift:Pastoral-industry ;
  skos:related agift:Viticultural-industry ;
.
agift:Agricultural-sciences
  a skos:Concept ;
  dcterms:contributor "KOdea" ;
  dcterms:created "2016-07-06T03:42:44+00:00"^^xsd:dateTime ;
  dcterms:creator "superadmin" ;
  dcterms:modified "2016-09-12T06:22:15+00:00"^^xsd:dateTime ;
  skos:altLabel "Agricultural research"@en ;
  skos:altLabel "Farm research"@en ;
  skos:altLabel "Farm sciences"@en ;
  skos:broader agift:SCIENCE ;
  skos:definition "Conducting research into forestry, food, fibre and other crops or plants grown for commercial purposes. Providing input into quality control for the processing of agricultural products. Includes scientific advice on soil, weed and pest management, and information on new plant species."@en ;
  skos:prefLabel "Agricultural sciences"@en ;
  skos:related agift:Agricultural-industry ;
  skos:related agift:Animal-and-veterinary-sciences ;
  skos:related agift:Biotechnology-development ;
  skos:related agift:Botany ;
  skos:related agift:Chemical-and-pesticide-regulation ;
  skos:related agift:Forestry-industry ;
  skos:related agift:Genetic-engineering ;
  skos:related agift:Horticultural-industry ;
  skos:related agift:Silvicultural-industry ;
  skos:related agift:Soil-preservation-programs ;
  skos:related agift:Viticultural-industry ;
.
agift:Air-Force
  a skos:Concept ;
  dcterms:contributor "KOdea" ;
  dcterms:created "2016-07-06T04:08:13+00:00"^^xsd:dateTime ;
  dcterms:creator "superadmin" ;
  dcterms:modified "2016-09-08T06:28:31+00:00"^^xsd:dateTime ;
  skos:altLabel "Airforce"@en ;
  skos:altLabel "RAAF"@en ;
  skos:altLabel "Royal Australian Air Force"@en ;
  skos:broader agift:Australian-Defence-Forces ;
  skos:definition "Raising, equipping and maintaining the air capacity of Australia's defence forces. Administering Air Force activities, implementing defence policy and coordinating joint defence force operations. Includes on-the-job and basic training of new Air Force recruits."@en ;
  skos:prefLabel "Air Force"@en ;
  skos:related agift:Air-transport ;
  skos:related agift:Reserves ;
.
agift:Air-transport
  a skos:Concept ;
  dcterms:contributor "KOdea" ;
  dcterms:created "2016-07-06T03:49:30+00:00"^^xsd:dateTime ;
  dcterms:creator "superadmin" ;
  dcterms:modified "2016-09-13T07:09:46+00:00"^^xsd:dateTime ;
  skos:altLabel "Aerospace"@en ;
  skos:altLabel "Airlines"@en ;
  skos:altLabel "Airspace"@en ;
  skos:altLabel "Aviation"@en ;
  skos:altLabel "Civil aviation"@en ;
  skos:broader agift:TRANSPORT ;
  skos:definition "Regulating the airline industry and developing policy relating to all aspects of private or commercial aviation. Administering air transport standards, security and services and maintaining air transport infrastructure. Includes liaison with other governments and international bodies to negotiate air lanes and airspace jurisdiction."@en ;
  skos:narrower agift:Air-transport-safety ;
  skos:narrower agift:Aircraft-standards ;
  skos:narrower agift:Airport-services ;
  skos:prefLabel "Air transport"@en ;
  skos:related agift:Air-Force ;
  skos:related agift:Freight-movement-regulation ;
.
agift:Air-transport-safety
  a skos:Concept ;
  dcterms:contributor "KOdea" ;
  dcterms:created "2016-07-06T05:14:26+00:00"^^xsd:dateTime ;
  dcterms:creator "superadmin" ;
  dcterms:modified "2016-09-13T07:10:41+00:00"^^xsd:dateTime ;
  skos:altLabel "Accident investigation"@en ;
  skos:altLabel "Air safety"@en ;
  skos:altLabel "Airport security"@en ;
  skos:altLabel "Safety investigation"@en ;
  skos:broader agift:Air-transport ;
  skos:definition "Regulating private and commercial aviation activities to improve security and reduce the risk of accidents or emergencies. Investigating accidents and incidents. Monitoring compliance with in-flight safety standards and regulations for security screening procedures. Includes training and advice, consultation and inspection services and cooperation on aviation safety issues across jurisdictions."@en ;
  skos:prefLabel "Air transport safety"@en ;
  skos:related agift:Aircraft-standards ;
  skos:related agift:Airport-services ;
.
agift:Aircraft-standards
  a skos:Concept ;
  dcterms:contributor "KOdea" ;
  dcterms:created "2016-07-06T05:14:33+00:00"^^xsd:dateTime ;
  dcterms:creator "superadmin" ;
  dcterms:modified "2016-09-13T07:11:31+00:00"^^xsd:dateTime ;
  skos:altLabel "Aeroplanes"@en ;
  skos:altLabel "Airline pilots"@en ;
  skos:altLabel "Airplanes"@en ;
  skos:altLabel "Pilots"@en ;
  skos:broader agift:Air-transport ;
  skos:definition "Regulating the design, construction, maintenance and operation of any machine supported for flight - such as airplanes, helicopters, gliders or hot air balloons. Registering aircraft to ensure they meet agreed specifications and are fit to fly. Monitoring conformance through inspections, testing and licensing. Includes certification of personnel such as flight crews, pilots, aviation engineers and others engaged in the maintenance of aircraft and equipment."@en ;
  skos:prefLabel "Aircraft standards"@en ;
  skos:related agift:Air-transport-safety ;
  skos:related agift:Atmospheric-sciences ;
  skos:related agift:Engineering-and-technology-sciences ;
.
agift:Airport-services
  a skos:Concept ;
  dcterms:contributor "KOdea" ;
  dcterms:created "2016-07-06T05:14:40+00:00"^^xsd:dateTime ;
  dcterms:creator "superadmin" ;
  dcterms:modified "2016-09-13T07:12:26+00:00"^^xsd:dateTime ;
  skos:altLabel "Aerodromes"@en ;
  skos:altLabel "Air navigation"@en ;
  skos:altLabel "Air traffic control"@en ;
  skos:altLabel "Airfields"@en ;
  skos:altLabel "Airports"@en ;
  skos:altLabel "Airstrips"@en ;
  skos:altLabel "Airways"@en ;
  skos:altLabel "Flight paths"@en ;
  skos:altLabel "Flight regulation"@en ;
  skos:altLabel "Runways"@en ;
  skos:broader agift:Air-transport ;
  skos:definition "Managing facilities for aircraft take-off, landing and storage. Regulating air traffic and providing air navigation support. Monitoring air lanes and registering flight paths for private or commercial aircraft. Includes maintenance of airports and air transport infrastructure."@en ;
  skos:prefLabel "Airport services"@en ;
  skos:related agift:Air-transport-safety ;
  skos:related agift:Passenger-services ;
  skos:related agift:Transport-infrastructure-development ;
.
agift:Ambulance-services
  a skos:Concept ;
  dcterms:contributor "KOdea" ;
  dcterms:created "2016-07-06T04:03:12+00:00"^^xsd:dateTime ;
  dcterms:creator "superadmin" ;
  dcterms:modified "2016-09-06T07:32:38+00:00"^^xsd:dateTime ;
  skos:altLabel "Aero-medical services"@en ;
  skos:altLabel "Emergency transport"@en ;
  skos:altLabel "Medical transport"@en ;
  skos:broader agift:Emergency-services ;
  skos:definition "Providing specially equipped vehicles and trained personnel to attend and transport sick or injured persons. Includes managing ambulance stations  and attendance at special events."@en ;
  skos:prefLabel "Ambulance services"@en ;
  skos:related agift:Community-education ;
  skos:related agift:Emergency-management ;
  skos:related agift:Natural-disasters ;
.
agift:Animal-and-veterinary-sciences
  a skos:Concept ;
  dcterms:contributor "KOdea" ;
  dcterms:created "2016-07-06T03:42:53+00:00"^^xsd:dateTime ;
  dcterms:creator "superadmin" ;
  dcterms:modified "2016-09-12T06:23:32+00:00"^^xsd:dateTime ;
  skos:altLabel "Animal sciences"@en ;
  skos:altLabel "Vet sciences"@en ;
  skos:altLabel "Veterinary research"@en ;
  skos:altLabel "Veterinary science"@en ;
  skos:broader agift:SCIENCE ;
  skos:definition "Conducting research into the health care and management of wild and domestic animals. Providing scientific advice on nutrition, breeding, diagnosis and treatment of diseases. Includes livestock, pets and other domestic animals, fish, birds and native animals - in the wild or in captivity."@en ;
  skos:prefLabel "Animal and veterinary sciences"@en ;
  skos:related agift:Agricultural-sciences ;
  skos:related agift:Aquaculture-industry ;
  skos:related agift:Chemical-and-pesticide-regulation ;
  skos:related agift:Entomology ;
  skos:related agift:Fisheries-industry ;
  skos:related agift:Pastoral-industry ;
  skos:related agift:Physiology ;
.
agift:Apparatus-licensing
  a skos:Concept ;
  dcterms:contributor "KOdea" ;
  dcterms:created "2016-07-06T03:59:55+00:00"^^xsd:dateTime ;
  dcterms:creator "superadmin" ;
  dcterms:modified "2016-09-05T07:55:21+00:00"^^xsd:dateTime ;
  skos:altLabel "Radio communication licensing"@en ;
  skos:broader agift:Radio-communication ;
  skos:definition "Administering standards for radio communications equipment. Monitoring compliance with government regulations. Processing licence applications for radio communications or transmission equipment. Administering standards for radio communications equipment. Ensuring that any emissions from apparatus, identified by qualified health authorities as being potentially are harmful, are properly controlled."@en ;
  skos:prefLabel "Apparatus licensing"@en ;
  skos:related agift:Medical-and-health-sciences ;
  skos:related agift:Mobile-telephone-services ;
.
agift:Applied-sciences
  a skos:Concept ;
  dcterms:contributor "KOdea" ;
  dcterms:created "2016-07-06T03:43:00+00:00"^^xsd:dateTime ;
  dcterms:creator "superadmin" ;
  dcterms:modified "2016-09-12T06:41:17+00:00"^^xsd:dateTime ;
  skos:altLabel "Industrial chemistry"@en ;
  skos:broader agift:SCIENCE ;
  skos:definition "Conducting research into the active use of scientific knowledge and principles from a range of fields and disciplines. Providing advice and practical solutions to problems in various sectors, such as industry, security, communications and health care."@en ;
  skos:narrower agift:Engineering-and-technology-sciences ;
  skos:narrower agift:Weights-and-measures-standards ;
  skos:prefLabel "Applied sciences"@en ;
  skos:related agift:Biotechnology-development ;
  skos:related agift:Mathematical-sciences ;
  skos:related agift:Medical-and-health-sciences ;
  skos:related agift:Mineral-exploration ;
  skos:related agift:Physical-sciences ;
  skos:related agift:Spatial-information-research ;
.
agift:Appointment-management
  a skos:Concept ;
  dcterms:contributor "superadmin" ;
  dcterms:created "2016-07-06T03:05:28+00:00"^^xsd:dateTime ;
  dcterms:creator "superadmin" ;
  dcterms:modified "2016-07-06T06:32:11+00:00"^^xsd:dateTime ;
  skos:broader agift:GOVERNANCE ;
  skos:definition "Management of appointments authorised by the Governor-General and Prime-Minister to support portfolio responsibilities."@en ;
  skos:prefLabel "Appointment management"@en ;
.
agift:Apprenticeship-programs
  a skos:Concept ;
  dcterms:contributor "KOdea" ;
  dcterms:created "2016-07-06T04:14:55+00:00"^^xsd:dateTime ;
  dcterms:creator "superadmin" ;
  dcterms:modified "2016-09-08T07:18:16+00:00"^^xsd:dateTime ;
  skos:altLabel "Trade apprenticeships"@en ;
  skos:broader agift:Vocational-education ;
  skos:definition "Administering programs of industry-based training for trade and technical vocations. Monitoring compliance with standards and guidelines. Managing accreditation processes. Implementing schemes to assist employers to take on apprentices."@en ;
  skos:prefLabel "Apprenticeship programs"@en ;
  skos:related agift:Industrial-awards-and-conditions ;
  skos:related agift:Trainee-programs ;
.
agift:Aquaculture-industry
  a skos:Concept ;
  dcterms:contributor "KOdea" ;
  dcterms:created "2016-07-06T05:02:25+00:00"^^xsd:dateTime ;
  dcterms:creator "superadmin" ;
  dcterms:modified "2016-09-12T06:14:42+00:00"^^xsd:dateTime ;
  skos:altLabel "Fish farming industry"@en ;
  skos:broader agift:Marine-and-rural-support ;
  skos:definition "Administering programs to support marine and freshwater fish or crop farming. Assisting industry growth and development. Encouraging businesses to adopt innovative practices, processes and products. Providing advice on production methods and business management to improve competitiveness."@en ;
  skos:prefLabel "Aquaculture industry"@en ;
  skos:related agift:Animal-and-veterinary-sciences ;
  skos:related agift:Fisheries-industry ;
  skos:related agift:Oceans-governance ;
.
agift:Architectural-services
  a skos:Concept ;
  dcterms:contributor "KOdea" ;
  dcterms:created "2016-07-06T03:53:03+00:00"^^xsd:dateTime ;
  dcterms:creator "superadmin" ;
  dcterms:modified "2016-09-05T07:02:44+00:00"^^xsd:dateTime ;
  skos:altLabel "Architect services"@en ;
  skos:altLabel "Architecture"@en ;
  skos:altLabel "Building design services"@en ;
  skos:altLabel "Heritage value assessments"@en ;
  skos:broader agift:Civic-management ;
  skos:definition "Providing professional advice and supervising the design and construction of public buildings.  Approving plans and conducting inspections to ensure building is completed in accordance with approved plans. Includes heritage value assessments."@en ;
  skos:prefLabel "Architectural services"@en ;
  skos:related agift:Building-preservation ;
  skos:related agift:Building-regulations-and-standards ;
  skos:related agift:Community-housing ;
  skos:related agift:Engineering-services ;
  skos:related agift:Public-housing-construction ;
.
agift:Army
  a skos:Concept ;
  dcterms:contributor "KOdea" ;
  dcterms:created "2016-07-06T04:08:19+00:00"^^xsd:dateTime ;
  dcterms:creator "superadmin" ;
  dcterms:modified "2016-09-08T06:29:23+00:00"^^xsd:dateTime ;
  skos:altLabel "Australian Army"@en ;
  skos:broader agift:Australian-Defence-Forces ;
  skos:definition "Raising, equipping and maintaining the land capability of Australia's defence forces. Administering Army activities, implementing defence policy and coordinating joint defence forces operations. Includes on-the-job and basic training of new Army recruits."@en ;
  skos:prefLabel "Army"@en ;
  skos:related agift:Army-reserve-training ;
  skos:related agift:Reserves ;
.
agift:Army-reserve-training
  a skos:Concept ;
  dcterms:contributor "KOdea" ;
  dcterms:created "2016-07-06T04:13:54+00:00"^^xsd:dateTime ;
  dcterms:creator "superadmin" ;
  dcterms:modified "2016-09-08T07:09:12+00:00"^^xsd:dateTime ;
  skos:altLabel "Army reserves"@en ;
  skos:altLabel "Reserve training"@en ;
  skos:broader agift:Military-education-and-training ;
  skos:definition "Administering educational programs for part-time voluntary defence units in the Army. Providing ongoing training through coursework and residential schools. Includes liaison with employers when sustained absence from work is required"@en ;
  skos:prefLabel "Army reserve training"@en ;
  skos:related agift:Army ;
  skos:related agift:Reserves ;
.
agift:Artefact-export-regulation
  skos:prefLabel "Artefact export regulation"@en ;
  owl:deprecated true ;
.
agift:Artefact-export-regulation
  a skos:Concept ;
  dcterms:contributor "fionamcl" ;
  dcterms:created "2016-09-08T01:34:09+00:00"^^xsd:dateTime ;
  dcterms:creator "fionamcl" ;
  skos:altLabel "Art export"@en ;
  skos:altLabel "Cultural material export regulation"@en ;
  skos:broader agift:Collection-management ;
  skos:definition "Negotiating the international movement of cultural material. Liaising with government and private sector bodies for the temporary import or export of artefacts for exhibition purposes. Obtaining valuations to confirm the worth of items. Assisting the return of illegally imported cultural property. Seeking export prevention orders for protected artefacts."@en ;
  skos:prefLabel "Artefact export regulation"@en ;
  skos:related agift:Cultural-artefact-repatriation ;
  skos:related agift:Prohibited-export-control ;
  skos:related agift:Prohibited-import-control ;
.
agift:Arts-development
  skos:prefLabel "Arts development"@en ;
  owl:deprecated true ;
.
agift:Arts-development
  a skos:Concept ;
  dcterms:contributor "fionamcl" ;
  dcterms:created "2016-09-08T01:21:58+00:00"^^xsd:dateTime ;
  dcterms:creator "fionamcl" ;
  dcterms:modified "2016-11-28T22:47:18+00:00"^^xsd:dateTime ;
  skos:altLabel "Arts councils"@en ;
  skos:altLabel "Ballet"@en ;
  skos:altLabel "Creative arts development"@en ;
  skos:altLabel "Dance"@en ;
  skos:altLabel "Film industry development"@en ;
  skos:altLabel "Fine arts development"@en ;
  skos:altLabel "Indigenous arts development"@en ;
  skos:altLabel "Literary arts development"@en ;
  skos:altLabel "Musical arts development"@en ;
  skos:altLabel "Opera"@en ;
  skos:altLabel "Performing arts development"@en ;
  skos:altLabel "Visual arts development"@en ;
  skos:broader agift:CULTURAL-AFFAIRS ;
  skos:definition "Providing support for the production of skilled performance or craft. Administering programs to develop funding and promotional strategies for the arts, and to encourage participation from across the community. Assisting the growth of artistic companies such as orchestras and dance companies through business advice and planning. Includes support for work spaces and liaison with education and exhibition facilities."@en ;
  skos:narrower agift:Arts-funding ;
  skos:narrower agift:Arts-incentive-schemes ;
  skos:narrower agift:Arts-promotion ;
  skos:prefLabel "Arts development"@en ;
  skos:related agift:Arts-education ;
  skos:related agift:Export-promotion ;
  skos:related agift:Trade-development-programs ;
.
agift:Arts-education
  a skos:Concept ;
  dcterms:contributor "KOdea" ;
  dcterms:created "2016-07-06T02:59:54+00:00"^^xsd:dateTime ;
  dcterms:creator "superadmin" ;
  dcterms:modified "2016-09-08T07:15:03+00:00"^^xsd:dateTime ;
  skos:altLabel "Arts councils"@en ;
  skos:broader agift:EDUCATION-AND-TRAINING ;
  skos:definition "Administering programs that offer training and facilities to support the production of skilled performance or craft. Managing specialised institutions or schemes to foster artistic talent at individual or community level. Includes the provision of scholarships and study grants."@en ;
  skos:prefLabel "Arts education"@en ;
  skos:related agift:Arts-development ;
  skos:related agift:Overseas-student-scholarship-programs ;
  skos:related agift:School-education ;
  skos:related agift:Tertiary-education ;
.
agift:Arts-funding
  skos:prefLabel "Arts funding"@en ;
  owl:deprecated true ;
.
agift:Arts-funding
  a skos:Concept ;
  dcterms:contributor "fionamcl" ;
  dcterms:created "2016-09-08T01:26:08+00:00"^^xsd:dateTime ;
  dcterms:creator "fionamcl" ;
  dcterms:modified "2016-11-28T22:46:25+00:00"^^xsd:dateTime ;
  skos:altLabel "Art subsidy schemes"@en ;
  skos:altLabel "Artistic grants"@en ;
  skos:broader agift:Arts-development ;
  skos:definition "Providing financial support for the production of skilled performance or craft. Assessing applications for funding. Allocating grants and subsidies to projects that meet selection criteria. Advising artists about funding programs and application procedures."@en ;
  skos:prefLabel "Arts funding"@en ;
.
agift:Arts-incentive-schemes
  skos:prefLabel "Arts incentive schemes"@en ;
  owl:deprecated true ;
.
agift:Arts-incentive-schemes
  a skos:Concept ;
  dcterms:contributor "fionamcl" ;
  dcterms:created "2016-09-08T01:26:13+00:00"^^xsd:dateTime ;
  dcterms:creator "fionamcl" ;
  dcterms:modified "2016-11-28T22:46:34+00:00"^^xsd:dateTime ;
  skos:altLabel "Register of cultural organisations"@en ;
  skos:altLabel "Taxation incentives for the arts"@en ;
  skos:broader agift:Arts-development ;
  skos:definition "Developing strategies to encourage investment in artistic activities or moveable cultural materials. Negotiating tax deductions for approved activities and setting guidelines for donor benefits. Certifying valuers to assess the worth of artistic works. Maintaining a register of cultural organisations qualified to offer incentives."@en ;
  skos:prefLabel "Arts incentive schemes"@en ;
  skos:related agift:Cultural-gifts-programs ;
.
agift:Arts-promotion
  skos:prefLabel "Arts promotion"@en ;
  owl:deprecated true ;
.
agift:Arts-promotion
  a skos:Concept ;
  dcterms:contributor "fionamcl" ;
  dcterms:created "2016-09-08T01:26:19+00:00"^^xsd:dateTime ;
  dcterms:creator "fionamcl" ;
  dcterms:modified "2016-11-28T22:46:40+00:00"^^xsd:dateTime ;
  skos:altLabel "Arts marketing"@en ;
  skos:broader agift:Arts-development ;
  skos:definition "Managing programs to encourage participation in artistic pursuits and support for performances or exhibitions. Developing strategies for marketing and information dissemination to raise community awareness of the arts."@en ;
  skos:prefLabel "Arts promotion"@en ;
  skos:related agift:Collection-promotion ;
.
agift:Asset-assessment
  a skos:Concept ;
  dcterms:contributor "KOdea" ;
  dcterms:created "2016-07-06T04:38:27+00:00"^^xsd:dateTime ;
  dcterms:creator "superadmin" ;
  dcterms:modified "2016-09-08T08:03:31+00:00"^^xsd:dateTime ;
  skos:altLabel "Retiree assets"@en ;
  skos:altLabel "Retirement assets"@en ;
  skos:broader agift:Retirement-income ;
  skos:definition "Estimating the value of resources owned by a retired individual in order to identify applicable taxes or benefits. Determining whether an asset meets criteria for exemption or inclusion for assessment purposes."@en ;
  skos:prefLabel "Asset assessment"@en ;
  skos:related agift:Financial-assistance ;
  skos:related agift:Income-support-schemes ;
.
agift:Associations-and-corporate-law
  a skos:Concept ;
  dcterms:contributor "KOdea" ;
  dcterms:created "2016-07-06T03:37:06+00:00"^^xsd:dateTime ;
  dcterms:creator "superadmin" ;
  dcterms:modified "2016-09-05T06:20:30+00:00"^^xsd:dateTime ;
  skos:altLabel "Business law"@en ;
  skos:altLabel "Corporate law"@en ;
  skos:altLabel "Corporations law"@en ;
  skos:broader agift:JUSTICE-ADMINISTRATION ;
  skos:definition "Administering the body of law that relates to companies or other organisations that have a distinct legal identity from that of their members. Regulating the formation, governance and dissolution of such organisations and establishing the limits of their powers or liability."@en ;
  skos:narrower agift:Bankruptcy-proceedings ;
  skos:narrower agift:Merger-regulation ;
  skos:prefLabel "Associations and corporate law"@en ;
  skos:related agift:Business-association ;
  skos:related agift:Business-registration-and-licensing ;
.
agift:Astronomical-sciences
  a skos:Concept ;
  dcterms:contributor "KOdea" ;
  dcterms:created "2016-07-06T05:05:43+00:00"^^xsd:dateTime ;
  dcterms:creator "superadmin" ;
  dcterms:modified "2016-09-05T07:52:22+00:00"^^xsd:dateTime ;
  skos:altLabel "Astronomy"@en ;
  skos:altLabel "Cosmology"@en ;
  skos:altLabel "Space research"@en ;
  skos:broader agift:Physical-sciences ;
  skos:definition "Conducting research into the properties of inanimate matter, substances and energy. Analysing and manipulating such material to identify the principles and processes that govern its behaviour. Includes the development of new methods to exploit physical substances or energy"@en ;
  skos:prefLabel "Astronomical sciences"@en ;
  skos:related agift:Satellite-communication ;
.
agift:Athlete-scholarship-programs
  a skos:Concept ;
  dcterms:contributor "KOdea" ;
  dcterms:created "2016-07-06T05:09:44+00:00"^^xsd:dateTime ;
  dcterms:creator "superadmin" ;
  dcterms:modified "2016-09-13T06:37:15+00:00"^^xsd:dateTime ;
  skos:altLabel "Athletics scholarships"@en ;
  skos:altLabel "Sports scholarships"@en ;
  skos:broader agift:Sport-and-fitness-development ;
  skos:definition "Administering schemes to encourage excellence in sport across local and national levels. Providing financial assistance to highly skilled athletes to attend advanced training programs. Enabling access to elite facilities, performance coaching, sports science services, career planning and education services. Sponsoring travel, accommodation and living expenses to support attendance at competitions."@en ;
  skos:prefLabel "Athlete scholarship programs"@en ;
  skos:related agift:Sporting-grants-administration ;
.
agift:Atmospheric-sciences
  a skos:Concept ;
  dcterms:contributor "KOdea" ;
  dcterms:created "2016-07-06T05:04:56+00:00"^^xsd:dateTime ;
  dcterms:creator "superadmin" ;
  dcterms:modified "2016-09-13T07:11:18+00:00"^^xsd:dateTime ;
  skos:altLabel "Atmospheric research"@en ;
  skos:altLabel "Climate change"@en ;
  skos:altLabel "Climate research"@en ;
  skos:altLabel "Global warming"@en ;
  skos:altLabel "Greenhouse effect"@en ;
  skos:altLabel "Ionospheric prediction"@en ;
  skos:altLabel "Meteorology"@en ;
  skos:altLabel "Weather research"@en ;
  skos:broader agift:Earth-sciences ;
  skos:definition "Conducting research into weather, climate and air pollution. Providing scientific advice on severe weather and climatic variation, such as acid deposition and ozone depletion. Includes middle atmosphere climate and space weather analysis, studies of the thermosphere and observatory experiments."@en ;
  skos:prefLabel "Atmospheric sciences"@en ;
  skos:related agift:Aircraft-standards ;
  skos:related agift:Climate-information-services ;
  skos:related agift:Natural-disasters ;
  skos:related agift:Pollutant-prevention-programs ;
  skos:related agift:Pollution-emission-control ;
.
agift:Atomic-and-molecular-sciences
  a skos:Concept ;
  dcterms:contributor "KOdea" ;
  dcterms:created "2016-07-06T05:05:51+00:00"^^xsd:dateTime ;
  dcterms:creator "superadmin" ;
  dcterms:modified "2016-09-12T06:42:31+00:00"^^xsd:dateTime ;
  skos:altLabel "Atomic research"@en ;
  skos:altLabel "Molecular science"@en ;
  skos:broader agift:Physical-sciences ;
  skos:definition "Conducting research into the structure and nature of the smallest particles of matter. Analysing the interaction of atoms with electromagnetic radiation, and changes to their chemical identity, weight or behaviour. Observing atomic reactions to identify or develop products or processes for use in medical, industrial or defence applications, or to support other fields of scientific research."@en ;
  skos:prefLabel "Atomic and molecular sciences"@en ;
  skos:related agift:Biochemistry ;
  skos:related agift:Nuclear-sciences ;
.
agift:Australian-Defence-Forces
  a skos:Concept ;
  dcterms:contributor "KOdea" ;
  dcterms:created "2016-07-06T02:58:17+00:00"^^xsd:dateTime ;
  dcterms:creator "superadmin" ;
  dcterms:modified "2016-09-08T06:58:04+00:00"^^xsd:dateTime ;
  skos:altLabel "ADF"@en ;
  skos:altLabel "Armed forces"@en ;
  skos:altLabel "Defence forces"@en ;
  skos:altLabel "Military forces"@en ;
  skos:broader agift:DEFENCE ;
  skos:definition "Maintaining and administering the combined Australian Defence Forces to ensure Australia's ability to resist foreign aggression or attack. Includes policies and programs for the development of the defence forces as a whole, arrangements for force generation, mobilisation and support."@en ;
  skos:narrower agift:Air-Force ;
  skos:narrower agift:Army ;
  skos:narrower agift:Badges-and-insignia ;
  skos:narrower agift:Cadets ;
  skos:narrower agift:Defence-force-commands ;
  skos:narrower agift:Military-bands ;
  skos:narrower agift:Navy ;
  skos:narrower agift:Reserves ;
  skos:prefLabel "Australian Defence Forces"@en ;
  skos:related agift:Defence-liaison ;
  skos:related agift:Military-education-and-training ;
  skos:related agift:Military-exercises ;
.
agift:Australian-theatre-of-war
  a skos:Concept ;
  dcterms:contributor "KOdea" ;
  dcterms:created "2016-07-06T04:12:09+00:00"^^xsd:dateTime ;
  dcterms:creator "superadmin" ;
  dcterms:modified "2016-09-08T06:57:41+00:00"^^xsd:dateTime ;
  skos:altLabel "Campaigns"@en ;
  skos:altLabel "Theatre of war"@en ;
  skos:broader agift:Military-operations ;
  skos:definition "Coordinating activities across the entire air, sea and land areas where Australia is likely to be directly involved in warfare or military action. Planning and conducting campaigns for the defence of Australia and its interests."@en ;
  skos:prefLabel "Australian theatre of war"@en ;
  skos:related agift:Special-operations ;
  skos:related agift:Warfare ;
.
agift:Authentication
  a skos:Concept ;
  dcterms:contributor "KOdea" ;
  dcterms:created "2016-07-06T03:57:01+00:00"^^xsd:dateTime ;
  dcterms:creator "superadmin" ;
  dcterms:modified "2016-09-12T06:50:06+00:00"^^xsd:dateTime ;
  skos:altLabel "Digital signatures"@en ;
  skos:altLabel "Electronic signatures"@en ;
  skos:altLabel "Encryption"@en ;
  skos:altLabel "Online security"@en ;
  skos:altLabel "PKI"@en ;
  skos:altLabel "Public Key Technology"@en ;
  skos:broader agift:Electronic-commerce ;
  skos:definition "Managing infrastructure to support the validation of electronic transactions to ensure commerce can be conducted free from abuse or fraud. Includes accreditation of certification authorities, management of public key certificates, related agreements and audits."@en ;
  skos:prefLabel "Authentication"@en ;
  skos:related agift:Information-security ;
.
agift:Award-conditions
  a skos:Concept ;
  dcterms:contributor "KOdea" ;
  dcterms:created "2016-07-06T04:21:48+00:00"^^xsd:dateTime ;
  dcterms:creator "superadmin" ;
  dcterms:modified "2016-09-08T07:29:58+00:00"^^xsd:dateTime ;
  skos:altLabel "Allowances"@en ;
  skos:altLabel "Annual leave"@en ;
  skos:altLabel "Award wages"@en ;
  skos:altLabel "Bereavement leave"@en ;
  skos:altLabel "Carer's leave"@en ;
  skos:altLabel "Employment conditions"@en ;
  skos:altLabel "Entitlements"@en ;
  skos:altLabel "Junior wages"@en ;
  skos:altLabel "Leave entitlements"@en ;
  skos:altLabel "Long service leave"@en ;
  skos:altLabel "Maternity leave"@en ;
  skos:altLabel "Minimum wage"@en ;
  skos:altLabel "Overtime rates"@en ;
  skos:altLabel "Parental leave"@en ;
  skos:altLabel "Penalty rates"@en ;
  skos:altLabel "Personal leave"@en ;
  skos:altLabel "Rates of pay and salary"@en ;
  skos:altLabel "Salary regulation"@en ;
  skos:altLabel "Shift penalties"@en ;
  skos:altLabel "Sick leave"@en ;
  skos:altLabel "Wages"@en ;
  skos:altLabel "Work life balance"@en ;
  skos:altLabel "Working conditions"@en ;
  skos:altLabel "Youth wages and allowances"@en ;
  skos:broader agift:Industrial-awards-and-conditions ;
  skos:definition "Implementing the provisions of industrial awards with regard to employment conditions and rates of pay. Providing advice on hours of work, working conditions, leave and other entitlements. Administering the payment of wages, allowances, overtime and penalties."@en ;
  skos:prefLabel "Award conditions"@en ;
  skos:related agift:Certified-employment-conditions ;
  skos:related agift:Occupational-health-and-safety ;
.
agift:BUSINESS-SUPPORT-AND-REGULATION
  a skos:Concept ;
  dcterms:contributor "KOdea" ;
  dcterms:created "2016-07-06T02:43:53+00:00"^^xsd:dateTime ;
  dcterms:creator "superadmin" ;
  dcterms:modified "2016-09-13T06:55:40+00:00"^^xsd:dateTime ;
  skos:altLabel "Industry"@en ;
  skos:definition "Formulating policy to regulate and support the private sector, including small business and non-profit organisations. Developing strategies to assist business growth and management. Implementing advocacy programs, providing funding and administering regulatory bodies."@en ;
  skos:narrower agift:Business-association ;
  skos:narrower agift:Business-process-auditing ;
  skos:narrower agift:Business-registration-and-licensing ;
  skos:narrower agift:Business-sponsorship ;
  skos:narrower agift:Consumer-protection ;
  skos:narrower agift:Fair-trading-compliance ;
  skos:narrower agift:Financial-institutions-regulation ;
  skos:narrower agift:Government-procurement-regulation ;
  skos:narrower agift:Industry-assistance-schemes ;
  skos:narrower agift:Industry-development ;
  skos:narrower agift:Insurance-regulation ;
  skos:narrower agift:Professional-accreditation ;
  skos:narrower agift:Small-business-services ;
  skos:narrower agift:Stock-market-regulation ;
  skos:prefLabel "BUSINESS SUPPORT AND REGULATION"@en ;
  skos:related agift:PRIMARY-INDUSTRIES ;
  skos:related agift:TRADE ;
  skos:topConceptOf agift:AGIFT ;
.
agift:Badges-and-insignia
  a skos:Concept ;
  dcterms:contributor "KOdea" ;
  dcterms:created "2016-07-06T04:08:27+00:00"^^xsd:dateTime ;
  dcterms:creator "superadmin" ;
  dcterms:modified "2016-09-08T06:29:52+00:00"^^xsd:dateTime ;
  skos:altLabel "Defence badges"@en ;
  skos:altLabel "Medals"@en ;
  skos:altLabel "Military awards"@en ;
  skos:altLabel "Military badges"@en ;
  skos:altLabel "Military insignia"@en ;
  skos:altLabel "Military medals"@en ;
  skos:broader agift:Australian-Defence-Forces ;
  skos:definition "Managing military badges, insignia, crests, medals and awards. Registering designs and regulating their use. Includes ceremonies for conferring military awards."@en ;
  skos:prefLabel "Badges and insignia"@en ;
  skos:related agift:Honours-and-awards-programs ;
.
agift:Bankruptcy-proceedings
  a skos:Concept ;
  dcterms:contributor "KOdea" ;
  dcterms:created "2016-07-06T04:55:35+00:00"^^xsd:dateTime ;
  dcterms:creator "superadmin" ;
  dcterms:modified "2016-08-26T08:09:58+00:00"^^xsd:dateTime ;
  skos:altLabel "Insolvency proceedings"@en ;
  skos:altLabel "Receivership management"@en ;
  skos:broader agift:Associations-and-corporate-law ;
  skos:definition "Administering insolvent parties' assets for the benefit of creditors. Includes providing bankruptcy notices, winding up of companies and the appointment of trustees."@en ;
  skos:prefLabel "Bankruptcy proceedings"@en ;
.
agift:Benefits
  a skos:Concept ;
  dcterms:contributor "KOdea" ;
  dcterms:created "2016-07-06T04:03:46+00:00"^^xsd:dateTime ;
  dcterms:creator "superadmin" ;
  dcterms:modified "2016-09-09T06:10:28+00:00"^^xsd:dateTime ;
  skos:altLabel "Allowances"@en ;
  skos:altLabel "Baby bonus"@en ;
  skos:altLabel "Entitlements"@en ;
  skos:altLabel "Farmer's rebate"@en ;
  skos:altLabel "Financial incentives"@en ;
  skos:altLabel "First homeowner's grant"@en ;
  skos:altLabel "Gap cover"@en ;
  skos:altLabel "LPG subsidy scheme"@en ;
  skos:altLabel "Maternity payment"@en ;
  skos:altLabel "Pharmaceutical benefits"@en ;
  skos:altLabel "Private health insurance rebate"@en ;
  skos:altLabel "Rebates"@en ;
  skos:altLabel "Seniors cards"@en ;
  skos:altLabel "Subsidies"@en ;
  skos:broader agift:Financial-assistance ;
  skos:definition "Administering programs to provide financial assistance to individuals, based on criteria other than income. Providing advice on entitlements. Assessing eligibility and processing payments. Includes ongoing benefits, one-off payments following a specific event, rebates for costs , rebates for costs already incurred or subsidies for upcoming expenses."@en ;
  skos:prefLabel "Benefits"@en ;
  skos:related agift:Health-insurance-schemes ;
  skos:related agift:Income-support-schemes ;
  skos:related agift:Indigenous-welfare-programs ;
  skos:related agift:Taxation-compliance ;
  skos:related agift:Veterans-entitlements ;
.
agift:Biochemistry
  a skos:Concept ;
  dcterms:contributor "KOdea" ;
  dcterms:created "2016-07-06T05:03:54+00:00"^^xsd:dateTime ;
  dcterms:creator "superadmin" ;
  dcterms:modified "2016-09-12T06:42:17+00:00"^^xsd:dateTime ;
  skos:altLabel "Cell biology"@en ;
  skos:altLabel "Molecular biology"@en ;
  skos:broader agift:Biological-sciences ;
  skos:definition "Conducting research into the chemical processes and molecular makeup of plants, animals and micro-organisms. Investigating the biological functions of plants and animals at a cellular level. Includes DNA and serum analysis."@en ;
  skos:prefLabel "Biochemistry"@en ;
  skos:related agift:Atomic-and-molecular-sciences ;
  skos:related agift:Biological-sciences ;
  skos:related agift:Genetic-engineering ;
.
agift:Biodiversity-preservation
  a skos:Concept ;
  dcterms:contributor "KOdea" ;
  dcterms:created "2016-07-06T05:04:02+00:00"^^xsd:dateTime ;
  dcterms:creator "superadmin" ;
  dcterms:modified "2016-09-08T07:39:46+00:00"^^xsd:dateTime ;
  skos:altLabel "Biodiversity management"@en ;
  skos:altLabel "Biodiversity"@en ;
  skos:broader agift:Biological-sciences ;
  skos:definition "Conducting research into the variety of plant and animal life in a region, and the actions necessary to conserve and sustain it. Identifying biota of environmental or economic significance. Includes studies of the origin, evolution and relationships between native plant and animal species, and programs to reintroduce in certain habitats."@en ;
  skos:prefLabel "Biodiversity preservation"@en ;
  skos:related agift:Conservation-programs ;
.
agift:Biological-sciences
  a skos:Concept ;
  dcterms:contributor "KOdea" ;
  dcterms:created "2016-07-06T03:43:09+00:00"^^xsd:dateTime ;
  dcterms:creator "superadmin" ;
  dcterms:modified "2016-09-12T06:41:30+00:00"^^xsd:dateTime ;
  skos:altLabel "Biology"@en ;
  skos:altLabel "Life sciences"@en ;
  skos:broader agift:SCIENCE ;
  skos:definition "Conducting research into the lives of plants, animals and micro-organisms. Investigating their origin, distribution, behaviour and physical makeup. Includes studies of evolution, ecosystem dynamics, identification and manipulation of biological processes."@en ;
  skos:narrower agift:Biochemistry ;
  skos:narrower agift:Biodiversity-preservation ;
  skos:narrower agift:Biotechnology-development ;
  skos:narrower agift:Botany ;
  skos:narrower agift:Entomology ;
  skos:narrower agift:Genetic-engineering ;
  skos:narrower agift:Physiology ;
  skos:prefLabel "Biological sciences"@en ;
  skos:related agift:Biochemistry ;
  skos:related agift:Marine-life-protection-programs ;
  skos:related agift:Medical-and-health-sciences ;
  skos:related agift:Oceanography ;
  skos:related agift:Physical-sciences ;
.
agift:Biotechnology-development
  a skos:Concept ;
  dcterms:contributor "KOdea" ;
  dcterms:created "2016-07-06T05:04:08+00:00"^^xsd:dateTime ;
  dcterms:creator "superadmin" ;
  dcterms:modified "2016-09-12T06:30:58+00:00"^^xsd:dateTime ;
  skos:altLabel "Fermentation"@en ;
  skos:altLabel "Genetically modified organisms"@en ;
  skos:altLabel "Grafting"@en ;
  skos:altLabel "Selective breeding"@en ;
  skos:broader agift:Biological-sciences ;
  skos:definition "Conducting research into the use of living things to make or alter organic material. Involves the use of micro-organisms or fungi, or strategies such as selective breeding to develop products for medical, agricultural and other commercial purposes. Includes health and environmental impact assessment of biotechnology products."@en ;
  skos:prefLabel "Biotechnology development"@en ;
  skos:related agift:Agricultural-sciences ;
  skos:related agift:Applied-sciences ;
  skos:related agift:Defence-science-and-technology ;
  skos:related agift:Food-quality-assurance ;
  skos:related agift:Genetic-engineering ;
.
agift:Blood-and-organ-donation-management
  a skos:Concept ;
  dcterms:contributor "KOdea" ;
  dcterms:created "2016-07-06T04:47:40+00:00"^^xsd:dateTime ;
  dcterms:creator "superadmin" ;
  dcterms:modified "2016-08-23T06:53:25+00:00"^^xsd:dateTime ;
  skos:broader agift:Public-health-services ;
  skos:definition "Developing policies and programs to establish a nationally coordinated approach to blood, organ and tissue donation. Promoting measures to raise community awareness of blood, organ and tissue donation."@en ;
  skos:prefLabel "Blood and organ donation management"@en ;
.
agift:Border-protection
  a skos:Concept ;
  dcterms:contributor "KOdea" ;
  dcterms:created "2016-07-06T05:08:30+00:00"^^xsd:dateTime ;
  dcterms:creator "superadmin" ;
  dcterms:modified "2016-09-13T07:00:26+00:00"^^xsd:dateTime ;
  skos:altLabel "Coastal defences"@en ;
  skos:altLabel "Coastal surveillance"@en ;
  skos:altLabel "Coastwatch"@en ;
  skos:altLabel "Maritme surveillance"@en ;
  skos:broader agift:National-security ;
  skos:definition "Coordinating operations to monitor Australian borders for unauthorised sea or air arrivals. Developing and implementing response procedures to prevent illegal entry. Includes liaison with law enforcement, immigration or defence services personnel to apprehend individuals who breach Australia's borders."@en ;
  skos:prefLabel "Border protection"@en ;
  skos:related agift:Detention-programs ;
  skos:related agift:Prohibited-import-control ;
  skos:related agift:Travel-authorisation ;
.
agift:Botany
  a skos:Concept ;
  dcterms:contributor "KOdea" ;
  dcterms:created "2016-07-06T05:04:15+00:00"^^xsd:dateTime ;
  dcterms:creator "superadmin" ;
  dcterms:modified "2016-09-12T06:22:00+00:00"^^xsd:dateTime ;
  skos:altLabel "Botanical research"@en ;
  skos:broader agift:Biological-sciences ;
  skos:definition "Conducting research into the structure, classification and distribution of plants. Developing taxonomic and geographic representations of botanical collections. Investigating potential uses for plant products in medicine or industry. Providing plant identification and botanical information services."@en ;
  skos:prefLabel "Botany"@en ;
  skos:related agift:Agricultural-sciences ;
.
agift:Broadcasting
  a skos:Concept ;
  dcterms:contributor "KOdea" ;
  dcterms:created "2016-07-06T02:53:28+00:00"^^xsd:dateTime ;
  dcterms:creator "superadmin" ;
  dcterms:modified "2016-09-09T07:14:59+00:00"^^xsd:dateTime ;
  skos:altLabel "Cable television services"@en ;
  skos:altLabel "Community broadcasting"@en ;
  skos:altLabel "Digital television services"@en ;
  skos:altLabel "Internet television services"@en ;
  skos:altLabel "Mass media services"@en ;
  skos:altLabel "Multicultural broadcasting"@en ;
  skos:altLabel "National broadcasters"@en ;
  skos:altLabel "Pay television services"@en ;
  skos:altLabel "Satellite television services"@en ;
  skos:broader agift:COMMUNICATIONS ;
  skos:definition "Developing policy to support and regulate industries that transmit content simultaneously to many recipients. Providing advice on the introduction of new technology and the effects of government communications policy on the broadcasting industry. Encouraging the use of mass marketing and content distribution strategies. Supporting the editorial and programming independence of national broadcasters. Includes liaison with arts and cultural sectors."@en ;
  skos:narrower agift:Broadcasting-standards ;
  skos:narrower agift:Radio-broadcasting ;
  skos:narrower agift:Television-broadcasting ;
  skos:prefLabel "Broadcasting"@en ;
.
agift:Broadcasting-standards
  a skos:Concept ;
  dcterms:contributor "KOdea" ;
  dcterms:created "2016-07-06T03:56:27+00:00"^^xsd:dateTime ;
  dcterms:creator "superadmin" ;
  dcterms:modified "2016-09-09T07:13:30+00:00"^^xsd:dateTime ;
  skos:altLabel "Australian broadcast standards"@en ;
  skos:altLabel "Broadband standards"@en ;
  skos:altLabel "Children's television standards"@en ;
  skos:altLabel "Film classification"@en ;
  skos:altLabel "Local content standards"@en ;
  skos:altLabel "Online content standards"@en ;
  skos:altLabel "Video classification"@en ;
  skos:broader agift:Broadcasting ;
  skos:definition "Establishing principles and criteria for the operation of industries that transmit content simultaneously to many recipients. Monitoring industry compliance with government standards and guidelines for all broadcasting media. Includes local content quotas, children's programming, codes of practice and the protection of special events."@en ;
  skos:prefLabel "Broadcasting standards"@en ;
  skos:related agift:Advertising-standards ;
  skos:related agift:Censorship-standards ;
  skos:related agift:Media-ownership-regulation ;
  skos:related agift:Radio-broadcasting ;
  skos:related agift:Television-broadcasting ;
.
agift:Building-acoustics
  a skos:Concept ;
  dcterms:contributor "KOdea" ;
  dcterms:created "2016-07-06T04:23:41+00:00"^^xsd:dateTime ;
  dcterms:creator "superadmin" ;
  dcterms:modified "2016-08-22T05:05:50+00:00"^^xsd:dateTime ;
  skos:altLabel "Structural integrity assessment"@en ;
  skos:broader agift:Built-environment ;
  skos:definition "Administering programs to assess the integrity of built structures. Conducting inspections to evaluate the safety of old buildings, transport infrastructure, dams and other elements of the built environment. Monitoring compliance with maintenance standards."@en ;
  skos:prefLabel "Building acoustics"@en ;
.
agift:Building-approval-services
  a skos:Concept ;
  dcterms:contributor "KOdea" ;
  dcterms:created "2016-07-06T03:53:12+00:00"^^xsd:dateTime ;
  dcterms:creator "superadmin" ;
  dcterms:modified "2016-09-05T06:48:30+00:00"^^xsd:dateTime ;
  skos:altLabel "Building alterations"@en ;
  skos:altLabel "Building applications"@en ;
  skos:altLabel "Construction approval services"@en ;
  skos:altLabel "Demolition approval services"@en ;
  skos:altLabel "Housing approval services"@en ;
  skos:broader agift:Civic-management ;
  skos:definition "Assessing applications for the building of new structures and the alteration or demolition of existing structures. Approving applications that meet town planning and building regulations. Providing advice on applications that cannot be supported.  Includes liaison across jurisdictions where joint approval is required."@en ;
  skos:prefLabel "Building approval services"@en ;
  skos:related agift:Land-use-zoning ;
  skos:related agift:Town-planning ;
.
agift:Building-preservation
  a skos:Concept ;
  dcterms:contributor "KOdea" ;
  dcterms:created "2016-07-06T04:32:34+00:00"^^xsd:dateTime ;
  dcterms:creator "superadmin" ;
  dcterms:modified "2016-09-05T06:45:27+00:00"^^xsd:dateTime ;
  skos:altLabel "Building conservation"@en ;
  skos:altLabel "Heritage building preservation"@en ;
  skos:broader agift:Built-environment ;
  skos:definition "Administering programs to maintain and protect built structures of particular historic, scientific or social significance. Issuing orders to prevent demolition, alteration or damage. Monitoring compliance with building preservation standards. Conducting inspections to ensure building modifications do not diminish heritage value."@en ;
  skos:prefLabel "Building preservation"@en ;
  skos:related agift:Architectural-services ;
.
agift:Building-regulations-and-standards
  a skos:Concept ;
  dcterms:contributor "KOdea" ;
  dcterms:created "2016-07-06T03:53:23+00:00"^^xsd:dateTime ;
  dcterms:creator "superadmin" ;
  dcterms:modified "2016-09-05T07:02:01+00:00"^^xsd:dateTime ;
  skos:altLabel "Building standards"@en ;
  skos:altLabel "Building surveyors"@en ;
  skos:broader agift:Civic-management ;
  skos:definition "Setting rules and guidelines for building new structures and altering or demolishing existing structures. Conducting assessments and inspections to ensure compliance with regulations and standards. Providing information and advice on building regulations and standards."@en ;
  skos:prefLabel "Building regulations and standards"@en ;
  skos:related agift:Architectural-services ;
  skos:related agift:Community-housing ;
  skos:related agift:Engineering-services ;
.
agift:Built-environment
  a skos:Concept ;
  dcterms:contributor "KOdea" ;
  dcterms:created "2016-07-06T03:02:25+00:00"^^xsd:dateTime ;
  dcterms:creator "superadmin" ;
  dcterms:modified "2016-09-08T07:38:09+00:00"^^xsd:dateTime ;
  skos:altLabel "National Estate preservation"@en ;
  skos:broader agift:ENVIRONMENT ;
  skos:definition "Developing policy and programs to protect structures of particular historic, scientific or social significance. Establishing standards for maintaining and preserving elements of the built environment. Providing funding for joint projects with business or the community."@en ;
  skos:narrower agift:Building-acoustics ;
  skos:narrower agift:Building-preservation ;
  skos:prefLabel "Built environment"@en ;
  skos:related agift:Conservation-programs ;
  skos:related agift:Historic-relic-protection ;
  skos:related agift:Indigenous-heritage-conservation ;
  skos:related agift:Natural-heritage-protection ;
.
agift:Burial-ground-management
  a skos:Concept ;
  dcterms:contributor "KOdea" ;
  dcterms:created "2016-07-06T03:55:02+00:00"^^xsd:dateTime ;
  dcterms:creator "superadmin" ;
  dcterms:modified "2016-09-05T07:05:02+00:00"^^xsd:dateTime ;
  skos:altLabel "Cemeteries"@en ;
  skos:altLabel "Cemetery management"@en ;
  skos:altLabel "Crematorium management"@en ;
  skos:altLabel "Graveyard management"@en ;
  skos:altLabel "War graves management"@en ;
  skos:broader agift:Public-land-management ;
  skos:definition "Administering areas of land set aside for depositing the bodies or ashes of the dead. Managing site layout. Ensuring facilities are kept clean and maintained. Monitoring rights of access and opening hours. Liaising with funeral directors, church and community groups. Includes war graves and overseas burial grounds managed by the Australian Government."@en ;
  skos:prefLabel "Burial ground management"@en ;
  skos:related agift:Memorial-maintenance ;
.
agift:Business-association
  a skos:Concept ;
  dcterms:contributor "KOdea" ;
  dcterms:created "2016-07-06T02:49:01+00:00"^^xsd:dateTime ;
  dcterms:creator "superadmin" ;
  dcterms:modified "2016-09-13T06:38:21+00:00"^^xsd:dateTime ;
  skos:altLabel "Association registration"@en ;
  skos:altLabel "Incorporation"@en ;
  skos:altLabel "Organisation registration"@en ;
  skos:broader agift:BUSINESS-SUPPORT-AND-REGULATION ;
  skos:definition "Recording the details of incorporated associations. Assessing applications and issuing registration numbers. Maintaining records of registered details. Processing registration updates and renewals."@en ;
  skos:prefLabel "Business association"@en ;
  skos:related agift:Associations-and-corporate-law ;
  skos:related agift:Business-registration-and-licensing ;
  skos:related agift:Fundraising-and-donation-schemes ;
  skos:related agift:Sport-and-fitness-development ;
.
agift:Business-process-auditing
  skos:prefLabel "Incorporation"@en ;
  owl:deprecated true ;
.
agift:Business-process-auditing
  a skos:Concept ;
  dcterms:contributor "KOdea" ;
  dcterms:created "2016-08-04T06:07:15+00:00"^^xsd:dateTime ;
  dcterms:creator "KOdea" ;
  dcterms:modified "2016-09-09T06:00:24+00:00"^^xsd:dateTime ;
  skos:altLabel "Auditing"@en ;
  skos:broader agift:BUSINESS-SUPPORT-AND-REGULATION ;
  skos:definition "Administering programs to examine the accounts and records of government or private sector bodies. Reviewing the performance or financial management of an organisation. Verifying statements or claims made in official reports. Providing recommendations for improvement."@en ;
  skos:prefLabel "Business process auditing"@en ;
  skos:related agift:Government-auditing ;
  skos:related agift:Recordkeeping-standards ;
.
agift:Business-registration-and-licensing
  a skos:Concept ;
  dcterms:contributor "KOdea" ;
  dcterms:created "2016-07-06T02:49:23+00:00"^^xsd:dateTime ;
  dcterms:creator "superadmin" ;
  dcterms:modified "2016-09-13T06:38:50+00:00"^^xsd:dateTime ;
  skos:altLabel "Australian Business Number"@en ;
  skos:altLabel "Australian Business Register"@en ;
  skos:altLabel "Australian Company Number"@en ;
  skos:altLabel "Australian Registered Body Number"@en ;
  skos:altLabel "Business licensing"@en ;
  skos:altLabel "Business names"@en ;
  skos:altLabel "Business permits and licences"@en ;
  skos:altLabel "Business registration number"@en ;
  skos:altLabel "Fundraising permits"@en ;
  skos:altLabel "GST registration"@en ;
  skos:altLabel "Liquor licensing"@en ;
  skos:altLabel "PAYG registration"@en ;
  skos:broader agift:BUSINESS-SUPPORT-AND-REGULATION ;
  skos:definition "Recording the details of companies and corporations. Assessing applications and issuing registration numbers. Maintaining records of registered details. Processing registration updates and renewals. Issuing licenses and permits, such as those required for fundraising, the sale of alcohol or signage and displays."@en ;
  skos:prefLabel "Business registration and licensing"@en ;
  skos:related agift:Associations-and-corporate-law ;
  skos:related agift:Business-association ;
  skos:related agift:Fundraising-and-donation-schemes ;
  skos:related agift:Gaming-industry-regulation ;
  skos:related agift:Income-assessment ;
.
agift:Business-sponsorship
  a skos:Concept ;
  dcterms:contributor "KOdea" ;
  dcterms:created "2016-07-06T02:49:33+00:00"^^xsd:dateTime ;
  dcterms:creator "superadmin" ;
  dcterms:modified "2016-09-13T06:39:03+00:00"^^xsd:dateTime ;
  skos:altLabel "Business sponsors"@en ;
  skos:altLabel "Corporate sponsors"@en ;
  skos:altLabel "Corporate sponsorship"@en ;
  skos:altLabel "Sponsorship"@en ;
  skos:altLabel "Sports advertising"@en ;
  skos:broader agift:BUSINESS-SUPPORT-AND-REGULATION ;
  skos:definition "Regulating corporate funding of organisations and events. Restricting the advertising of some types of products or services at events. Providing information about sponsorship applications and how to meet obligations in relation to marketing and merchandising."@en ;
  skos:prefLabel "Business sponsorship"@en ;
  skos:related agift:Advertising-standards ;
  skos:related agift:Fair-trading-compliance ;
  skos:related agift:Fundraising-and-donation-schemes ;
.
agift:CIVIC-INFRASTRUCTURE
  a skos:Concept ;
  dcterms:contributor "KOdea" ;
  dcterms:created "2016-07-06T02:44:12+00:00"^^xsd:dateTime ;
  dcterms:creator "superadmin" ;
  dcterms:modified "2016-09-12T06:44:11+00:00"^^xsd:dateTime ;
  skos:altLabel "Bridges"@en ;
  skos:altLabel "Buildings"@en ;
  skos:altLabel "Dams"@en ;
  skos:altLabel "Public works"@en ;
  skos:definition "Developing policy to support the growth of towns and cities. Implementing programs to manage urban development and maintain essential services. Installing buildings and services to meet the administrative, social and recreational needs of local residents."@en ;
  skos:narrower agift:Civic-management ;
  skos:narrower agift:Energy-supply ;
  skos:narrower agift:Housing-industry-policy ;
  skos:narrower agift:Infrastructure-planning ;
  skos:narrower agift:Integrated-services-planning ;
  skos:narrower agift:Place-names ;
  skos:narrower agift:Public-housing ;
  skos:narrower agift:Public-land-management ;
  skos:narrower agift:Regional-development ;
  skos:narrower agift:Transport-network-maintenance ;
  skos:narrower agift:Waste-management ;
  skos:prefLabel "CIVIC INFRASTRUCTURE"@en ;
  skos:related agift:Crown-land-administration ;
  skos:related agift:Mobile-telephone-services ;
  skos:related agift:Spatial-information-research ;
  skos:topConceptOf agift:AGIFT ;
.
agift:COMMUNICATIONS
  a skos:Concept ;
  dcterms:contributor "KOdea" ;
  dcterms:created "2016-07-06T02:44:29+00:00"^^xsd:dateTime ;
  dcterms:creator "superadmin" ;
  dcterms:modified "2016-09-12T06:45:12+00:00"^^xsd:dateTime ;
  skos:definition "Supporting the growth and management of industries that facilitate the transmission of information. Regulating the provision of postal and telecommunication services to all citizens. Encouraging the development of standards for information management, information dissemination and information technology."@en ;
  skos:narrower agift:Advertising-standards ;
  skos:narrower agift:Broadcasting ;
  skos:narrower agift:Call-centre-administration ;
  skos:narrower agift:Electronic-commerce ;
  skos:narrower agift:Government-media ;
  skos:narrower agift:Information-management-standards ;
  skos:narrower agift:Internet ;
  skos:narrower agift:Media-ownership-regulation ;
  skos:narrower agift:Postal-services ;
  skos:narrower agift:Publishing ;
  skos:narrower agift:Radio-communication ;
  skos:narrower agift:Satellite-communication ;
  skos:narrower agift:Telecommunications ;
  skos:prefLabel "COMMUNICATIONS"@en ;
  skos:related agift:Navigation-systems-development ;
  skos:related agift:Search-technology-development ;
  skos:related agift:Spatial-information-research ;
  skos:topConceptOf agift:AGIFT ;
.
agift:COMMUNITY-SERVICES
  a skos:Concept ;
  dcterms:contributor "KOdea" ;
  dcterms:created "2016-07-06T02:44:41+00:00"^^xsd:dateTime ;
  dcterms:creator "superadmin" ;
  dcterms:modified "2016-08-08T06:37:52+00:00"^^xsd:dateTime ;
  skos:altLabel "Welfare"@en ;
  skos:definition "Developing policy to assist citizens in a particular district or those with common interests and needs. Providing welfare services and financial support. Administering disaster and emergency assistance programs."@en ;
  skos:narrower agift:Accommodation-services ;
  skos:narrower agift:Community-engagement ;
  skos:narrower agift:Community-support ;
  skos:narrower agift:Counselling-services ;
  skos:narrower agift:Emergency-services ;
  skos:narrower agift:Financial-assistance ;
  skos:narrower agift:Natural-disasters ;
  skos:narrower agift:Rural-community-development ;
  skos:narrower agift:Social-justice-and-equity ;
  skos:narrower agift:Social-research ;
  skos:narrower agift:Transport-access-schemes ;
  skos:prefLabel "COMMUNITY SERVICES"@en ;
  skos:topConceptOf agift:AGIFT ;
.
agift:CULTURAL-AFFAIRS
  a skos:Concept ;
  dcterms:contributor "KOdea" ;
  dcterms:created "2016-09-08T01:21:39+00:00"^^xsd:dateTime ;
  dcterms:creator "fionamcl" ;
  dcterms:modified "2016-09-09T07:47:02+00:00"^^xsd:dateTime ;
  skos:altLabel "Archives"@en ;
  skos:altLabel "Art galleries"@en ;
  skos:altLabel "Cultural institutions"@en ;
  skos:altLabel "Culture"@en ;
  skos:altLabel "Galleries"@en ;
  skos:altLabel "Libraries"@en ;
  skos:altLabel "Museums"@en ;
  skos:altLabel "Theatres"@en ;
  skos:definition "Developing policy to support the arts and cultural organisations such as museums, libraries and galleries. Establishing programs to develop and manage cultural collections and artefacts, and to stimulate growth in cultural industries. Sponsoring activities and events to celebrate the diversity of Australian culture."@en ;
  skos:narrower agift:Arts-development ;
  skos:narrower agift:Collection-access ;
  skos:narrower agift:Collection-management ;
  skos:narrower agift:Collection-promotion ;
  skos:narrower agift:Cultural-awards-and-scholarships ;
  skos:narrower agift:Cultural-festivals ;
  skos:narrower agift:Cultural-gifts-programs ;
  skos:narrower agift:Multicultural-heritage-promotion ;
  skos:prefLabel "CULTURAL AFFAIRS"@en ;
  skos:related agift:Cultural-centre-management ;
  skos:related agift:IMMIGRATION ;
  skos:topConceptOf agift:AGIFT ;
.
agift:Cadets
  a skos:Concept ;
  dcterms:contributor "KOdea" ;
  dcterms:created "2016-07-06T04:08:33+00:00"^^xsd:dateTime ;
  dcterms:creator "superadmin" ;
  dcterms:modified "2016-09-08T06:31:30+00:00"^^xsd:dateTime ;
  skos:altLabel "Cadet training"@en ;
  skos:altLabel "Military cadets"@en ;
  skos:broader agift:Australian-Defence-Forces ;
  skos:definition "Managing the Australian Defence Force Cadets and similar programs to recruit and develop young service personnel. Developing, sponsoring and promoting Cadet activity programs and recruitment procedures. Includes Officers and Instructors of Cadets, Australian Navy Cadets, Australian Army Cadets and Australian Air Force Cadets."@en ;
  skos:prefLabel "Cadets"@en ;
  skos:related agift:Military-education-and-training ;
.
agift:Call-centre-administration
  a skos:Concept ;
  dcterms:contributor "KOdea" ;
  dcterms:created "2016-07-06T02:53:35+00:00"^^xsd:dateTime ;
  dcterms:creator "superadmin" ;
  dcterms:modified "2016-08-05T05:09:34+00:00"^^xsd:dateTime ;
  skos:altLabel "Advice lines"@en ;
  skos:altLabel "Telephone assistance services"@en ;
  skos:broader agift:COMMUNICATIONS ;
  skos:definition "Managing facilities where trained staff are available to answer questions or provide advice via the telephone. Promoting the use of call centres to facilitate public access to government information."@en ;
  skos:prefLabel "Call centre administration"@en ;
.
agift:Capital-equipment-programs
  a skos:Concept ;
  dcterms:contributor "KOdea" ;
  dcterms:created "2016-07-06T04:10:54+00:00"^^xsd:dateTime ;
  dcterms:creator "superadmin" ;
  dcterms:modified "2016-09-08T06:45:03+00:00"^^xsd:dateTime ;
  skos:altLabel "Capital equipment acquisition"@en ;
  skos:altLabel "Defence equipment"@en ;
  skos:altLabel "Military equipment"@en ;
  skos:broader agift:Defence-strategic-support ;
  skos:definition "Administering projects to purchase or build the physical resources to support Australia's defence forces and military operations. Cataloguing major equipment and scheduling refurbishment or disposal. Includes, but is not limited to, the management of weaponry, vehicles, aircraft, seagoing vessels, communications and surveillance equipment."@en ;
  skos:prefLabel "Capital equipment programs"@en ;
  skos:related agift:Defence-industry ;
.
agift:Caravan-and-camping-services
  a skos:Concept ;
  dcterms:contributor "KOdea" ;
  dcterms:created "2016-07-06T03:45:20+00:00"^^xsd:dateTime ;
  dcterms:creator "superadmin" ;
  dcterms:modified "2016-09-13T06:26:46+00:00"^^xsd:dateTime ;
  skos:altLabel "Camping grounds"@en ;
  skos:altLabel "Campsites"@en ;
  skos:altLabel "Caravan parks"@en ;
  skos:broader agift:SPORT-AND-RECREATION ;
  skos:definition "Regulating the provision of sites where caravans, tents and other temporary dwellings may be erected. Certifying the safety of campsite facilities and the hygiene of amenities. Providing advice to operators on administration, emergency procedures and insurance. Includes public information services, such as the production of maps and promotional literature."@en ;
  skos:prefLabel "Caravan and camping services"@en ;
  skos:related agift:Tourism-industry-development ;
.
agift:Cargo-control
  a skos:Concept ;
  dcterms:contributor "KOdea" ;
  dcterms:created "2016-07-06T03:39:08+00:00"^^xsd:dateTime ;
  dcterms:creator "superadmin" ;
  dcterms:modified "2016-09-13T07:12:59+00:00"^^xsd:dateTime ;
  skos:altLabel "Hazardous materials management"@en ;
  skos:altLabel "Hazardous waste management"@en ;
  skos:altLabel "Stevedores"@en ;
  skos:altLabel "Stevedoring"@en ;
  skos:broader agift:MARITIME-SERVICES ;
  skos:definition "Developing policy for the transportation of goods by sea. Monitoring compliance with regulations and international standards for carriage of hazardous materials, dangerous goods and oversize containers. Includes advice on best practice cargo handling, loading and management."@en ;
  skos:prefLabel "Cargo control"@en ;
  skos:related agift:Export-regulation ;
  skos:related agift:Freight-movement-regulation ;
  skos:related agift:Import-regulation ;
  skos:related agift:Occupational-health-and-safety ;
  skos:related agift:Port-regulation ;
.
agift:Carriage-service-providers
  a skos:Concept ;
  dcterms:contributor "KOdea" ;
  dcterms:created "2016-07-06T04:00:20+00:00"^^xsd:dateTime ;
  dcterms:creator "superadmin" ;
  dcterms:modified "2016-08-05T05:56:57+00:00"^^xsd:dateTime ;
  skos:altLabel "Telecommunications carriers"@en ;
  skos:broader agift:Telecommunications ;
  skos:definition "Monitoring the activities of suppliers of telecommunications services. Regulating the construction of facilities, installation and maintenance of equipment such as cables and optical fibre. Ensuring compliance with pricing guidelines and standards of service."@en ;
  skos:prefLabel "Carriage service providers"@en ;
.
agift:Carrier-licensing
  a skos:Concept ;
  dcterms:contributor "KOdea" ;
  dcterms:created "2016-07-06T04:00:31+00:00"^^xsd:dateTime ;
  dcterms:creator "superadmin" ;
  dcterms:modified "2016-08-05T05:58:01+00:00"^^xsd:dateTime ;
  skos:altLabel "Telecommunications licensing"@en ;
  skos:broader agift:Telecommunications ;
  skos:definition "Processing applications and issuing licenses to suppliers of telecommunications services. Drafting licence conditions. Monitoring compliance with legislative obligations and reporting requirements."@en ;
  skos:prefLabel "Carrier licensing"@en ;
.
agift:Censorship-standards
  a skos:Concept ;
  dcterms:contributor "KOdea" ;
  dcterms:created "2016-07-06T04:54:41+00:00"^^xsd:dateTime ;
  dcterms:creator "superadmin" ;
  dcterms:modified "2016-09-09T07:14:59+00:00"^^xsd:dateTime ;
  skos:altLabel "Film classification"@en ;
  skos:altLabel "Radio censorship"@en ;
  skos:altLabel "Television censorship"@en ;
  skos:altLabel "Video classification"@en ;
  skos:broader agift:Administrative-law ;
  skos:definition "Regulating the accessibility of various kinds of content for television, literature, film, radio or theatre. Establishing criteria to classify content and determine its availability to the public."@en ;
  skos:prefLabel "Censorship standards"@en ;
  skos:related agift:Advertising-standards ;
  skos:related agift:Broadcasting-standards ;
  skos:related agift:Publishing-standards ;
.
agift:Ceremonial-events-and-representation
  a skos:Concept ;
  dcterms:contributor "KOdea" ;
  dcterms:created "2016-07-06T04:42:07+00:00"^^xsd:dateTime ;
  dcterms:creator "superadmin" ;
  dcterms:modified "2016-09-09T05:54:07+00:00"^^xsd:dateTime ;
  skos:altLabel "Official representation"@en ;
  skos:broader agift:Official-protocol ;
  skos:definition "Organising the attendance of high-level government officials at formal public occasions, either in Australia or overseas. Providing advice on conduct during ritual or traditional proceedings. Making arrangements to support official protocol such as determining guest lists, producing formal invitations, providing acceptances or apologies."@en ;
  skos:prefLabel "Ceremonial events and representation"@en ;
  skos:related agift:Head-of-Government-protocol ;
  skos:related agift:Official-hospitality ;
  skos:related agift:Official-visits ;
.
agift:Certified-employment-conditions
  a skos:Concept ;
  dcterms:contributor "KOdea" ;
  dcterms:created "2016-07-06T04:22:58+00:00"^^xsd:dateTime ;
  dcterms:creator "superadmin" ;
  dcterms:modified "2016-09-08T07:35:26+00:00"^^xsd:dateTime ;
  skos:altLabel "Certified agreement disputes"@en ;
  skos:altLabel "Workplace agreement disputes"@en ;
  skos:broader agift:Workplace-agreement-processes ;
  skos:definition "Implementing the provisions of workplace agreements with regard to working conditions, rates of pay and performance management. Providing advice on hours of work, employment conditions, leave and other entitlements. Administering the payment of wages, allowances, overtime and penalties."@en ;
  skos:prefLabel "Certified employment conditions"@en ;
  skos:related agift:Award-conditions ;
  skos:related agift:Occupational-health-and-safety ;
.
agift:Charting-sea-lanes
  a skos:Concept ;
  dcterms:contributor "KOdea" ;
  dcterms:created "2016-07-06T04:58:00+00:00"^^xsd:dateTime ;
  dcterms:creator "superadmin" ;
  dcterms:modified "2016-09-09T07:32:20+00:00"^^xsd:dateTime ;
  skos:altLabel "Sea lane mapping"@en ;
  skos:altLabel "Shipping channel mapping"@en ;
  skos:broader agift:Navigation ;
  skos:definition "Administering programs to map the location of shipping channels and established routes for watercraft. Developing graphic representations to record special conditions or geographical features."@en ;
  skos:prefLabel "Charting sea lanes"@en ;
  skos:related agift:Port-regulation ;
  skos:related agift:Spatial-information-research ;
.
agift:Chemical-and-pesticide-regulation
  a skos:Concept ;
  dcterms:contributor "KOdea" ;
  dcterms:created "2016-07-06T03:41:43+00:00"^^xsd:dateTime ;
  dcterms:creator "superadmin" ;
  dcterms:modified "2016-09-12T06:32:01+00:00"^^xsd:dateTime ;
  skos:altLabel "Herbicide regulation"@en ;
  skos:altLabel "Insecticide regulation"@en ;
  skos:altLabel "Maximum residue limits"@en ;
  skos:altLabel "Pesticide regulation"@en ;
  skos:altLabel "Veterinary chemical regulation"@en ;
  skos:broader agift:PRIMARY-INDUSTRIES ;
  skos:definition "Monitoring the use of substances to control weeds, insects and other pests that affect primary production. Maintaining a register of approved agricultural or veterinary chemicals and pesticides. Assessing product applications, specifying conditions of use and maximum residue limits. Conducting routine inspections to ensure compliance."@en ;
  skos:prefLabel "Chemical and pesticide regulation"@en ;
  skos:related agift:Agricultural-sciences ;
  skos:related agift:Animal-and-veterinary-sciences ;
  skos:related agift:Drugs-and-poisons-regulation ;
  skos:related agift:Entomology ;
  skos:related agift:Food-quality-assurance ;
  skos:related agift:Soil-preservation-programs ;
  skos:related agift:Warfare ;
.
agift:Child-and-youth-support
  a skos:Concept ;
  dcterms:contributor "KOdea" ;
  dcterms:created "2016-07-06T04:02:22+00:00"^^xsd:dateTime ;
  dcterms:creator "superadmin" ;
  dcterms:modified "2016-09-09T07:23:40+00:00"^^xsd:dateTime ;
  skos:altLabel "Child protection services"@en ;
  skos:altLabel "Child welfare"@en ;
  skos:altLabel "Children's services"@en ;
  skos:altLabel "Parental education programs"@en ;
  skos:altLabel "Youth support services"@en ;
  skos:broader agift:Community-support ;
  skos:definition "Providing and monitoring services for young people. Assisting those who are disadvantaged or at risk of abuse or domestic violence. Running parent education programs and managing youth centres. Includes funding and support for community-based or volunteer programs providing child and youth support."@en ;
  skos:prefLabel "Child and youth support"@en ;
  skos:related agift:Adult-education-programs ;
  skos:related agift:Child-care-services ;
  skos:related agift:Discipline-programs ;
  skos:related agift:Early-childhood-education ;
  skos:related agift:Health-promotion ;
  skos:related agift:Juvenile-justice ;
  skos:related agift:Taxation-compliance ;
.
agift:Child-care-services
  a skos:Concept ;
  dcterms:contributor "KOdea" ;
  dcterms:created "2016-07-06T04:02:29+00:00"^^xsd:dateTime ;
  dcterms:creator "superadmin" ;
  dcterms:modified "2016-09-06T07:20:16+00:00"^^xsd:dateTime ;
  skos:altLabel "Babysitting services"@en ;
  skos:altLabel "Child minding services"@en ;
  skos:altLabel "Child-care centres"@en ;
  skos:altLabel "Day care services"@en ;
  skos:altLabel "Nursery schools"@en ;
  skos:altLabel "Playgroup services"@en ;
  skos:broader agift:Community-support ;
  skos:definition "Providing services for the supervision of children when their parents are not available. Monitoring private sector staff and facilities for compliance with industry standards. Includes temporary arrangements for emergency or foster care."@en ;
  skos:prefLabel "Child-care services"@en ;
  skos:related agift:Adoption-services ;
  skos:related agift:Child-and-youth-support ;
  skos:related agift:Early-childhood-education ;
  skos:related agift:Financial-assistance ;
  skos:related agift:Taxation-compliance ;
.
agift:Citizenship
  a skos:Concept ;
  dcterms:contributor "KOdea" ;
  dcterms:created "2016-07-06T03:33:41+00:00"^^xsd:dateTime ;
  dcterms:creator "superadmin" ;
  dcterms:modified "2016-09-09T06:30:08+00:00"^^xsd:dateTime ;
  skos:altLabel "Dual citizenship"@en ;
  skos:altLabel "Nationality"@en ;
  skos:altLabel "Naturalisation policy"@en ;
  skos:broader agift:IMMIGRATION ;
  skos:definition "Developing policy for Australian nationality, including the rights and obligations of citizens. Defining the legal status of Australian citizens, and the management of citizenship when people migrate. Establishing criteria for the naturalisation of immigrants. Promoting the value of Australian citizenship."@en ;
  skos:narrower agift:Naturalisation-assessment ;
  skos:narrower agift:Presentation-arrangements ;
  skos:prefLabel "Citizenship"@en ;
  skos:related agift:Travel-authorisation ;
.
agift:Civic-celebrations
  a skos:Concept ;
  dcterms:contributor "KOdea" ;
  dcterms:created "2016-07-06T03:05:34+00:00"^^xsd:dateTime ;
  dcterms:creator "superadmin" ;
  dcterms:modified "2016-09-09T05:40:34+00:00"^^xsd:dateTime ;
  skos:altLabel "ANZAC Day services"@en ;
  skos:altLabel "Australia Day celebrations"@en ;
  skos:altLabel "Celebrations"@en ;
  skos:altLabel "Centenary of Federation"@en ;
  skos:altLabel "Commemorative services"@en ;
  skos:altLabel "Federation celebrations"@en ;
  skos:altLabel "Queen's birthday celebrations"@en ;
  skos:broader agift:GOVERNANCE ;
  skos:definition "Organising community events and ceremonies to mark significant occasions. Coordinating security, publicity and entertainment. Arranging adequate public facilities, car parking and seating. Includes liaison with local businesses, volunteers and community groups."@en ;
  skos:prefLabel "Civic celebrations"@en ;
  skos:related agift:Cultural-festivals ;
  skos:related agift:Multicultural-festivals ;
  skos:related agift:Presentation-arrangements ;
.
agift:Civic-management
  a skos:Concept ;
  dcterms:contributor "KOdea" ;
  dcterms:created "2016-07-06T02:51:20+00:00"^^xsd:dateTime ;
  dcterms:creator "superadmin" ;
  dcterms:modified "2016-08-05T01:43:07+00:00"^^xsd:dateTime ;
  skos:altLabel "Urban development"@en ;
  skos:broader agift:CIVIC-INFRASTRUCTURE ;
  skos:definition "Developing programs to provide integrated support for town planning and building projects. Coordinating government building projects and managing input from multiple parties. Defining responsibilities for projects that cross jurisdictional boundaries."@en ;
  skos:narrower agift:Architectural-services ;
  skos:narrower agift:Building-approval-services ;
  skos:narrower agift:Building-regulations-and-standards ;
  skos:narrower agift:Engineering-services ;
  skos:narrower agift:Town-planning ;
  skos:prefLabel "Civic management"@en ;
.
agift:Civil-community-assistance
  a skos:Concept ;
  dcterms:contributor "KOdea" ;
  dcterms:created "2016-07-06T04:11:29+00:00"^^xsd:dateTime ;
  dcterms:creator "superadmin" ;
  dcterms:modified "2016-09-09T07:38:03+00:00"^^xsd:dateTime ;
  skos:altLabel "Civil defence"@en ;
  skos:altLabel "Civil disaster support"@en ;
  skos:altLabel "Community disaster support"@en ;
  skos:altLabel "Defence forces assistance"@en ;
  skos:altLabel "Military assistance"@en ;
  skos:broader agift:Emergency-management ;
  skos:definition "Managing the allocation of defence resources to protect the civilian population from the effects of hostilities or emergencies. Providing support to civil emergency services in times of natural disaster. Includes identifying lines of communication, chain of command, and establishing criteria for situations warranting defence forces assistance."@en ;
  skos:prefLabel "Civil community assistance"@en ;
  skos:related agift:Disaster-recovery ;
  skos:related agift:Disaster-support ;
  skos:related agift:Natural-disasters ;
  skos:related agift:Search-and-rescue ;
.
agift:Civil-law
  a skos:Concept ;
  dcterms:contributor "superadmin" ;
  dcterms:created "2016-07-06T03:37:12+00:00"^^xsd:dateTime ;
  dcterms:creator "superadmin" ;
  dcterms:modified "2016-07-06T06:52:05+00:00"^^xsd:dateTime ;
  skos:broader agift:JUSTICE-ADMINISTRATION ;
  skos:definition "Administering the body of law that relates to social behaviour and the ordinary private matters of individuals. Establishing property rights, determining legal relationships and responsibilities."@en ;
  skos:narrower agift:Civil-registration ;
  skos:narrower agift:Conveyancing ;
  skos:narrower agift:Dispute-mediation-programs ;
  skos:narrower agift:Family-law-proceedings ;
  skos:narrower agift:Probate-applications ;
  skos:prefLabel "Civil law"@en ;
.
agift:Civil-registration
  a skos:Concept ;
  dcterms:contributor "KOdea" ;
  dcterms:created "2016-07-06T04:55:57+00:00"^^xsd:dateTime ;
  dcterms:creator "superadmin" ;
  dcterms:modified "2016-08-29T06:14:21+00:00"^^xsd:dateTime ;
  skos:altLabel "Birth certificates"@en ;
  skos:altLabel "Death certificates"@en ;
  skos:altLabel "Marriage certificates"@en ;
  skos:altLabel "Registrar"@en ;
  skos:broader agift:Civil-law ;
  skos:definition "Administering the registration of major life events, such as births, marriages and deaths. Issuing certificates and keeping records to support other civil law processes."@en ;
  skos:prefLabel "Civil registration"@en ;
.
agift:Climate-information-services
  a skos:Concept ;
  dcterms:contributor "KOdea" ;
  dcterms:created "2016-07-06T03:02:33+00:00"^^xsd:dateTime ;
  dcterms:creator "superadmin" ;
  dcterms:modified "2016-09-08T07:37:43+00:00"^^xsd:dateTime ;
  skos:altLabel "Weather forecasting"@en ;
  skos:broader agift:ENVIRONMENT ;
  skos:definition "Providing climatic advice, information on prevailing conditions and weather forecasts. Issuing alerts for severe weather. Includes drought monitoring and updates on seasonal climate variability."@en ;
  skos:prefLabel "Climate information services"@en ;
  skos:related agift:Atmospheric-sciences ;
  skos:related agift:Natural-disasters ;
.
agift:Clinical-health-services
  a skos:Concept ;
  dcterms:contributor "KOdea" ;
  dcterms:created "2016-07-06T04:44:56+00:00"^^xsd:dateTime ;
  dcterms:creator "superadmin" ;
  dcterms:modified "2016-09-09T06:22:08+00:00"^^xsd:dateTime ;
  skos:altLabel "Family medical centres"@en ;
  skos:altLabel "General practitioners"@en ;
  skos:altLabel "Health clinics"@en ;
  skos:altLabel "Medical centres"@en ;
  skos:altLabel "Travel health clinics"@en ;
  skos:broader agift:Community-health-services ;
  skos:definition "Administering health programs that operate out of medical centres. Providing consultation services to allow diagnosis and treatment based on direct observation of the patient. Developing treatment care plans for medication or rehabilitation, and issuing referrals to support services."@en ;
  skos:prefLabel "Clinical health services"@en ;
  skos:related agift:Counselling-services ;
  skos:related agift:Medical-quarantine-services ;
  skos:related agift:Primary-health-care ;
  skos:related agift:Special-needs-services ;
.
agift:Collection-access
  skos:prefLabel "Collection access"@en ;
  owl:deprecated true ;
.
agift:Collection-access
  a skos:Concept ;
  dcterms:contributor "fionamcl" ;
  dcterms:created "2016-09-08T01:22:05+00:00"^^xsd:dateTime ;
  dcterms:creator "fionamcl" ;
  dcterms:modified "2016-11-28T22:47:11+00:00"^^xsd:dateTime ;
  skos:broader agift:CULTURAL-AFFAIRS ;
  skos:definition "Developing policy to assist the location and use of items held by cultural institutions. Establishing access procedures to meet legislative requirements. Providing advice about opening hours and membership or registration requirements. Includes development of online information to support remote access."@en ;
  skos:narrower agift:Descriptive-standards ;
  skos:narrower agift:Finding-aids-development ;
  skos:narrower agift:Reference-services ;
  skos:prefLabel "Collection access"@en ;
  skos:related agift:Reference-services ;
.
agift:Collection-accessioning
  skos:prefLabel "Collection accessioning"@en ;
  owl:deprecated true ;
.
agift:Collection-accessioning
  a skos:Concept ;
  dcterms:contributor "fionamcl" ;
  dcterms:created "2016-09-08T01:34:13+00:00"^^xsd:dateTime ;
  dcterms:creator "fionamcl" ;
  dcterms:modified "2016-11-28T22:47:43+00:00"^^xsd:dateTime ;
  skos:altLabel "Accessioning"@en ;
  skos:altLabel "Collection listing"@en ;
  skos:altLabel "Index development"@en ;
  skos:broader agift:Collection-management ;
  skos:definition "Applying intellectual and physical control over items held by cultural institutions. Recording the essential details of materials as they are acquired. Includes accessioning (and de-accessioning) items for touring exhibitions and those on loan from other collections."@en ;
  skos:prefLabel "Collection accessioning"@en ;
  skos:related agift:Collection-acquisition ;
  skos:related agift:Descriptive-standards ;
  skos:related agift:Finding-aids-development ;
.
agift:Collection-acquisition
  skos:prefLabel "Collection acquisition"@en ;
  owl:deprecated true ;
.
agift:Collection-acquisition
  a skos:Concept ;
  dcterms:contributor "fionamcl" ;
  dcterms:created "2016-09-08T01:34:18+00:00"^^xsd:dateTime ;
  dcterms:creator "fionamcl" ;
  dcterms:modified "2016-11-28T22:47:48+00:00"^^xsd:dateTime ;
  skos:altLabel "Acquisitions"@en ;
  skos:altLabel "Art acquisitions"@en ;
  skos:altLabel "Cultural materials acquisition"@en ;
  skos:broader agift:Collection-management ;
  skos:definition "Seeking and receiving new materials for cultural institutions. Building a collection in accordance with policy and guidelines. Negotiating temporary use of items from other collections. Developing mechanisms to support a range of acquisition methods, such as purchases, donations, loans and joint investments."@en ;
  skos:prefLabel "Collection acquisition"@en ;
  skos:related agift:Collection-accessioning ;
  skos:related agift:Cultural-gifts-programs ;
  skos:related agift:Exhibition-programs ;
.
agift:Collection-management
  skos:prefLabel "Collection management"@en ;
  owl:deprecated true ;
.
agift:Collection-management
  a skos:Concept ;
  dcterms:contributor "fionamcl" ;
  dcterms:created "2016-09-08T01:22:10+00:00"^^xsd:dateTime ;
  dcterms:creator "fionamcl" ;
  dcterms:modified "2016-11-28T22:47:06+00:00"^^xsd:dateTime ;
  skos:altLabel "Archival holdings management"@en ;
  skos:altLabel "Collection development policy"@en ;
  skos:altLabel "Holdings management"@en ;
  skos:altLabel "Library collection management"@en ;
  skos:altLabel "Museum collection management"@en ;
  skos:broader agift:CULTURAL-AFFAIRS ;
  skos:definition "Developing policy for the acquisition, storage and preservation of cultural material and artefacts. Producing standards and guidelines for collection management procedures to ensure the safety of fragile or highly valuable items. Includes liaison with other institutions about the management of cultural materials."@en ;
  skos:narrower agift:Artefact-export-regulation ;
  skos:narrower agift:Collection-accessioning ;
  skos:narrower agift:Collection-acquisition ;
  skos:narrower agift:Collection-storage ;
  skos:narrower agift:Preservation-services ;
  skos:prefLabel "Collection management"@en ;
.
agift:Collection-promotion
  skos:prefLabel "Collection promotion"@en ;
  owl:deprecated true ;
.
agift:Collection-promotion
  a skos:Concept ;
  dcterms:contributor "fionamcl" ;
  dcterms:created "2016-09-08T01:22:31+00:00"^^xsd:dateTime ;
  dcterms:creator "fionamcl" ;
  dcterms:modified "2016-11-28T22:48:19+00:00"^^xsd:dateTime ;
  skos:altLabel "Cultural collection marketing"@en ;
  skos:broader agift:CULTURAL-AFFAIRS ;
  skos:definition "Developing strategies to raise the profiles of cultural institutions and their holdings. Coordinating programs of events and publications. Establishing policy and guidelines to support exhibitions and marketing campaigns."@en ;
  skos:narrower agift:Exhibition-programs ;
  skos:narrower agift:Publicity-programs ;
  skos:prefLabel "Collection promotion"@en ;
  skos:related agift:Arts-promotion ;
  skos:related agift:Publishing ;
.
agift:Collection-storage
  skos:prefLabel "Collection storage"@en ;
  owl:deprecated true ;
.
agift:Collection-storage
  a skos:Concept ;
  dcterms:contributor "fionamcl" ;
  dcterms:created "2016-09-08T01:34:22+00:00"^^xsd:dateTime ;
  dcterms:creator "fionamcl" ;
  dcterms:modified "2016-11-28T22:47:53+00:00"^^xsd:dateTime ;
  skos:altLabel "Records storage"@en ;
  skos:altLabel "Repository management"@en ;
  skos:altLabel "Stack management"@en ;
  skos:broader agift:Collection-management ;
  skos:definition "Designing and managing facilities to house materials held by cultural institutions. Ensuring environmental conditions meet appropriate industry standards. Arranging facilities to support access and preservation guidelines."@en ;
  skos:prefLabel "Collection storage"@en ;
  skos:related agift:Cultural-centre-management ;
  skos:related agift:Preservation-services ;
.
agift:Commissions-of-inquiry
  a skos:Concept ;
  dcterms:contributor "KOdea" ;
  dcterms:created "2016-07-06T03:37:18+00:00"^^xsd:dateTime ;
  dcterms:creator "superadmin" ;
  dcterms:modified "2016-08-29T06:21:40+00:00"^^xsd:dateTime ;
  skos:altLabel "Inquiries"@en ;
  skos:altLabel "Royal Commissions"@en ;
  skos:altLabel "Senate committees"@en ;
  skos:broader agift:JUSTICE-ADMINISTRATION ;
  skos:definition "Establishing a body to investigate a special matter or designated subject. Conducting inquiries, hearing evidence, receiving submissions and reporting findings. Includes Royal Commissions and other bodies charged with similar duties."@en ;
  skos:prefLabel "Commissions of inquiry"@en ;
.
agift:Commonwealth-State-funding
  a skos:Concept ;
  dcterms:contributor "KOdea" ;
  dcterms:created "2016-07-06T03:03:49+00:00"^^xsd:dateTime ;
  dcterms:creator "superadmin" ;
  dcterms:modified "2016-09-09T05:44:03+00:00"^^xsd:dateTime ;
  skos:altLabel "Commonwealth funding"@en ;
  skos:altLabel "Funding allocations"@en ;
  skos:altLabel "State funding"@en ;
  skos:altLabel "Vertical-fiscal balance"@en ;
  skos:broader agift:FINANCE-MANAGEMENT ;
  skos:definition "Administering the allocation of Commonwealth financial support to State governments. Conducting analysis to determine the appropriate distribution across jurisdictions. Includes general grants and specific-purpose payments as negotiated at Heads of Governments meetings."@en ;
  skos:prefLabel "Commonwealth State funding"@en ;
  skos:related agift:Intergovernmental-relations ;
.
agift:Communications-infrastructure
  a skos:Concept ;
  dcterms:contributor "KOdea" ;
  dcterms:created "2016-07-06T04:00:36+00:00"^^xsd:dateTime ;
  dcterms:creator "superadmin" ;
  dcterms:modified "2016-08-05T05:58:53+00:00"^^xsd:dateTime ;
  skos:broader agift:Telecommunications ;
  skos:definition "Developing policy and programs to support the provision and  management of physical communication infrastructure. Facilitating  communication industries including access for people with special needs and advising on the availability of new communications technology."@en ;
  skos:prefLabel "Communications infrastructure"@en ;
.
agift:Community-based-corrections
  a skos:Concept ;
  dcterms:contributor "KOdea" ;
  dcterms:created "2016-07-06T05:06:26+00:00"^^xsd:dateTime ;
  dcterms:creator "superadmin" ;
  dcterms:modified "2016-09-12T06:45:00+00:00"^^xsd:dateTime ;
  skos:altLabel "Prison employment schemes"@en ;
  skos:altLabel "Probation programs"@en ;
  skos:altLabel "Reintegration programs"@en ;
  skos:altLabel "Sentenced probation"@en ;
  skos:broader agift:Corrective-services ;
  skos:definition "Administering programs that facilitate the reintegration of offenders into society. Aiding the development of independent living skills through a combination of sentenced probation, supervision, pre-parole reporting and pre-sentence reporting, unpaid community work and personal development opportunities."@en ;
  skos:prefLabel "Community based corrections"@en ;
  skos:related agift:Spatial-information-research ;
  skos:related agift:Vocational-education ;
.
agift:Community-education
  a skos:Concept ;
  dcterms:contributor "KOdea" ;
  dcterms:created "2016-07-06T03:00:01+00:00"^^xsd:dateTime ;
  dcterms:creator "superadmin" ;
  dcterms:modified "2016-09-08T07:31:41+00:00"^^xsd:dateTime ;
  skos:altLabel "Fire safety training"@en ;
  skos:altLabel "First aid training"@en ;
  skos:broader agift:EDUCATION-AND-TRAINING ;
  skos:definition "Developing training programs designed to assist target groups of citizens. Initiating joint ventures with not-for-profit groups and local businesses. Community education is usually offered outside formal institutional structures. Includes first aid and fire safety training."@en ;
  skos:narrower agift:Adult-education-programs ;
  skos:narrower agift:Adult-migrant-education ;
  skos:narrower agift:Road-safety-awareness ;
  skos:prefLabel "Community education"@en ;
  skos:related agift:Ambulance-services ;
  skos:related agift:Firefighting-services ;
  skos:related agift:Job-placement-programs ;
.
agift:Community-engagement
  a skos:Concept ;
  dcterms:contributor "KOdea" ;
  dcterms:created "2016-07-06T02:55:32+00:00"^^xsd:dateTime ;
  dcterms:creator "superadmin" ;
  dcterms:modified "2016-09-05T07:39:17+00:00"^^xsd:dateTime ;
  skos:altLabel "Community consultation"@en ;
  skos:broader agift:COMMUNITY-SERVICES ;
  skos:definition "Inviting the community to participate in many forms of community consultations."@en ;
  skos:prefLabel "Community engagement"@en ;
  skos:related agift:Government-media ;
  skos:related agift:Social-media ;
.
agift:Community-health-services
  a skos:Concept ;
  dcterms:contributor "KOdea" ;
  dcterms:created "2016-07-06T03:07:06+00:00"^^xsd:dateTime ;
  dcterms:creator "superadmin" ;
  dcterms:modified "2016-09-09T06:18:39+00:00"^^xsd:dateTime ;
  skos:altLabel "Local health services"@en ;
  skos:altLabel "Regional health services"@en ;
  skos:broader agift:HEALTH-CARE ;
  skos:definition "Developing policy to provide for the physical and mental wellbeing of citizens in a particular district. Establishing programs that offer direct assistance to individuals or groups, and address the needs of the local community. Monitoring community health services to ensure adequate levels of care."@en ;
  skos:narrower agift:Clinical-health-services ;
  skos:narrower agift:Health-promotion ;
  skos:narrower agift:Primary-health-care ;
  skos:prefLabel "Community health services"@en ;
  skos:related agift:Counselling-services ;
  skos:related agift:Mental-health-services ;
  skos:related agift:Public-health-services ;
  skos:related agift:Special-needs-services ;
.
agift:Community-housing
  a skos:Concept ;
  dcterms:contributor "KOdea" ;
  dcterms:created "2016-07-06T03:54:18+00:00"^^xsd:dateTime ;
  dcterms:creator "superadmin" ;
  dcterms:modified "2016-09-05T07:02:01+00:00"^^xsd:dateTime ;
  skos:broader agift:Public-housing ;
  skos:definition "Developing community housing programs delivered by community organisations and local governments to eligible individuals and families."@en ;
  skos:prefLabel "Community housing"@en ;
  skos:related agift:Architectural-services ;
  skos:related agift:Building-regulations-and-standards ;
.
agift:Community-policing
  a skos:Concept ;
  dcterms:contributor "KOdea" ;
  dcterms:created "2016-07-06T05:07:55+00:00"^^xsd:dateTime ;
  dcterms:creator "superadmin" ;
  dcterms:modified "2016-08-30T07:22:32+00:00"^^xsd:dateTime ;
  skos:altLabel "Crime prevention"@en ;
  skos:altLabel "Drink driving"@en ;
  skos:altLabel "Local police"@en ;
  skos:altLabel "Police activities"@en ;
  skos:altLabel "Police"@en ;
  skos:altLabel "Public safety"@en ;
  skos:broader agift:Law-enforcement ;
  skos:definition "Administering programs that address local problems and crime reduction amongst target groups. Developing cooperative strategies involving police, local business and communities. Conducting safety audits of priority public sites, undertaking public safety patrols, identifying crime prone areas and advocating safe street and building design features."@en ;
  skos:prefLabel "Community policing"@en ;
.
agift:Community-recreational-programs
  a skos:Concept ;
  dcterms:contributor "KOdea" ;
  dcterms:created "2016-07-06T03:45:29+00:00"^^xsd:dateTime ;
  dcterms:creator "superadmin" ;
  dcterms:modified "2016-09-13T06:27:44+00:00"^^xsd:dateTime ;
  skos:altLabel "Recreation programs"@en ;
  skos:altLabel "School holiday activities"@en ;
  skos:altLabel "Senior citizen activities"@en ;
  skos:broader agift:SPORT-AND-RECREATION ;
  skos:definition "Administering schemes to provide organised activities to members of the public. Holding events for exercise, relaxation and enjoyment. Developing programs for specific groups, such as school children or senior citizens. Includes activities provided across public facilities such as swimming pools, libraries, community halls, sports centres, arts and cultural centres."@en ;
  skos:narrower agift:Gambling-support-services ;
  skos:narrower agift:Public-fitness-promotion ;
  skos:narrower agift:Social-club-support ;
  skos:narrower agift:Volunteer-support-programs ;
  skos:prefLabel "Community recreational programs"@en ;
  skos:related agift:Community-support ;
.
agift:Community-support
  a skos:Concept ;
  dcterms:contributor "KOdea" ;
  dcterms:created "2016-07-06T02:55:39+00:00"^^xsd:dateTime ;
  dcterms:creator "superadmin" ;
  dcterms:modified "2016-09-13T06:27:44+00:00"^^xsd:dateTime ;
  skos:altLabel "Disability services"@en ;
  skos:altLabel "Family support"@en ;
  skos:altLabel "Non-profit organisations support"@en ;
  skos:broader agift:COMMUNITY-SERVICES ;
  skos:definition "Managing programs to assist family units. Developing targeted services and programs to foster relationships and develop community self-reliance. Includes cooperation with other jurisdictions and non-government organisations."@en ;
  skos:narrower agift:Adoption-services ;
  skos:narrower agift:Aged-care-services ;
  skos:narrower agift:Child-and-youth-support ;
  skos:narrower agift:Child-care-services ;
  skos:narrower agift:Defence-community-programs ;
  skos:narrower agift:Family-reunion-programs ;
  skos:narrower agift:Veterans-entitlements ;
  skos:prefLabel "Community support"@en ;
  skos:related agift:Community-recreational-programs ;
  skos:related agift:Rural-community-development ;
  skos:related agift:Social-justice-and-equity ;
.
agift:Conservation-programs
  a skos:Concept ;
  dcterms:contributor "KOdea" ;
  dcterms:created "2016-07-06T03:02:39+00:00"^^xsd:dateTime ;
  dcterms:creator "superadmin" ;
  dcterms:modified "2016-09-08T07:39:46+00:00"^^xsd:dateTime ;
  skos:altLabel "Environmental conservation programs"@en ;
  skos:broader agift:ENVIRONMENT ;
  skos:definition "Maintaining land-based areas of the natural environment that are culturally or scientifically significant in their native state. Developing schemes to conserve plant or animal life in a region to protect and sustain ecosystems. Promoting community awareness of and participation in conservation activities. Promoting community awareness of and participation in sustainability activities."@en ;
  skos:narrower agift:Endangered-species-protection ;
  skos:narrower agift:Landcare-programs ;
  skos:narrower agift:Soil-preservation-programs ;
  skos:prefLabel "Conservation programs"@en ;
  skos:related agift:Biodiversity-preservation ;
  skos:related agift:Built-environment ;
  skos:related agift:Marine-life-protection-programs ;
  skos:related agift:Natural-heritage-protection ;
  skos:related agift:Waterway-management ;
.
agift:Constitutional-conventions
  a skos:Concept ;
  dcterms:contributor "KOdea" ;
  dcterms:created "2016-07-06T04:39:51+00:00"^^xsd:dateTime ;
  dcterms:creator "superadmin" ;
  dcterms:modified "2016-08-22T06:41:37+00:00"^^xsd:dateTime ;
  skos:broader agift:Constitutional-matters ;
  skos:definition "Organising forums for discussing and voting on change to the governance model embodied in a constitution. Selecting or appointing delegates. Providing advice on the rules of debate, order of proceedings and movement of motions and amendments. Producing, distributing and tabling of documents, notices and resolutions."@en ;
  skos:prefLabel "Constitutional conventions"@en ;
.
agift:Constitutional-matters
  a skos:Concept ;
  dcterms:contributor "KOdea" ;
  dcterms:created "2016-07-06T03:05:41+00:00"^^xsd:dateTime ;
  dcterms:creator "superadmin" ;
  dcterms:modified "2016-08-22T06:41:02+00:00"^^xsd:dateTime ;
  skos:altLabel "Australian Constitution"@en ;
  skos:altLabel "Governing charter"@en ;
  skos:altLabel "Sovereignty"@en ;
  skos:broader agift:GOVERNANCE ;
  skos:definition "Managing the system of fundamental principles that provide the governance framework for a nation, state or municipality. Administering policy and procedures for constitutional review and amendment. Providing advice on the implications of intervention in constitutional litigation. Includes the activities of committees involved in constitutional matters."@en ;
  skos:narrower agift:Constitutional-conventions ;
  skos:narrower agift:Constitutional-referenda ;
  skos:prefLabel "Constitutional matters"@en ;
.
agift:Constitutional-referenda
  a skos:Concept ;
  dcterms:contributor "KOdea" ;
  dcterms:created "2016-07-06T04:39:58+00:00"^^xsd:dateTime ;
  dcterms:creator "superadmin" ;
  dcterms:modified "2016-09-09T05:41:22+00:00"^^xsd:dateTime ;
  skos:altLabel "Referendums"@en ;
  skos:broader agift:Constitutional-matters ;
  skos:definition "Implementing the processes by which the governance model can be amended. Drafting and tabling a Bill proposing alteration to the constitution. Preparing and lodging the 'yes' and 'no' cases with the appropriate electoral commission."@en ;
  skos:prefLabel "Constitutional referenda"@en ;
  skos:related agift:Electoral-matters ;
.
agift:Consular-services
  a skos:Concept ;
  dcterms:contributor "KOdea" ;
  dcterms:created "2016-07-06T03:35:43+00:00"^^xsd:dateTime ;
  dcterms:creator "superadmin" ;
  dcterms:modified "2016-09-09T07:00:27+00:00"^^xsd:dateTime ;
  skos:altLabel "Consulates"@en ;
  skos:altLabel "Embassies"@en ;
  skos:altLabel "Expatriates"@en ;
  skos:altLabel "High Commissions"@en ;
  skos:broader agift:INTERNATIONAL-RELATIONS ;
  skos:definition "Establishing and maintaining Australian government representation overseas, such as high commissions, embassies or consulates. Protecting the interests of Australian citizens travelling or living overseas. Providing country-specific trade or travel advice, and direct assistance where necessary. Includes services to Australians who are hospitalised or imprisoned in other countries, advising the families of Australians who are missing and coordinating evacuations from high-risk areas."@en ;
  skos:prefLabel "Consular services"@en ;
  skos:related agift:Defence-attaches ;
  skos:related agift:Diplomatic-missions ;
  skos:related agift:International-affairs ;
  skos:related agift:Passport-services ;
.
agift:Consumer-protection
  a skos:Concept ;
  dcterms:contributor "KOdea" ;
  dcterms:created "2016-07-06T02:49:44+00:00"^^xsd:dateTime ;
  dcterms:creator "superadmin" ;
  dcterms:modified "2016-09-05T07:21:53+00:00"^^xsd:dateTime ;
  skos:altLabel "Consumer affairs"@en ;
  skos:altLabel "Customer protection"@en ;
  skos:broader agift:BUSINESS-SUPPORT-AND-REGULATION ;
  skos:definition "Administering programs to safeguard the purchasers of goods and services. Providing information to consumers and business about their rights and obligations. Handling complaints and managing dispute resolution procedures."@en ;
  skos:prefLabel "Consumer protection"@en ;
  skos:related agift:Advertising-standards ;
  skos:related agift:Fair-trading-compliance ;
.
agift:Contract-management
  a skos:Concept ;
  dcterms:contributor "KOdea" ;
  dcterms:created "2016-07-06T04:37:37+00:00"^^xsd:dateTime ;
  dcterms:creator "superadmin" ;
  dcterms:modified "2016-08-22T06:12:57+00:00"^^xsd:dateTime ;
  skos:altLabel "Government contracts"@en ;
  skos:broader agift:Resource-management ;
  skos:definition "Developing procedures to administer agreements for the provision of goods and services, in accordance with government policy. Monitoring contracts to ensure the agreed terms are met and requirements fulfilled."@en ;
  skos:prefLabel "Contract management"@en ;
.
agift:Conveyancing
  a skos:Concept ;
  dcterms:contributor "KOdea" ;
  dcterms:created "2016-07-06T04:56:03+00:00"^^xsd:dateTime ;
  dcterms:creator "superadmin" ;
  dcterms:modified "2016-08-29T06:15:07+00:00"^^xsd:dateTime ;
  skos:altLabel "Measurement standards"@en ;
  skos:broader agift:Civil-law ;
  skos:definition "Administering the transfer of property rights between parties. Managing legal instruments that regulate the sale or purchase of domestic or commercial property."@en ;
  skos:prefLabel "Conveyancing"@en ;
.
agift:Copyright-regulation
  a skos:Concept ;
  dcterms:contributor "KOdea" ;
  dcterms:created "2016-07-06T04:54:47+00:00"^^xsd:dateTime ;
  dcterms:creator "superadmin" ;
  dcterms:modified "2016-09-13T07:06:37+00:00"^^xsd:dateTime ;
  skos:broader agift:Administrative-law ;
  skos:definition "Administering the legislation that governs the rights of ownership or control of literary, musical, dramatic or artistic works. Includes legal processes to resolve disputes over copyright ownership."@en ;
  skos:prefLabel "Copyright regulation"@en ;
  skos:related agift:Publishing ;
  skos:related agift:Trademark-registration ;
.
agift:Coronial-law
  a skos:Concept ;
  dcterms:contributor "KOdea" ;
  dcterms:created "2016-07-06T03:37:29+00:00"^^xsd:dateTime ;
  dcterms:creator "superadmin" ;
  dcterms:modified "2016-08-29T06:22:34+00:00"^^xsd:dateTime ;
  skos:altLabel "Coroner"@en ;
  skos:altLabel "Coroner's court"@en ;
  skos:altLabel "Coronial investigation"@en ;
  skos:broader agift:JUSTICE-ADMINISTRATION ;
  skos:definition "Administering the body of law that supports inquests into any death clearly not due to natural causes. Undertaking investigations on behalf of the coroner into the manner and cause of examinable deaths, or fires and explosions which damage property."@en ;
  skos:prefLabel "Coronial law"@en ;
.
agift:Corrective-services
  a skos:Concept ;
  dcterms:contributor "KOdea" ;
  dcterms:created "2016-07-06T03:44:23+00:00"^^xsd:dateTime ;
  dcterms:creator "superadmin" ;
  dcterms:modified "2016-09-09T07:27:31+00:00"^^xsd:dateTime ;
  skos:altLabel "Correctional services"@en ;
  skos:altLabel "Corrections"@en ;
  skos:altLabel "Criminal punishment"@en ;
  skos:altLabel "Parole services"@en ;
  skos:altLabel "Penalties"@en ;
  skos:broader agift:SECURITY ;
  skos:definition "Developing policy and programs for the punishment of individuals who have been convicted of an offence. Establishing standards and guidelines for correctional facilities and staff. Managing probation and parole activities. Includes support programs for inmates' families."@en ;
  skos:narrower agift:Community-based-corrections ;
  skos:narrower agift:Detention-centre-management ;
  skos:prefLabel "Corrective services"@en ;
  skos:related agift:Detention-programs ;
  skos:related agift:Prosecution-services ;
.
agift:Corruption-prevention
  a skos:Concept ;
  dcterms:contributor "KOdea" ;
  dcterms:created "2016-07-06T04:43:32+00:00"^^xsd:dateTime ;
  dcterms:creator "superadmin" ;
  dcterms:modified "2016-09-12T06:57:14+00:00"^^xsd:dateTime ;
  skos:broader agift:Public-administration ;
  skos:definition "Preventing, detecting and investigating serious and systemic corruption issues in government  agencies."@en ;
  skos:prefLabel "Corruption prevention"@en ;
  skos:related agift:Criminal-law ;
  skos:related agift:Government-auditing ;
  skos:related agift:Integrity-compliance ;
  skos:related agift:Law-enforcement ;
  skos:related agift:Whistleblowing ;
.
agift:Counselling-services
  a skos:Concept ;
  dcterms:contributor "KOdea" ;
  dcterms:created "2016-07-06T02:55:47+00:00"^^xsd:dateTime ;
  dcterms:creator "superadmin" ;
  dcterms:modified "2016-09-09T07:19:12+00:00"^^xsd:dateTime ;
  skos:altLabel "Anger management"@en ;
  skos:altLabel "Domestic violence programs"@en ;
  skos:altLabel "Drug abuse counselling"@en ;
  skos:altLabel "Grief counselling"@en ;
  skos:altLabel "Group therapy"@en ;
  skos:altLabel "Health counselling"@en ;
  skos:altLabel "Marriage counselling"@en ;
  skos:altLabel "Psychiatric counselling"@en ;
  skos:altLabel "Psychiatry"@en ;
  skos:altLabel "Psychological counselling"@en ;
  skos:altLabel "Psychology"@en ;
  skos:altLabel "Suicide prevention"@en ;
  skos:altLabel "Therapy"@en ;
  skos:broader agift:COMMUNITY-SERVICES ;
  skos:definition "Providing group therapy or psychological advice to individuals, families and community groups. Managing programs to treat drug addiction, emotional or behavioural problems. Includes assistance to people who have been ordered through the courts to undertake counselling."@en ;
  skos:prefLabel "Counselling services"@en ;
  skos:related agift:Clinical-health-services ;
  skos:related agift:Community-health-services ;
  skos:related agift:Defence-community-programs ;
  skos:related agift:Discipline-programs ;
  skos:related agift:Dispute-mediation-programs ;
  skos:related agift:Gambling-support-services ;
  skos:related agift:Independent-living-services ;
  skos:related agift:Mental-health-services ;
  skos:related agift:Residential-services ;
  skos:related agift:Special-needs-services ;
.
agift:Counterfeiting-control
  a skos:Concept ;
  dcterms:contributor "KOdea" ;
  dcterms:created "2016-07-06T04:35:23+00:00"^^xsd:dateTime ;
  dcterms:creator "superadmin" ;
  dcterms:modified "2016-09-08T07:52:13+00:00"^^xsd:dateTime ;
  skos:broader agift:Currency ;
  skos:definition "Setting penalties for making or distributing forged currency. Includes procedures for reporting suspected counterfeit currency and related activities."@en ;
  skos:prefLabel "Counterfeiting control"@en ;
  skos:related agift:Currency ;
  skos:related agift:Law-enforcement ;
.
agift:Courier-services
  a skos:Concept ;
  dcterms:contributor "KOdea" ;
  dcterms:created "2016-07-06T03:58:44+00:00"^^xsd:dateTime ;
  dcterms:creator "superadmin" ;
  dcterms:modified "2016-08-05T05:43:05+00:00"^^xsd:dateTime ;
  skos:altLabel "Certified mail services"@en ;
  skos:altLabel "Express post services"@en ;
  skos:altLabel "Registered mail services"@en ;
  skos:broader agift:Postal-services ;
  skos:definition "Administering special services to collect and deliver letters, parcels and other mail with guaranteed speed or security. Includes managing contracts with private courier companies and monitoring standards of service."@en ;
  skos:prefLabel "Courier services"@en ;
.
agift:Court-reporting
  a skos:Concept ;
  dcterms:contributor "KOdea" ;
  dcterms:created "2016-07-06T03:37:39+00:00"^^xsd:dateTime ;
  dcterms:creator "superadmin" ;
  dcterms:modified "2016-09-09T07:21:49+00:00"^^xsd:dateTime ;
  skos:altLabel "Transcription services"@en ;
  skos:broader agift:JUSTICE-ADMINISTRATION ;
  skos:definition "Capturing and making accessible a record of what is said in a court or other judicial decision-making body. Includes recording and publishing a statement of facts, arguments and judgements of a proceeding in the form of a transcript."@en ;
  skos:prefLabel "Court reporting"@en ;
  skos:related agift:Hansard-services ;
  skos:related agift:Parliamentary-papers ;
.
agift:Criminal-law
  a skos:Concept ;
  dcterms:contributor "KOdea" ;
  dcterms:created "2016-07-06T03:37:47+00:00"^^xsd:dateTime ;
  dcterms:creator "superadmin" ;
  dcterms:modified "2016-09-09T07:22:30+00:00"^^xsd:dateTime ;
  skos:altLabel "Crime prevention"@en ;
  skos:altLabel "Crime"@en ;
  skos:altLabel "Criminal confiscation"@en ;
  skos:broader agift:JUSTICE-ADMINISTRATION ;
  skos:definition "Administering the body of law that governs actions punishable by the state. Establishing rules of statute and common law to define criminal behaviour, specific penalties and the conduct of legal proceedings."@en ;
  skos:prefLabel "Criminal law"@en ;
  skos:related agift:Corruption-prevention ;
  skos:related agift:Integrity-compliance ;
.
agift:Criminology
  a skos:Concept ;
  dcterms:contributor "KOdea" ;
  dcterms:created "2016-07-06T05:08:01+00:00"^^xsd:dateTime ;
  dcterms:creator "superadmin" ;
  dcterms:modified "2016-08-30T07:23:15+00:00"^^xsd:dateTime ;
  skos:altLabel "Crime research"@en ;
  skos:broader agift:Law-enforcement ;
  skos:definition "Conducting research into crime and criminal justice in Australia. Analysing the causes of illegal behaviour and evaluating the operation of law enforcement agencies, the courts and correctional systems. Providing advice for the development of policy on crime control."@en ;
  skos:prefLabel "Criminology"@en ;
.
agift:Cross-border-cooperation
  a skos:Concept ;
  dcterms:contributor "KOdea" ;
  dcterms:created "2016-07-06T04:40:54+00:00"^^xsd:dateTime ;
  dcterms:creator "superadmin" ;
  dcterms:modified "2016-09-09T05:45:31+00:00"^^xsd:dateTime ;
  skos:broader agift:Intergovernmental-relations ;
  skos:definition "Implementing the terms and conditions of formal agreements made between Australian government jurisdictions. Monitoring compliance with provisions and obligations. Assessing the ongoing benefits of interstate agreements."@en ;
  skos:prefLabel "Cross-border cooperation"@en ;
  skos:related agift:Intergovernmental-relations ;
  skos:related agift:Interstate-trade-agreements ;
.
agift:Crown-land-administration
  a skos:Concept ;
  dcterms:contributor "KOdea" ;
  dcterms:created "2016-07-06T03:40:34+00:00"^^xsd:dateTime ;
  dcterms:creator "superadmin" ;
  dcterms:modified "2016-09-12T05:50:02+00:00"^^xsd:dateTime ;
  skos:altLabel "Crown land use"@en ;
  skos:altLabel "Crown land"@en ;
  skos:broader agift:NATURAL-RESOURCES ;
  skos:definition "Managing tenure of government property. Administering the sale, purchase, resumption, lease, license or transfer of Crown land. Providing property services to government agencies, such as those associated with national parks and government housing."@en ;
  skos:prefLabel "Crown land administration"@en ;
  skos:related agift:CIVIC-INFRASTRUCTURE ;
  skos:related agift:Public-housing ;
  skos:related agift:Public-land-management ;
.
agift:Cultural-artefact-repatriation
  a skos:Concept ;
  dcterms:contributor "fionamcl" ;
  dcterms:created "2016-07-06T04:51:22+00:00"^^xsd:dateTime ;
  dcterms:creator "superadmin" ;
  dcterms:modified "2016-09-08T01:37:11+00:00"^^xsd:dateTime ;
  skos:altLabel "Return of Cultural Property programs"@en ;
  skos:altLabel "Sacred object protection"@en ;
  skos:broader agift:Indigenous-cultural-heritage ;
  skos:definition "Developing policy to safeguard custodial rights over indigenous cultural heritage property. Implementing programs to return indigenous relics, artworks, human remains and other items of cultural significance to their traditional owners or custodians."@en ;
  skos:prefLabel "Cultural artefact repatriation"@en ;
  skos:related agift:Artefact-export-regulation ;
.
agift:Cultural-awards-and-scholarships
  skos:prefLabel "Cultural awards and scholarships"@en ;
  owl:deprecated true ;
.
agift:Cultural-awards-and-scholarships
  a skos:Concept ;
  dcterms:contributor "fionamcl" ;
  dcterms:created "2016-09-08T01:22:37+00:00"^^xsd:dateTime ;
  dcterms:creator "fionamcl" ;
  dcterms:modified "2016-11-28T22:48:31+00:00"^^xsd:dateTime ;
  skos:altLabel "Awards and scholarships"@en ;
  skos:altLabel "Cultural scholarship programs"@en ;
  skos:altLabel "Scholarship programs"@en ;
  skos:broader agift:CULTURAL-AFFAIRS ;
  skos:definition "Developing schemes to confer prizes for achievement in artistic, literary or heritage-related activities. Providing grants to cultural-sector students of high merit. Includes promotional activities, assessing applications and managing payments."@en ;
  skos:prefLabel "Cultural awards and scholarships"@en ;
  skos:related agift:Honours-and-awards-programs ;
.
agift:Cultural-centre-management
  a skos:Concept ;
  dcterms:contributor "KOdea" ;
  dcterms:created "2016-07-06T03:55:08+00:00"^^xsd:dateTime ;
  dcterms:creator "superadmin" ;
  dcterms:modified "2016-09-09T07:47:02+00:00"^^xsd:dateTime ;
  skos:altLabel "Archive management"@en ;
  skos:altLabel "Art gallery management"@en ;
  skos:altLabel "Community centre management"@en ;
  skos:altLabel "Community hall management"@en ;
  skos:altLabel "Gallery management"@en ;
  skos:altLabel "Library management"@en ;
  skos:altLabel "Museum management"@en ;
  skos:altLabel "Public library management"@en ;
  skos:altLabel "Theatre management"@en ;
  skos:broader agift:Public-land-management ;
  skos:definition "Administering buildings that house cultural collections or are set aside for community use. Ensuring facilities are kept clean and maintained. Monitoring rights of access and opening hours. Taking bookings and liaising with event organisers."@en ;
  skos:prefLabel "Cultural centre management"@en ;
  skos:related agift:CULTURAL-AFFAIRS ;
  skos:related agift:Collection-storage ;
.
agift:Cultural-festivals
  skos:prefLabel "Cultural festivals"@en ;
  owl:deprecated true ;
.
agift:Cultural-festivals
  a skos:Concept ;
  dcterms:contributor "fionamcl" ;
  dcterms:created "2016-09-08T01:22:40+00:00"^^xsd:dateTime ;
  dcterms:creator "fionamcl" ;
  dcterms:modified "2016-11-28T22:48:37+00:00"^^xsd:dateTime ;
  skos:altLabel "Arts festivals"@en ;
  skos:altLabel "Book festivals"@en ;
  skos:altLabel "Festivals"@en ;
  skos:altLabel "Heritage festivals"@en ;
  skos:broader agift:CULTURAL-AFFAIRS ;
  skos:definition "Promoting and funding events that highlight artistic, literary or heritage related activities. Organising festivals, performances and joint ventures with community groups where events focus on a particular genre or collection. Includes participation in international cultural festivals."@en ;
  skos:prefLabel "Cultural festivals"@en ;
  skos:related agift:Civic-celebrations ;
  skos:related agift:Multicultural-festivals ;
  skos:related agift:Overseas-promotion ;
.
agift:Cultural-gifts-programs
  skos:prefLabel "Cultural gifts programs"@en ;
  owl:deprecated true ;
.
agift:Cultural-gifts-programs
  a skos:Concept ;
  dcterms:contributor "fionamcl" ;
  dcterms:created "2016-09-08T01:22:44+00:00"^^xsd:dateTime ;
  dcterms:creator "fionamcl" ;
  dcterms:modified "2016-11-28T22:48:43+00:00"^^xsd:dateTime ;
  skos:altLabel "Art donation schemes"@en ;
  skos:altLabel "Public donations"@en ;
  skos:broader agift:CULTURAL-AFFAIRS ;
  skos:definition "Managing donations of cultural materials, made under arts incentive schemes. Examining materials to ensure they conform to collection development policies. Setting guidelines for the acceptance of gifts. Determining access restrictions, intellectual property rights and legal title over materials. Organising independent valuations and making submissions to the relevant taxation incentives body."@en ;
  skos:prefLabel "Cultural gifts programs"@en ;
  skos:related agift:Arts-incentive-schemes ;
  skos:related agift:Collection-acquisition ;
.
agift:Currency
  a skos:Concept ;
  dcterms:contributor "KOdea" ;
  dcterms:created "2016-07-06T03:03:56+00:00"^^xsd:dateTime ;
  dcterms:creator "superadmin" ;
  dcterms:modified "2016-09-08T07:52:13+00:00"^^xsd:dateTime ;
  skos:altLabel "Coinage"@en ;
  skos:altLabel "Coins"@en ;
  skos:altLabel "Money"@en ;
  skos:altLabel "Notes"@en ;
  skos:broader agift:FINANCE-MANAGEMENT ;
  skos:definition "Developing policy for the minting and distribution of monetary notes and coins. Designing security techniques such as watermarks to prevent counterfeiting. Includes procedures for issuing new or commemorative coins."@en ;
  skos:narrower agift:Counterfeiting-control ;
  skos:prefLabel "Currency"@en ;
  skos:related agift:Counterfeiting-control ;
.
agift:Curriculum-development
  a skos:Concept ;
  dcterms:contributor "KOdea" ;
  dcterms:created "2016-07-06T03:00:07+00:00"^^xsd:dateTime ;
  dcterms:creator "superadmin" ;
  dcterms:modified "2016-09-08T07:15:19+00:00"^^xsd:dateTime ;
  skos:altLabel "School curriculum development"@en ;
  skos:altLabel "Syllabus development"@en ;
  skos:broader agift:EDUCATION-AND-TRAINING ;
  skos:definition "Researching and drafting outline study programs for any education sector. Outlining the courses and units to be completed. Includes liaison across jurisdictions to support consistency across education authorities."@en ;
  skos:prefLabel "Curriculum development"@en ;
  skos:related agift:School-education ;
  skos:related agift:Tertiary-education ;
.
agift:Cybersafety
  a skos:Concept ;
  dcterms:contributor "KOdea" ;
  dcterms:created "2016-07-06T03:58:20+00:00"^^xsd:dateTime ;
  dcterms:creator "superadmin" ;
  dcterms:modified "2016-09-05T07:38:50+00:00"^^xsd:dateTime ;
  skos:altLabel "Cybersecurity"@en ;
  skos:broader agift:Internet ;
  skos:definition "Developing policy and programs designed to protect consumers shopping online, vulnerable people from exposure to inappropriate material and invasion of personal privacy online."@en ;
  skos:prefLabel "Cybersafety"@en ;
  skos:related agift:Electronic-commerce ;
  skos:related agift:Information-management-standards ;
  skos:related agift:Privacy ;
.
agift:DEFENCE
  a skos:Concept ;
  dcterms:contributor "KOdea" ;
  dcterms:created "2016-07-06T02:45:01+00:00"^^xsd:dateTime ;
  dcterms:creator "superadmin" ;
  dcterms:modified "2016-09-08T06:26:15+00:00"^^xsd:dateTime ;
  skos:definition "Ensuring the safety of Australia by building, maintaining and deploying military resources. Developing policy and programs for defence of the nation, region and allies. Includes high-level administration of the Australian Defence Forces (ADF)."@en ;
  skos:narrower agift:Australian-Defence-Forces ;
  skos:narrower agift:Defence-estate-management ;
  skos:narrower agift:Defence-force-careers ;
  skos:narrower agift:Defence-strategic-development ;
  skos:narrower agift:Defence-strategic-policy ;
  skos:narrower agift:Defence-strategic-support ;
  skos:narrower agift:Emergency-management ;
  skos:narrower agift:Military-law ;
  skos:narrower agift:Military-operations ;
  skos:prefLabel "DEFENCE"@en ;
  skos:related agift:SECURITY ;
  skos:topConceptOf agift:AGIFT ;
.
agift:Data-management
  a skos:Concept ;
  dcterms:contributor "KOdea" ;
  dcterms:created "2016-07-06T03:57:37+00:00"^^xsd:dateTime ;
  dcterms:creator "superadmin" ;
  dcterms:modified "2016-09-05T07:34:12+00:00"^^xsd:dateTime ;
  skos:altLabel "Data matching guidelines"@en ;
  skos:altLabel "Metadata standards"@en ;
  skos:broader agift:Information-management-standards ;
  skos:definition "Developing standards for the exchange or transfer of information between government agencies or systems. Providing guidelines for cross-matching data. Promoting the use of metadata to support resource discovery or interoperability"@en ;
  skos:prefLabel "Data management"@en ;
  skos:related agift:Information-security ;
  skos:related agift:Information-technology-standards ;
  skos:related agift:Online-transaction-standards ;
.
agift:Declaration-of-interests
  a skos:Concept ;
  dcterms:contributor "KOdea" ;
  dcterms:created "2016-07-06T04:40:16+00:00"^^xsd:dateTime ;
  dcterms:creator "superadmin" ;
  dcterms:modified "2016-08-22T06:44:17+00:00"^^xsd:dateTime ;
  skos:altLabel "Pecuniary interests"@en ;
  skos:altLabel "Register of interests"@en ;
  skos:broader agift:Electoral-matters ;
  skos:definition "Managing the disclosure of election campaign funding details. Facilitating the lodgement of returns by candidates and political parties. Includes notifications from broadcasters regarding electoral advertisements run during an election period."@en ;
  skos:prefLabel "Declaration of interests"@en ;
.
agift:Defence-attaches
  a skos:Concept ;
  dcterms:contributor "KOdea" ;
  dcterms:created "2016-07-06T04:52:17+00:00"^^xsd:dateTime ;
  dcterms:creator "superadmin" ;
  dcterms:modified "2016-09-09T07:00:45+00:00"^^xsd:dateTime ;
  skos:broader agift:Defence-liaison ;
  skos:definition "Providing diplomatic representation of Australia's military interests. Liaising with governments and international bodies to build strategic alliances and defence partnerships."@en ;
  skos:prefLabel "Defence attaches"@en ;
  skos:related agift:Consular-services ;
  skos:related agift:Defence-strategic-policy ;
  skos:related agift:Military-advisors ;
.
agift:Defence-career-development
  a skos:Concept ;
  dcterms:contributor "KOdea" ;
  dcterms:created "2016-07-06T04:09:24+00:00"^^xsd:dateTime ;
  dcterms:creator "superadmin" ;
  dcterms:modified "2016-09-08T06:37:09+00:00"^^xsd:dateTime ;
  skos:broader agift:Defence-force-careers ;
  skos:definition "Providing career counselling, career planning, professional development and training advice to regular and reserve members of the Australian Defence Forces. Includes career transition assistance, redeployment, discharge and retirement services."@en ;
  skos:prefLabel "Defence career development"@en ;
  skos:related agift:Defence-community-programs ;
  skos:related agift:Military-education-and-training ;
  skos:related agift:Military-employment-services ;
.
agift:Defence-college-training
  a skos:Concept ;
  dcterms:contributor "KOdea" ;
  dcterms:created "2016-07-06T04:14:00+00:00"^^xsd:dateTime ;
  dcterms:creator "superadmin" ;
  dcterms:modified "2016-08-19T01:51:32+00:00"^^xsd:dateTime ;
  skos:altLabel "Military colleges"@en ;
  skos:altLabel "Officer college training"@en ;
  skos:broader agift:Military-education-and-training ;
  skos:definition "Administering educational programs through institutions that cater specifically to military personnel, officers and cadets. Determining entry requirements. Providing scholarships and study grants."@en ;
  skos:prefLabel "Defence college training"@en ;
.
agift:Defence-community-programs
  a skos:Concept ;
  dcterms:contributor "KOdea" ;
  dcterms:created "2016-07-06T04:02:36+00:00"^^xsd:dateTime ;
  dcterms:creator "superadmin" ;
  dcterms:modified "2016-09-06T07:21:57+00:00"^^xsd:dateTime ;
  skos:altLabel "Defence families"@en ;
  skos:broader agift:Community-support ;
  skos:definition "Providing services to support military personnel and their families. Establishing social networks and activities. Facilitating communication between family members separated by service requirements. Arranging access to support groups or counselling in times of tragedy."@en ;
  skos:prefLabel "Defence community programs"@en ;
  skos:related agift:Counselling-services ;
  skos:related agift:Defence-career-development ;
  skos:related agift:Defence-housing ;
  skos:related agift:Veterans-entitlements ;
.
agift:Defence-cooperation-programs
  a skos:Concept ;
  dcterms:contributor "KOdea" ;
  dcterms:created "2016-07-06T04:52:23+00:00"^^xsd:dateTime ;
  dcterms:creator "superadmin" ;
  dcterms:modified "2016-09-09T07:01:14+00:00"^^xsd:dateTime ;
  skos:broader agift:Defence-liaison ;
  skos:definition "Promoting international defence relations through a series of high-level dialogue, official visits and collaboration with regional and allied defence organisations. Developing a coordinated international response to a potential or imminent threat."@en ;
  skos:prefLabel "Defence cooperation programs"@en ;
  skos:related agift:Peacekeeping-forces ;
.
agift:Defence-efficiency-review
  a skos:Concept ;
  dcterms:contributor "KOdea" ;
  dcterms:created "2016-07-06T04:09:58+00:00"^^xsd:dateTime ;
  dcterms:creator "superadmin" ;
  dcterms:modified "2016-08-11T07:22:42+00:00"^^xsd:dateTime ;
  skos:broader agift:Defence-strategic-development ;
  skos:definition "Investigating current defence operations to assess performance against the use of resources. Reviewing processes and consulting stakeholders. Developing strategies for efficient expenditure of funds, to maximise defence capability."@en ;
  skos:prefLabel "Defence efficiency review"@en ;
.
agift:Defence-estate-management
  a skos:Concept ;
  dcterms:contributor "KOdea" ;
  dcterms:created "2016-07-06T02:58:24+00:00"^^xsd:dateTime ;
  dcterms:creator "superadmin" ;
  dcterms:modified "2016-09-08T06:34:25+00:00"^^xsd:dateTime ;
  skos:broader agift:DEFENCE ;
  skos:definition "Administering buildings, infrastructure, property and other corporate assets of the Defence portfolio. Developing acquisition and disposal policy. Managing repair and maintenance programs. Reviewing facilities and capital works."@en ;
  skos:prefLabel "Defence estate management"@en ;
  skos:related agift:Defence-housing ;
.
agift:Defence-force-careers
  a skos:Concept ;
  dcterms:contributor "KOdea" ;
  dcterms:created "2016-07-06T02:58:30+00:00"^^xsd:dateTime ;
  dcterms:creator "superadmin" ;
  dcterms:modified "2016-09-08T07:25:37+00:00"^^xsd:dateTime ;
  skos:altLabel "Air force careers"@en ;
  skos:altLabel "Army careers"@en ;
  skos:altLabel "Defence personnel"@en ;
  skos:altLabel "Enlistment"@en ;
  skos:altLabel "Military enlistment"@en ;
  skos:altLabel "Navy careers"@en ;
  skos:broader agift:DEFENCE ;
  skos:definition "Developing human resources policy for defence force personnel. Conducting research into recruitment, retention and demographics. Administering recruitment programs and activities to promote defence force careers."@en ;
  skos:narrower agift:Defence-career-development ;
  skos:narrower agift:Military-employment-services ;
  skos:prefLabel "Defence force careers"@en ;
  skos:related agift:Defence-personnel-exchanges ;
  skos:related agift:Human-resources-development ;
  skos:related agift:Military-education-and-training ;
  skos:related agift:Recruitment-programs ;
  skos:related agift:Workplace-discrimination-monitoring ;
.
agift:Defence-force-commands
  a skos:Concept ;
  dcterms:contributor "KOdea" ;
  dcterms:created "2016-07-06T04:08:39+00:00"^^xsd:dateTime ;
  dcterms:creator "superadmin" ;
  dcterms:modified "2016-08-11T07:12:41+00:00"^^xsd:dateTime ;
  skos:altLabel "Air force commands"@en ;
  skos:altLabel "Army commands"@en ;
  skos:altLabel "Command and control"@en ;
  skos:altLabel "Defence commands"@en ;
  skos:altLabel "Military commands"@en ;
  skos:altLabel "Navy commands"@en ;
  skos:altLabel "RAAF commands"@en ;
  skos:altLabel "RAN commands"@en ;
  skos:broader agift:Australian-Defence-Forces ;
  skos:definition "Managing and operating command centres of the Army, Navy or Air Force, which exercise authority over a specific geographical area, a discrete function or specialised programs."@en ;
  skos:prefLabel "Defence force commands"@en ;
.
agift:Defence-housing
  a skos:Concept ;
  dcterms:contributor "KOdea" ;
  dcterms:created "2016-07-06T04:01:34+00:00"^^xsd:dateTime ;
  dcterms:creator "superadmin" ;
  dcterms:modified "2016-09-08T06:34:25+00:00"^^xsd:dateTime ;
  skos:altLabel "ADF housing"@en ;
  skos:altLabel "Defence families"@en ;
  skos:altLabel "War service home schemes"@en ;
  skos:broader agift:Accommodation-services ;
  skos:definition "Administering schemes to provide accommodation for defence forces personnel. Includes criteria for eligibility, subsidy entitlements, leasing arrangements, relocation and maintenance programs. Planning for housing construction and the movement of defence personnel. Liaising with local authorities and acquiring land."@en ;
  skos:prefLabel "Defence housing"@en ;
  skos:related agift:Defence-community-programs ;
  skos:related agift:Defence-estate-management ;
.
agift:Defence-industry
  a skos:Concept ;
  dcterms:contributor "KOdea" ;
  dcterms:created "2016-07-06T04:11:00+00:00"^^xsd:dateTime ;
  dcterms:creator "superadmin" ;
  dcterms:modified "2016-09-08T06:45:57+00:00"^^xsd:dateTime ;
  skos:broader agift:Defence-strategic-support ;
  skos:definition "Administering programs to build relationships with Australian industry to support defence activities. Providing funding, investment opportunities and incentives for research and development. Establishing advisory forums and other communication strategies. Operating endorsement schemes to certify products that meet Australian defence specifications. Encouraging participation in the international defence market and managing materiel cooperative activities."@en ;
  skos:prefLabel "Defence industry"@en ;
  skos:related agift:Capital-equipment-programs ;
  skos:related agift:Defence-science-and-technology ;
.
agift:Defence-liaison
  a skos:Concept ;
  dcterms:contributor "KOdea" ;
  dcterms:created "2016-07-06T03:35:50+00:00"^^xsd:dateTime ;
  dcterms:creator "superadmin" ;
  dcterms:modified "2016-09-09T07:05:23+00:00"^^xsd:dateTime ;
  skos:broader agift:INTERNATIONAL-RELATIONS ;
  skos:definition "Cooperating with other countries to ensure Australia's ability to resist foreign aggression or attack. Providing defence and strategic advice, negotiating agreements for the deployment of defence resources. Includes participation in joint exercises and development programs."@en ;
  skos:narrower agift:Defence-attaches ;
  skos:narrower agift:Defence-cooperation-programs ;
  skos:narrower agift:Defence-personnel-exchanges ;
  skos:narrower agift:Military-advisors ;
  skos:prefLabel "Defence liaison"@en ;
  skos:related agift:Australian-Defence-Forces ;
  skos:related agift:External-security ;
  skos:related agift:International-affairs ;
  skos:related agift:International-treaties ;
.
agift:Defence-personnel-exchanges
  a skos:Concept ;
  dcterms:contributor "KOdea" ;
  dcterms:created "2016-07-06T04:52:31+00:00"^^xsd:dateTime ;
  dcterms:creator "superadmin" ;
  dcterms:modified "2016-09-08T06:35:55+00:00"^^xsd:dateTime ;
  skos:broader agift:Defence-liaison ;
  skos:definition "Designing and implementing programs for temporary reassignment of defence personnel, to support professional development and promote relationships between defence forces. Providing services and training to staff on exchange, to help realise the full benefits of the program."@en ;
  skos:prefLabel "Defence personnel exchanges"@en ;
  skos:related agift:Defence-force-careers ;
.
agift:Defence-reform-program
  a skos:Concept ;
  dcterms:contributor "KOdea" ;
  dcterms:created "2016-07-06T04:10:07+00:00"^^xsd:dateTime ;
  dcterms:creator "superadmin" ;
  dcterms:modified "2016-08-11T07:23:15+00:00"^^xsd:dateTime ;
  skos:broader agift:Defence-strategic-development ;
  skos:definition "Implementing improvements in defence operations, to support long-term capability development. Evaluating the effects of reforms, to determine their impact on performance, efficiency and personnel."@en ;
  skos:prefLabel "Defence reform program"@en ;
.
agift:Defence-science-and-technology
  a skos:Concept ;
  dcterms:contributor "KOdea" ;
  dcterms:created "2016-07-06T04:11:06+00:00"^^xsd:dateTime ;
  dcterms:creator "superadmin" ;
  dcterms:modified "2016-09-12T06:46:09+00:00"^^xsd:dateTime ;
  skos:altLabel "Biological weapons"@en ;
  skos:broader agift:Defence-strategic-support ;
  skos:definition "Conducting research into the application of specialist knowledge and equipment to support military operations. Providing technical advice on the purchase of defence equipment. Includes designing, testing and overseeing the manufacture of new products."@en ;
  skos:prefLabel "Defence science and technology"@en ;
  skos:related agift:Biotechnology-development ;
  skos:related agift:Defence-industry ;
  skos:related agift:Engineering-and-technology-sciences ;
  skos:related agift:Nuclear-sciences ;
  skos:related agift:Spatial-information-research ;
.
agift:Defence-strategic-development
  a skos:Concept ;
  dcterms:contributor "KOdea" ;
  dcterms:created "2016-07-06T02:58:38+00:00"^^xsd:dateTime ;
  dcterms:creator "superadmin" ;
  dcterms:modified "2016-09-08T06:43:38+00:00"^^xsd:dateTime ;
  skos:broader agift:DEFENCE ;
  skos:definition "Identifying issues for the effective growth and advancement of defence operations. Assessing current infrastructure and facilities, and forecasting future needs. Conducting long-term planning for capability development, science and technology, acquisition, training and logistics."@en ;
  skos:narrower agift:Defence-efficiency-review ;
  skos:narrower agift:Defence-reform-program ;
  skos:prefLabel "Defence strategic development"@en ;
  skos:related agift:Strategic-planning ;
.
agift:Defence-strategic-policy
  a skos:Concept ;
  dcterms:contributor "KOdea" ;
  dcterms:created "2016-07-06T02:58:44+00:00"^^xsd:dateTime ;
  dcterms:creator "superadmin" ;
  dcterms:modified "2016-09-08T06:41:41+00:00"^^xsd:dateTime ;
  skos:altLabel "Military equipment strategy"@en ;
  skos:broader agift:DEFENCE ;
  skos:definition "Formulating high-level policy to direct the development and deployment of Australia's defence capability. Directing the management of international defence activities and setting guidelines and priorities for military planning and decision making."@en ;
  skos:narrower agift:Strategic-decisions ;
  skos:narrower agift:Strategic-planning ;
  skos:prefLabel "Defence strategic policy"@en ;
  skos:related agift:Defence-attaches ;
  skos:related agift:Defence-strategic-support ;
.
agift:Defence-strategic-support
  a skos:Concept ;
  dcterms:contributor "KOdea" ;
  dcterms:created "2016-07-06T02:58:56+00:00"^^xsd:dateTime ;
  dcterms:creator "superadmin" ;
  dcterms:modified "2016-09-12T06:45:47+00:00"^^xsd:dateTime ;
  skos:altLabel "Military equipment strategy"@en ;
  skos:broader agift:DEFENCE ;
  skos:definition "Developing programs to ensure military operations are fully equipped and assisted. Building a coordinated network of infrastructure, facilities and knowledge. Formulating policy for contracting, acquisitions and defence export activities."@en ;
  skos:narrower agift:Capital-equipment-programs ;
  skos:narrower agift:Defence-industry ;
  skos:narrower agift:Defence-science-and-technology ;
  skos:narrower agift:Logistics ;
  skos:prefLabel "Defence strategic support"@en ;
  skos:related agift:Defence-strategic-policy ;
.
agift:Dental-health-services
  a skos:Concept ;
  dcterms:contributor "KOdea" ;
  dcterms:created "2016-07-06T04:48:59+00:00"^^xsd:dateTime ;
  dcterms:creator "superadmin" ;
  dcterms:modified "2016-08-24T07:22:19+00:00"^^xsd:dateTime ;
  skos:altLabel "Dentists"@en ;
  skos:altLabel "Oral health services"@en ;
  skos:altLabel "Orthodontic services"@en ;
  skos:altLabel "Teeth"@en ;
  skos:broader agift:Special-needs-services ;
  skos:definition "Administering programs that provide treatments for oral hygiene and problems with teeth. Managing school dental services and schemes to provide access to low-income earners or disadvantaged groups. Monitoring the activities of private dental health providers."@en ;
  skos:prefLabel "Dental health services"@en ;
.
agift:Deportation
  a skos:Concept ;
  dcterms:contributor "KOdea" ;
  dcterms:created "2016-07-06T03:33:49+00:00"^^xsd:dateTime ;
  dcterms:creator "superadmin" ;
  dcterms:modified "2016-09-09T06:31:36+00:00"^^xsd:dateTime ;
  skos:altLabel "Criminal deportation"@en ;
  skos:altLabel "Extradition"@en ;
  skos:altLabel "Illegal immigrants"@en ;
  skos:broader agift:IMMIGRATION ;
  skos:definition "Administering the removal of foreign nationals whose presence in Australia is unlawful or poses an unacceptable level of threat to the community. Arranging the deportation of non-citizens who have committed serious crimes and those whose visas have expired. Includes the exclusion of unauthorised arrivals who are not refugees."@en ;
  skos:prefLabel "Deportation"@en ;
  skos:related agift:Administrative-law ;
  skos:related agift:Detention-programs ;
  skos:related agift:National-security ;
  skos:related agift:Refugee-services ;
.
agift:Descriptive-standards
  skos:prefLabel "Descriptive standards"@en ;
  owl:deprecated true ;
.
agift:Descriptive-standards
  a skos:Concept ;
  dcterms:contributor "fionamcl" ;
  dcterms:created "2016-09-08T01:29:14+00:00"^^xsd:dateTime ;
  dcterms:creator "fionamcl" ;
  dcterms:modified "2016-11-28T22:46:48+00:00"^^xsd:dateTime ;
  skos:altLabel "Cataloguing standards"@en ;
  skos:altLabel "Classification standards"@en ;
  skos:altLabel "Curatorial standards"@en ;
  skos:altLabel "Indexing standards"@en ;
  skos:broader agift:Collection-access ;
  skos:definition "Developing and implementing agreed models to explain the content, extent and format of items in cultural collections. Includes cooperative efforts to promote common descriptive standards across a range of cultural institutions."@en ;
  skos:prefLabel "Descriptive standards"@en ;
  skos:related agift:Collection-accessioning ;
  skos:related agift:Finding-aids-development ;
.
agift:Design-rights-management
  a skos:Concept ;
  dcterms:contributor "KOdea" ;
  dcterms:created "2016-07-06T05:13:34+00:00"^^xsd:dateTime ;
  dcterms:creator "superadmin" ;
  dcterms:modified "2016-09-13T07:05:25+00:00"^^xsd:dateTime ;
  skos:broader agift:Intellectual-property-management ;
  skos:definition "Conferring legal ownership over applied intellectual property such as structures, machinery, industrial plans or complex artworks (eg those with intricate configuration or moving parts). Includes processing and approving applications for design registration, liaising with designers and licensing the use of designs."@en ;
  skos:prefLabel "Design rights management"@en ;
  skos:related agift:Patent-rights-management ;
  skos:related agift:Plant-breeders-rights-management ;
  skos:related agift:Trademark-registration ;
.
agift:Detention-centre-management
  a skos:Concept ;
  dcterms:contributor "KOdea" ;
  dcterms:created "2016-07-06T05:06:32+00:00"^^xsd:dateTime ;
  dcterms:creator "superadmin" ;
  dcterms:modified "2016-09-12T06:47:58+00:00"^^xsd:dateTime ;
  skos:altLabel "Detention centres"@en ;
  skos:altLabel "Jail management"@en ;
  skos:altLabel "Juvenile detention centres"@en ;
  skos:altLabel "Police cells"@en ;
  skos:altLabel "Prison farms"@en ;
  skos:altLabel "Prison management"@en ;
  skos:altLabel "Remand centres"@en ;
  skos:broader agift:Corrective-services ;
  skos:definition "Administering humane and appropriately secure facilities where convicted offenders are incarcerated. Providing food and amenities, recreation, medical care, mail services and education. Monitoring standards where detention centre management activities are outsourced"@en ;
  skos:prefLabel "Detention centre management"@en ;
  skos:related agift:Detention-programs ;
  skos:related agift:Military-law ;
.
agift:Detention-programs
  a skos:Concept ;
  dcterms:contributor "KOdea" ;
  dcterms:created "2016-07-06T03:33:55+00:00"^^xsd:dateTime ;
  dcterms:creator "superadmin" ;
  dcterms:modified "2016-09-28T07:01:59+00:00"^^xsd:dateTime ;
  skos:altLabel "Migrant processing centres"@en ;
  skos:broader agift:IMMIGRATION ;
  skos:definition "Administering custodial schemes for people who have entered Australia illegally, those refused entry at international airports and seaports, and those whose visas are cancelled or expired. Managing facilities for the detention of illegal immigrants. Providing food and amenities, medical care, recreation, social support and education."@en ;
  skos:prefLabel "Detention programs"@en ;
  skos:related agift:Border-protection ;
  skos:related agift:Corrective-services ;
  skos:related agift:Deportation ;
  skos:related agift:Detention-centre-management ;
  skos:related agift:Migrant-accommodation-services ;
  skos:related agift:Military-law ;
  skos:related agift:National-security ;
  skos:related agift:Refugee-services ;
.
agift:Development-assistance-programs
  a skos:Concept ;
  dcterms:contributor "KOdea" ;
  dcterms:created "2016-07-06T04:53:45+00:00"^^xsd:dateTime ;
  dcterms:creator "superadmin" ;
  dcterms:modified "2016-09-13T07:08:24+00:00"^^xsd:dateTime ;
  skos:broader agift:Overseas-aid-programs ;
  skos:definition "Administering schemes to support growth and improvement in overseas communities. Providing advice and training and delivering projects in sectors such as governance, health, education, rural and infrastructure development. Includes emergency, humanitarian and reconstruction assistance in times of  crisis."@en ;
  skos:prefLabel "Development assistance programs"@en ;
  skos:related agift:Disaster-recovery ;
  skos:related agift:Disaster-support ;
  skos:related agift:Overseas-student-scholarship-programs ;
  skos:related agift:Peacekeeping-forces ;
  skos:related agift:Trade-development-programs ;
.
agift:Diplomatic-missions
  a skos:Concept ;
  dcterms:contributor "KOdea" ;
  dcterms:created "2016-07-06T03:35:56+00:00"^^xsd:dateTime ;
  dcterms:creator "superadmin" ;
  dcterms:modified "2016-09-09T07:02:28+00:00"^^xsd:dateTime ;
  skos:altLabel "Ambassadors"@en ;
  skos:altLabel "Diplomatic Corps"@en ;
  skos:altLabel "International representatives"@en ;
  skos:broader agift:INTERNATIONAL-RELATIONS ;
  skos:definition "Providing services to representatives of foreign governments or international organisations. Assisting representatives to establish and maintain diplomatic missions, such as high commissions, embassies or consulates. Includes developing protocol guidelines and consular responsibilities for countries without diplomatic representation in Australia."@en ;
  skos:prefLabel "Diplomatic missions"@en ;
  skos:related agift:Consular-services ;
  skos:related agift:International-affairs ;
.
agift:Disarmament-and-arms-control
  a skos:Concept ;
  dcterms:contributor "KOdea" ;
  dcterms:created "2016-07-06T04:53:00+00:00"^^xsd:dateTime ;
  dcterms:creator "superadmin" ;
  dcterms:modified "2016-09-09T07:06:38+00:00"^^xsd:dateTime ;
  skos:altLabel "Arms control"@en ;
  skos:altLabel "Chemical weapons"@en ;
  skos:altLabel "Nuclear weapons"@en ;
  skos:altLabel "Weapons inspections"@en ;
  skos:altLabel "Weapons of mass destruction"@en ;
  skos:broader agift:International-affairs ;
  skos:definition "Implementing the terms and conditions of formal agreements to reduce or limit levels of military resources. Administering regulatory mechanisms to enable Australia to fulfil its obligations under international treaties. Includes disseminating information to stakeholders, inspecting significant facilities and declaring notable activities."@en ;
  skos:prefLabel "Disarmament and arms control"@en ;
  skos:related agift:International-treaties ;
  skos:related agift:Nuclear-safeguards ;
  skos:related agift:Treaty-administration ;
.
agift:Disaster-recovery
  a skos:Concept ;
  dcterms:contributor "KOdea" ;
  dcterms:created "2016-07-06T04:04:15+00:00"^^xsd:dateTime ;
  dcterms:creator "superadmin" ;
  dcterms:modified "2016-09-06T07:51:05+00:00"^^xsd:dateTime ;
  skos:broader agift:Natural-disasters ;
  skos:definition "Coordinating programs to repair the damage caused by natural disasters - such as floods, earthquakes, cyclones, storms or major bushfires. Developing strategies for timely restoration of essential services and clearing debris. Initiating plans for demolition and rebuilding of damaged facilities."@en ;
  skos:prefLabel "Disaster recovery"@en ;
  skos:related agift:Civil-community-assistance ;
  skos:related agift:Development-assistance-programs ;
  skos:related agift:Disaster-relief ;
  skos:related agift:Disaster-support ;
.
agift:Disaster-relief
  a skos:Concept ;
  dcterms:contributor "KOdea" ;
  dcterms:created "2016-07-06T04:04:22+00:00"^^xsd:dateTime ;
  dcterms:creator "superadmin" ;
  dcterms:modified "2016-09-12T06:14:01+00:00"^^xsd:dateTime ;
  skos:altLabel "Drought relief"@en ;
  skos:altLabel "Flood relief"@en ;
  skos:altLabel "Relief funding"@en ;
  skos:broader agift:Natural-disasters ;
  skos:definition "Providing financial assistance to communities, individuals and businesses affected by natural disasters such as floods, earthquakes, cyclones, storms or major bushfires. Includes negotiating terms for compensation payments or low interest loans, processing claims and liaising with community services for other forms of support."@en ;
  skos:prefLabel "Disaster relief"@en ;
  skos:related agift:Disaster-recovery ;
  skos:related agift:Emergency-accommodation ;
  skos:related agift:Emergency-funding ;
  skos:related agift:Financial-assistance ;
  skos:related agift:Marine-and-rural-support ;
.
agift:Disaster-support
  a skos:Concept ;
  dcterms:contributor "KOdea" ;
  dcterms:created "2016-07-06T04:11:44+00:00"^^xsd:dateTime ;
  dcterms:creator "superadmin" ;
  dcterms:modified "2016-09-08T06:54:02+00:00"^^xsd:dateTime ;
  skos:broader agift:Emergency-management ;
  skos:definition "Managing the allocation of Australian Defence Force resources to assist overseas communities in times of crisis. Providing support to humanitarian and reconstruction efforts after natural disaster or other emergency. Includes identifying lines of communication, chain of command, and establishing criteria for situations warranting defence forces assistance."@en ;
  skos:prefLabel "Disaster support"@en ;
  skos:related agift:Civil-community-assistance ;
  skos:related agift:Development-assistance-programs ;
  skos:related agift:Disaster-recovery ;
  skos:related agift:Peacekeeping-forces ;
.
agift:Discipline-programs
  a skos:Concept ;
  dcterms:contributor "KOdea" ;
  dcterms:created "2016-07-06T04:14:16+00:00"^^xsd:dateTime ;
  dcterms:creator "superadmin" ;
  dcterms:modified "2016-09-08T07:12:51+00:00"^^xsd:dateTime ;
  skos:altLabel "Bullying prevention programs"@en ;
  skos:altLabel "School detention"@en ;
  skos:altLabel "School discipline"@en ;
  skos:broader agift:School-education ;
  skos:definition "Developing and implementing programs to reduce or prevent behavioural problems in schools. Assisting those experiencing behavioural problems, and victims of unacceptable behaviour. Providing guidance to teachers about appropriate forms of discipline. Includes liaison with community groups, police and families to deal with behavioural problems."@en ;
  skos:prefLabel "Discipline programs"@en ;
  skos:related agift:Child-and-youth-support ;
  skos:related agift:Counselling-services ;
.
agift:Dispute-mediation-programs
  a skos:Concept ;
  dcterms:contributor "KOdea" ;
  dcterms:created "2016-07-06T04:56:09+00:00"^^xsd:dateTime ;
  dcterms:creator "superadmin" ;
  dcterms:modified "2016-09-09T07:20:26+00:00"^^xsd:dateTime ;
  skos:altLabel "Court counselling"@en ;
  skos:altLabel "Dispute resolution services"@en ;
  skos:altLabel "Legal dispute mediation"@en ;
  skos:altLabel "Legal mediation programs"@en ;
  skos:altLabel "Mandatory counselling"@en ;
  skos:altLabel "Mediation programs"@en ;
  skos:broader agift:Civil-law ;
  skos:definition "Establishing procedures to settle legal debates or reconcile competing interests. Acting as an intermediary between opposing parties to bring about agreement. Includes facilitating access to these programs."@en ;
  skos:prefLabel "Dispute mediation programs"@en ;
  skos:related agift:Administrative-decision-appeal ;
  skos:related agift:Agreement-dispute-mediation ;
  skos:related agift:Counselling-services ;
  skos:related agift:Native-title-mediation-programs ;
  skos:related agift:Workplace-equity-and-justice-programs ;
.
agift:Doping-detection-research
  a skos:Concept ;
  dcterms:contributor "KOdea" ;
  dcterms:created "2016-07-06T05:10:36+00:00"^^xsd:dateTime ;
  dcterms:creator "superadmin" ;
  dcterms:modified "2016-09-12T06:40:35+00:00"^^xsd:dateTime ;
  skos:broader agift:Sports-drugs-monitoring ;
  skos:prefLabel "Doping detection research"@en ;
  skos:related agift:Medical-and-health-sciences ;
.
agift:Draft-Bill-amendment-process
  a skos:Concept ;
  dcterms:contributor "KOdea" ;
  dcterms:created "2016-07-06T04:41:25+00:00"^^xsd:dateTime ;
  dcterms:creator "superadmin" ;
  dcterms:modified "2016-09-09T05:49:06+00:00"^^xsd:dateTime ;
  skos:broader agift:Legislative-drafting ;
  skos:definition "Revising and modifying proposed legal instruments, during their passage through parliament. Incorporating changes in government policy and other developments."@en ;
  skos:prefLabel "Draft Bill amendment process"@en ;
  skos:related agift:Legislation-review ;
  skos:related agift:Parliamentary-papers ;
  skos:related agift:Tabling-of-official-documents ;
.
agift:Driving-licences-administration
  a skos:Concept ;
  dcterms:contributor "KOdea" ;
  dcterms:created "2016-07-06T05:16:03+00:00"^^xsd:dateTime ;
  dcterms:creator "superadmin" ;
  dcterms:modified "2016-09-13T07:22:04+00:00"^^xsd:dateTime ;
  skos:altLabel "Driver's licenses"@en ;
  skos:broader agift:Road-transport ;
  skos:definition "Managing the system to approve applications to operate various types of motor vehicles. Testing drivers, issuing or renewing permits and licenses. Includes variation, suspension and cancellation of licenses, administering demerit points and liaison to promote consistency across jurisdictions."@en ;
  skos:prefLabel "Driving licences administration"@en ;
  skos:related agift:Road-safety-awareness ;
  skos:related agift:Road-traffic-regulation ;
  skos:related agift:Road-transport-safety ;
  skos:related agift:Vehicle-standards ;
.
agift:Drugs-and-poisons-regulation
  a skos:Concept ;
  dcterms:contributor "KOdea" ;
  dcterms:created "2016-07-06T04:45:29+00:00"^^xsd:dateTime ;
  dcterms:creator "superadmin" ;
  dcterms:modified "2016-09-09T06:12:14+00:00"^^xsd:dateTime ;
  skos:altLabel "Medicine regulation"@en ;
  skos:altLabel "Pharmaceutical regulation"@en ;
  skos:altLabel "Poisons regulation"@en ;
  skos:broader agift:Health-protocol-administration ;
  skos:definition "Monitoring substances used for medicinal purposes, which may have toxic or lethal effects if administered incorrectly or in large doses. Maintaining a register of approved substances. Assessing product applications and manufacturing quality. Restricting the availability of drugs or poisons, and specifying conditions of use."@en ;
  skos:prefLabel "Drugs and poisons regulation"@en ;
  skos:related agift:Chemical-and-pesticide-regulation ;
.
agift:EDUCATION-AND-TRAINING
  a skos:Concept ;
  dcterms:contributor "KOdea" ;
  dcterms:created "2016-07-06T02:45:11+00:00"^^xsd:dateTime ;
  dcterms:creator "superadmin" ;
  dcterms:modified "2016-09-09T07:08:50+00:00"^^xsd:dateTime ;
  skos:altLabel "Teachers"@en ;
  skos:altLabel "Teaching"@en ;
  skos:definition "Formulating policy to support programs that provide skills and knowledge to citizens. Developing strategies to make education available to the broadest possible cross-section of the community. Providing funding to schools, universities, colleges, academies or community groups that provide education and training. Establishing programs to develop and manage educational institutions."@en ;
  skos:narrower agift:Arts-education ;
  skos:narrower agift:Community-education ;
  skos:narrower agift:Curriculum-development ;
  skos:narrower agift:Early-childhood-education ;
  skos:narrower agift:Military-education-and-training ;
  skos:narrower agift:Overseas-skills-recognition ;
  skos:narrower agift:School-education ;
  skos:narrower agift:Tertiary-education ;
  skos:narrower agift:Vocational-education ;
  skos:prefLabel "EDUCATION AND TRAINING"@en ;
  skos:related agift:Overseas-student-scholarship-programs ;
  skos:topConceptOf agift:AGIFT ;
.
agift:EMPLOYMENT
  a skos:Concept ;
  dcterms:contributor "KOdea" ;
  dcterms:created "2016-07-06T02:45:21+00:00"^^xsd:dateTime ;
  dcterms:creator "superadmin" ;
  dcterms:modified "2016-09-09T06:01:04+00:00"^^xsd:dateTime ;
  skos:altLabel "Industrial relations"@en ;
  skos:altLabel "Public service employment"@en ;
  skos:altLabel "Workplace management"@en ;
  skos:altLabel "Workplace relations"@en ;
  skos:definition "Formulating policy to support employment growth and regulate public or private sector working environments. Developing strategies to improve workplace relations, productivity and performance. Implementing labour market programs and providing funding. Administering regulatory bodies and arbitration services."@en ;
  skos:narrower agift:Human-resources-development ;
  skos:narrower agift:Industrial-awards-and-conditions ;
  skos:narrower agift:Labour-market-programs ;
  skos:narrower agift:Workplace-agreement-processes ;
  skos:prefLabel "EMPLOYMENT"@en ;
  skos:related agift:Public-service ;
  skos:related agift:Vocational-education ;
  skos:topConceptOf agift:AGIFT ;
.
agift:ENVIRONMENT
  a skos:Concept ;
  dcterms:contributor "KOdea" ;
  dcterms:created "2016-07-06T02:45:29+00:00"^^xsd:dateTime ;
  dcterms:creator "superadmin" ;
  dcterms:modified "2016-09-12T06:08:45+00:00"^^xsd:dateTime ;
  skos:altLabel "Environmental monitoring"@en ;
  skos:definition "Developing policy to support the management of the surrounding natural and built environments. Balancing competing requirements to generate long term sustainable benefits for industry, tourism and the community. Protecting elements of the natural and built environment that are of special significance. Includes conservation of the national estate and world heritage concerns."@en ;
  skos:narrower agift:Built-environment ;
  skos:narrower agift:Climate-information-services ;
  skos:narrower agift:Conservation-programs ;
  skos:narrower agift:Environmental-impact-assessment ;
  skos:narrower agift:Historic-relic-protection ;
  skos:narrower agift:Marine-life-protection-programs ;
  skos:narrower agift:Natural-heritage-protection ;
  skos:narrower agift:Oceans-governance ;
  skos:narrower agift:Pollutant-prevention-programs ;
  skos:narrower agift:World-heritage-listings ;
  skos:prefLabel "ENVIRONMENT"@en ;
  skos:related agift:Marine-and-rural-regulation ;
  skos:related agift:NATURAL-RESOURCES ;
  skos:related agift:Water-conservation-plans ;
  skos:related agift:Waterway-management ;
  skos:topConceptOf agift:AGIFT ;
.
agift:Early-childhood-education
  a skos:Concept ;
  dcterms:contributor "KOdea" ;
  dcterms:created "2016-07-06T03:00:15+00:00"^^xsd:dateTime ;
  dcterms:creator "superadmin" ;
  dcterms:modified "2016-09-08T07:11:41+00:00"^^xsd:dateTime ;
  skos:altLabel "Kindergarten education"@en ;
  skos:altLabel "Preschool education"@en ;
  skos:broader agift:EDUCATION-AND-TRAINING ;
  skos:definition "Administering learning programs and related services designed to foster the development of young children, usually under the age of five years. Implementing standards and guidelines to support teachers. Includes determining enrolment criteria."@en ;
  skos:prefLabel "Early childhood education"@en ;
  skos:related agift:Child-and-youth-support ;
  skos:related agift:Child-care-services ;
  skos:related agift:School-education ;
.
agift:Earth-sciences
  a skos:Concept ;
  dcterms:contributor "KOdea" ;
  dcterms:created "2016-07-06T03:43:17+00:00"^^xsd:dateTime ;
  dcterms:creator "superadmin" ;
  dcterms:modified "2016-09-12T05:59:58+00:00"^^xsd:dateTime ;
  skos:altLabel "Geography"@en ;
  skos:altLabel "Geological sciences"@en ;
  skos:altLabel "Geology"@en ;
  skos:broader agift:SCIENCE ;
  skos:definition "Conducting research into geological, water and atmospheric processes. Providing scientific advice on the sustainable management of land and water resources, exploitation of mineral resources, hazard and disaster assessment."@en ;
  skos:narrower agift:Atmospheric-sciences ;
  skos:narrower agift:Hydrology ;
  skos:narrower agift:Mineral-exploration ;
  skos:narrower agift:Oceanography ;
  skos:narrower agift:Seismology ;
  skos:prefLabel "Earth sciences"@en ;
  skos:related agift:Mining-regulations ;
.
agift:Economic-research
  a skos:Concept ;
  dcterms:contributor "KOdea" ;
  dcterms:created "2016-07-06T03:04:04+00:00"^^xsd:dateTime ;
  dcterms:creator "superadmin" ;
  dcterms:modified "2016-09-08T07:56:49+00:00"^^xsd:dateTime ;
  skos:altLabel "Economic modelling"@en ;
  skos:broader agift:FINANCE-MANAGEMENT ;
  skos:definition "Developing new economic measurements and models, estimating quantitative models of economic behaviour, assessing the effects of public policies on the Australian economy, and projecting the effects of alternative policy proposals."@en ;
  skos:prefLabel "Economic research"@en ;
  skos:related agift:Financial-system-management ;
  skos:related agift:Fiscal-policy ;
  skos:related agift:Monetary-policy ;
.
agift:Election-campaigning
  a skos:Concept ;
  dcterms:contributor "KOdea" ;
  dcterms:created "2016-07-06T04:40:22+00:00"^^xsd:dateTime ;
  dcterms:creator "superadmin" ;
  dcterms:modified "2016-09-09T05:42:45+00:00"^^xsd:dateTime ;
  skos:altLabel "Political campaigning"@en ;
  skos:broader agift:Electoral-matters ;
  skos:definition "Regulating the presentation of policies and platforms by election candidates and political parties. Providing advice on the content of television and newspaper advertisements, media reporting, distribution of pamphlets, shopping centre tours and door-to-door canvassing. Establishing eligibility criteria for parliamentary and non-parliamentary parties, and the nomination and registration of political parties."@en ;
  skos:prefLabel "Election campaigning"@en ;
  skos:related agift:Advertising-standards ;
  skos:related agift:Government-media ;
.
agift:Electoral-boundary-assessment
  a skos:Concept ;
  dcterms:contributor "KOdea" ;
  dcterms:created "2016-07-06T04:40:31+00:00"^^xsd:dateTime ;
  dcterms:creator "superadmin" ;
  dcterms:modified "2016-08-22T06:47:05+00:00"^^xsd:dateTime ;
  skos:altLabel "Electorates"@en ;
  skos:altLabel "Gerrymander prevention"@en ;
  skos:altLabel "Redistribution Committee"@en ;
  skos:broader agift:Electoral-matters ;
  skos:definition "Assessing and reviewing the margins of electoral divisions to maintain equal representation. Assessing population projection figures, conducting quota calculations and public consultation. Publicising final boundary determinations."@en ;
  skos:prefLabel "Electoral boundary assessment"@en ;
.
agift:Electoral-matters
  a skos:Concept ;
  dcterms:contributor "KOdea" ;
  dcterms:created "2016-07-06T03:05:47+00:00"^^xsd:dateTime ;
  dcterms:creator "superadmin" ;
  dcterms:modified "2016-09-09T05:41:22+00:00"^^xsd:dateTime ;
  skos:broader agift:GOVERNANCE ;
  skos:definition "Administering voting to elect representatives for public office. Conducting referenda to amend the constitution. Maintaining electoral rolls and enrolment procedures. Providing polling booths, ballot papers and scrutiny of electoral processes. Distributing the results of elections via any medium. Includes electoral information and education programs."@en ;
  skos:narrower agift:Declaration-of-interests ;
  skos:narrower agift:Election-campaigning ;
  skos:narrower agift:Electoral-boundary-assessment ;
  skos:prefLabel "Electoral matters"@en ;
  skos:related agift:Constitutional-referenda ;
.
agift:Electronic-commerce
  a skos:Concept ;
  dcterms:contributor "KOdea" ;
  dcterms:created "2016-07-06T02:53:43+00:00"^^xsd:dateTime ;
  dcterms:creator "superadmin" ;
  dcterms:modified "2016-09-05T07:37:16+00:00"^^xsd:dateTime ;
  skos:altLabel "Digital commerce"@en ;
  skos:altLabel "E-Business"@en ;
  skos:altLabel "E-Commerce"@en ;
  skos:altLabel "Information economy"@en ;
  skos:altLabel "Internet commerce"@en ;
  skos:altLabel "Online commerce"@en ;
  skos:broader agift:COMMUNICATIONS ;
  skos:definition "Developing policy to support and regulate Australian participation in the global information economy. Administering programs to promote the implementation of information and communications technology for conducting business. Providing funding to foster initiatives in electronic commerce."@en ;
  skos:narrower agift:Authentication ;
  skos:narrower agift:Online-transaction-standards ;
  skos:prefLabel "Electronic commerce"@en ;
  skos:related agift:Cybersafety ;
  skos:related agift:Internet ;
.
agift:Electronic-postal-services
  a skos:Concept ;
  dcterms:contributor "KOdea" ;
  dcterms:created "2016-07-06T03:58:51+00:00"^^xsd:dateTime ;
  dcterms:creator "superadmin" ;
  dcterms:modified "2016-08-05T05:44:26+00:00"^^xsd:dateTime ;
  skos:altLabel "Internet postal services"@en ;
  skos:broader agift:Postal-services ;
  skos:definition "Administering special services through the postal communications network. Providing electronic transactions such as banking, bill payments and business lodgements. Managing electronic mail processing activities, such as barcoding and postcode scanning mechanisms."@en ;
  skos:prefLabel "Electronic postal services"@en ;
.
agift:Electronic-publishing
  a skos:Concept ;
  dcterms:contributor "KOdea" ;
  dcterms:created "2016-07-06T03:59:21+00:00"^^xsd:dateTime ;
  dcterms:creator "superadmin" ;
  dcterms:modified "2016-09-05T07:47:09+00:00"^^xsd:dateTime ;
  skos:broader agift:Publishing ;
  skos:definition "Compiling, editing and disseminating government information in electronic form. Developing website content and multi-media programs."@en ;
  skos:prefLabel "Electronic publishing"@en ;
  skos:related agift:Government-media ;
  skos:related agift:Information-dissemination ;
  skos:related agift:Website-development ;
.
agift:Emergency-accommodation
  a skos:Concept ;
  dcterms:contributor "KOdea" ;
  dcterms:created "2016-07-06T04:01:41+00:00"^^xsd:dateTime ;
  dcterms:creator "superadmin" ;
  dcterms:modified "2016-09-08T06:52:14+00:00"^^xsd:dateTime ;
  skos:broader agift:Accommodation-services ;
  skos:definition "Managing services to provide housing for the community in the event of crisis or disaster. Assisting individuals and families following a house fire, natural disaster, or other emergency. Includes accommodation placements in government and non-government housing."@en ;
  skos:prefLabel "Emergency accommodation"@en ;
  skos:related agift:Disaster-relief ;
  skos:related agift:Emergency-funding ;
  skos:related agift:Emergency-management ;
  skos:related agift:Emergency-services ;
.
agift:Emergency-funding
  a skos:Concept ;
  dcterms:contributor "KOdea" ;
  dcterms:created "2016-07-06T04:03:18+00:00"^^xsd:dateTime ;
  dcterms:creator "superadmin" ;
  dcterms:modified "2016-09-06T07:52:03+00:00"^^xsd:dateTime ;
  skos:altLabel "Disaster funds"@en ;
  skos:altLabel "Emergency funds"@en ;
  skos:broader agift:Emergency-services ;
  skos:definition "Managing financial resources allocated for the provision of emergency services. Includes receiving revenue, investing funds and making payments to eligible organisations."@en ;
  skos:prefLabel "Emergency funding"@en ;
  skos:related agift:Disaster-relief ;
  skos:related agift:Emergency-accommodation ;
  skos:related agift:Emergency-management ;
  skos:related agift:Natural-disasters ;
.
agift:Emergency-management
  a skos:Concept ;
  dcterms:contributor "KOdea" ;
  dcterms:created "2016-07-06T02:59:03+00:00"^^xsd:dateTime ;
  dcterms:creator "superadmin" ;
  dcterms:modified "2016-09-12T06:48:29+00:00"^^xsd:dateTime ;
  skos:altLabel "Counter-terrorism activities"@en ;
  skos:altLabel "Emergencies"@en ;
  skos:altLabel "Martial law"@en ;
  skos:altLabel "National emergency"@en ;
  skos:altLabel "State of emergency"@en ;
  skos:altLabel "Terrorism"@en ;
  skos:broader agift:DEFENCE ;
  skos:definition "Managing cross-jurisdictional operations to deal with large-scale crises. Developing policy and strategies for emergency prevention, response and recovery. Coordinating services and resources to provide a comprehensive and integrated emergency management framework."@en ;
  skos:narrower agift:Civil-community-assistance ;
  skos:narrower agift:Disaster-support ;
  skos:prefLabel "Emergency management"@en ;
  skos:related agift:Ambulance-services ;
  skos:related agift:Emergency-accommodation ;
  skos:related agift:Emergency-funding ;
  skos:related agift:Emergency-services ;
  skos:related agift:External-security ;
  skos:related agift:Firefighting-services ;
  skos:related agift:Health-disaster-preparedness ;
  skos:related agift:Law-enforcement ;
  skos:related agift:Military-law ;
  skos:related agift:Natural-disasters ;
  skos:related agift:Search-and-rescue ;
  skos:related agift:Special-operations ;
.
agift:Emergency-services
  a skos:Concept ;
  dcterms:contributor "KOdea" ;
  dcterms:created "2016-07-06T02:55:54+00:00"^^xsd:dateTime ;
  dcterms:creator "superadmin" ;
  dcterms:modified "2016-09-06T07:31:30+00:00"^^xsd:dateTime ;
  skos:altLabel "Carelink"@en ;
  skos:broader agift:COMMUNITY-SERVICES ;
  skos:definition "Managing programs to provide urgent assistance in times of crisis or unforeseen circumstances. Monitoring compliance with equipment standards and regulating the use of volunteers. Coordinating government and community-based services within a region, in times of emergency. Includes land-based search and rescue operations outside urban areas."@en ;
  skos:narrower agift:Ambulance-services ;
  skos:narrower agift:Emergency-funding ;
  skos:narrower agift:Firefighting-services ;
  skos:prefLabel "Emergency services"@en ;
  skos:related agift:Emergency-accommodation ;
  skos:related agift:Emergency-management ;
  skos:related agift:Firefighting-services ;
  skos:related agift:Health-disaster-preparedness ;
  skos:related agift:Law-enforcement ;
  skos:related agift:Natural-disasters ;
  skos:related agift:Rescue-coordination ;
.
agift:Employment-advocacy-services
  a skos:Concept ;
  dcterms:contributor "KOdea" ;
  dcterms:created "2016-07-06T04:23:12+00:00"^^xsd:dateTime ;
  dcterms:creator "superadmin" ;
  dcterms:modified "2016-08-19T07:26:34+00:00"^^xsd:dateTime ;
  skos:altLabel "Advocacy services"@en ;
  skos:altLabel "Workplace advocacy services"@en ;
  skos:broader agift:Workplace-agreement-processes ;
  skos:definition "Providing workplace relations information to employers and employees. Offering advice on rights and obligations, union membership or the implications of industrial action. Developing guidance for the negotiation and implementation of workplace agreements."@en ;
  skos:prefLabel "Employment advocacy services"@en ;
.
agift:Employment-services-marketing
  a skos:Concept ;
  dcterms:contributor "KOdea" ;
  dcterms:created "2016-07-06T04:22:09+00:00"^^xsd:dateTime ;
  dcterms:creator "superadmin" ;
  dcterms:modified "2016-09-08T07:31:06+00:00"^^xsd:dateTime ;
  skos:altLabel "Employment marketing"@en ;
  skos:altLabel "Job creation programs"@en ;
  skos:altLabel "Job search"@en ;
  skos:altLabel "JobSearch"@en ;
  skos:altLabel "Supported wages"@en ;
  skos:altLabel "VolunteerSearch"@en ;
  skos:altLabel "Wage assistance"@en ;
  skos:broader agift:Labour-market-programs ;
  skos:definition "Administering programs that encourage and assist businesses to employ more staff. Liaising with employers to evaluate their needs for support. Providing information and resources to help locate suitable staff. Managing wage assistance and subsidy schemes. Includes promotional strategies and advertising campaigns to advocate employment in particular industries."@en ;
  skos:prefLabel "Employment services marketing"@en ;
  skos:related agift:Industry-collaboration ;
  skos:related agift:Vocational-education ;
.
agift:Endangered-species-protection
  a skos:Concept ;
  dcterms:contributor "KOdea" ;
  dcterms:created "2016-07-06T04:33:05+00:00"^^xsd:dateTime ;
  dcterms:creator "superadmin" ;
  dcterms:modified "2016-09-08T07:40:36+00:00"^^xsd:dateTime ;
  skos:altLabel "Rare species"@en ;
  skos:altLabel "Threatened species"@en ;
  skos:altLabel "Vulnerable species"@en ;
  skos:broader agift:Conservation-programs ;
  skos:definition "Identifying groups of plants or animals that are under threat or at risk of extinction. Evaluating the source of the danger, whether direct harm to individual organisms or the indirect impacts of environmental change. Administering programs to protect and repopulate specific areas. Includes liaison with national parks, scientific research bodies and community groups."@en ;
  skos:prefLabel "Endangered species protection"@en ;
  skos:related agift:Wilderness-area-management ;
  skos:related agift:Wildlife-sanctuary-management ;
.
agift:Energy-resources
  a skos:Concept ;
  dcterms:contributor "fionamcl" ;
  dcterms:created "2016-07-06T03:40:42+00:00"^^xsd:dateTime ;
  dcterms:creator "superadmin" ;
  dcterms:modified "2016-09-20T00:08:13+00:00"^^xsd:dateTime ;
  skos:altLabel "Electricity"@en ;
  skos:altLabel "Fuel prices"@en ;
  skos:altLabel "Nuclear energy"@en ;
  skos:broader agift:NATURAL-RESOURCES ;
  skos:definition "Developing policy and administering legislation relating to fossil fuels, renewable and other energy industries. Providing advice on energy market reform, research and development, and environmental assessments."@en ;
  skos:narrower agift:Fossil-fuel-management ;
  skos:narrower agift:Renewable-energy-development ;
  skos:prefLabel "Energy resources"@en ;
  skos:related agift:Energy-supply ;
  skos:related agift:SCIENCE ;
.
agift:Energy-supply
  a skos:Concept ;
  dcterms:contributor "KOdea" ;
  dcterms:created "2016-07-06T02:51:29+00:00"^^xsd:dateTime ;
  dcterms:creator "superadmin" ;
  dcterms:modified "2016-09-12T06:01:19+00:00"^^xsd:dateTime ;
  skos:altLabel "Electricity services"@en ;
  skos:altLabel "Gas services"@en ;
  skos:altLabel "Public utilities management"@en ;
  skos:altLabel "Water services"@en ;
  skos:broader agift:CIVIC-INFRASTRUCTURE ;
  skos:definition "Regulating the provision of energy resources and other utilities. Installing infrastructure to facilitate energy supply. Monitoring providers to ensure all citizens receive an adequate level of service to meet basic requirements. Encouraging consumers to conserve energy, and to support renewable energy development."@en ;
  skos:prefLabel "Energy supply"@en ;
  skos:related agift:Energy-resources ;
  skos:related agift:Prices-surveillance ;
  skos:related agift:Water-resources ;
.
agift:Engineering-and-technology-sciences
  a skos:Concept ;
  dcterms:contributor "KOdea" ;
  dcterms:created "2016-07-06T05:03:31+00:00"^^xsd:dateTime ;
  dcterms:creator "superadmin" ;
  dcterms:modified "2016-09-13T07:11:31+00:00"^^xsd:dateTime ;
  skos:altLabel "Chemical engineering"@en ;
  skos:altLabel "Electrical engineering"@en ;
  skos:altLabel "Information technology"@en ;
  skos:altLabel "Mechanical engineering"@en ;
  skos:altLabel "Software engineering"@en ;
  skos:altLabel "Systems engineering"@en ;
  skos:altLabel "Technology research"@en ;
  skos:broader agift:Applied-sciences ;
  skos:definition "Conducting research into the practical application of scientific knowledge for systematic design, construction and management activities. Developing products and processes to support industry, communications, defence and civic infrastructure. Includes component analysis, design and manipulation of systems to solve complex problems."@en ;
  skos:prefLabel "Engineering and technology sciences"@en ;
  skos:related agift:Aircraft-standards ;
  skos:related agift:Defence-science-and-technology ;
  skos:related agift:Engineering-services ;
  skos:related agift:Genetic-engineering ;
  skos:related agift:Intellectual-property-management ;
  skos:related agift:Mathematical-sciences ;
.
agift:Engineering-services
  a skos:Concept ;
  dcterms:contributor "KOdea" ;
  dcterms:created "2016-07-06T03:53:34+00:00"^^xsd:dateTime ;
  dcterms:creator "superadmin" ;
  dcterms:modified "2016-09-13T07:22:37+00:00"^^xsd:dateTime ;
  skos:altLabel "Civil engineering"@en ;
  skos:broader agift:Civic-management ;
  skos:definition "Providing professional advice and supervising the design and construction of public works, such as roads, bridges, dams or harbours. Approving plans and conducting inspections to ensure building is completed in accordance with approved plans."@en ;
  skos:prefLabel "Engineering services"@en ;
  skos:related agift:Architectural-services ;
  skos:related agift:Building-regulations-and-standards ;
  skos:related agift:Engineering-and-technology-sciences ;
  skos:related agift:Transport-infrastructure-development ;
.
agift:Entomology
  a skos:Concept ;
  dcterms:contributor "KOdea" ;
  dcterms:created "2016-07-06T05:04:21+00:00"^^xsd:dateTime ;
  dcterms:creator "superadmin" ;
  dcterms:modified "2016-09-12T06:32:01+00:00"^^xsd:dateTime ;
  skos:broader agift:Biological-sciences ;
  skos:definition "Conducting research into insects and their management by understanding the role of insects and other invertebrates in the natural, urban and rural environments. Developing safe, sustainable methods of pest management."@en ;
  skos:prefLabel "Entomology"@en ;
  skos:related agift:Animal-and-veterinary-sciences ;
  skos:related agift:Chemical-and-pesticide-regulation ;
.
agift:Environmental-impact-assessment
  a skos:Concept ;
  dcterms:contributor "KOdea" ;
  dcterms:created "2016-07-06T03:02:46+00:00"^^xsd:dateTime ;
  dcterms:creator "superadmin" ;
  dcterms:modified "2016-09-12T05:59:34+00:00"^^xsd:dateTime ;
  skos:broader agift:ENVIRONMENT ;
  skos:definition "Evaluating the effects of industry, tourism or community use on the natural and built environments. Conducting inspections of premises, equipment or operations. Providing advice on proposed infrastructure projects, commercial or residential developments. Includes emergency assessments following industrial accidents or natural disasters."@en ;
  skos:prefLabel "Environmental impact assessment"@en ;
  skos:related agift:Mining-regulations ;
.
agift:Epidemiology
  a skos:Concept ;
  dcterms:contributor "KOdea" ;
  dcterms:created "2016-07-06T04:47:46+00:00"^^xsd:dateTime ;
  dcterms:creator "superadmin" ;
  dcterms:modified "2016-09-09T06:20:18+00:00"^^xsd:dateTime ;
  skos:broader agift:Public-health-services ;
  skos:definition "Administering programs to identify and prevent the large-scale outbreak of disease. Conducting research into the presence of communicable diseases and their distribution within the population. Developing strategies to monitor the incidence of infection and predict a possible epidemic."@en ;
  skos:prefLabel "Epidemiology"@en ;
  skos:related agift:Medical-and-health-sciences ;
  skos:related agift:Notifiable-disease-management ;
  skos:related agift:Population-based-research ;
.
agift:Equipment-licensing
  a skos:Concept ;
  dcterms:contributor "KOdea" ;
  dcterms:created "2016-07-06T04:00:45+00:00"^^xsd:dateTime ;
  dcterms:creator "superadmin" ;
  dcterms:modified "2016-08-05T05:59:49+00:00"^^xsd:dateTime ;
  skos:altLabel "Equipment licenses"@en ;
  skos:broader agift:Telecommunications ;
  skos:definition "Processing applications and issuing licenses for telecommunications equipment, such as transmitters, wireless rooftop links or cable capacity. Drafting licence conditions. Establishing standards for connecting or labelling telecommunications equipment."@en ;
  skos:prefLabel "Equipment licensing"@en ;
.
agift:Ethical-compliance
  a skos:Concept ;
  dcterms:contributor "KOdea" ;
  dcterms:created "2016-07-06T03:43:26+00:00"^^xsd:dateTime ;
  dcterms:creator "superadmin" ;
  dcterms:modified "2016-08-30T06:43:49+00:00"^^xsd:dateTime ;
  skos:altLabel "Research ethics"@en ;
  skos:broader agift:SCIENCE ;
  skos:definition "Administering programs to ensure research is carried out in an acceptable manner. Assessing research methods against accepted moral principles and standards of conduct. Monitoring activities, performing inspections and handling complaints."@en ;
  skos:prefLabel "Ethical compliance"@en ;
.
agift:Exchange-rates
  a skos:Concept ;
  dcterms:contributor "KOdea" ;
  dcterms:created "2016-07-06T04:37:04+00:00"^^xsd:dateTime ;
  dcterms:creator "superadmin" ;
  dcterms:modified "2016-08-22T06:09:45+00:00"^^xsd:dateTime ;
  skos:altLabel "Currency rates"@en ;
  skos:altLabel "Foreign exchange rates"@en ;
  skos:altLabel "International exchange rates"@en ;
  skos:altLabel "Money rates"@en ;
  skos:broader agift:Monetary-policy ;
  skos:definition "Monitoring the value of the Australian dollar currency against the value of other currencies. Forecasting the consequences and economic impact of fluctuations in exchange rates. Developing strategies to minimise those effects."@en ;
  skos:prefLabel "Exchange rates"@en ;
.
agift:Exhibition-programs
  skos:prefLabel "Exhibition programs"@en ;
  owl:deprecated true ;
.
agift:Exhibition-programs
  a skos:Concept ;
  dcterms:contributor "fionamcl" ;
  dcterms:created "2016-09-08T01:41:27+00:00"^^xsd:dateTime ;
  dcterms:creator "fionamcl" ;
  dcterms:modified "2016-11-28T22:48:13+00:00"^^xsd:dateTime ;
  skos:altLabel "Displays and exhibitions"@en ;
  skos:broader agift:Collection-promotion ;
  skos:definition "Planning and implementing displays of material from cultural collections. Conducting research and selecting items for inclusion in displays. Identifying relevant material in other collections. Ensuring installations meet preservation requirements."@en ;
  skos:prefLabel "Exhibition programs"@en ;
  skos:related agift:Collection-acquisition ;
  skos:related agift:Publicity-programs ;
.
agift:Export-promotion
  a skos:Concept ;
  dcterms:contributor "KOdea" ;
  dcterms:created "2016-07-06T05:12:32+00:00"^^xsd:dateTime ;
  dcterms:creator "superadmin" ;
  dcterms:modified "2016-09-13T06:56:56+00:00"^^xsd:dateTime ;
  skos:altLabel "Export incentives"@en ;
  skos:broader agift:Export-regulation ;
  skos:definition "Promoting Australian businesses in the global marketplace. Developing long term sustainable exports and diversifying markets through grants schemes. Providing export advice and statistics. Includes conducting promotional programs overseas to enhance the awareness and image of Australian products."@en ;
  skos:prefLabel "Export promotion"@en ;
  skos:related agift:Arts-development ;
  skos:related agift:Overseas-promotion ;
  skos:related agift:Trade-expositions ;
.
agift:Export-regulation
  a skos:Concept ;
  dcterms:contributor "KOdea" ;
  dcterms:created "2016-07-06T03:48:00+00:00"^^xsd:dateTime ;
  dcterms:creator "superadmin" ;
  dcterms:modified "2016-09-13T06:56:19+00:00"^^xsd:dateTime ;
  skos:altLabel "Export monitoring"@en ;
  skos:broader agift:TRADE ;
  skos:definition "Controlling the international sale and movement of goods from Australia. Ensuring compliance with domestic and international protocols and guidelines. Issuing export permits and licences, directing price regulation at port terminals and exit points. Includes monitoring international trade and consulting with primary producers, industry organisations and other stakeholders."@en ;
  skos:narrower agift:Export-promotion ;
  skos:narrower agift:Prohibited-export-control ;
  skos:prefLabel "Export regulation"@en ;
  skos:related agift:Cargo-control ;
  skos:related agift:Freight-movement-regulation ;
  skos:related agift:Port-regulation ;
.
agift:External-security
  a skos:Concept ;
  dcterms:contributor "KOdea" ;
  dcterms:created "2016-07-06T03:44:29+00:00"^^xsd:dateTime ;
  dcterms:creator "superadmin" ;
  dcterms:modified "2016-09-12T06:58:42+00:00"^^xsd:dateTime ;
  skos:altLabel "International security liaison"@en ;
  skos:altLabel "International security"@en ;
  skos:broader agift:SECURITY ;
  skos:definition "Developing policy and procedures to protect Australia's international security interests Implementing strategies to maintain peace in external territories and the region. Evaluating risks to Australian citizens, territories and property overseas. Includes liaison with international security and law enforcement bodies."@en ;
  skos:narrower agift:Peacekeeping-forces ;
  skos:prefLabel "External security"@en ;
  skos:related agift:Defence-liaison ;
  skos:related agift:Emergency-management ;
  skos:related agift:Intelligence ;
  skos:related agift:International-affairs ;
.
agift:FINANCE-MANAGEMENT
  a skos:Concept ;
  dcterms:contributor "KOdea" ;
  dcterms:created "2016-07-06T02:45:37+00:00"^^xsd:dateTime ;
  dcterms:creator "superadmin" ;
  dcterms:modified "2016-08-22T05:46:04+00:00"^^xsd:dateTime ;
  skos:altLabel "Financial policy"@en ;
  skos:definition "Developing policy for the administration of public funds and other resources. Determining appropriate strategies for raising revenue and regulating expenditure. Monitoring economic indicators and forecasting trends to enable financial planning."@en ;
  skos:narrower agift:Commonwealth-State-funding ;
  skos:narrower agift:Currency ;
  skos:narrower agift:Economic-research ;
  skos:narrower agift:Financial-investment ;
  skos:narrower agift:Financial-system-management ;
  skos:narrower agift:Fiscal-policy ;
  skos:narrower agift:Foreign-investment-control ;
  skos:narrower agift:International-monetary-regulation ;
  skos:narrower agift:Monetary-policy ;
  skos:narrower agift:Resource-management ;
  skos:narrower agift:Retirement-income ;
  skos:narrower agift:Taxation ;
  skos:prefLabel "FINANCE MANAGEMENT"@en ;
  skos:topConceptOf agift:AGIFT ;
.
agift:Fair-trading-compliance
  a skos:Concept ;
  dcterms:contributor "KOdea" ;
  dcterms:created "2016-07-06T02:49:53+00:00"^^xsd:dateTime ;
  dcterms:creator "superadmin" ;
  dcterms:modified "2016-09-05T06:24:18+00:00"^^xsd:dateTime ;
  skos:altLabel "Commerce"@en ;
  skos:altLabel "Fair trading"@en ;
  skos:altLabel "Industry code"@en ;
  skos:altLabel "Market regulation"@en ;
  skos:altLabel "Trade Practices Act"@en ;
  skos:broader agift:BUSINESS-SUPPORT-AND-REGULATION ;
  skos:definition "Developing policy to ensure the ethical conduct of business, and protect consumers from excessive prices or faulty products. Promoting trading practices that support market competition."@en ;
  skos:narrower agift:Prices-surveillance ;
  skos:narrower agift:Product-safety ;
  skos:narrower agift:Trade-practices-compliance ;
  skos:prefLabel "Fair trading compliance"@en ;
  skos:related agift:Business-sponsorship ;
  skos:related agift:Consumer-protection ;
.
agift:Family-law-proceedings
  a skos:Concept ;
  dcterms:contributor "KOdea" ;
  dcterms:created "2016-07-06T04:56:16+00:00"^^xsd:dateTime ;
  dcterms:creator "superadmin" ;
  dcterms:modified "2016-09-09T07:20:54+00:00"^^xsd:dateTime ;
  skos:altLabel "Child custody"@en ;
  skos:altLabel "Child support"@en ;
  skos:altLabel "Custody proceedings"@en ;
  skos:altLabel "Divorce proceedings"@en ;
  skos:altLabel "Divorce settlements"@en ;
  skos:altLabel "Family courts"@en ;
  skos:altLabel "Family support"@en ;
  skos:broader agift:Civil-law ;
  skos:definition "Administering the body of law relating to the rights of parents and their children, especially during break-up of the family unit. Hearing matters of divorce, custody and child support."@en ;
  skos:prefLabel "Family law proceedings"@en ;
  skos:related agift:Income-support-schemes ;
.
agift:Family-reunion-programs
  a skos:Concept ;
  dcterms:contributor "KOdea" ;
  dcterms:created "2016-07-06T04:02:43+00:00"^^xsd:dateTime ;
  dcterms:creator "superadmin" ;
  dcterms:modified "2016-09-09T06:37:54+00:00"^^xsd:dateTime ;
  skos:altLabel "Child migration schemes"@en ;
  skos:altLabel "Family research"@en ;
  skos:altLabel "Indigenous family reunion services"@en ;
  skos:altLabel "Link up programs"@en ;
  skos:altLabel "Separated families"@en ;
  skos:altLabel "Stolen generations"@en ;
  skos:broader agift:Community-support ;
  skos:definition "Assisting groups and individuals to locate and contact relatives from whom they have become separated. Helping reunite birth parents and adopted children. Providing referral and research services to Indigenous and other families separated by foster programs or migration schemes."@en ;
  skos:prefLabel "Family reunion programs"@en ;
  skos:related agift:Adoption-services ;
  skos:related agift:Indigenous-welfare-programs ;
  skos:related agift:Migrant-services ;
  skos:related agift:Migrant-settlement-programs ;
.
agift:Feral-pest-control
  a skos:Concept ;
  dcterms:contributor "KOdea" ;
  dcterms:created "2016-07-06T04:33:53+00:00"^^xsd:dateTime ;
  dcterms:creator "superadmin" ;
  dcterms:modified "2016-09-08T07:44:54+00:00"^^xsd:dateTime ;
  skos:broader agift:Natural-heritage-protection ;
  skos:definition "Operating programs to remove feral animals and  plants from national parks and wilderness areas."@en ;
  skos:prefLabel "Feral pest control"@en ;
  skos:related agift:National-park-management ;
  skos:related agift:Nature-reserve-management ;
  skos:related agift:Wilderness-area-management ;
.
agift:Financial-administration
  a skos:Concept ;
  dcterms:contributor "KOdea" ;
  dcterms:created "2016-07-06T04:37:49+00:00"^^xsd:dateTime ;
  dcterms:creator "superadmin" ;
  dcterms:modified "2016-09-08T08:01:58+00:00"^^xsd:dateTime ;
  skos:broader agift:Resource-management ;
  skos:definition "Developing procedures to control the income and expenditure of government organisations. Making payments to employees and suppliers. Managing revenue generated by sales of goods or services. Includes financial planning activities."@en ;
  skos:prefLabel "Financial administration"@en ;
  skos:related agift:Financial-budgeting ;
.
agift:Financial-assistance
  a skos:Concept ;
  dcterms:contributor "KOdea" ;
  dcterms:created "2016-07-06T02:56:02+00:00"^^xsd:dateTime ;
  dcterms:creator "superadmin" ;
  dcterms:modified "2016-09-12T06:13:46+00:00"^^xsd:dateTime ;
  skos:altLabel "Social security"@en ;
  skos:altLabel "Welfare payments"@en ;
  skos:broader agift:COMMUNITY-SERVICES ;
  skos:definition "Developing policy and programs to provide monetary support to individuals. Setting eligibility criteria and determining appropriate delivery mechanisms for providing financial assistance. Making payments and setting policy on entitlements for those in the community in need. Includes ongoing and one-off payments following a specific event."@en ;
  skos:narrower agift:Benefits ;
  skos:narrower agift:Income-support-schemes ;
  skos:prefLabel "Financial assistance"@en ;
  skos:related agift:Aged-care-services ;
  skos:related agift:Asset-assessment ;
  skos:related agift:Child-care-services ;
  skos:related agift:Disaster-relief ;
  skos:related agift:Income-support-schemes ;
  skos:related agift:Indigenous-welfare-programs ;
  skos:related agift:Marine-and-rural-support ;
  skos:related agift:Public-housing-entitlements ;
  skos:related agift:Taxation ;
  skos:related agift:Taxation-compliance ;
  skos:related agift:Transport-access-schemes ;
  skos:related agift:Veterans-entitlements ;
.
agift:Financial-budgeting
  a skos:Concept ;
  dcterms:contributor "KOdea" ;
  dcterms:created "2016-07-06T04:37:58+00:00"^^xsd:dateTime ;
  dcterms:creator "superadmin" ;
  dcterms:modified "2016-09-08T08:01:58+00:00"^^xsd:dateTime ;
  skos:altLabel "Accounting"@en ;
  skos:altLabel "Budget"@en ;
  skos:altLabel "Financial statements"@en ;
  skos:broader agift:Resource-management ;
  skos:definition "Providing estimates and documentation for the annual budgeting cycle. Preparing financial statements to justify the allocation of resources. Accounting for expenditure and forecasting revenues"@en ;
  skos:prefLabel "Financial budgeting"@en ;
  skos:related agift:Financial-administration ;
  skos:related agift:Fiscal-policy ;
  skos:related agift:Public-expenditure ;
.
agift:Financial-institutions-regulation
  a skos:Concept ;
  dcterms:contributor "KOdea" ;
  dcterms:created "2016-07-06T02:50:02+00:00"^^xsd:dateTime ;
  dcterms:creator "superadmin" ;
  dcterms:modified "2016-09-05T06:27:25+00:00"^^xsd:dateTime ;
  skos:altLabel "ADI regulation"@en ;
  skos:altLabel "Authorised Deposit-Taking Institutions regulation"@en ;
  skos:altLabel "Authorised capital regulation"@en ;
  skos:altLabel "Banking regulation"@en ;
  skos:altLabel "Banks"@en ;
  skos:altLabel "Building society regulation"@en ;
  skos:altLabel "Credit union regulation"@en ;
  skos:altLabel "Friendly society regulation"@en ;
  skos:altLabel "Provident society regulation"@en ;
  skos:altLabel "Prudential regulation"@en ;
  skos:broader agift:BUSINESS-SUPPORT-AND-REGULATION ;
  skos:definition "Developing policy to control banks, credit unions, building societies and friendly societies. Establishing rules for capital adequacy. Monitoring the activities of financial institutions. Investigating suspected breaches of prudential regulations and applying penalties when appropriate."@en ;
  skos:prefLabel "Financial institutions regulation"@en ;
  skos:related agift:Financial-investment ;
  skos:related agift:Insurance-regulation ;
  skos:related agift:Retirement-income ;
.
agift:Financial-investment
  a skos:Concept ;
  dcterms:contributor "KOdea" ;
  dcterms:created "2016-07-06T03:04:11+00:00"^^xsd:dateTime ;
  dcterms:creator "superadmin" ;
  dcterms:modified "2016-09-08T07:54:47+00:00"^^xsd:dateTime ;
  skos:altLabel "Investment control"@en ;
  skos:altLabel "Investment"@en ;
  skos:broader agift:FINANCE-MANAGEMENT ;
  skos:definition "Developing policy to encourage safe and legitimate investment practices. Maintaining prudential oversight of financial instruments and participants in financial markets. Setting penalties for breaches of prudential regulations relating to investment."@en ;
  skos:narrower agift:Investment-scheme-regulation ;
  skos:prefLabel "Financial investment"@en ;
  skos:related agift:Financial-institutions-regulation ;
  skos:related agift:Insurance-regulation ;
  skos:related agift:Superannuation-regulation ;
.
agift:Financial-system-management
  a skos:Concept ;
  dcterms:contributor "KOdea" ;
  dcterms:created "2016-07-06T03:04:19+00:00"^^xsd:dateTime ;
  dcterms:creator "superadmin" ;
  dcterms:modified "2016-09-08T07:55:42+00:00"^^xsd:dateTime ;
  skos:broader agift:FINANCE-MANAGEMENT ;
  skos:definition "Developing policy to maintain stability in the financial system. Includes managing arrangements that allow consumers, business, other organisations, and financial institutions to transfer funds from one to another."@en ;
  skos:narrower agift:Financial-system-monitoring ;
  skos:narrower agift:Payments-management ;
  skos:prefLabel "Financial system management"@en ;
  skos:related agift:Economic-research ;
  skos:related agift:Productivity ;
.
agift:Financial-system-monitoring
  a skos:Concept ;
  dcterms:contributor "KOdea" ;
  dcterms:created "2016-07-06T04:36:00+00:00"^^xsd:dateTime ;
  dcterms:creator "superadmin" ;
  dcterms:modified "2016-09-08T07:56:49+00:00"^^xsd:dateTime ;
  skos:altLabel "Financial reporting standards"@en ;
  skos:altLabel "Financial system standards"@en ;
  skos:broader agift:Financial-system-management ;
  skos:definition "Developing policy to maintain stability in the financial system. Developing strategies to counteract the effects of instability."@en ;
  skos:prefLabel "Financial system monitoring"@en ;
.
agift:Finding-aids-development
  skos:prefLabel "Finding aids development"@en ;
  owl:deprecated true ;
.
agift:Finding-aids-development
  a skos:Concept ;
  dcterms:contributor "fionamcl" ;
  dcterms:created "2016-09-08T01:29:18+00:00"^^xsd:dateTime ;
  dcterms:creator "fionamcl" ;
  dcterms:modified "2016-11-28T22:46:54+00:00"^^xsd:dateTime ;
  skos:altLabel "Catalogue development"@en ;
  skos:altLabel "Cataloguing"@en ;
  skos:altLabel "Classification schemes"@en ;
  skos:altLabel "Collection description"@en ;
  skos:altLabel "Guide development"@en ;
  skos:altLabel "Indexing"@en ;
  skos:broader agift:Collection-access ;
  skos:definition "Creating tools to promote and enable access to items in cultural collections. Researching and developing content for guides, information sheets or websites. Preparing entries for catalogues, indexes and databases."@en ;
  skos:prefLabel "Finding aids development"@en ;
  skos:related agift:Collection-accessioning ;
  skos:related agift:Descriptive-standards ;
  skos:related agift:Reference-services ;
.
agift:Firefighting-services
  a skos:Concept ;
  dcterms:contributor "KOdea" ;
  dcterms:created "2016-07-06T04:03:30+00:00"^^xsd:dateTime ;
  dcterms:creator "superadmin" ;
  dcterms:modified "2016-09-09T07:38:43+00:00"^^xsd:dateTime ;
  skos:altLabel "Bushfire prevention"@en ;
  skos:altLabel "Fire brigade"@en ;
  skos:altLabel "Fire fighting"@en ;
  skos:altLabel "Fire prevention programs"@en ;
  skos:altLabel "Hazardous materials management"@en ;
  skos:altLabel "Hazardous waste management"@en ;
  skos:altLabel "Urban search and rescue"@en ;
  skos:broader agift:Emergency-services ;
  skos:definition "Providing specially equipped vehicles and trained personnel to prevent, control or extinguish fires. Conducting urban search and rescue operations and managing hazardous materials incidents. Includes managing fire stations, attendance at special events and support for community-based or volunteer fire fighting services."@en ;
  skos:prefLabel "Firefighting services"@en ;
  skos:related agift:Community-education ;
  skos:related agift:Emergency-management ;
  skos:related agift:Emergency-services ;
  skos:related agift:Natural-disasters ;
  skos:related agift:Rescue-coordination ;
  skos:related agift:Search-and-rescue ;
.
agift:Fiscal-policy
  a skos:Concept ;
  dcterms:contributor "KOdea" ;
  dcterms:created "2016-07-06T03:04:25+00:00"^^xsd:dateTime ;
  dcterms:creator "superadmin" ;
  dcterms:modified "2016-09-08T07:57:38+00:00"^^xsd:dateTime ;
  skos:broader agift:FINANCE-MANAGEMENT ;
  skos:definition "Developing policy for the strategic management and distribution of public money. Determining overall levels of public spending required to maintain economic stability. Regulating public borrowing and levels of public debt."@en ;
  skos:narrower agift:Public-borrowing ;
  skos:narrower agift:Public-debt ;
  skos:narrower agift:Public-expenditure ;
  skos:prefLabel "Fiscal policy"@en ;
  skos:related agift:Economic-research ;
  skos:related agift:Financial-budgeting ;
  skos:related agift:Productivity ;
.
agift:Fisheries-industry
  a skos:Concept ;
  dcterms:contributor "KOdea" ;
  dcterms:created "2016-07-06T05:01:53+00:00"^^xsd:dateTime ;
  dcterms:creator "superadmin" ;
  dcterms:modified "2016-09-12T06:16:06+00:00"^^xsd:dateTime ;
  skos:altLabel "Bycatch regulation"@en ;
  skos:altLabel "Fishing industry regulation"@en ;
  skos:altLabel "Seafood industry regulation"@en ;
  skos:broader agift:Marine-and-rural-regulation ;
  skos:definition "Regulating recreational fishing practices and commercial fishing industries. Administering quotas and issuing licenses for controlled activities. Certifying products and methods of catching or harvesting. Conducting assessments and inspections to ensure compliance with standards and policy. Applying penalties for breaches of regulations."@en ;
  skos:prefLabel "Fisheries industry"@en ;
  skos:related agift:Animal-and-veterinary-sciences ;
  skos:related agift:Aquaculture-industry ;
  skos:related agift:Oceans-governance ;
.
agift:Food-hygiene-regulation
  a skos:Concept ;
  dcterms:contributor "KOdea" ;
  dcterms:created "2016-07-06T04:45:36+00:00"^^xsd:dateTime ;
  dcterms:creator "superadmin" ;
  dcterms:modified "2016-09-09T06:13:09+00:00"^^xsd:dateTime ;
  skos:altLabel "Food safety"@en ;
  skos:altLabel "Meat inspection"@en ;
  skos:broader agift:Health-protocol-administration ;
  skos:definition "Administering programs to ensure food is produced and handled without risk of contamination. Evaluating performance against established standards and codes of practice. Investigating complaints and initiating disciplinary proceedings or applying penalties when appropriate. Includes product recall or closure of premises found in breach of regulations."@en ;
  skos:prefLabel "Food hygiene regulation"@en ;
  skos:related agift:Food-quality-assurance ;
  skos:related agift:Health-promotion ;
  skos:related agift:Medical-and-health-sciences ;
.
agift:Food-quality-assurance
  a skos:Concept ;
  dcterms:contributor "KOdea" ;
  dcterms:created "2016-07-06T05:02:00+00:00"^^xsd:dateTime ;
  dcterms:creator "superadmin" ;
  dcterms:modified "2016-09-12T06:12:27+00:00"^^xsd:dateTime ;
  skos:altLabel "Australian food industry"@en ;
  skos:altLabel "Food industry regulation"@en ;
  skos:altLabel "Food standards code"@en ;
  skos:broader agift:Marine-and-rural-regulation ;
  skos:definition "Regulating food and beverage production industries. Administering labelling and packaging requirements. Certifying products and methods of production or processing. Conducting assessments and inspections to ensure compliance with standards and policy. Applying penalties for breaches of regulations."@en ;
  skos:prefLabel "Food quality assurance"@en ;
  skos:related agift:Biotechnology-development ;
  skos:related agift:Chemical-and-pesticide-regulation ;
  skos:related agift:Food-hygiene-regulation ;
  skos:related agift:Genetic-engineering ;
.
agift:Foreign-investment-control
  a skos:Concept ;
  dcterms:contributor "KOdea" ;
  dcterms:created "2016-07-06T03:04:32+00:00"^^xsd:dateTime ;
  dcterms:creator "superadmin" ;
  dcterms:modified "2016-09-08T07:59:44+00:00"^^xsd:dateTime ;
  skos:altLabel "Foreign investment review"@en ;
  skos:altLabel "International investment control"@en ;
  skos:altLabel "Investment management"@en ;
  skos:altLabel "Overseas investment control"@en ;
  skos:broader agift:FINANCE-MANAGEMENT ;
  skos:definition "Regulating the participation of overseas parties in Australian commercial or financial ventures. Restricting the ownership of Australian assets by foreigners. Includes advice to Australian governments entering into partnerships with foreign investors."@en ;
  skos:prefLabel "Foreign investment control"@en ;
.
agift:Forensic-analysis
  a skos:Concept ;
  dcterms:contributor "KOdea" ;
  dcterms:created "2016-07-06T05:07:05+00:00"^^xsd:dateTime ;
  dcterms:creator "superadmin" ;
  dcterms:modified "2016-08-30T07:15:37+00:00"^^xsd:dateTime ;
  skos:altLabel "Computer forensics"@en ;
  skos:altLabel "Criminal forensics"@en ;
  skos:altLabel "Forensic medicine"@en ;
  skos:broader agift:Intelligence ;
  skos:definition "Applying investigative strategies and technologies to gather intelligence or evidence that may be used in a court of law. Analysing available information to reach a conclusion and identifying data that will substantiate the results."@en ;
  skos:prefLabel "Forensic analysis"@en ;
.
agift:Forestry-industry
  a skos:Concept ;
  dcterms:contributor "KOdea" ;
  dcterms:created "2016-07-06T05:02:07+00:00"^^xsd:dateTime ;
  dcterms:creator "superadmin" ;
  dcterms:modified "2016-09-12T06:12:58+00:00"^^xsd:dateTime ;
  skos:altLabel "Regional Forest Agreements"@en ;
  skos:altLabel "Timber industry regulation"@en ;
  skos:altLabel "Wood products industry"@en ;
  skos:broader agift:Marine-and-rural-regulation ;
  skos:definition "Regulating timber cultivation industries. Administering quotas and issuing licenses for controlled activities. Certifying products and methods of growing or harvesting. Conducting assessments and inspections to ensure compliance with standards and policy. Applying penalties for breaches of regulations."@en ;
  skos:prefLabel "Forestry industry"@en ;
  skos:related agift:Agricultural-sciences ;
  skos:related agift:Silvicultural-industry ;
.
agift:Fossil-fuel-management
  a skos:Concept ;
  dcterms:contributor "KOdea" ;
  dcterms:created "2016-07-06T04:59:56+00:00"^^xsd:dateTime ;
  dcterms:creator "superadmin" ;
  dcterms:modified "2016-09-12T05:53:44+00:00"^^xsd:dateTime ;
  skos:altLabel "Coal"@en ;
  skos:altLabel "Gas resources"@en ;
  skos:altLabel "Natural gas resources"@en ;
  skos:altLabel "Oil resources"@en ;
  skos:altLabel "Petroleum resources"@en ;
  skos:broader agift:Energy-resources ;
  skos:definition "Regulating the exploitation of coal, oil and natural gas resources. Licensing infrastructure and operational activities. Conducting exploration and mapping deposits of fossil fuels. Granting acreage release for vacant onshore, offshore and coastal areas."@en ;
  skos:prefLabel "Fossil fuel management"@en ;
  skos:related agift:Mineral-exploration ;
  skos:related agift:Mineral-resources ;
.
agift:Freedom-of-information
  a skos:Concept ;
  dcterms:contributor "KOdea" ;
  dcterms:created "2016-07-06T04:54:54+00:00"^^xsd:dateTime ;
  dcterms:creator "superadmin" ;
  dcterms:modified "2016-09-09T07:16:53+00:00"^^xsd:dateTime ;
  skos:altLabel "FOI"@en ;
  skos:broader agift:Administrative-law ;
  skos:definition "Allowing individuals to see what information government holds about them, and to seek correction of that information if they consider it wrong or misleading. Requiring agencies to publish government information and  providing for a right of access by the public to government documents."@en ;
  skos:prefLabel "Freedom of information"@en ;
  skos:related agift:Open-government ;
  skos:related agift:Privacy ;
  skos:related agift:Recordkeeping-standards ;
.
agift:Freight-movement-regulation
  a skos:Concept ;
  dcterms:contributor "KOdea" ;
  dcterms:created "2016-07-06T03:49:38+00:00"^^xsd:dateTime ;
  dcterms:creator "superadmin" ;
  dcterms:modified "2016-09-13T07:20:28+00:00"^^xsd:dateTime ;
  skos:altLabel "Freight control"@en ;
  skos:altLabel "Freight"@en ;
  skos:altLabel "Hazardous materials management"@en ;
  skos:altLabel "Hazardous waste management"@en ;
  skos:broader agift:TRANSPORT ;
  skos:definition "Developing policy for the transportation of goods by air, rail or road. Monitoring compliance with regulations for carriage of hazardous materials, dangerous goods and oversize containers. Includes advice on best practice logistics and standardised freight movement across jurisdictions."@en ;
  skos:prefLabel "Freight movement regulation"@en ;
  skos:related agift:Air-transport ;
  skos:related agift:Cargo-control ;
  skos:related agift:Export-regulation ;
  skos:related agift:Import-regulation ;
  skos:related agift:Rail-transport ;
  skos:related agift:Road-transport-safety ;
.
agift:Fundraising-and-donation-schemes
  a skos:Concept ;
  dcterms:contributor "KOdea" ;
  dcterms:created "2016-07-06T05:09:51+00:00"^^xsd:dateTime ;
  dcterms:creator "superadmin" ;
  dcterms:modified "2016-09-13T06:42:05+00:00"^^xsd:dateTime ;
  skos:altLabel "Donation schemes"@en ;
  skos:altLabel "Sports funding"@en ;
  skos:broader agift:Sport-and-fitness-development ;
  skos:definition "Administering programs to encourage investment in sporting events. Visiting individuals and corporations to request gifts, contributions or sponsorship. Providing advice on advertising opportunities, donation of prizes, tax incentives and bequests."@en ;
  skos:prefLabel "Fundraising and donation schemes"@en ;
  skos:related agift:Business-association ;
  skos:related agift:Business-registration-and-licensing ;
  skos:related agift:Business-sponsorship ;
  skos:related agift:Games-administration ;
  skos:related agift:Games-promotion ;
.
agift:GOVERNANCE
  a skos:Concept ;
  dcterms:contributor "KOdea" ;
  dcterms:created "2016-07-06T02:45:44+00:00"^^xsd:dateTime ;
  dcterms:creator "superadmin" ;
  dcterms:modified "2016-08-22T06:37:23+00:00"^^xsd:dateTime ;
  skos:altLabel "City councils"@en ;
  skos:altLabel "Councils"@en ;
  skos:altLabel "Federal government"@en ;
  skos:altLabel "Government"@en ;
  skos:altLabel "Houses of parliament"@en ;
  skos:altLabel "Local government"@en ;
  skos:altLabel "Shire councils"@en ;
  skos:altLabel "State government"@en ;
  skos:altLabel "Territory government"@en ;
  skos:definition "Executing legislative processes in Houses of Parliament, assemblies or councils, where officers are elected to represent citizens. Administering committees that report to legislative bodies. Managing elections of government representatives and sponsoring major community celebrations. Includes official duties carried out by the titular head of the government or municipality. Includes managing the machinery of government processes at all levels of government."@en ;
  skos:narrower agift:Appointment-management ;
  skos:narrower agift:Civic-celebrations ;
  skos:narrower agift:Constitutional-matters ;
  skos:narrower agift:Electoral-matters ;
  skos:narrower agift:Honours-and-awards-programs ;
  skos:narrower agift:Intergovernmental-relations ;
  skos:narrower agift:Legislative-drafting ;
  skos:narrower agift:Official-protocol ;
  skos:narrower agift:Open-government ;
  skos:narrower agift:Parliamentary-chamber-support ;
  skos:narrower agift:Parliamentary-committee-and-member-support ;
  skos:narrower agift:Public-administration ;
  skos:prefLabel "GOVERNANCE"@en ;
  skos:topConceptOf agift:AGIFT ;
.
agift:Gambling-support-services
  a skos:Concept ;
  dcterms:contributor "KOdea" ;
  dcterms:created "2016-07-06T05:08:59+00:00"^^xsd:dateTime ;
  dcterms:creator "superadmin" ;
  dcterms:modified "2016-09-13T06:31:00+00:00"^^xsd:dateTime ;
  skos:altLabel "Gambling addiction"@en ;
  skos:altLabel "Gambling services"@en ;
  skos:broader agift:Community-recreational-programs ;
  skos:definition "Administering programs to assist people with compulsive betting problems or gambling addictions. Providing services such as group support and positive reinforcement activities. Arranging access to counselling for gamblers and their families. Includes community information services and advice to the gaming industry."@en ;
  skos:prefLabel "Gambling support services"@en ;
  skos:related agift:Counselling-services ;
  skos:related agift:Gaming-industry-regulation ;
.
agift:Games-administration
  a skos:Concept ;
  dcterms:contributor "KOdea" ;
  dcterms:created "2016-07-06T05:09:57+00:00"^^xsd:dateTime ;
  dcterms:creator "superadmin" ;
  dcterms:modified "2016-09-13T06:42:23+00:00"^^xsd:dateTime ;
  skos:altLabel "Commonwealth Games administration"@en ;
  skos:altLabel "Olympic Games administration"@en ;
  skos:altLabel "Sporting event administration"@en ;
  skos:broader agift:Sport-and-fitness-development ;
  skos:definition "Organising and managing major sporting events. Strategic planning and coordination of activities. Liaising with sporting bodies, sponsors, volunteers and organising committees. Arranging access to venues or facilities and overseeing tenders and infrastructure development."@en ;
  skos:prefLabel "Games administration"@en ;
  skos:related agift:Fundraising-and-donation-schemes ;
  skos:related agift:Games-promotion ;
  skos:related agift:Sport-and-fitness-development ;
  skos:related agift:Volunteer-support-programs ;
.
agift:Games-promotion
  a skos:Concept ;
  dcterms:contributor "KOdea" ;
  dcterms:created "2016-07-06T05:10:08+00:00"^^xsd:dateTime ;
  dcterms:creator "superadmin" ;
  dcterms:modified "2016-09-13T06:52:13+00:00"^^xsd:dateTime ;
  skos:altLabel "Commonwealth Games promotion"@en ;
  skos:altLabel "Olympic Games promotion"@en ;
  skos:altLabel "Sporting event promotion"@en ;
  skos:broader agift:Sport-and-fitness-development ;
  skos:definition "Developing advertising campaigns for major sporting events. Organising strategic marketing activities to reach target audiences. Liaising with sponsors, journalists and the media, locally and internationally."@en ;
  skos:prefLabel "Games promotion"@en ;
  skos:related agift:Fundraising-and-donation-schemes ;
  skos:related agift:Games-administration ;
  skos:related agift:Overseas-promotion ;
  skos:related agift:Tourist-event-promotion ;
.
agift:Gaming-industry-regulation
  a skos:Concept ;
  dcterms:contributor "KOdea" ;
  dcterms:created "2016-07-06T03:45:37+00:00"^^xsd:dateTime ;
  dcterms:creator "superadmin" ;
  dcterms:modified "2016-09-13T06:31:00+00:00"^^xsd:dateTime ;
  skos:altLabel "Casino regulation"@en ;
  skos:altLabel "Gambling industry"@en ;
  skos:altLabel "Greyhound racing"@en ;
  skos:altLabel "Horse racing"@en ;
  skos:altLabel "Poker machine licensing"@en ;
  skos:broader agift:SPORT-AND-RECREATION ;
  skos:definition "Monitoring gambling and betting activities to ensure compliance with legislation. Conducting audits of accounts, procedures and machines in organisations with gaming facilities. Issuing licences and providing training to licence holders. Promoting responsible gambling practices and allocating revenue from gaming activities to community projects."@en ;
  skos:prefLabel "Gaming industry regulation"@en ;
  skos:related agift:Business-registration-and-licensing ;
  skos:related agift:Gambling-support-services ;
.
agift:Garden-management
  a skos:Concept ;
  dcterms:contributor "KOdea" ;
  dcterms:created "2016-07-06T03:55:15+00:00"^^xsd:dateTime ;
  dcterms:creator "superadmin" ;
  dcterms:modified "2016-09-13T06:31:47+00:00"^^xsd:dateTime ;
  skos:altLabel "Botanic gardens"@en ;
  skos:altLabel "Community gardens"@en ;
  skos:broader agift:Public-land-management ;
  skos:definition "Administering public land where ornamental or useful plants are cultivated. Managing site layout, planting and landscaping. Ensuring facilities are kept clean and maintained. Monitoring rights of access and opening hours. Organising seasonal public events"@en ;
  skos:prefLabel "Garden management"@en ;
  skos:related agift:National-park-management ;
  skos:related agift:Nature-reserve-management ;
  skos:related agift:Park-and-reserve-services ;
  skos:related agift:Recreational-park-management ;
  skos:related agift:Wilderness-area-management ;
.
agift:General-insurance
  a skos:Concept ;
  dcterms:contributor "KOdea" ;
  dcterms:created "2016-07-06T03:51:59+00:00"^^xsd:dateTime ;
  dcterms:creator "superadmin" ;
  dcterms:modified "2016-09-09T06:11:06+00:00"^^xsd:dateTime ;
  skos:altLabel "Accident insurance"@en ;
  skos:altLabel "Business insurance"@en ;
  skos:altLabel "Car insurance"@en ;
  skos:altLabel "Contents insurance"@en ;
  skos:altLabel "Fire insurance"@en ;
  skos:altLabel "Home insurance"@en ;
  skos:altLabel "Indemnity insurance"@en ;
  skos:altLabel "Private health insurance"@en ;
  skos:altLabel "Travel insurance"@en ;
  skos:broader agift:Insurance-regulation ;
  skos:definition "Monitoring the activities of general insurance providers to ensure compliance with government policy and standards. Investigating suspected breaches of prudential regulations and applying penalties when appropriate."@en ;
  skos:prefLabel "General insurance"@en ;
  skos:related agift:Health-insurance-schemes ;
  skos:related agift:Life-insurance ;
.
agift:Genetic-engineering
  a skos:Concept ;
  dcterms:contributor "KOdea" ;
  dcterms:created "2016-07-06T05:04:30+00:00"^^xsd:dateTime ;
  dcterms:creator "superadmin" ;
  dcterms:modified "2016-09-12T06:33:07+00:00"^^xsd:dateTime ;
  skos:altLabel "Gene sciences"@en ;
  skos:altLabel "Genetic modification"@en ;
  skos:broader agift:Biological-sciences ;
  skos:definition "Conducting research into the chromosome structure of reproductive cells. Copying, modifying and transferring genetic material to produce or reduce biological products, traits and characteristics in animals or plants. Includes health and environmental impact studies for genetically modified organisms (GMOs)."@en ;
  skos:prefLabel "Genetic engineering"@en ;
  skos:related agift:Agricultural-sciences ;
  skos:related agift:Biochemistry ;
  skos:related agift:Biotechnology-development ;
  skos:related agift:Engineering-and-technology-sciences ;
  skos:related agift:Food-quality-assurance ;
  skos:related agift:Intellectual-property-management ;
.
agift:Government-auditing
  a skos:Concept ;
  dcterms:contributor "KOdea" ;
  dcterms:created "2016-07-06T04:43:39+00:00"^^xsd:dateTime ;
  dcterms:creator "superadmin" ;
  dcterms:modified "2016-09-09T06:00:43+00:00"^^xsd:dateTime ;
  skos:broader agift:Public-administration ;
  skos:definition "Reviewing the financial or performance management of a government organisation or entity and reporting findings to the legislative body."@en ;
  skos:prefLabel "Government auditing"@en ;
  skos:related agift:Business-process-auditing ;
  skos:related agift:Corruption-prevention ;
  skos:related agift:Integrity-compliance ;
  skos:related agift:Whistleblowing ;
.
agift:Government-media
  a skos:Concept ;
  dcterms:contributor "KOdea" ;
  dcterms:created "2016-07-06T02:53:50+00:00"^^xsd:dateTime ;
  dcterms:creator "superadmin" ;
  dcterms:modified "2016-09-13T06:53:56+00:00"^^xsd:dateTime ;
  skos:altLabel "Government advertising"@en ;
  skos:altLabel "Government communications"@en ;
  skos:altLabel "Media releases"@en ;
  skos:altLabel "Public relations"@en ;
  skos:broader agift:COMMUNICATIONS ;
  skos:definition "Managing government advertising and communications activities. Developing advertisements and advertising campaign material. Includes production of media releases, public notices, commercial and employment opportunities."@en ;
  skos:prefLabel "Government media"@en ;
  skos:related agift:Advertising-campaigns ;
  skos:related agift:Community-engagement ;
  skos:related agift:Election-campaigning ;
  skos:related agift:Electronic-publishing ;
  skos:related agift:Government-procurement-regulation ;
  skos:related agift:Information-dissemination ;
  skos:related agift:Publicity-programs ;
  skos:related agift:Publishing ;
  skos:related agift:Recruitment-programs ;
  skos:related agift:Social-media ;
.
agift:Government-procurement-regulation
  a skos:Concept ;
  dcterms:contributor "KOdea" ;
  dcterms:created "2016-07-06T02:50:10+00:00"^^xsd:dateTime ;
  dcterms:creator "superadmin" ;
  dcterms:modified "2016-09-05T07:28:58+00:00"^^xsd:dateTime ;
  skos:altLabel "Endorsed Supplier Arrangements"@en ;
  skos:altLabel "Government purchasing"@en ;
  skos:altLabel "Government tendering"@en ;
  skos:altLabel "Preferred supplier arrangements"@en ;
  skos:altLabel "Procurement policy"@en ;
  skos:altLabel "Purchasing"@en ;
  skos:altLabel "Request for Proposal"@en ;
  skos:altLabel "Tender management"@en ;
  skos:broader agift:BUSINESS-SUPPORT-AND-REGULATION ;
  skos:definition "Administering the processes of tendering and awarding government contracts for the provision of goods and services. Developing policy and guidelines to direct procurement activities. Managing preferred supplier arrangements."@en ;
  skos:prefLabel "Government procurement regulation"@en ;
  skos:related agift:Government-media ;
  skos:related agift:Resource-management ;
.
agift:HEALTH-CARE
  a skos:Concept ;
  dcterms:contributor "KOdea" ;
  dcterms:created "2016-07-06T02:45:53+00:00"^^xsd:dateTime ;
  dcterms:creator "superadmin" ;
  dcterms:modified "2016-08-23T06:06:58+00:00"^^xsd:dateTime ;
  skos:altLabel "Health services"@en ;
  skos:definition "Providing and coordinating programs for the prevention, diagnosis and treatment of disease or injury. Developing policy to support the provision of health care services and medical research. Administering regulatory schemes for health care products and pharmaceuticals."@en ;
  skos:narrower agift:Community-health-services ;
  skos:narrower agift:Health-insurance-schemes ;
  skos:narrower agift:Health-protocol-administration ;
  skos:narrower agift:Hospital-services ;
  skos:narrower agift:Medical-research ;
  skos:narrower agift:Public-health-services ;
  skos:narrower agift:Special-needs-services ;
  skos:narrower agift:Veterans-health-services ;
  skos:prefLabel "HEALTH CARE"@en ;
  skos:topConceptOf agift:AGIFT ;
.
agift:Hansard-services
  a skos:Concept ;
  dcterms:contributor "KOdea" ;
  dcterms:created "2016-07-06T04:43:00+00:00"^^xsd:dateTime ;
  dcterms:creator "superadmin" ;
  dcterms:modified "2016-09-09T07:21:49+00:00"^^xsd:dateTime ;
  skos:altLabel "Parliamentary proceedings"@en ;
  skos:broader agift:Parliamentary-chamber-support ;
  skos:definition "Producing the official record of the proceedings of Parliament. Documenting the debates and speeches of Members, public and private hearings and parliamentary committees. Transcribing and publishing proceedings in paper and electronic format. Managing databases of Hansard reports. Includes all chambers in all levels of government."@en ;
  skos:prefLabel "Hansard services"@en ;
  skos:related agift:Court-reporting ;
  skos:related agift:Parliamentary-committee-and-member-support ;
.
agift:Harbour-management
  a skos:Concept ;
  dcterms:contributor "KOdea" ;
  dcterms:created "2016-07-06T03:39:15+00:00"^^xsd:dateTime ;
  dcterms:creator "superadmin" ;
  dcterms:modified "2016-09-12T06:04:36+00:00"^^xsd:dateTime ;
  skos:altLabel "Breakwaters"@en ;
  skos:altLabel "Sea walls"@en ;
  skos:broader agift:MARITIME-SERVICES ;
  skos:definition "Building and maintaining infrastructure to provide protection for ships from wind, waves and currents. Developing policy for commercial and recreational use of harbour facilities, and monitoring the environmental impact of activities. Includes liaison to promote coordination and consistency among harbour authorities from different jurisdictions."@en ;
  skos:prefLabel "Harbour management"@en ;
  skos:related agift:Marina-management ;
  skos:related agift:Oceans-governance ;
  skos:related agift:Port-regulation ;
  skos:related agift:Waterway-management ;
.
agift:Head-of-Government-protocol
  a skos:Concept ;
  dcterms:contributor "KOdea" ;
  dcterms:created "2016-07-06T04:42:15+00:00"^^xsd:dateTime ;
  dcterms:creator "superadmin" ;
  dcterms:modified "2016-09-09T05:52:45+00:00"^^xsd:dateTime ;
  skos:altLabel "Governor-General's protocol"@en ;
  skos:altLabel "Lord Mayor's protocol"@en ;
  skos:altLabel "Mayoral protocol"@en ;
  skos:altLabel "Premier's protocol"@en ;
  skos:altLabel "Prime Ministerial protocol"@en ;
  skos:altLabel "Vice regal protocol"@en ;
  skos:broader agift:Official-protocol ;
  skos:definition "Organising the activities of Heads of Government in carrying out their constitutional, statutory, ceremonial and public duties. Making arrangements to support official protocol such as dress code, official decoration, customs and procedures."@en ;
  skos:prefLabel "Head of Government protocol"@en ;
  skos:related agift:Ceremonial-events-and-representation ;
  skos:related agift:Official-establishment-management ;
  skos:related agift:Official-hospitality ;
  skos:related agift:Official-visits ;
.
agift:Health-disaster-preparedness
  a skos:Concept ;
  dcterms:contributor "KOdea" ;
  dcterms:created "2016-07-06T04:47:52+00:00"^^xsd:dateTime ;
  dcterms:creator "superadmin" ;
  dcterms:modified "2016-09-09T06:21:06+00:00"^^xsd:dateTime ;
  skos:altLabel "Health contingency"@en ;
  skos:altLabel "Health disasters"@en ;
  skos:broader agift:Public-health-services ;
  skos:definition "Developing strategies to handle a large-scale medical emergency. Planning a coordinated counter-disaster response to and recovery from health disasters. Ensuring adequate supplies of drugs and blood, and the availability of medical equipment and trained personnel."@en ;
  skos:prefLabel "Health disaster preparedness"@en ;
  skos:related agift:Emergency-management ;
  skos:related agift:Emergency-services ;
  skos:related agift:Medical-quarantine-services ;
  skos:related agift:Notifiable-disease-management ;
.
agift:Health-hazard-prevention
  a skos:Concept ;
  dcterms:contributor "KOdea" ;
  dcterms:created "2016-07-06T04:47:58+00:00"^^xsd:dateTime ;
  dcterms:creator "superadmin" ;
  dcterms:modified "2016-09-09T06:05:29+00:00"^^xsd:dateTime ;
  skos:altLabel "Anti-smoking campaigns"@en ;
  skos:altLabel "Biosafety"@en ;
  skos:altLabel "Drug and alcohol awareness"@en ;
  skos:altLabel "Early detection"@en ;
  skos:altLabel "Health risk management"@en ;
  skos:altLabel "Manual handling standards"@en ;
  skos:altLabel "Needle disposal"@en ;
  skos:altLabel "Passive smoking guidelines"@en ;
  skos:altLabel "Repetitive strain injury"@en ;
  skos:broader agift:Public-health-services ;
  skos:definition "Managing programs to reduce public exposure to health risks. Developing campaigns to raise community awareness of dangerous substances or potential sources of injury. Establishing standards and guidelines to protect individuals who come into contact with hazardous substances or environments."@en ;
  skos:prefLabel "Health hazard prevention"@en ;
  skos:related agift:Health-promotion ;
  skos:related agift:Occupational-health-and-safety ;
.
agift:Health-insurance-schemes
  a skos:Concept ;
  dcterms:contributor "KOdea" ;
  dcterms:created "2016-07-06T03:07:12+00:00"^^xsd:dateTime ;
  dcterms:creator "superadmin" ;
  dcterms:modified "2016-09-09T06:11:32+00:00"^^xsd:dateTime ;
  skos:altLabel "Medical indemnity"@en ;
  skos:altLabel "Medical insurance"@en ;
  skos:altLabel "Medicare"@en ;
  skos:altLabel "Pharmaceutical benefits"@en ;
  skos:altLabel "Public health insurance"@en ;
  skos:broader agift:HEALTH-CARE ;
  skos:definition "Administering programs that provide financial guarantees against risk of disease or injury. Developing policy to support the operation of universal health insurance schemes, allowing subsidised medical treatment within the public health system."@en ;
  skos:prefLabel "Health insurance schemes"@en ;
  skos:related agift:Benefits ;
  skos:related agift:General-insurance ;
  skos:related agift:Workers-compensation-schemes ;
.
agift:Health-promotion
  a skos:Concept ;
  dcterms:contributor "KOdea" ;
  dcterms:created "2016-07-06T04:45:03+00:00"^^xsd:dateTime ;
  dcterms:creator "superadmin" ;
  dcterms:modified "2016-09-13T06:29:41+00:00"^^xsd:dateTime ;
  skos:altLabel "Consumers health forum"@en ;
  skos:altLabel "Food and nutrition"@en ;
  skos:altLabel "Health information"@en ;
  skos:altLabel "Healthy eating"@en ;
  skos:altLabel "Nutrition advice"@en ;
  skos:altLabel "Safe sex awareness"@en ;
  skos:altLabel "Sanitation advice"@en ;
  skos:broader agift:Community-health-services ;
  skos:definition "Administering information programs to improve the physical and mental wellbeing of individuals in the community. Developing campaigns to encourage activities that result in good health. Providing advice on basic aspects of health care, and disease or injury prevention."@en ;
  skos:prefLabel "Health promotion"@en ;
  skos:related agift:Adult-education-programs ;
  skos:related agift:Child-and-youth-support ;
  skos:related agift:Food-hygiene-regulation ;
  skos:related agift:Health-hazard-prevention ;
  skos:related agift:Primary-health-care ;
  skos:related agift:Public-fitness-promotion ;
  skos:related agift:School-education ;
.
agift:Health-protocol-administration
  a skos:Concept ;
  dcterms:contributor "KOdea" ;
  dcterms:created "2016-07-06T03:07:19+00:00"^^xsd:dateTime ;
  dcterms:creator "superadmin" ;
  dcterms:modified "2016-08-23T06:21:12+00:00"^^xsd:dateTime ;
  skos:altLabel "Health care standards"@en ;
  skos:altLabel "Health regulation"@en ;
  skos:broader agift:HEALTH-CARE ;
  skos:definition "Developing policy to regulate activities that are fundamental to the promotion of health and prevention of disease. Establishing standards and guidelines to support consistent procedures across jurisdictions."@en ;
  skos:narrower agift:Drugs-and-poisons-regulation ;
  skos:narrower agift:Food-hygiene-regulation ;
  skos:narrower agift:Practitioner-discipline ;
  skos:narrower agift:Practitioner-registration ;
  skos:prefLabel "Health protocol administration"@en ;
.
agift:Historic-relic-protection
  a skos:Concept ;
  dcterms:contributor "KOdea" ;
  dcterms:created "2016-07-06T03:02:53+00:00"^^xsd:dateTime ;
  dcterms:creator "superadmin" ;
  dcterms:modified "2016-09-08T07:42:38+00:00"^^xsd:dateTime ;
  skos:altLabel "Artefact protection"@en ;
  skos:altLabel "Community relic protection"@en ;
  skos:altLabel "Maritime heritage"@en ;
  skos:altLabel "Relic protection"@en ;
  skos:altLabel "Shipwreck relic protection"@en ;
  skos:altLabel "Space debris protection"@en ;
  skos:broader agift:ENVIRONMENT ;
  skos:definition "Developing policy and programs to protect built artefacts of particular heritage, scientific or social significance. Establishing standards for maintaining and preserving historic relics. Providing funding for joint projects with business or the community."@en ;
  skos:prefLabel "Historic relic protection"@en ;
  skos:related agift:Built-environment ;
  skos:related agift:Indigenous-heritage-conservation ;
  skos:related agift:Natural-heritage-protection ;
.
agift:Honours-and-awards-programs
  a skos:Concept ;
  dcterms:contributor "KOdea" ;
  dcterms:created "2016-07-06T03:05:55+00:00"^^xsd:dateTime ;
  dcterms:creator "superadmin" ;
  dcterms:modified "2016-09-08T06:29:52+00:00"^^xsd:dateTime ;
  skos:altLabel "Australian Service medal"@en ;
  skos:altLabel "Australian of the Year"@en ;
  skos:altLabel "Awards programs"@en ;
  skos:altLabel "Commonwealth Recognition Awards"@en ;
  skos:altLabel "Investiture programs"@en ;
  skos:broader agift:GOVERNANCE ;
  skos:definition "Coordinating and promoting ceremonies to pay tribute to notable achievements. Establishing selection criteria and the framework of levels of honour. Designing and producing medals. Researching and evaluating nominations. Maintaining a register of awards. Preparing congratulatory messages."@en ;
  skos:prefLabel "Honours and awards programs"@en ;
  skos:related agift:Badges-and-insignia ;
  skos:related agift:Cultural-awards-and-scholarships ;
.
agift:Horticultural-industry
  a skos:Concept ;
  dcterms:contributor "KOdea" ;
  dcterms:created "2016-07-06T05:02:39+00:00"^^xsd:dateTime ;
  dcterms:creator "superadmin" ;
  dcterms:modified "2016-09-12T06:16:43+00:00"^^xsd:dateTime ;
  skos:altLabel "Flower industry"@en ;
  skos:altLabel "Fruit growing industry"@en ;
  skos:altLabel "Gardening industry"@en ;
  skos:altLabel "Horticulture"@en ;
  skos:altLabel "Vegetable farming industry"@en ;
  skos:broader agift:Marine-and-rural-support ;
  skos:definition "Administering programs to support the commercial production of fruit, vegetables and flowers. Assisting industry growth and development. Encouraging businesses to adopt innovative practices, processes and products. Providing advice on cultivation methods and business management to improve competitiveness."@en ;
  skos:prefLabel "Horticultural industry"@en ;
  skos:related agift:Agricultural-industry ;
  skos:related agift:Agricultural-sciences ;
  skos:related agift:Pastoral-industry ;
  skos:related agift:Viticultural-industry ;
.
agift:Hospital-administration
  a skos:Concept ;
  dcterms:contributor "KOdea" ;
  dcterms:created "2016-07-06T04:46:06+00:00"^^xsd:dateTime ;
  dcterms:creator "superadmin" ;
  dcterms:modified "2016-08-23T06:35:40+00:00"^^xsd:dateTime ;
  skos:altLabel "Infirmary administration"@en ;
  skos:broader agift:Hospital-services ;
  skos:definition "Providing trained personnel to assist citizens who are injured or ill and require medical treatment. Managing staff and facilities at hospitals. Administering internal security, investigation and disciplinary procedures. Monitoring standards where hospital management activities are outsourced."@en ;
  skos:prefLabel "Hospital administration"@en ;
.
agift:Hospital-services
  a skos:Concept ;
  dcterms:contributor "KOdea" ;
  dcterms:created "2016-07-06T03:07:26+00:00"^^xsd:dateTime ;
  dcterms:creator "superadmin" ;
  dcterms:modified "2016-08-23T06:34:53+00:00"^^xsd:dateTime ;
  skos:altLabel "Hospitals"@en ;
  skos:broader agift:HEALTH-CARE ;
  skos:definition "Developing policy for the provision of health care through institutions offering a wide range of treatments and services. Establishing programs to support the provision of hospital services. Includes liaison across jurisdictions to coordinate services and operations."@en ;
  skos:narrower agift:Hospital-administration ;
  skos:narrower agift:Patient-care ;
  skos:narrower agift:Pharmaceutical-and-drug-support ;
  skos:prefLabel "Hospital services"@en ;
.
agift:Hospital-teaching-programs
  a skos:Concept ;
  dcterms:contributor "KOdea" ;
  dcterms:created "2016-07-06T04:15:10+00:00"^^xsd:dateTime ;
  dcterms:creator "superadmin" ;
  dcterms:modified "2016-08-19T02:14:04+00:00"^^xsd:dateTime ;
  skos:altLabel "Medical internship programs"@en ;
  skos:altLabel "Nursing education programs"@en ;
  skos:altLabel "Student doctor programs"@en ;
  skos:altLabel "Teaching hospitals"@en ;
  skos:broader agift:Vocational-education ;
  skos:definition "Administering programs of on-the-job training for professionals within the hospital system. Managing joint ventures with tertiary institutions. Monitoring compliance with standards and guidelines. Includes nursing courses, internships and work experience for medical students."@en ;
  skos:prefLabel "Hospital teaching programs"@en ;
.
agift:Housing-industry-policy
  a skos:Concept ;
  dcterms:contributor "KOdea" ;
  dcterms:created "2016-07-06T02:51:38+00:00"^^xsd:dateTime ;
  dcterms:creator "superadmin" ;
  dcterms:modified "2016-09-05T06:52:12+00:00"^^xsd:dateTime ;
  skos:altLabel "Housing affordability"@en ;
  skos:altLabel "Housing supply"@en ;
  skos:broader agift:CIVIC-INFRASTRUCTURE ;
  skos:definition "Developing policy and programs to ensure the adequacy of land supply and construction activity to meet demand and improve housing affordability."@en ;
  skos:prefLabel "Housing industry policy"@en ;
  skos:related agift:Land-use-planning ;
  skos:related agift:Town-planning ;
.
agift:Human-resources-development
  a skos:Concept ;
  dcterms:contributor "KOdea" ;
  dcterms:created "2016-07-06T03:01:45+00:00"^^xsd:dateTime ;
  dcterms:creator "superadmin" ;
  dcterms:modified "2016-09-08T07:20:29+00:00"^^xsd:dateTime ;
  skos:altLabel "Career development"@en ;
  skos:altLabel "Personnel management"@en ;
  skos:altLabel "Staff development"@en ;
  skos:altLabel "Staffing"@en ;
  skos:broader agift:EMPLOYMENT ;
  skos:definition "Developing policy and programs for staff support and management. Providing career planning advice, professional development and training. Conducting research into recruitment, retention and organisational demographics, to support long-term planning for human resources development."@en ;
  skos:narrower agift:Occupational-health-and-safety ;
  skos:narrower agift:Recruitment-programs ;
  skos:narrower agift:Termination-processes ;
  skos:narrower agift:Workers-compensation-schemes ;
  skos:narrower agift:Workplace-discrimination-monitoring ;
  skos:narrower agift:Workplace-equity-and-justice-programs ;
  skos:prefLabel "Human resources development"@en ;
  skos:related agift:Defence-force-careers ;
  skos:related agift:Workplace-training ;
.
agift:Human-rights-obligations
  a skos:Concept ;
  dcterms:contributor "KOdea" ;
  dcterms:created "2016-07-06T03:37:55+00:00"^^xsd:dateTime ;
  dcterms:creator "superadmin" ;
  dcterms:modified "2016-09-09T07:23:17+00:00"^^xsd:dateTime ;
  skos:altLabel "Civil liberties"@en ;
  skos:altLabel "Civil rights"@en ;
  skos:broader agift:JUSTICE-ADMINISTRATION ;
  skos:definition "Administering programs to ensure the freedoms to which all people are entitled, are upheld. Monitoring compliance with principles which may be constitutionally entrenched and guaranteed, recognised at common law, or declared by an international legal instrument. Includes investigations into breaches and promotion of human rights obligations and principles."@en ;
  skos:prefLabel "Human rights obligations"@en ;
  skos:related agift:Military-law ;
  skos:related agift:Privacy ;
  skos:related agift:Refugee-services ;
  skos:related agift:Treaty-administration ;
.
agift:Hydrology
  a skos:Concept ;
  dcterms:contributor "KOdea" ;
  dcterms:created "2016-07-06T05:05:03+00:00"^^xsd:dateTime ;
  dcterms:creator "superadmin" ;
  dcterms:modified "2016-09-12T06:34:30+00:00"^^xsd:dateTime ;
  skos:altLabel "Flood research"@en ;
  skos:altLabel "Water catchment studies"@en ;
  skos:altLabel "Water sciences"@en ;
  skos:broader agift:Earth-sciences ;
  skos:definition "Conducting research into water systems, on land and underground. Providing scientific advice on water cycles and flood warning information. Environmental and commercial assessment of projects such as dams and hydropower stations. Determining the impact of changes in land use, stream flow and climate on sediment and nutrient levels, and local ecology. Includes rivers, glaciers, catchment areas and geysers."@en ;
  skos:prefLabel "Hydrology"@en ;
  skos:related agift:Oceans-governance ;
  skos:related agift:Water-resources ;
.
agift:IMMIGRATION
  a skos:Concept ;
  dcterms:contributor "KOdea" ;
  dcterms:created "2016-07-06T02:46:01+00:00"^^xsd:dateTime ;
  dcterms:creator "superadmin" ;
  dcterms:modified "2016-09-09T06:29:24+00:00"^^xsd:dateTime ;
  skos:altLabel "Ethnic affairs"@en ;
  skos:altLabel "Migrants"@en ;
  skos:altLabel "Migration policy"@en ;
  skos:definition "Assisting people wishing to enter Australia on a permanent or temporary basis. Developing policy to establish entry or deportation requirements for migrants and visitors. Includes strategies for the management of illegal immigrants."@en ;
  skos:narrower agift:Citizenship ;
  skos:narrower agift:Deportation ;
  skos:narrower agift:Detention-programs ;
  skos:narrower agift:Migrant-services ;
  skos:narrower agift:Refugee-services ;
  skos:narrower agift:Travel-authorisation ;
  skos:prefLabel "IMMIGRATION"@en ;
  skos:related agift:CULTURAL-AFFAIRS ;
  skos:topConceptOf agift:AGIFT ;
.
agift:INDIGENOUS-AFFAIRS
  a skos:Concept ;
  dcterms:contributor "KOdea" ;
  dcterms:created "2016-07-06T02:46:09+00:00"^^xsd:dateTime ;
  dcterms:creator "superadmin" ;
  dcterms:modified "2016-08-26T07:29:53+00:00"^^xsd:dateTime ;
  skos:altLabel "Aboriginal affairs"@en ;
  skos:altLabel "Islander affairs"@en ;
  skos:altLabel "Torres Strait Islander affairs"@en ;
  skos:definition "Developing policy to support the advancement of Aboriginal and Torres Strait Islander people. Establishing programs to develop, manage and deliver services to Aboriginal and Torres Strait Islander people. Includes protecting areas directly associated with Aboriginal and Torres Strait Islander culture."@en ;
  skos:narrower agift:Indigenous-advocacy ;
  skos:narrower agift:Indigenous-cultural-heritage ;
  skos:narrower agift:Indigenous-enterprise-development ;
  skos:narrower agift:Indigenous-health-services ;
  skos:narrower agift:Indigenous-land-management ;
  skos:narrower agift:Indigenous-reconciliation ;
  skos:narrower agift:Indigenous-welfare-programs ;
  skos:prefLabel "INDIGENOUS AFFAIRS"@en ;
  skos:topConceptOf agift:AGIFT ;
.
agift:INTERNATIONAL-RELATIONS
  a skos:Concept ;
  dcterms:contributor "KOdea" ;
  dcterms:created "2016-07-06T02:46:18+00:00"^^xsd:dateTime ;
  dcterms:creator "superadmin" ;
  dcterms:modified "2016-09-09T05:44:42+00:00"^^xsd:dateTime ;
  skos:altLabel "Australian foreign policy"@en ;
  skos:altLabel "Foreign relations"@en ;
  skos:altLabel "International liaison"@en ;
  skos:altLabel "Overseas relations"@en ;
  skos:altLabel "United Nations"@en ;
  skos:definition "Building and maintaining relationships with other countries and international organisations. Developing strategies to protect and advance national interests. Contributing to international security, economic development, the environment, democratic principles and human rights through aid programs, treaties and diplomatic services."@en ;
  skos:narrower agift:Consular-services ;
  skos:narrower agift:Defence-liaison ;
  skos:narrower agift:Diplomatic-missions ;
  skos:narrower agift:International-affairs ;
  skos:narrower agift:International-treaties ;
  skos:narrower agift:Overseas-aid-programs ;
  skos:narrower agift:Overseas-promotion ;
  skos:narrower agift:Passport-services ;
  skos:prefLabel "INTERNATIONAL RELATIONS"@en ;
  skos:related agift:Intergovernmental-relations ;
  skos:topConceptOf agift:AGIFT ;
.
agift:Import-regulation
  a skos:Concept ;
  dcterms:contributor "KOdea" ;
  dcterms:created "2016-07-06T03:48:12+00:00"^^xsd:dateTime ;
  dcterms:creator "superadmin" ;
  dcterms:modified "2016-09-13T07:00:26+00:00"^^xsd:dateTime ;
  skos:altLabel "Customs regulation"@en ;
  skos:altLabel "Imports"@en ;
  skos:altLabel "Inspection services"@en ;
  skos:altLabel "Inspections"@en ;
  skos:broader agift:TRADE ;
  skos:definition "Controlling the international purchase and movement of goods into Australia. Ensuring compliance with domestic and international protocols and guidelines. Setting quotas, import licensing arrangements and customs regulations. Includes inspections and cargo clearance."@en ;
  skos:narrower agift:Prohibited-import-control ;
  skos:narrower agift:Tariff-regulation ;
  skos:prefLabel "Import regulation"@en ;
  skos:related agift:Cargo-control ;
  skos:related agift:Freight-movement-regulation ;
  skos:related agift:Port-regulation ;
.
agift:Income-assessment
  a skos:Concept ;
  dcterms:contributor "KOdea" ;
  dcterms:created "2016-07-06T04:39:07+00:00"^^xsd:dateTime ;
  dcterms:creator "superadmin" ;
  dcterms:modified "2016-09-08T08:08:19+00:00"^^xsd:dateTime ;
  skos:altLabel "Company tax"@en ;
  skos:altLabel "Income tax"@en ;
  skos:altLabel "Medicare levy"@en ;
  skos:altLabel "Personal tax"@en ;
  skos:altLabel "Tax file numbers"@en ;
  skos:altLabel "Tax returns"@en ;
  skos:broader agift:Taxation ;
  skos:definition "Evaluating earnings to determine the amount of taxation payable by an individual or organisation. Developing lodgement procedures for tax returns and issuing guidelines for tax agents. Processing notices of assessment and refunds. Issuing tax file numbers to individuals."@en ;
  skos:prefLabel "Income assessment"@en ;
  skos:related agift:Business-registration-and-licensing ;
  skos:related agift:Taxation-compliance ;
.
agift:Income-support-schemes
  a skos:Concept ;
  dcterms:contributor "KOdea" ;
  dcterms:created "2016-07-06T04:03:53+00:00"^^xsd:dateTime ;
  dcterms:creator "superadmin" ;
  dcterms:modified "2016-09-09T07:20:54+00:00"^^xsd:dateTime ;
  skos:altLabel "Abstudy"@en ;
  skos:altLabel "Age pensions"@en ;
  skos:altLabel "Aged concession"@en ;
  skos:altLabel "Aged pensions"@en ;
  skos:altLabel "Allowances"@en ;
  skos:altLabel "Carer's pensions"@en ;
  skos:altLabel "Concession cards"@en ;
  skos:altLabel "Defence service pensions"@en ;
  skos:altLabel "Disability support pension"@en ;
  skos:altLabel "Domestic assistance"@en ;
  skos:altLabel "Entitlements"@en ;
  skos:altLabel "Farm help"@en ;
  skos:altLabel "Health care cards"@en ;
  skos:altLabel "Invalid pensions"@en ;
  skos:altLabel "Old age pensions"@en ;
  skos:altLabel "Pension cards"@en ;
  skos:altLabel "Pensions"@en ;
  skos:altLabel "Rates rebate"@en ;
  skos:altLabel "Rebates"@en ;
  skos:altLabel "Rental assistance"@en ;
  skos:altLabel "Service pensions"@en ;
  skos:altLabel "Sickness benefits"@en ;
  skos:altLabel "Single parent pensions"@en ;
  skos:altLabel "Student benefits"@en ;
  skos:altLabel "Unemployment benefits"@en ;
  skos:altLabel "War pensions"@en ;
  skos:altLabel "War widows pensions"@en ;
  skos:altLabel "Widows' pensions"@en ;
  skos:broader agift:Financial-assistance ;
  skos:definition "Administering programs to provide financial assistance to individuals with low earnings. Providing advice on entitlements. Assessing eligibility and processing payments."@en ;
  skos:prefLabel "Income support schemes"@en ;
  skos:related agift:Asset-assessment ;
  skos:related agift:Benefits ;
  skos:related agift:Family-law-proceedings ;
  skos:related agift:Financial-assistance ;
  skos:related agift:Indigenous-welfare-programs ;
  skos:related agift:Public-housing ;
  skos:related agift:Taxation-compliance ;
  skos:related agift:Veterans-entitlements ;
.
agift:Independent-living-services
  a skos:Concept ;
  dcterms:contributor "KOdea" ;
  dcterms:created "2016-07-06T04:49:10+00:00"^^xsd:dateTime ;
  dcterms:creator "superadmin" ;
  dcterms:modified "2016-09-09T06:26:42+00:00"^^xsd:dateTime ;
  skos:altLabel "Carers"@en ;
  skos:altLabel "Community care"@en ;
  skos:altLabel "Disability services"@en ;
  skos:altLabel "Halfway houses"@en ;
  skos:altLabel "Home care"@en ;
  skos:altLabel "Nursing aide"@en ;
  skos:altLabel "Personal care"@en ;
  skos:altLabel "Sheltered accommodation"@en ;
  skos:altLabel "Supervised residences"@en ;
  skos:broader agift:Special-needs-services ;
  skos:definition "Managing programs to provide in-home support for aged or disabled persons, those recovering from injury, suffering disease or mental illness. Providing trained staff, carers and assistance to enable patients to remain at home. Includes 'halfway' or group houses where residents live independently under supervision."@en ;
  skos:prefLabel "Independent living services"@en ;
  skos:related agift:Aged-care-services ;
  skos:related agift:Counselling-services ;
  skos:related agift:Mental-health-services ;
  skos:related agift:Patient-care ;
  skos:related agift:Residential-services ;
.
agift:Indigenous-advocacy
  a skos:Concept ;
  dcterms:contributor "KOdea" ;
  dcterms:created "2016-07-06T03:34:41+00:00"^^xsd:dateTime ;
  dcterms:creator "superadmin" ;
  dcterms:modified "2016-09-09T06:49:01+00:00"^^xsd:dateTime ;
  skos:altLabel "Aboriginal cultural heritage"@en ;
  skos:altLabel "Torres Strait Islander cultural heritage"@en ;
  skos:broader agift:INDIGENOUS-AFFAIRS ;
  skos:definition "Providing access to information regarding rights, protections and entitlements for Aboriginal and Torres Strait Islander peoples. Representing and supporting individuals or groups to ensure rights are upheld."@en ;
  skos:prefLabel "Indigenous advocacy"@en ;
  skos:related agift:Indigenous-reconciliation ;
  skos:related agift:Social-justice-and-equity ;
.
agift:Indigenous-cultural-heritage
  a skos:Concept ;
  dcterms:contributor "KOdea" ;
  dcterms:created "2016-07-06T03:34:52+00:00"^^xsd:dateTime ;
  dcterms:creator "superadmin" ;
  dcterms:modified "2016-09-09T06:56:35+00:00"^^xsd:dateTime ;
  skos:broader agift:INDIGENOUS-AFFAIRS ;
  skos:definition "Managing programs to protect and promote the material, intellectual and spiritual traditions of Aboriginal and Torres Strait Islander peoples. Encouraging research into Indigenous culture. Establishing and maintaining cultural resource collections. Negotiating special custodial arrangements with Indigenous peoples. Initiating projects to compile and record indigenous oral histories, genealogies and languages."@en ;
  skos:narrower agift:Cultural-artefact-repatriation ;
  skos:prefLabel "Indigenous cultural heritage"@en ;
  skos:related agift:Indigenous-enterprise-development ;
  skos:related agift:Indigenous-heritage-conservation ;
  skos:related agift:Indigenous-reconciliation ;
  skos:related agift:Multicultural-heritage-promotion ;
.
agift:Indigenous-enterprise-development
  a skos:Concept ;
  dcterms:contributor "KOdea" ;
  dcterms:created "2016-07-06T03:34:59+00:00"^^xsd:dateTime ;
  dcterms:creator "superadmin" ;
  dcterms:modified "2016-09-09T06:53:08+00:00"^^xsd:dateTime ;
  skos:altLabel "Aboriginal enterprise development"@en ;
  skos:altLabel "Torres Strait Islander enterprise development"@en ;
  skos:broader agift:INDIGENOUS-AFFAIRS ;
  skos:definition "Administering programs to support the growth of businesses owned or operated by Aboriginal and Torres Strait Islander communities or individuals. Providing advice and services to assist the establishment of new ventures."@en ;
  skos:prefLabel "Indigenous enterprise development"@en ;
  skos:related agift:Indigenous-cultural-heritage ;
  skos:related agift:Indigenous-heritage-conservation ;
.
agift:Indigenous-health-services
  a skos:Concept ;
  dcterms:contributor "KOdea" ;
  dcterms:created "2016-07-06T03:35:06+00:00"^^xsd:dateTime ;
  dcterms:creator "superadmin" ;
  dcterms:modified "2016-09-09T06:57:13+00:00"^^xsd:dateTime ;
  skos:altLabel "Aboriginal health services"@en ;
  skos:altLabel "Torres Strait Islander health services"@en ;
  skos:broader agift:INDIGENOUS-AFFAIRS ;
  skos:definition "Developing policy and programs to support the physical and mental wellbeing of citizens in Aboriginal or Torres Strait Islander communities. Conducting planning and evaluation in consultation with local authorities. Encouraging participation to ensure community needs are adequately addressed."@en ;
  skos:prefLabel "Indigenous health services"@en ;
  skos:related agift:Indigenous-welfare-programs ;
  skos:related agift:Primary-health-care ;
  skos:related agift:Special-needs-services ;
.
agift:Indigenous-heritage-conservation
  a skos:Concept ;
  dcterms:contributor "KOdea" ;
  dcterms:created "2016-07-06T04:51:43+00:00"^^xsd:dateTime ;
  dcterms:creator "superadmin" ;
  dcterms:modified "2016-09-13T06:33:19+00:00"^^xsd:dateTime ;
  skos:altLabel "Aboriginal heritage conservation"@en ;
  skos:altLabel "Aboriginal rock paintings"@en ;
  skos:altLabel "Archaeological site conservation"@en ;
  skos:altLabel "Heritage protection"@en ;
  skos:altLabel "Islander heritage conservation"@en ;
  skos:altLabel "Native heritage conservation"@en ;
  skos:altLabel "Sacred site protection"@en ;
  skos:altLabel "Torres Strait Islander heritage conservation"@en ;
  skos:broader agift:Indigenous-land-management ;
  skos:definition "Developing policy and programs to protect areas directly associated with Aboriginal and Torres Strait Islander culture. Establishing standards for maintaining and preserving Indigenous heritage areas, such as control of public access. Providing funding for joint projects with business or the community. Developing land use agreements and site management plans."@en ;
  skos:prefLabel "Indigenous heritage conservation"@en ;
  skos:related agift:Built-environment ;
  skos:related agift:Historic-relic-protection ;
  skos:related agift:Indigenous-cultural-heritage ;
  skos:related agift:Indigenous-enterprise-development ;
  skos:related agift:Land-use-planning ;
  skos:related agift:National-park-management ;
  skos:related agift:Native-title-claims ;
  skos:related agift:Natural-heritage-protection ;
  skos:related agift:Park-and-reserve-services ;
  skos:related agift:Wilderness-area-management ;
.
agift:Indigenous-land-management
  a skos:Concept ;
  dcterms:contributor "KOdea" ;
  dcterms:created "2016-07-06T03:35:13+00:00"^^xsd:dateTime ;
  dcterms:creator "superadmin" ;
  dcterms:modified "2016-09-09T06:55:48+00:00"^^xsd:dateTime ;
  skos:broader agift:INDIGENOUS-AFFAIRS ;
  skos:definition "Developing policies and programs to manage traditional lands and seas owned by Aboriginal and Torres Strait Islander peoples. Assisting in the acquisition and management of lands and seas to achieve economic, environmental, social and cultural benefits."@en ;
  skos:narrower agift:Indigenous-heritage-conservation ;
  skos:narrower agift:Land-councils ;
  skos:prefLabel "Indigenous land management"@en ;
  skos:related agift:Land-councils ;
  skos:related agift:Native-title-claims ;
.
agift:Indigenous-reconciliation
  a skos:Concept ;
  dcterms:contributor "KOdea" ;
  dcterms:created "2016-07-06T03:35:20+00:00"^^xsd:dateTime ;
  dcterms:creator "superadmin" ;
  dcterms:modified "2016-09-09T06:56:35+00:00"^^xsd:dateTime ;
  skos:altLabel "Aboriginal reconciliation"@en ;
  skos:altLabel "Reconciliation programs"@en ;
  skos:altLabel "Torres Strait Islander reconciliation"@en ;
  skos:broader agift:INDIGENOUS-AFFAIRS ;
  skos:definition "Administering programs and services to promote understanding and agreement between Indigenous and non-Indigenous Australians. Ensuring government policy encompasses respect for the aspirations and rights of Aboriginal and Torres Strait Islander communities. Supporting activities to increase tolerance and cross-cultural awareness."@en ;
  skos:prefLabel "Indigenous reconciliation"@en ;
  skos:related agift:Indigenous-advocacy ;
  skos:related agift:Indigenous-cultural-heritage ;
.
agift:Indigenous-welfare-programs
  a skos:Concept ;
  dcterms:contributor "KOdea" ;
  dcterms:created "2016-07-06T03:35:27+00:00"^^xsd:dateTime ;
  dcterms:creator "superadmin" ;
  dcterms:modified "2016-09-09T06:57:13+00:00"^^xsd:dateTime ;
  skos:altLabel "Torres Strait Islander reconciliation"@en ;
  skos:altLabel "Torres Strait Islander welfare programs"@en ;
  skos:broader agift:INDIGENOUS-AFFAIRS ;
  skos:definition "Providing social support services specific to Aboriginal or Torres Strait Islander communities. Includes programs to expand Indigenous access to education and employment services, improve living conditions and assist families in crisis."@en ;
  skos:prefLabel "Indigenous welfare programs"@en ;
  skos:related agift:Benefits ;
  skos:related agift:Family-reunion-programs ;
  skos:related agift:Financial-assistance ;
  skos:related agift:Income-support-schemes ;
  skos:related agift:Indigenous-health-services ;
  skos:related agift:Rural-community-development ;
.
agift:Industrial-awards-and-conditions
  a skos:Concept ;
  dcterms:contributor "KOdea" ;
  dcterms:created "2016-07-06T03:01:52+00:00"^^xsd:dateTime ;
  dcterms:creator "superadmin" ;
  dcterms:modified "2016-09-08T07:34:59+00:00"^^xsd:dateTime ;
  skos:altLabel "Arbitration"@en ;
  skos:altLabel "Income awards and conditions"@en ;
  skos:broader agift:EMPLOYMENT ;
  skos:definition "Regulating the conduct of employers and employees across a particular industry or occupation. Issuing awards with regard to rates of pay and working conditions. Developing policy to support the establishment and use of industrial awards. Hearing disputes and offering independent arbitration services."@en ;
  skos:narrower agift:Award-conditions ;
  skos:narrower agift:Remuneration-review ;
  skos:prefLabel "Industrial awards and conditions"@en ;
  skos:related agift:Agreement-dispute-mediation ;
  skos:related agift:Apprenticeship-programs ;
  skos:related agift:Military-employment-services ;
  skos:related agift:Occupational-health-and-safety ;
  skos:related agift:Workplace-agreement-processes ;
.
agift:Industry-assistance-schemes
  a skos:Concept ;
  dcterms:contributor "KOdea" ;
  dcterms:created "2016-07-06T02:50:20+00:00"^^xsd:dateTime ;
  dcterms:creator "superadmin" ;
  dcterms:modified "2016-09-12T06:08:28+00:00"^^xsd:dateTime ;
  skos:altLabel "Manufacturing industry support"@en ;
  skos:altLabel "Secondary industry support"@en ;
  skos:altLabel "Services industry support"@en ;
  skos:broader agift:BUSINESS-SUPPORT-AND-REGULATION ;
  skos:definition "Developing policy to support the growth and management of secondary and tertiary industries. Identifying markets or investment opportunities. Encouraging businesses to adopt innovative practices, processes and products. Providing advice on production methods and business management to improve competitiveness."@en ;
  skos:prefLabel "Industry assistance schemes"@en ;
  skos:related agift:Industry-collaboration ;
  skos:related agift:Marine-and-rural-regulation ;
  skos:related agift:Small-business-advocacy ;
.
agift:Industry-collaboration
  a skos:Concept ;
  dcterms:contributor "KOdea" ;
  dcterms:created "2016-07-06T04:15:17+00:00"^^xsd:dateTime ;
  dcterms:creator "superadmin" ;
  dcterms:modified "2016-09-08T07:30:37+00:00"^^xsd:dateTime ;
  skos:broader agift:Vocational-education ;
  skos:definition "Connecting partnerships between industry and tertiary and vocational education to train a responsive workforce based on the skillsets needed by Australian enterprises and industry sectors"@en ;
  skos:prefLabel "Industry collaboration"@en ;
  skos:related agift:Employment-services-marketing ;
  skos:related agift:Industry-assistance-schemes ;
  skos:related agift:Labour-market-programs ;
.
agift:Industry-development
  a skos:Concept ;
  dcterms:contributor "KOdea" ;
  dcterms:created "2016-07-06T02:50:29+00:00"^^xsd:dateTime ;
  dcterms:creator "superadmin" ;
  dcterms:modified "2016-09-12T06:13:32+00:00"^^xsd:dateTime ;
  skos:altLabel "Innovation"@en ;
  skos:altLabel "Manufacturing industry regulation"@en ;
  skos:altLabel "Secondary industry regulation"@en ;
  skos:altLabel "Services industry regulation"@en ;
  skos:altLabel "Tertiary industry regulation"@en ;
  skos:broader agift:BUSINESS-SUPPORT-AND-REGULATION ;
  skos:definition "Monitoring the management of secondary and tertiary industries. Developing quality assurance programs, operating standards and other regulatory mechanisms. Issuing licenses for controlled activities. Certifying products and production methods. Conducting assessments and inspections to ensure compliance with standards and policy. Applying penalties for breaches of regulations."@en ;
  skos:prefLabel "Industry development"@en ;
  skos:related agift:Marine-and-rural-regulation ;
  skos:related agift:Marine-and-rural-support ;
  skos:related agift:Small-business-development ;
.
agift:Inflation
  a skos:Concept ;
  dcterms:contributor "KOdea" ;
  dcterms:created "2016-07-06T04:37:12+00:00"^^xsd:dateTime ;
  dcterms:creator "superadmin" ;
  dcterms:modified "2016-08-22T06:10:48+00:00"^^xsd:dateTime ;
  skos:altLabel "Price rises"@en ;
  skos:broader agift:Monetary-policy ;
  skos:definition "Establishing inflation targets. Monitoring relative amounts of currency in circulation and the resulting price increases or decreases. Forecasting the effects of inflation and developing strategies to minimise those effects."@en ;
  skos:prefLabel "Inflation"@en ;
.
agift:Information-dissemination
  a skos:Concept ;
  dcterms:contributor "KOdea" ;
  dcterms:created "2016-07-06T03:57:44+00:00"^^xsd:dateTime ;
  dcterms:creator "superadmin" ;
  dcterms:modified "2016-09-05T07:45:00+00:00"^^xsd:dateTime ;
  skos:altLabel "Government shopfronts"@en ;
  skos:altLabel "Portals"@en ;
  skos:altLabel "Web portals"@en ;
  skos:broader agift:Information-management-standards ;
  skos:definition "Developing strategies to effectively communicate government information. Promoting government-wide or cross-jurisdictional initiatives to provide access to government services and information. Planning advertising campaigns. Includes government shopfronts, remote access points and kiosks."@en ;
  skos:prefLabel "Information dissemination"@en ;
  skos:related agift:Electronic-publishing ;
  skos:related agift:Government-media ;
  skos:related agift:Publishing ;
  skos:related agift:Website-development ;
.
agift:Information-management-standards
  a skos:Concept ;
  dcterms:contributor "KOdea" ;
  dcterms:created "2016-07-06T02:53:57+00:00"^^xsd:dateTime ;
  dcterms:creator "superadmin" ;
  dcterms:modified "2016-09-05T07:32:37+00:00"^^xsd:dateTime ;
  skos:altLabel "Accessibility standards"@en ;
  skos:broader agift:COMMUNICATIONS ;
  skos:definition "Developing policy to support the organisation and use of government information. Providing advice on the availability of new communications technology and the implications for government business. Encouraging the implementation of best practice information management strategies. Includes guidelines for ensuring the accessibility of government information to individuals with special needs."@en ;
  skos:narrower agift:Data-management ;
  skos:narrower agift:Information-dissemination ;
  skos:narrower agift:Information-technology-standards ;
  skos:prefLabel "Information management standards"@en ;
  skos:related agift:Cybersafety ;
  skos:related agift:Information-security ;
  skos:related agift:Online-transaction-standards ;
  skos:related agift:Privacy ;
  skos:related agift:Recordkeeping-standards ;
.
agift:Information-security
  a skos:Concept ;
  dcterms:contributor "KOdea" ;
  dcterms:created "2016-07-06T03:44:36+00:00"^^xsd:dateTime ;
  dcterms:creator "superadmin" ;
  dcterms:modified "2016-09-12T06:50:43+00:00"^^xsd:dateTime ;
  skos:altLabel "Communication security"@en ;
  skos:altLabel "Cryptology"@en ;
  skos:altLabel "Cybersecurity"@en ;
  skos:altLabel "Data security standards"@en ;
  skos:broader agift:SECURITY ;
  skos:definition "Administering guidelines and standards for the protection of government networks and information systems. Conducting research into cryptology and the development of codes. Monitoring compliance with government security policy. Providing advice and tools to assist organisations to assess and improve their information systems."@en ;
  skos:prefLabel "Information security"@en ;
  skos:related agift:Authentication ;
  skos:related agift:Data-management ;
  skos:related agift:Information-management-standards ;
  skos:related agift:Information-technology-standards ;
  skos:related agift:Privacy ;
  skos:related agift:Recordkeeping-standards ;
.
agift:Information-technology-standards
  a skos:Concept ;
  dcterms:contributor "KOdea" ;
  dcterms:created "2016-07-06T03:57:52+00:00"^^xsd:dateTime ;
  dcterms:creator "superadmin" ;
  dcterms:modified "2016-09-05T07:37:16+00:00"^^xsd:dateTime ;
  skos:altLabel "Data transfer protocols"@en ;
  skos:altLabel "Interoperability standards"@en ;
  skos:broader agift:Information-management-standards ;
  skos:definition "Establishing guidelines and models to regulate the implementation of government hardware and software. Promoting the application of information technology standards to support interoperability and data exchange. Providing advice on the implementation of standards and monitoring compliance."@en ;
  skos:prefLabel "Information technology standards"@en ;
  skos:related agift:Data-management ;
  skos:related agift:Information-security ;
  skos:related agift:Online-transaction-standards ;
.
agift:Infrastructure-planning
  a skos:Concept ;
  dcterms:contributor "KOdea" ;
  dcterms:created "2016-07-06T02:51:47+00:00"^^xsd:dateTime ;
  dcterms:creator "superadmin" ;
  dcterms:modified "2016-09-05T06:56:29+00:00"^^xsd:dateTime ;
  skos:broader agift:CIVIC-INFRASTRUCTURE ;
  skos:definition "Identifying strategic investment priorities, policy, and regulatory reforms in the transport, water, energy and communications sectors, and providing advice on nationally-significant economic infrastructure to governments, investors and owners."@en ;
  skos:prefLabel "Infrastructure planning"@en ;
  skos:related agift:Integrated-services-planning ;
  skos:related agift:Land-use-planning ;
  skos:related agift:Regional-development ;
  skos:related agift:Town-planning ;
.
agift:Insurance-regulation
  a skos:Concept ;
  dcterms:contributor "KOdea" ;
  dcterms:created "2016-07-06T02:50:38+00:00"^^xsd:dateTime ;
  dcterms:creator "superadmin" ;
  dcterms:modified "2016-09-08T07:54:47+00:00"^^xsd:dateTime ;
  skos:broader agift:BUSINESS-SUPPORT-AND-REGULATION ;
  skos:definition "Developing policy to control schemes that provide financial guarantees against risk of loss or harm. Maintaining prudential oversight of insurance providers. Setting penalties for breaches of prudential regulations relating to insurance. Providing assistance and advice to citizens seeking insurance."@en ;
  skos:narrower agift:General-insurance ;
  skos:narrower agift:Life-insurance ;
  skos:prefLabel "Insurance regulation"@en ;
  skos:related agift:Financial-institutions-regulation ;
  skos:related agift:Financial-investment ;
  skos:related agift:Retirement-income ;
  skos:related agift:Workers-compensation-schemes ;
.
agift:Integrated-services-planning
  a skos:Concept ;
  dcterms:contributor "KOdea" ;
  dcterms:created "2016-07-06T02:51:59+00:00"^^xsd:dateTime ;
  dcterms:creator "superadmin" ;
  dcterms:modified "2016-09-05T06:59:33+00:00"^^xsd:dateTime ;
  skos:altLabel "Planning"@en ;
  skos:broader agift:CIVIC-INFRASTRUCTURE ;
  skos:definition "Developing strategies to provide essential community services in a coordinated and equitable manner. Evaluating land use data and town planning objectives. Identifying the requirements of particular districts. Bringing together related services, according to target audience."@en ;
  skos:prefLabel "Integrated services planning"@en ;
  skos:related agift:Infrastructure-planning ;
  skos:related agift:Land-use-planning ;
  skos:related agift:Land-use-zoning ;
  skos:related agift:Regional-development ;
  skos:related agift:Town-planning ;
  skos:related agift:Transport-network-maintenance ;
.
agift:Integrity-compliance
  a skos:Concept ;
  dcterms:contributor "KOdea" ;
  dcterms:created "2016-07-06T04:43:49+00:00"^^xsd:dateTime ;
  dcterms:creator "superadmin" ;
  dcterms:modified "2016-09-12T06:57:27+00:00"^^xsd:dateTime ;
  skos:broader agift:Public-administration ;
  skos:definition "Encouraging ethical behaviour and compliance with official codes of conduct."@en ;
  skos:prefLabel "Integrity compliance"@en ;
  skos:related agift:Corruption-prevention ;
  skos:related agift:Criminal-law ;
  skos:related agift:Government-auditing ;
  skos:related agift:Law-enforcement ;
  skos:related agift:Whistleblowing ;
.
agift:Intellectual-property-management
  a skos:Concept ;
  dcterms:contributor "KOdea" ;
  dcterms:created "2016-07-06T03:48:20+00:00"^^xsd:dateTime ;
  dcterms:creator "superadmin" ;
  dcterms:modified "2016-09-12T06:33:07+00:00"^^xsd:dateTime ;
  skos:broader agift:TRADE ;
  skos:definition "Developing policy to protect the rights of creative workers in literary, artistic, industrial or scientific fields. Regulating the administration of copyright, patents, trademarks and design registration. Includes proprietary knowledge such as development of new plant varieties or commercial trade secrets."@en ;
  skos:narrower agift:Design-rights-management ;
  skos:narrower agift:Patent-rights-management ;
  skos:narrower agift:Plant-breeders-rights-management ;
  skos:narrower agift:Trademark-registration ;
  skos:prefLabel "Intellectual property management"@en ;
  skos:related agift:Engineering-and-technology-sciences ;
  skos:related agift:Genetic-engineering ;
.
agift:Intelligence
  a skos:Concept ;
  dcterms:contributor "KOdea" ;
  dcterms:created "2016-07-06T03:44:43+00:00"^^xsd:dateTime ;
  dcterms:creator "superadmin" ;
  dcterms:modified "2016-09-12T06:55:20+00:00"^^xsd:dateTime ;
  skos:altLabel "Aerial surveillance"@en ;
  skos:altLabel "Espionage"@en ;
  skos:altLabel "Surveillance"@en ;
  skos:broader agift:SECURITY ;
  skos:definition "Developing policy and procedures to support the collection of information by covert means, to protect Australia from threats to national security. Conducting surveillance operations and investigating the use of technology to facilitate intelligence gathering. Includes foreign intelligence gathering in relation to strategic, political, economic or scientific activities."@en ;
  skos:narrower agift:Forensic-analysis ;
  skos:narrower agift:Intelligence-liaison ;
  skos:narrower agift:Intelligence-support ;
  skos:prefLabel "Intelligence"@en ;
  skos:related agift:External-security ;
  skos:related agift:Protective-services ;
.
agift:Intelligence-liaison
  a skos:Concept ;
  dcterms:contributor "KOdea" ;
  dcterms:created "2016-07-06T05:07:14+00:00"^^xsd:dateTime ;
  dcterms:creator "superadmin" ;
  dcterms:modified "2016-09-12T06:56:15+00:00"^^xsd:dateTime ;
  skos:altLabel "Criminal intelligence"@en ;
  skos:altLabel "Intelligence exchange"@en ;
  skos:broader agift:Intelligence ;
  skos:definition "Gathering information on illegal activity in support of law enforcement operations. Developing national and international networks of officers and agencies to facilitate the interchange of intelligence and reporting on criminal trends."@en ;
  skos:prefLabel "Intelligence liaison"@en ;
  skos:related agift:Intelligence-support ;
.
agift:Intelligence-support
  a skos:Concept ;
  dcterms:contributor "KOdea" ;
  dcterms:created "2016-07-06T05:07:23+00:00"^^xsd:dateTime ;
  dcterms:creator "superadmin" ;
  dcterms:modified "2016-09-12T06:58:12+00:00"^^xsd:dateTime ;
  skos:altLabel "Military intelligence"@en ;
  skos:altLabel "Reconnaissance"@en ;
  skos:broader agift:Intelligence ;
  skos:definition "Gathering military information in support of special operations. Compiling knowledge that might prove detrimental to an enemy. Conducting investigations and surveillance to support the planning and conduct of exceptional defence or security activities."@en ;
  skos:prefLabel "Intelligence support"@en ;
  skos:related agift:Intelligence-liaison ;
  skos:related agift:Protective-services ;
  skos:related agift:Special-operations ;
.
agift:Interest-rates
  a skos:Concept ;
  dcterms:contributor "KOdea" ;
  dcterms:created "2016-07-06T04:37:19+00:00"^^xsd:dateTime ;
  dcterms:creator "superadmin" ;
  dcterms:modified "2016-08-22T06:11:27+00:00"^^xsd:dateTime ;
  skos:broader agift:Monetary-policy ;
  skos:definition "Setting interest rates by buying and selling in money markets. Monitoring interest rates and forecasting the consequences and economic impact of fluctuations in interest rates. Developing strategies to minimise those effects."@en ;
  skos:prefLabel "Interest rates"@en ;
.
agift:Intergovernment-policy-dissemination
  a skos:Concept ;
  dcterms:contributor "KOdea" ;
  dcterms:created "2016-07-06T04:41:04+00:00"^^xsd:dateTime ;
  dcterms:creator "superadmin" ;
  dcterms:modified "2016-09-09T05:47:14+00:00"^^xsd:dateTime ;
  skos:altLabel "Cross-jurisdictional policy dissemination"@en ;
  skos:altLabel "Interstate policy dissemination"@en ;
  skos:broader agift:Intergovernmental-relations ;
  skos:definition "Managing the distribution of advice on decisions and strategies that require cooperative action across jurisdictions. Administering intergovernmental ministerial councils or committees responsible for policy reform."@en ;
  skos:prefLabel "Intergovernment policy dissemination"@en ;
.
agift:Intergovernmental-relations
  a skos:Concept ;
  dcterms:contributor "KOdea" ;
  dcterms:created "2016-07-06T03:06:02+00:00"^^xsd:dateTime ;
  dcterms:creator "superadmin" ;
  dcterms:modified "2016-09-09T05:44:56+00:00"^^xsd:dateTime ;
  skos:altLabel "Commonwealth State relations"@en ;
  skos:altLabel "Governmental relations"@en ;
  skos:altLabel "Interstate governmental relations"@en ;
  skos:broader agift:GOVERNANCE ;
  skos:definition "Developing cooperative associations between Australian government jurisdictions. Hosting forums and consultation processes to assess policy proposals and their potential impacts. Administering inter-jurisdictional bodies, grants and reforms. Negotiating interstate agreements on matters other than trade."@en ;
  skos:narrower agift:Cross-border-cooperation ;
  skos:narrower agift:Intergovernment-policy-dissemination ;
  skos:prefLabel "Intergovernmental relations"@en ;
  skos:related agift:Commonwealth-State-funding ;
  skos:related agift:Cross-border-cooperation ;
  skos:related agift:INTERNATIONAL-RELATIONS ;
  skos:related agift:Interstate-trade-agreements ;
.
agift:International-affairs
  a skos:Concept ;
  dcterms:contributor "KOdea" ;
  dcterms:created "2016-07-06T03:36:03+00:00"^^xsd:dateTime ;
  dcterms:creator "superadmin" ;
  dcterms:modified "2016-09-12T06:48:53+00:00"^^xsd:dateTime ;
  skos:altLabel "Attaches"@en ;
  skos:altLabel "Diplomacy"@en ;
  skos:altLabel "Diplomatic advisors"@en ;
  skos:altLabel "Foreign affairs"@en ;
  skos:altLabel "United Nations"@en ;
  skos:broader agift:INTERNATIONAL-RELATIONS ;
  skos:definition "Representing the Australian government and providing diplomatic advice overseas. Conducting consultations with foreign governments and international organisations to maintain relationships and protect national interests."@en ;
  skos:narrower agift:Disarmament-and-arms-control ;
  skos:narrower agift:Nuclear-safeguards ;
  skos:prefLabel "International affairs"@en ;
  skos:related agift:Consular-services ;
  skos:related agift:Defence-liaison ;
  skos:related agift:Diplomatic-missions ;
  skos:related agift:External-security ;
  skos:related agift:International-treaties ;
.
agift:International-monetary-regulation
  a skos:Concept ;
  dcterms:contributor "KOdea" ;
  dcterms:created "2016-07-06T03:04:39+00:00"^^xsd:dateTime ;
  dcterms:creator "superadmin" ;
  dcterms:modified "2016-08-22T06:06:15+00:00"^^xsd:dateTime ;
  skos:altLabel "Currency markets"@en ;
  skos:altLabel "International currency markets"@en ;
  skos:broader agift:FINANCE-MANAGEMENT ;
  skos:definition "Monitoring international currency markets and identifying trends. Forecasting market movements and developing strategies to maintain stable Australian markets"@en ;
  skos:prefLabel "International monetary regulation"@en ;
.
agift:International-trade-agreements
  a skos:Concept ;
  dcterms:contributor "KOdea" ;
  dcterms:created "2016-07-06T03:48:32+00:00"^^xsd:dateTime ;
  dcterms:creator "superadmin" ;
  dcterms:modified "2016-09-13T07:07:10+00:00"^^xsd:dateTime ;
  skos:altLabel "Regional trade agreements"@en ;
  skos:altLabel "Trade agreements"@en ;
  skos:altLabel "World Trade Organisation"@en ;
  skos:broader agift:TRADE ;
  skos:definition "Developing legislation, policy and protocols to support the supply and consumption of goods and services between countries. Negotiating treaties to reduce international trade restrictions and promote regional economic links."@en ;
  skos:prefLabel "International trade agreements"@en ;
  skos:related agift:International-treaties ;
  skos:related agift:Treaty-administration ;
.
agift:International-treaties
  a skos:Concept ;
  dcterms:contributor "KOdea" ;
  dcterms:created "2016-07-06T03:36:11+00:00"^^xsd:dateTime ;
  dcterms:creator "superadmin" ;
  dcterms:modified "2016-09-09T07:05:53+00:00"^^xsd:dateTime ;
  skos:altLabel "Bilateral agreements"@en ;
  skos:altLabel "Bilateral treaties"@en ;
  skos:altLabel "International agreements"@en ;
  skos:altLabel "International protocols"@en ;
  skos:altLabel "International treaty participation"@en ;
  skos:altLabel "Multilateral treaties"@en ;
  skos:altLabel "Treaties"@en ;
  skos:altLabel "Treaty negotiations"@en ;
  skos:broader agift:INTERNATIONAL-RELATIONS ;
  skos:definition "Negotiating a formal agreement or convention between Australia and one or more other countries. Forming a bilateral partnership or a multilateral alliance which is binding under international law. Amending an existing treaty or withdrawing from a treaty. Includes consultation with stakeholders, the development of declarations that may contribute to the development or interpretation of treaties, and monitoring of treaty, convention or agreement conditions."@en ;
  skos:narrower agift:Treaty-administration ;
  skos:prefLabel "International treaties"@en ;
  skos:related agift:Defence-liaison ;
  skos:related agift:Disarmament-and-arms-control ;
  skos:related agift:International-affairs ;
  skos:related agift:International-trade-agreements ;
.
agift:Internet
  a skos:Concept ;
  dcterms:contributor "KOdea" ;
  dcterms:created "2016-07-06T02:54:06+00:00"^^xsd:dateTime ;
  dcterms:creator "superadmin" ;
  dcterms:modified "2016-09-05T07:27:56+00:00"^^xsd:dateTime ;
  skos:broader agift:COMMUNICATIONS ;
  skos:definition "Developing policy and programs to regulate and promote Australia's role in the internet."@en ;
  skos:narrower agift:Cybersafety ;
  skos:narrower agift:Social-media ;
  skos:prefLabel "Internet"@en ;
  skos:related agift:Electronic-commerce ;
.
agift:Interpreter-services
  a skos:Concept ;
  dcterms:contributor "KOdea" ;
  dcterms:created "2016-07-06T04:50:19+00:00"^^xsd:dateTime ;
  dcterms:creator "superadmin" ;
  dcterms:modified "2016-09-09T06:33:59+00:00"^^xsd:dateTime ;
  skos:altLabel "Interpreters"@en ;
  skos:altLabel "Language services"@en ;
  skos:altLabel "Language"@en ;
  skos:altLabel "Translation services"@en ;
  skos:broader agift:Migrant-services ;
  skos:definition "Administering programs that offer oral and written translations between English and other languages. Providing face-to-face interpreter services, telephone interpretation and document translations. Includes services to community organisations that may assist migrants and refugees."@en ;
  skos:prefLabel "Interpreter services"@en ;
  skos:related agift:Adult-migrant-education ;
.
agift:Interstate-trade-agreements
  a skos:Concept ;
  dcterms:contributor "KOdea" ;
  dcterms:created "2016-07-07T00:42:04+00:00"^^xsd:dateTime ;
  dcterms:creator "superadmin" ;
  dcterms:modified "2016-09-13T07:07:55+00:00"^^xsd:dateTime ;
  skos:altLabel "Trade agreements"@en ;
  skos:broader agift:TRADE ;
  skos:definition "Developing legislation, policy and protocols to support the supply and consumption of goods and services across Australia. Negotiating agreements that promote commerce between states and encourage competition. Includes agreements on quarantine zones, transport and infrastructure arrangements in support of trade."@en ;
  skos:prefLabel "Interstate trade agreements"@en ;
  skos:related agift:Cross-border-cooperation ;
  skos:related agift:Intergovernmental-relations ;
  skos:related agift:Quarantine ;
.
agift:Investment-scheme-regulation
  a skos:Concept ;
  dcterms:contributor "KOdea" ;
  dcterms:created "2016-07-06T04:35:39+00:00"^^xsd:dateTime ;
  dcterms:creator "superadmin" ;
  dcterms:modified "2016-09-08T08:05:19+00:00"^^xsd:dateTime ;
  skos:altLabel "Investment management"@en ;
  skos:altLabel "Prudential regulation"@en ;
  skos:broader agift:Financial-investment ;
  skos:definition "Monitoring financial investment practices to ensure compliance with government policy and standards. Investigating suspected breaches of prudential regulations and applying penalties when appropriate."@en ;
  skos:prefLabel "Investment scheme regulation"@en ;
  skos:related agift:Superannuation-regulation ;
.
agift:JUSTICE-ADMINISTRATION
  a skos:Concept ;
  dcterms:contributor "KOdea" ;
  dcterms:created "2016-07-06T02:46:26+00:00"^^xsd:dateTime ;
  dcterms:creator "superadmin" ;
  dcterms:modified "2016-09-09T07:11:28+00:00"^^xsd:dateTime ;
  skos:altLabel "Courts"@en ;
  skos:altLabel "Judiciary"@en ;
  skos:altLabel "Law"@en ;
  skos:definition "Developing, interpreting and applying legislation, regulations or by-laws. Regulating the conduct of individuals, business and government, to conform to agreed rules and principles. Establishing programs and services to support the operation of the justice system."@en ;
  skos:narrower agift:Administrative-law ;
  skos:narrower agift:Associations-and-corporate-law ;
  skos:narrower agift:Civil-law ;
  skos:narrower agift:Commissions-of-inquiry ;
  skos:narrower agift:Coronial-law ;
  skos:narrower agift:Court-reporting ;
  skos:narrower agift:Criminal-law ;
  skos:narrower agift:Human-rights-obligations ;
  skos:narrower agift:Juvenile-justice ;
  skos:narrower agift:Legal-aid-services ;
  skos:narrower agift:Local-laws-and-ordinances ;
  skos:narrower agift:Native-title-claims ;
  skos:narrower agift:Privacy ;
  skos:narrower agift:Prosecution-services ;
  skos:prefLabel "JUSTICE ADMINISTRATION"@en ;
  skos:related agift:SECURITY ;
  skos:topConceptOf agift:AGIFT ;
.
agift:Job-placement-programs
  a skos:Concept ;
  dcterms:contributor "KOdea" ;
  dcterms:created "2016-07-06T04:22:17+00:00"^^xsd:dateTime ;
  dcterms:creator "superadmin" ;
  dcterms:modified "2016-09-08T07:32:12+00:00"^^xsd:dateTime ;
  skos:altLabel "Aboriginal employment services"@en ;
  skos:altLabel "Community work"@en ;
  skos:altLabel "Disability employment services"@en ;
  skos:altLabel "Employment National"@en ;
  skos:altLabel "Job Network"@en ;
  skos:altLabel "Job centres"@en ;
  skos:altLabel "Job seekers"@en ;
  skos:altLabel "Recruitment services"@en ;
  skos:altLabel "Torres Strait Islander employment services"@en ;
  skos:altLabel "Transition to work"@en ;
  skos:altLabel "Work for the Dole"@en ;
  skos:broader agift:Labour-market-programs ;
  skos:definition "Administering programs that encourage and assist individuals to enter the workforce. Liaising with jobseekers to evaluate their needs for support. Providing information and resources to help locate suitable employment. Assessing jobseeker eligibility for subsidy schemes. Includes promotional strategies and advertising campaigns to advocate the employment of individuals from target groups."@en ;
  skos:prefLabel "Job placement programs"@en ;
  skos:related agift:Community-education ;
  skos:related agift:Labour-market-programs ;
  skos:related agift:Vocational-education ;
.
agift:Job-vacancy-data-management
  a skos:Concept ;
  dcterms:contributor "KOdea" ;
  dcterms:created "2016-07-06T04:22:24+00:00"^^xsd:dateTime ;
  dcterms:creator "superadmin" ;
  dcterms:modified "2016-08-19T07:11:25+00:00"^^xsd:dateTime ;
  skos:altLabel "Unemployment figures"@en ;
  skos:broader agift:Labour-market-programs ;
  skos:definition "Administering information about employment opportunities. Evaluating and monitoring unemployment levels. Collecting statistics on skill shortages and vacancy trends. Managing resources and facilities for the advertisement of job vacancies."@en ;
  skos:prefLabel "Job vacancy data management"@en ;
.
agift:Juvenile-justice
  a skos:Concept ;
  dcterms:contributor "KOdea" ;
  dcterms:created "2016-07-06T03:38:02+00:00"^^xsd:dateTime ;
  dcterms:creator "superadmin" ;
  dcterms:modified "2016-09-09T07:23:40+00:00"^^xsd:dateTime ;
  skos:altLabel "Children's court"@en ;
  skos:altLabel "Children's crime"@en ;
  skos:altLabel "Juvenile crime"@en ;
  skos:altLabel "Youth crime"@en ;
  skos:broader agift:JUSTICE-ADMINISTRATION ;
  skos:definition "Administering special courts for the trial of children and young persons under a statutory age. Developing diversionary programs as an alternative to sentencing, opportunities for restorative justice and reintegration into the community."@en ;
  skos:prefLabel "Juvenile justice"@en ;
  skos:related agift:Child-and-youth-support ;
.
agift:Labour-market-programs
  a skos:Concept ;
  dcterms:contributor "KOdea" ;
  dcterms:created "2016-07-06T03:01:59+00:00"^^xsd:dateTime ;
  dcterms:creator "superadmin" ;
  dcterms:modified "2016-09-08T07:32:12+00:00"^^xsd:dateTime ;
  skos:altLabel "Employment marketing"@en ;
  skos:altLabel "Employment services"@en ;
  skos:altLabel "Job creation"@en ;
  skos:altLabel "Unemployment policy"@en ;
  skos:broader agift:EMPLOYMENT ;
  skos:definition "Developing policy and programs to support the growth and stability of labour markets. Includes programs to increase employment among individuals in target groups or across specific industries. Establishing mechanisms for managing and disseminating job vacancy data. Issuing licenses to organisations or individuals who provide employment services."@en ;
  skos:narrower agift:Employment-services-marketing ;
  skos:narrower agift:Job-placement-programs ;
  skos:narrower agift:Job-vacancy-data-management ;
  skos:prefLabel "Labour market programs"@en ;
  skos:related agift:Industry-collaboration ;
  skos:related agift:Job-placement-programs ;
.
agift:Land-councils
  a skos:Concept ;
  dcterms:contributor "KOdea" ;
  dcterms:created "2016-07-06T04:51:50+00:00"^^xsd:dateTime ;
  dcterms:creator "superadmin" ;
  dcterms:modified "2016-09-09T06:56:05+00:00"^^xsd:dateTime ;
  skos:broader agift:Indigenous-land-management ;
  skos:definition "Consulting with stakeholders and providing assistance for the development of land rights for Aboriginal and Torres Strait Islander peoples. Supports land and sea acquisition, establishment of commercial enterprises and community benefit schemes."@en ;
  skos:prefLabel "Land councils"@en ;
  skos:related agift:Indigenous-land-management ;
  skos:related agift:Native-title-claims ;
.
agift:Land-rehabilitation-programs
  a skos:Concept ;
  dcterms:contributor "KOdea" ;
  dcterms:created "2016-07-06T05:00:36+00:00"^^xsd:dateTime ;
  dcterms:creator "superadmin" ;
  dcterms:modified "2016-09-08T07:41:44+00:00"^^xsd:dateTime ;
  skos:altLabel "Land regeneration"@en ;
  skos:altLabel "Natural regeneration"@en ;
  skos:altLabel "Restoration programs"@en ;
  skos:broader agift:Mineral-resources ;
  skos:definition "Administering environmental support schemes to restore areas damaged by mineral excavation and extraction. Includes reviewing proposed projects and providing advice on rehabilitation strategies."@en ;
  skos:prefLabel "Land rehabilitation programs"@en ;
  skos:related agift:Landcare-programs ;
  skos:related agift:Soil-preservation-programs ;
.
agift:Land-use-planning
  a skos:Concept ;
  dcterms:contributor "KOdea" ;
  dcterms:created "2016-07-06T03:40:52+00:00"^^xsd:dateTime ;
  dcterms:creator "superadmin" ;
  dcterms:modified "2016-09-12T05:56:44+00:00"^^xsd:dateTime ;
  skos:altLabel "Commercial land use"@en ;
  skos:altLabel "Land planning"@en ;
  skos:broader agift:NATURAL-RESOURCES ;
  skos:definition "Developing policy for the effective management and allocation of land resources. Promoting strategies for integrated land use and balancing competing interests. Providing advice on rural and urban developments. Conducting surveys and demographic analysis, forecasting needs for infrastructure and facilities, and identifying heritage and significant areas."@en ;
  skos:narrower agift:Land-use-zoning ;
  skos:prefLabel "Land use planning"@en ;
  skos:related agift:Housing-industry-policy ;
  skos:related agift:Indigenous-heritage-conservation ;
  skos:related agift:Infrastructure-planning ;
  skos:related agift:Integrated-services-planning ;
.
agift:Land-use-zoning
  a skos:Concept ;
  dcterms:contributor "KOdea" ;
  dcterms:created "2016-07-06T05:00:19+00:00"^^xsd:dateTime ;
  dcterms:creator "superadmin" ;
  dcterms:modified "2016-09-12T05:57:38+00:00"^^xsd:dateTime ;
  skos:altLabel "Commercial land use"@en ;
  skos:altLabel "Commercial zoning"@en ;
  skos:altLabel "Development approval services"@en ;
  skos:altLabel "Land zoning"@en ;
  skos:altLabel "Public land zoning"@en ;
  skos:altLabel "Residential zoning"@en ;
  skos:altLabel "Zoning"@en ;
  skos:broader agift:Land-use-planning ;
  skos:definition "Marking out areas of land with regard to their use. Implementing strategic land use plans for the allocation of land resources. Administering land zones and assessing  development applications."@en ;
  skos:prefLabel "Land use zoning"@en ;
  skos:related agift:Building-approval-services ;
  skos:related agift:Integrated-services-planning ;
  skos:related agift:Town-planning ;
.
agift:Land-valuation
  a skos:Concept ;
  dcterms:contributor "KOdea" ;
  dcterms:created "2016-07-06T03:40:59+00:00"^^xsd:dateTime ;
  dcterms:creator "superadmin" ;
  dcterms:modified "2016-08-29T07:11:51+00:00"^^xsd:dateTime ;
  skos:altLabel "Land value"@en ;
  skos:altLabel "Valuation services"@en ;
  skos:broader agift:NATURAL-RESOURCES ;
  skos:definition "Assessing land resources to estimate their material worth for rating and taxation purposes. Providing advice on the unimproved value of land or in acquisition compensation disputes. Includes valuations for heritage listed land and rating concessions where land is held under nominated lease or tenure from the Crown."@en ;
  skos:prefLabel "Land valuation"@en ;
.
agift:Landcare-programs
  a skos:Concept ;
  dcterms:contributor "KOdea" ;
  dcterms:created "2016-07-06T04:33:19+00:00"^^xsd:dateTime ;
  dcterms:creator "superadmin" ;
  dcterms:modified "2016-09-08T07:41:01+00:00"^^xsd:dateTime ;
  skos:altLabel "Community land care"@en ;
  skos:altLabel "Land conservation programs"@en ;
  skos:altLabel "Sustainable agriculture"@en ;
  skos:broader agift:Conservation-programs ;
  skos:definition "Managing programs to prevent or repair damage to the natural environment. Restoring specific areas to their native state or preventing further degradation. Conducting activities such as planting or feral weed control. Includes funding for joint projects with local business or community groups."@en ;
  skos:prefLabel "Landcare programs"@en ;
  skos:related agift:Land-rehabilitation-programs ;
.
agift:Law-enforcement
  a skos:Concept ;
  dcterms:contributor "KOdea" ;
  dcterms:created "2016-07-06T03:44:50+00:00"^^xsd:dateTime ;
  dcterms:creator "superadmin" ;
  dcterms:modified "2016-09-13T07:20:15+00:00"^^xsd:dateTime ;
  skos:altLabel "Detector dog programs"@en ;
  skos:altLabel "Enforcement"@en ;
  skos:altLabel "Federal police"@en ;
  skos:altLabel "National police"@en ;
  skos:altLabel "Police"@en ;
  skos:broader agift:SECURITY ;
  skos:definition "Formulating policy to support the maintenance of rules and regulations that govern the actions of citizens. Coordinating the services of law enforcement agencies across jurisdictions. Developing programs to reduce violence and the use of illicit substances, improve public safety and reduce repeat offences. Includes activities to address 'white-collar' and corporate crime."@en ;
  skos:narrower agift:Community-policing ;
  skos:narrower agift:Criminology ;
  skos:narrower agift:Police-administration ;
  skos:narrower agift:Protective-services ;
  skos:prefLabel "Law enforcement"@en ;
  skos:related agift:Corruption-prevention ;
  skos:related agift:Counterfeiting-control ;
  skos:related agift:Emergency-management ;
  skos:related agift:Emergency-services ;
  skos:related agift:Integrity-compliance ;
  skos:related agift:Prosecution-services ;
  skos:related agift:Road-safety-awareness ;
  skos:related agift:Road-transport-safety ;
.
agift:Legal-aid-services
  a skos:Concept ;
  dcterms:contributor "KOdea" ;
  dcterms:created "2016-07-06T03:38:11+00:00"^^xsd:dateTime ;
  dcterms:creator "superadmin" ;
  dcterms:modified "2016-09-09T07:27:16+00:00"^^xsd:dateTime ;
  skos:altLabel "Aboriginal legal services"@en ;
  skos:altLabel "Community legal centres"@en ;
  skos:altLabel "Public defenders"@en ;
  skos:broader agift:JUSTICE-ADMINISTRATION ;
  skos:definition "Providing financial assistance for the purpose of legal proceedings in courts. Facilitating access to legal advice and services according to an income-based scale."@en ;
  skos:prefLabel "Legal aid services"@en ;
  skos:related agift:Prosecution-services ;
.
agift:Legislation-review
  a skos:Concept ;
  dcterms:contributor "KOdea" ;
  dcterms:created "2016-07-06T04:41:35+00:00"^^xsd:dateTime ;
  dcterms:creator "superadmin" ;
  dcterms:modified "2016-09-09T05:48:31+00:00"^^xsd:dateTime ;
  skos:altLabel "Law reform"@en ;
  skos:altLabel "Legislative amendment"@en ;
  skos:broader agift:Legislative-drafting ;
  skos:definition "Revising or amending legal instruments that already exist on statute books. Incorporating changes in government policy and other developments to ensure laws are relevant and equitable. Managing legislative review programs. Administering inter-departmental committees. Conducting enquiries, consultation and research. Providing advice on law reform."@en ;
  skos:prefLabel "Legislation review"@en ;
  skos:related agift:Draft-Bill-amendment-process ;
.
agift:Legislative-drafting
  a skos:Concept ;
  dcterms:contributor "KOdea" ;
  dcterms:created "2016-07-06T03:06:09+00:00"^^xsd:dateTime ;
  dcterms:creator "superadmin" ;
  dcterms:modified "2016-09-09T05:47:31+00:00"^^xsd:dateTime ;
  skos:altLabel "Acts of Parliament"@en ;
  skos:altLabel "Law-making"@en ;
  skos:altLabel "Legislation development"@en ;
  skos:broader agift:GOVERNANCE ;
  skos:definition "Preparing legal instruments for the parliament of any jurisdiction. Analysing government policy and the constitutional environment. Interpreting the legal effect of existing legislation. Providing advice on legislative proposals."@en ;
  skos:narrower agift:Draft-Bill-amendment-process ;
  skos:narrower agift:Legislation-review ;
  skos:narrower agift:Preparation-of-legislative-regulations ;
  skos:prefLabel "Legislative drafting"@en ;
  skos:related agift:Parliamentary-papers ;
  skos:related agift:Tabling-of-official-documents ;
.
agift:Life-insurance
  a skos:Concept ;
  dcterms:contributor "KOdea" ;
  dcterms:created "2016-07-06T03:52:06+00:00"^^xsd:dateTime ;
  dcterms:creator "superadmin" ;
  dcterms:modified "2016-09-05T06:39:24+00:00"^^xsd:dateTime ;
  skos:altLabel "Death insurance"@en ;
  skos:altLabel "Disablement insurance"@en ;
  skos:altLabel "Total and permanent disablement insurance"@en ;
  skos:broader agift:Insurance-regulation ;
  skos:definition "Monitoring the activities of life insurance providers to ensure compliance with government policy and standards. Investigating suspected breaches of prudential regulations and applying penalties when appropriate."@en ;
  skos:prefLabel "Life insurance"@en ;
  skos:related agift:General-insurance ;
.
agift:Light-station-maintenance
  a skos:Concept ;
  dcterms:contributor "KOdea" ;
  dcterms:created "2016-07-06T04:58:08+00:00"^^xsd:dateTime ;
  dcterms:creator "superadmin" ;
  dcterms:modified "2016-09-09T07:33:06+00:00"^^xsd:dateTime ;
  skos:altLabel "Beacon maintenance"@en ;
  skos:altLabel "Lighthouse maintenance"@en ;
  skos:altLabel "Lighthouses"@en ;
  skos:altLabel "Navigation aid maintenance"@en ;
  skos:broader agift:Navigation ;
  skos:definition "Administering programs to plan and manage navigational aids and markers for maritime transport. Supervising upgrades and regular maintenance to ensure the safe movement of vessels through shipping channels and approaches to ports. Includes decommissioning of light stations."@en ;
  skos:prefLabel "Light station maintenance"@en ;
  skos:related agift:Navigation-systems-development ;
.
agift:Local-laws-and-ordinances
  a skos:Concept ;
  dcterms:contributor "KOdea" ;
  dcterms:created "2016-07-06T03:38:24+00:00"^^xsd:dateTime ;
  dcterms:creator "superadmin" ;
  dcterms:modified "2016-09-08T08:07:52+00:00"^^xsd:dateTime ;
  skos:altLabel "Animal welfare"@en ;
  skos:altLabel "Councils"@en ;
  skos:altLabel "Dog registration"@en ;
  skos:altLabel "Domestic animal registration"@en ;
  skos:altLabel "Domestic animal services"@en ;
  skos:altLabel "Fines"@en ;
  skos:altLabel "Native animal registration"@en ;
  skos:altLabel "Ordinances"@en ;
  skos:altLabel "Permits and licence applications"@en ;
  skos:altLabel "Rates"@en ;
  skos:broader agift:JUSTICE-ADMINISTRATION ;
  skos:definition "Administering legal processes at town or district level. Establishing public regulations and courts with limited civil or criminal jurisdiction. Includes management of permits, rates and registration of domestic or native animals."@en ;
  skos:prefLabel "Local laws and ordinances"@en ;
  skos:related agift:Revenue-raising ;
  skos:related agift:Taxation ;
.
agift:Logistics
  a skos:Concept ;
  dcterms:contributor "KOdea" ;
  dcterms:created "2016-07-06T04:11:12+00:00"^^xsd:dateTime ;
  dcterms:creator "superadmin" ;
  dcterms:modified "2016-08-12T06:28:30+00:00"^^xsd:dateTime ;
  skos:altLabel "Army logistics"@en ;
  skos:altLabel "Defence logistics"@en ;
  skos:altLabel "Defence supply systems"@en ;
  skos:broader agift:Defence-strategic-support ;
  skos:definition "Administering programs to manage military transportation and supply. Developing procedural frameworks and systems to move bodies of troops or deliver services and equipment."@en ;
  skos:prefLabel "Logistics"@en ;
.
agift:MARITIME-SERVICES
  a skos:Concept ;
  dcterms:contributor "KOdea" ;
  dcterms:created "2016-07-06T02:46:33+00:00"^^xsd:dateTime ;
  dcterms:creator "superadmin" ;
  dcterms:modified "2016-09-09T07:28:38+00:00"^^xsd:dateTime ;
  skos:altLabel "Marine authorities"@en ;
  skos:altLabel "Merchant shipping"@en ;
  skos:altLabel "Shipping"@en ;
  skos:definition "Developing policy to regulate use of the sea as a means of transport. Negotiating passage for sea transport and maritime jurisdiction. Planning and managing maritime infrastructure. Monitoring the safety of seagoing vessels, pilots and personnel. Administering programs for marine search and rescue. Providing resources for the development of navigational aids."@en ;
  skos:narrower agift:Cargo-control ;
  skos:narrower agift:Harbour-management ;
  skos:narrower agift:Marina-management ;
  skos:narrower agift:Navigation ;
  skos:narrower agift:Pilotage-management ;
  skos:narrower agift:Port-regulation ;
  skos:narrower agift:Sea-passengers ;
  skos:narrower agift:Search-and-rescue ;
  skos:narrower agift:Ship-personnel ;
  skos:narrower agift:Ship-safety ;
  skos:prefLabel "MARITIME SERVICES"@en ;
  skos:related agift:Navy ;
  skos:related agift:TRANSPORT ;
  skos:topConceptOf agift:AGIFT ;
.
agift:Marina-management
  a skos:Concept ;
  dcterms:contributor "KOdea" ;
  dcterms:created "2016-07-06T03:39:21+00:00"^^xsd:dateTime ;
  dcterms:creator "superadmin" ;
  dcterms:modified "2016-09-12T06:04:46+00:00"^^xsd:dateTime ;
  skos:altLabel "Marina"@en ;
  skos:altLabel "Marinas"@en ;
  skos:broader agift:MARITIME-SERVICES ;
  skos:definition "Building and maintaining facilities offering dockage and other services for watercraft. Licensing operators of private marinas. Regulating boating activities, to protect waterways and marine industries from environmental impact. Includes inspections and assessment of procedures for managing sewage, spills and other discharge."@en ;
  skos:prefLabel "Marina management"@en ;
  skos:related agift:Harbour-management ;
  skos:related agift:Oceans-governance ;
  skos:related agift:Port-regulation ;
  skos:related agift:Waterway-management ;
.
agift:Marine-and-rural-regulation
  a skos:Concept ;
  dcterms:contributor "KOdea" ;
  dcterms:created "2016-07-06T03:41:52+00:00"^^xsd:dateTime ;
  dcterms:creator "superadmin" ;
  dcterms:modified "2016-09-12T06:08:45+00:00"^^xsd:dateTime ;
  skos:altLabel "Marine industries regulation"@en ;
  skos:altLabel "Rural industries regulation"@en ;
  skos:broader agift:PRIMARY-INDUSTRIES ;
  skos:definition "Monitoring the management of sea-based and farming industries. Encouraging efficient and sustainable cultivation practices. Developing quality assurance programs, operating standards and other regulatory mechanisms."@en ;
  skos:narrower agift:Agricultural-industry ;
  skos:narrower agift:Fisheries-industry ;
  skos:narrower agift:Food-quality-assurance ;
  skos:narrower agift:Forestry-industry ;
  skos:prefLabel "Marine and rural regulation"@en ;
  skos:related agift:ENVIRONMENT ;
  skos:related agift:Industry-assistance-schemes ;
  skos:related agift:Industry-development ;
  skos:related agift:Oceans-governance ;
.
agift:Marine-and-rural-support
  a skos:Concept ;
  dcterms:contributor "KOdea" ;
  dcterms:created "2016-07-06T03:42:00+00:00"^^xsd:dateTime ;
  dcterms:creator "superadmin" ;
  dcterms:modified "2016-09-12T06:19:21+00:00"^^xsd:dateTime ;
  skos:broader agift:PRIMARY-INDUSTRIES ;
  skos:definition "Developing policy to assist the growth and management of sea-based or farming industries. Identifying markets and facilitating trade or investment opportunities. Providing grants, financial incentives or subsidies for initiatives."@en ;
  skos:narrower agift:Aquaculture-industry ;
  skos:narrower agift:Horticultural-industry ;
  skos:narrower agift:Pastoral-industry ;
  skos:narrower agift:Silvicultural-industry ;
  skos:narrower agift:Viticultural-industry ;
  skos:prefLabel "Marine and rural support"@en ;
  skos:related agift:Disaster-relief ;
  skos:related agift:Financial-assistance ;
  skos:related agift:Industry-development ;
  skos:related agift:Rural-partnership-programs ;
  skos:related agift:Small-business-advocacy ;
.
agift:Marine-life-protection-programs
  a skos:Concept ;
  dcterms:contributor "KOdea" ;
  dcterms:created "2016-07-06T03:02:59+00:00"^^xsd:dateTime ;
  dcterms:creator "superadmin" ;
  dcterms:modified "2016-09-08T07:43:28+00:00"^^xsd:dateTime ;
  skos:altLabel "Aquarium programs"@en ;
  skos:altLabel "Marine protection programs"@en ;
  skos:altLabel "Ocean conservation programs"@en ;
  skos:altLabel "Sea conservation programs"@en ;
  skos:broader agift:ENVIRONMENT ;
  skos:definition "Maintaining sea-based areas of the natural environment that are culturally or scientifically significant in their native state. Developing schemes to conserve plant or animal life in a region, to protect and sustain ecosystems. Promoting community awareness and participation in conservation activities."@en ;
  skos:prefLabel "Marine life protection programs"@en ;
  skos:related agift:Biological-sciences ;
  skos:related agift:Conservation-programs ;
  skos:related agift:Oceanography ;
  skos:related agift:Oceans-governance ;
.
agift:Mathematical-sciences
  a skos:Concept ;
  dcterms:contributor "KOdea" ;
  dcterms:created "2016-07-06T03:43:34+00:00"^^xsd:dateTime ;
  dcterms:creator "superadmin" ;
  dcterms:modified "2016-09-12T06:39:32+00:00"^^xsd:dateTime ;
  skos:altLabel "Statistical research"@en ;
  skos:broader agift:SCIENCE ;
  skos:definition "Conducting research into quantities, magnitudes and forms by the use of numbers. Providing data analysis, simulation or mathematical modelling to illustrate trends and predict outcomes. Performing optimisation tests to determine the best operating conditions for a process. Includes training and consultancy in mathematical analysis."@en ;
  skos:prefLabel "Mathematical sciences"@en ;
  skos:related agift:Applied-sciences ;
  skos:related agift:Engineering-and-technology-sciences ;
  skos:related agift:STATISTICAL-SERVICES ;
.
agift:Media-ownership-regulation
  a skos:Concept ;
  dcterms:contributor "KOdea" ;
  dcterms:created "2016-07-06T02:54:15+00:00"^^xsd:dateTime ;
  dcterms:creator "superadmin" ;
  dcterms:modified "2016-09-05T07:39:55+00:00"^^xsd:dateTime ;
  skos:altLabel "Mass media services"@en ;
  skos:altLabel "Media ownership"@en ;
  skos:broader agift:COMMUNICATIONS ;
  skos:definition "Developing policy and legislation to support Australian control of domestic communication channels. Setting limits on who can own and control Australian media outlets. Encouraging diversity among the more influential broadcasting services."@en ;
  skos:prefLabel "Media ownership regulation"@en ;
  skos:related agift:Broadcasting-standards ;
.
agift:Medical-aids-regulation
  a skos:Concept ;
  dcterms:contributor "KOdea" ;
  dcterms:created "2016-07-06T04:46:40+00:00"^^xsd:dateTime ;
  dcterms:creator "superadmin" ;
  dcterms:modified "2016-08-23T06:44:30+00:00"^^xsd:dateTime ;
  skos:altLabel "Disability aids"@en ;
  skos:altLabel "Disabled equipment"@en ;
  skos:altLabel "Hearing aids"@en ;
  skos:altLabel "Medical alert devices"@en ;
  skos:altLabel "Prosthetics"@en ;
  skos:altLabel "Respirators"@en ;
  skos:altLabel "Vehicle modifications"@en ;
  skos:altLabel "Walking aids"@en ;
  skos:altLabel "Wheelchairs"@en ;
  skos:broader agift:Medical-research ;
  skos:definition "Monitoring the availability and manufacturing quality of appliances that assist people suffering from disease or disability. Assessing products to determine eligibility for subsidies, special tax treatment or limited distribution, in accordance with government policy."@en ;
  skos:prefLabel "Medical aids regulation"@en ;
.
agift:Medical-and-health-sciences
  a skos:Concept ;
  dcterms:contributor "KOdea" ;
  dcterms:created "2016-07-06T03:43:42+00:00"^^xsd:dateTime ;
  dcterms:creator "superadmin" ;
  dcterms:modified "2016-09-12T06:40:35+00:00"^^xsd:dateTime ;
  skos:altLabel "Health sciences"@en ;
  skos:altLabel "Medicine"@en ;
  skos:broader agift:SCIENCE ;
  skos:definition "Conducting experimental research into the causes, effects and symptoms of illness. Applying knowledge from a range of scientific disciplines to advance the diagnosis, treatment and prevention of disease. Developing products and processes to improve community health. Providing advice on diet, nutrition and the use of pharmaceuticals. Includes safety assessments for therapeutic goods, and the development of new surgical techniques."@en ;
  skos:prefLabel "Medical and health sciences"@en ;
  skos:related agift:Apparatus-licensing ;
  skos:related agift:Applied-sciences ;
  skos:related agift:Biological-sciences ;
  skos:related agift:Doping-detection-research ;
  skos:related agift:Epidemiology ;
  skos:related agift:Food-hygiene-regulation ;
  skos:related agift:Medical-research ;
  skos:related agift:National-referral-laboratory-services ;
  skos:related agift:Physiology ;
  skos:related agift:Population-based-research ;
.
agift:Medical-quarantine-services
  a skos:Concept ;
  dcterms:contributor "KOdea" ;
  dcterms:created "2016-07-06T04:48:06+00:00"^^xsd:dateTime ;
  dcterms:creator "superadmin" ;
  dcterms:modified "2016-09-09T06:22:35+00:00"^^xsd:dateTime ;
  skos:broader agift:Public-health-services ;
  skos:definition "Protecting the health of human populations from risks associated with exotic or infectious disease. Providing surveillance and isolation of persons who have potentially been exposed to a particular disease. Managing facilities at Antarctic stations, airports and seaports."@en ;
  skos:prefLabel "Medical quarantine services"@en ;
  skos:related agift:Clinical-health-services ;
  skos:related agift:Health-disaster-preparedness ;
  skos:related agift:Notifiable-disease-management ;
  skos:related agift:Quarantine ;
.
agift:Medical-radiation-services
  a skos:Concept ;
  dcterms:contributor "KOdea" ;
  dcterms:created "2016-07-06T04:48:16+00:00"^^xsd:dateTime ;
  dcterms:creator "superadmin" ;
  dcterms:modified "2016-09-12T06:43:35+00:00"^^xsd:dateTime ;
  skos:broader agift:Public-health-services ;
  skos:prefLabel "Medical radiation services"@en ;
  skos:related agift:Nuclear-sciences ;
  skos:related agift:Radiation-protection ;
.
agift:Medical-research
  a skos:Concept ;
  dcterms:contributor "KOdea" ;
  dcterms:created "2016-07-06T03:07:33+00:00"^^xsd:dateTime ;
  dcterms:creator "superadmin" ;
  dcterms:modified "2016-09-09T06:16:25+00:00"^^xsd:dateTime ;
  skos:altLabel "Health research regulation"@en ;
  skos:altLabel "Medical technologies"@en ;
  skos:broader agift:HEALTH-CARE ;
  skos:definition "Regulating the scientific investigation of human health and disease. Endorsing standards for ethical conduct. Developing policy to support the availability of medical equipment or research services. Establishing criteria for the allocation of funding to medical research."@en ;
  skos:narrower agift:Medical-aids-regulation ;
  skos:narrower agift:Medical-research-funding ;
  skos:narrower agift:National-referral-laboratory-services ;
  skos:narrower agift:Population-based-research ;
  skos:prefLabel "Medical research"@en ;
  skos:related agift:Medical-and-health-sciences ;
.
agift:Medical-research-funding
  a skos:Concept ;
  dcterms:contributor "KOdea" ;
  dcterms:created "2016-07-06T04:46:50+00:00"^^xsd:dateTime ;
  dcterms:creator "superadmin" ;
  dcterms:modified "2016-08-23T06:47:50+00:00"^^xsd:dateTime ;
  skos:altLabel "Health research funding"@en ;
  skos:broader agift:Medical-research ;
  skos:definition "Providing financial support for the scientific investigation of human health and disease. Assessing proposals and applications against established criteria. Allocating funds to successful projects and providing advice to unsuccessful applicants."@en ;
  skos:prefLabel "Medical research funding"@en ;
.
agift:Memorial-maintenance
  a skos:Concept ;
  dcterms:contributor "KOdea" ;
  dcterms:created "2016-07-06T03:55:22+00:00"^^xsd:dateTime ;
  dcterms:creator "superadmin" ;
  dcterms:modified "2016-09-05T07:05:02+00:00"^^xsd:dateTime ;
  skos:altLabel "Commemorative monument maintenance"@en ;
  skos:altLabel "Memorials"@en ;
  skos:altLabel "Monument maintenance"@en ;
  skos:altLabel "War memorial maintenance"@en ;
  skos:broader agift:Public-land-management ;
  skos:definition "Administering areas of land set aside to commemorate a person or event. Managing site layout. Ensuring facilities are kept clean and maintained. Monitoring rights of access and opening hours."@en ;
  skos:prefLabel "Memorial maintenance"@en ;
  skos:related agift:Burial-ground-management ;
.
agift:Mental-health-services
  a skos:Concept ;
  dcterms:contributor "KOdea" ;
  dcterms:created "2016-07-06T04:49:17+00:00"^^xsd:dateTime ;
  dcterms:creator "superadmin" ;
  dcterms:modified "2016-09-09T06:27:02+00:00"^^xsd:dateTime ;
  skos:altLabel "Psychiatric health services"@en ;
  skos:altLabel "Psychological health services"@en ;
  skos:altLabel "Suicide prevention"@en ;
  skos:broader agift:Special-needs-services ;
  skos:definition "Administering programs to treat or manage disorders and diseases of the mind. Monitoring the activities of private mental health providers. Includes assessment, therapeutic intervention, referral to support services and mental health advocacy"@en ;
  skos:prefLabel "Mental health services"@en ;
  skos:related agift:Community-health-services ;
  skos:related agift:Counselling-services ;
  skos:related agift:Independent-living-services ;
  skos:related agift:Residential-services ;
.
agift:Merger-regulation
  a skos:Concept ;
  dcterms:contributor "KOdea" ;
  dcterms:created "2016-07-06T04:55:41+00:00"^^xsd:dateTime ;
  dcterms:creator "superadmin" ;
  dcterms:modified "2016-08-26T08:12:02+00:00"^^xsd:dateTime ;
  skos:altLabel "Business mergers"@en ;
  skos:altLabel "Company takeovers"@en ;
  skos:altLabel "Corporate takeovers"@en ;
  skos:altLabel "Mergers"@en ;
  skos:altLabel "Takeovers"@en ;
  skos:broader agift:Associations-and-corporate-law ;
  skos:definition "Regulating the statutory combination of two or more corporations by transfer of assets and property to a single enterprise. Assessing possible economic consequences of mergers, such as inflated prices, reduced quality or anti-competitive behaviour."@en ;
  skos:prefLabel "Merger regulation"@en ;
.
agift:Migrant-accommodation-services
  a skos:Concept ;
  dcterms:contributor "KOdea" ;
  dcterms:created "2016-07-06T04:50:27+00:00"^^xsd:dateTime ;
  dcterms:creator "superadmin" ;
  dcterms:modified "2016-09-28T07:00:41+00:00"^^xsd:dateTime ;
  skos:altLabel "Immigrant accommodation"@en ;
  skos:altLabel "Migrant camps"@en ;
  skos:altLabel "Migrant hostels"@en ;
  skos:altLabel "Migrant housing"@en ;
  skos:broader agift:Migrant-services ;
  skos:definition "Administering programs to assist new immigrants or refugees to find housing. Assessing eligibility and allocating accommodation to approved applicants. Providing advice to tenants about their rights and obligations. Includes interim housing in camps or hostels"@en ;
  skos:prefLabel "Migrant accommodation services"@en ;
  skos:related agift:Accommodation-services ;
  skos:related agift:Detention-programs ;
  skos:related agift:Public-housing ;
.
agift:Migrant-services
  a skos:Concept ;
  dcterms:contributor "KOdea" ;
  dcterms:created "2016-07-06T03:34:02+00:00"^^xsd:dateTime ;
  dcterms:creator "superadmin" ;
  dcterms:modified "2016-09-09T06:39:49+00:00"^^xsd:dateTime ;
  skos:altLabel "Assisted migration"@en ;
  skos:altLabel "Immigration services"@en ;
  skos:broader agift:IMMIGRATION ;
  skos:definition "Developing programs to provide information and support to foreign nationals who intend to settle in Australia. Evaluating the needs of migrants and providing advice before embarkation and upon arrival. Includes liaison with community groups and across jurisdictions to ensure appropriate support."@en ;
  skos:narrower agift:Interpreter-services ;
  skos:narrower agift:Migrant-accommodation-services ;
  skos:narrower agift:Migrant-settlement-programs ;
  skos:prefLabel "Migrant services"@en ;
  skos:related agift:Adult-migrant-education ;
  skos:related agift:Family-reunion-programs ;
  skos:related agift:Multicultural-services ;
  skos:related agift:Permanent-entry-arrangements ;
  skos:related agift:Refugee-services ;
.
agift:Migrant-settlement-programs
  a skos:Concept ;
  dcterms:contributor "KOdea" ;
  dcterms:created "2016-07-06T04:50:34+00:00"^^xsd:dateTime ;
  dcterms:creator "superadmin" ;
  dcterms:modified "2016-09-09T06:38:25+00:00"^^xsd:dateTime ;
  skos:altLabel "Migrant resource centres"@en ;
  skos:broader agift:Migrant-services ;
  skos:definition "Administering schemes to assist new immigrants or refugees to become established in Australia. Managing migrant resource centres. Providing orientation information and support services. Includes advice about bringing family members to Australia and liaison with immigration officials on behalf of migrants."@en ;
  skos:prefLabel "Migrant settlement programs"@en ;
  skos:related agift:Adult-migrant-education ;
  skos:related agift:Family-reunion-programs ;
  skos:related agift:Refugee-services ;
.
agift:Military-advisors
  a skos:Concept ;
  dcterms:contributor "KOdea" ;
  dcterms:created "2016-07-06T04:52:41+00:00"^^xsd:dateTime ;
  dcterms:creator "superadmin" ;
  dcterms:modified "2016-09-09T07:00:45+00:00"^^xsd:dateTime ;
  skos:altLabel "Defence advisors"@en ;
  skos:altLabel "Military advice"@en ;
  skos:broader agift:Defence-liaison ;
  skos:definition "Providing defence counsel to senior government representatives. Developing guidance on defence capability and the conduct of military operations. Making recommendations to support command and control of the Australian Defence Force and strategic preparation of its service elements."@en ;
  skos:prefLabel "Military advisors"@en ;
  skos:related agift:Defence-attaches ;
  skos:related agift:Military-operations ;
  skos:related agift:Strategic-decisions ;
  skos:related agift:Strategic-planning ;
.
agift:Military-bands
  a skos:Concept ;
  dcterms:contributor "KOdea" ;
  dcterms:created "2016-07-06T04:08:45+00:00"^^xsd:dateTime ;
  dcterms:creator "superadmin" ;
  dcterms:modified "2016-08-11T07:14:05+00:00"^^xsd:dateTime ;
  skos:altLabel "Bands"@en ;
  skos:altLabel "Military tattoo"@en ;
  skos:broader agift:Australian-Defence-Forces ;
  skos:definition "Raising, developing and maintaining companies of musicians to provide musical support for defence force ceremonies, community events and other activities. Administering bookings, arranging concerts and tours."@en ;
  skos:prefLabel "Military bands"@en ;
.
agift:Military-education-and-training
  a skos:Concept ;
  dcterms:contributor "KOdea" ;
  dcterms:created "2016-07-06T03:00:22+00:00"^^xsd:dateTime ;
  dcterms:creator "superadmin" ;
  dcterms:modified "2016-09-08T07:33:44+00:00"^^xsd:dateTime ;
  skos:altLabel "Air training units"@en ;
  skos:altLabel "Army training units"@en ;
  skos:altLabel "Navy training units"@en ;
  skos:broader agift:EDUCATION-AND-TRAINING ;
  skos:definition "Developing programs designed to instruct and exercise defence recruits. Managing specialised institutions or facilities to provide suitable training for active personnel. Initiating joint ventures to provide tertiary level education or residential schools for service personnel."@en ;
  skos:narrower agift:Army-reserve-training ;
  skos:narrower agift:Defence-college-training ;
  skos:prefLabel "Military education and training"@en ;
  skos:related agift:Australian-Defence-Forces ;
  skos:related agift:Cadets ;
  skos:related agift:Defence-career-development ;
  skos:related agift:Defence-force-careers ;
  skos:related agift:Military-exercises ;
  skos:related agift:Reserves ;
  skos:related agift:Vocational-education ;
  skos:related agift:Workplace-agreement-processes ;
  skos:related agift:Workplace-training ;
.
agift:Military-employment-services
  a skos:Concept ;
  dcterms:contributor "KOdea" ;
  dcterms:created "2016-07-06T04:09:31+00:00"^^xsd:dateTime ;
  dcterms:creator "superadmin" ;
  dcterms:modified "2016-09-08T07:28:43+00:00"^^xsd:dateTime ;
  skos:altLabel "Defence employment services"@en ;
  skos:altLabel "Discharge processes"@en ;
  skos:altLabel "Military discharge"@en ;
  skos:broader agift:Defence-force-careers ;
  skos:definition "Administering personnel support services for regular and reserve members of the Australian Defence Forces. Providing advice on wages and employment conditions, leave and other entitlements. Managing complaints, health and safety or harassment issues. Initiating disciplinary proceedings. Includes work experience placements and spouse employment services."@en ;
  skos:prefLabel "Military employment services"@en ;
  skos:related agift:Defence-career-development ;
  skos:related agift:Industrial-awards-and-conditions ;
  skos:related agift:Military-law ;
  skos:related agift:Termination-processes ;
  skos:related agift:Workplace-equity-and-justice-programs ;
.
agift:Military-exercises
  a skos:Concept ;
  dcterms:contributor "KOdea" ;
  dcterms:created "2016-07-06T04:12:15+00:00"^^xsd:dateTime ;
  dcterms:creator "superadmin" ;
  dcterms:modified "2016-09-08T06:58:15+00:00"^^xsd:dateTime ;
  skos:altLabel "Defence exercises"@en ;
  skos:altLabel "Military training exercises"@en ;
  skos:altLabel "War games"@en ;
  skos:broader agift:Military-operations ;
  skos:definition "Executing air, sea and land training manoeuvres in preparation for warfare. Managing war games and other practical exercises in real or simulated environments. Testing communications and information systems that support operations. Evaluating exercises and conducting research to develop strategies for future operations. Includes activities to meet environmental obligations and safety standards during exercises."@en ;
  skos:prefLabel "Military exercises"@en ;
  skos:related agift:Australian-Defence-Forces ;
  skos:related agift:Military-education-and-training ;
.
agift:Military-law
  a skos:Concept ;
  dcterms:contributor "KOdea" ;
  dcterms:created "2016-07-06T02:59:11+00:00"^^xsd:dateTime ;
  dcterms:creator "superadmin" ;
  dcterms:modified "2016-09-08T06:59:08+00:00"^^xsd:dateTime ;
  skos:altLabel "Courts martial"@en ;
  skos:altLabel "Military courts"@en ;
  skos:altLabel "Military detention"@en ;
  skos:altLabel "Prisoners of war"@en ;
  skos:broader agift:DEFENCE ;
  skos:definition "Administering the body of law that relates to the discipline, trial and punishment of defence personnel. Establishing military courts and conducting hearings to determine whether a command is lawful, or if service personnel have met their obligations. Regulating the treatment of prisoners of war and captured civilians in times of war."@en ;
  skos:prefLabel "Military law"@en ;
  skos:related agift:Detention-centre-management ;
  skos:related agift:Detention-programs ;
  skos:related agift:Emergency-management ;
  skos:related agift:Human-rights-obligations ;
  skos:related agift:Military-employment-services ;
  skos:related agift:Special-operations ;
  skos:related agift:Treaty-administration ;
.
agift:Military-operations
  a skos:Concept ;
  dcterms:contributor "KOdea" ;
  dcterms:created "2016-07-06T02:59:18+00:00"^^xsd:dateTime ;
  dcterms:creator "superadmin" ;
  dcterms:modified "2016-09-08T06:56:49+00:00"^^xsd:dateTime ;
  skos:altLabel "Defence operations"@en ;
  skos:broader agift:DEFENCE ;
  skos:definition "Implementing strategic decisions for the deployment of Australia's defence capability. Directing the conduct of campaigns and other activities for the defence of Australia and its interests. Evaluating joint operations and exercises to prepare for future action."@en ;
  skos:narrower agift:Australian-theatre-of-war ;
  skos:narrower agift:Military-exercises ;
  skos:narrower agift:Special-operations ;
  skos:narrower agift:Warfare ;
  skos:prefLabel "Military operations"@en ;
  skos:related agift:Military-advisors ;
  skos:related agift:Peacekeeping-forces ;
  skos:related agift:Strategic-decisions ;
.
agift:Mineral-exploration
  a skos:Concept ;
  dcterms:contributor "KOdea" ;
  dcterms:created "2016-07-06T05:05:10+00:00"^^xsd:dateTime ;
  dcterms:creator "superadmin" ;
  dcterms:modified "2016-09-12T06:36:05+00:00"^^xsd:dateTime ;
  skos:altLabel "Mine exploration"@en ;
  skos:altLabel "Mining activities"@en ;
  skos:altLabel "Mining exploration"@en ;
  skos:altLabel "Mining"@en ;
  skos:broader agift:Earth-sciences ;
  skos:definition "Conducting research into ore deposits and their environmental settings. Applying geological and geochemical methods to advance the understanding of mineral origin and distribution. Developing tools and models to support deposit location, excavation and extraction processes. Promoting collaborative programs across government, university and industry sectors. Includes training programs for geologists, industry researchers and students."@en ;
  skos:prefLabel "Mineral exploration"@en ;
  skos:related agift:Applied-sciences ;
  skos:related agift:Fossil-fuel-management ;
  skos:related agift:Mineral-resources ;
  skos:related agift:Seismology ;
.
agift:Mineral-resources
  a skos:Concept ;
  dcterms:contributor "KOdea" ;
  dcterms:created "2016-07-06T03:41:06+00:00"^^xsd:dateTime ;
  dcterms:creator "superadmin" ;
  dcterms:modified "2016-09-12T05:58:29+00:00"^^xsd:dateTime ;
  skos:altLabel "Mining"@en ;
  skos:broader agift:NATURAL-RESOURCES ;
  skos:definition "Administering legislation relating to mining and mineral processing. Developing policy to support the management of mineral resources and the economic development of related industries. Negotiating partnership programs with the traditional owners of mineral-rich lands."@en ;
  skos:narrower agift:Land-rehabilitation-programs ;
  skos:narrower agift:Mining-regulations ;
  skos:prefLabel "Mineral resources"@en ;
  skos:related agift:Fossil-fuel-management ;
  skos:related agift:Mineral-exploration ;
.
agift:Mining-regulations
  a skos:Concept ;
  dcterms:contributor "KOdea" ;
  dcterms:created "2016-07-06T05:00:45+00:00"^^xsd:dateTime ;
  dcterms:creator "superadmin" ;
  dcterms:modified "2016-09-12T06:35:20+00:00"^^xsd:dateTime ;
  skos:altLabel "Mining activities"@en ;
  skos:altLabel "Mining exploration"@en ;
  skos:broader agift:Mineral-resources ;
  skos:definition "Managing the exploitation of ores and mineral resources. Licensing infrastructure and operational activities. Conducting exploration and mapping mineral deposits. Granting mining titles and leases for excavation and extraction. Monitoring compliance with standards, regulations and risk management procedures."@en ;
  skos:prefLabel "Mining regulations"@en ;
  skos:related agift:Earth-sciences ;
  skos:related agift:Environmental-impact-assessment ;
.
agift:Mobile-telephone-services
  a skos:Concept ;
  dcterms:contributor "KOdea" ;
  dcterms:created "2016-07-06T04:00:53+00:00"^^xsd:dateTime ;
  dcterms:creator "superadmin" ;
  dcterms:modified "2016-09-05T07:56:06+00:00"^^xsd:dateTime ;
  skos:altLabel "Cellular telephone services"@en ;
  skos:altLabel "Mobile phones"@en ;
  skos:altLabel "Wireless telecommunications services"@en ;
  skos:broader agift:Telecommunications ;
  skos:definition "Monitoring the activities of suppliers of wireless telecommunications services. Ensuring compliance with pricing guidelines, standards of service and maintenance requirements. Encouraging the development of the mobile telephone industry."@en ;
  skos:prefLabel "Mobile telephone services"@en ;
  skos:related agift:Apparatus-licensing ;
  skos:related agift:CIVIC-INFRASTRUCTURE ;
  skos:related agift:Radio-communication ;
  skos:related agift:Telephone-services ;
.
agift:Monetary-policy
  a skos:Concept ;
  dcterms:contributor "KOdea" ;
  dcterms:created "2016-07-06T03:04:46+00:00"^^xsd:dateTime ;
  dcterms:creator "superadmin" ;
  dcterms:modified "2016-09-08T08:00:31+00:00"^^xsd:dateTime ;
  skos:altLabel "Economic policy"@en ;
  skos:altLabel "Interest rate policy"@en ;
  skos:altLabel "Macroeconomic policy"@en ;
  skos:broader agift:FINANCE-MANAGEMENT ;
  skos:definition "Developing policy to maintain stability of the currency, improve economic performance and employment levels. Setting interest rates by buying and selling in money markets. Includes activities to control inflation within predefined limits."@en ;
  skos:narrower agift:Exchange-rates ;
  skos:narrower agift:Inflation ;
  skos:narrower agift:Interest-rates ;
  skos:prefLabel "Monetary policy"@en ;
  skos:related agift:Economic-research ;
  skos:related agift:Prices-surveillance ;
  skos:related agift:Productivity ;
.
agift:Multicultural-festivals
  skos:prefLabel "Multicultural festivals"@en ;
  owl:deprecated true ;
.
agift:Multicultural-festivals
  a skos:Concept ;
  dcterms:contributor "fionamcl" ;
  dcterms:created "2016-09-08T01:46:59+00:00"^^xsd:dateTime ;
  dcterms:creator "fionamcl" ;
  dcterms:modified "2016-11-28T22:48:56+00:00"^^xsd:dateTime ;
  skos:altLabel "Ethnic festivals"@en ;
  skos:altLabel "Food fairs"@en ;
  skos:altLabel "International cultural displays"@en ;
  skos:altLabel "International food fairs"@en ;
  skos:broader agift:Multicultural-heritage-promotion ;
  skos:definition "Promoting and funding events that reflect Australia's cultural diversity and multi-ethnic population. Organising festivals, performances and joint ventures with community groups where events highlight the origin of particular cultural activities. Includes participation in international cultural festivals."@en ;
  skos:prefLabel "Multicultural festivals"@en ;
  skos:related agift:Civic-celebrations ;
  skos:related agift:Cultural-festivals ;
  skos:related agift:Overseas-promotion ;
.
agift:Multicultural-heritage-promotion
  skos:prefLabel "Multicultural heritage promotion"@en ;
  owl:deprecated true ;
.
agift:Multicultural-heritage-promotion
  a skos:Concept ;
  dcterms:contributor "fionamcl" ;
  dcterms:created "2016-09-08T01:23:27+00:00"^^xsd:dateTime ;
  dcterms:creator "fionamcl" ;
  dcterms:modified "2016-11-28T22:48:48+00:00"^^xsd:dateTime ;
  skos:broader agift:CULTURAL-AFFAIRS ;
  skos:definition "Managing programs to protect and promote Australia's cultural diversity. Sponsoring community events and activities. Recognising internationally significant dates and events. Encouraging research into multicultural experiences. Initiating projects to compile and document ethnic oral histories and folklore."@en ;
  skos:narrower agift:Multicultural-festivals ;
  skos:narrower agift:Multicultural-services ;
  skos:prefLabel "Multicultural heritage promotion"@en ;
  skos:related agift:Indigenous-cultural-heritage ;
.
agift:Multicultural-services
  skos:prefLabel "Multicultural services"@en ;
  owl:deprecated true ;
.
agift:Multicultural-services
  a skos:Concept ;
  dcterms:contributor "fionamcl" ;
  dcterms:created "2016-09-08T01:47:02+00:00"^^xsd:dateTime ;
  dcterms:creator "fionamcl" ;
  dcterms:modified "2016-11-28T22:49:03+00:00"^^xsd:dateTime ;
  skos:altLabel "Cultural diversity programs"@en ;
  skos:altLabel "Ethnic services"@en ;
  skos:broader agift:Multicultural-heritage-promotion ;
  skos:definition "Encouraging migrant communities to retain their cultural identity. Establishing and maintaining ethnic cultural resource collections. Providing assistance in the conduct of religious ceremonies or social events. Includes liaison across jurisdictions to support and promote multiculturalism."@en ;
  skos:prefLabel "Multicultural services"@en ;
  skos:related agift:Migrant-services ;
  skos:related agift:Social-club-support ;
.
agift:NATURAL-RESOURCES
  a skos:Concept ;
  dcterms:contributor "fionamcl" ;
  dcterms:created "2016-07-06T02:46:42+00:00"^^xsd:dateTime ;
  dcterms:creator "superadmin" ;
  dcterms:modified "2016-09-20T00:08:41+00:00"^^xsd:dateTime ;
  skos:altLabel "Natural resource management"@en ;
  skos:definition "Developing policy for the sustainable use and management of energy, mineral, land and water supplies. Administering programs to evaluate resource consumption and exploitation practices. Regulating and supporting industries that realise the economic potential of resources."@en ;
  skos:narrower agift:Crown-land-administration ;
  skos:narrower agift:Energy-resources ;
  skos:narrower agift:Land-use-planning ;
  skos:narrower agift:Land-valuation ;
  skos:narrower agift:Mineral-resources ;
  skos:narrower agift:Pollution-emission-control ;
  skos:narrower agift:Water-resources ;
  skos:prefLabel "NATURAL RESOURCES"@en ;
  skos:related agift:ENVIRONMENT ;
  skos:related agift:PRIMARY-INDUSTRIES ;
  skos:related agift:SCIENCE ;
  skos:topConceptOf agift:AGIFT ;
.
agift:National-park-management
  a skos:Concept ;
  dcterms:contributor "KOdea" ;
  dcterms:created "2016-07-06T04:34:12+00:00"^^xsd:dateTime ;
  dcterms:creator "superadmin" ;
  dcterms:modified "2016-09-13T06:32:29+00:00"^^xsd:dateTime ;
  skos:altLabel "Forest management"@en ;
  skos:altLabel "Marine parks"@en ;
  skos:altLabel "National park access and permits"@en ;
  skos:altLabel "National parks"@en ;
  skos:altLabel "Parks"@en ;
  skos:broader agift:Natural-heritage-protection ;
  skos:definition "Administering designated national park areas. Monitoring access restrictions and maintaining public amenities. Issuing permits for commercial or recreational activities. Assessing applications for development within national parks. Implementing plans for regeneration following erosion or natural disasters."@en ;
  skos:prefLabel "National park management"@en ;
  skos:related agift:Feral-pest-control ;
  skos:related agift:Garden-management ;
  skos:related agift:Indigenous-heritage-conservation ;
  skos:related agift:Nature-reserve-management ;
  skos:related agift:Park-and-reserve-services ;
  skos:related agift:Recreational-park-management ;
  skos:related agift:Wilderness-area-management ;
  skos:related agift:Wildlife-sanctuary-management ;
.
agift:National-referral-laboratory-services
  a skos:Concept ;
  dcterms:contributor "KOdea" ;
  dcterms:created "2016-07-06T04:47:00+00:00"^^xsd:dateTime ;
  dcterms:creator "superadmin" ;
  dcterms:modified "2016-09-09T06:17:08+00:00"^^xsd:dateTime ;
  skos:altLabel "Analytical testing"@en ;
  skos:altLabel "Health testing services"@en ;
  skos:altLabel "Laboratory services"@en ;
  skos:altLabel "Medical testing services"@en ;
  skos:altLabel "Pathology"@en ;
  skos:altLabel "Specimen collection services"@en ;
  skos:broader agift:Medical-research ;
  skos:definition "Managing programs that administer scientific testing on behalf of health and medical practitioners. Packaging and transporting specimens for analysis. Conducting screening and assessment of patients. Examining specimens and providing results."@en ;
  skos:prefLabel "National referral laboratory services"@en ;
  skos:related agift:Medical-and-health-sciences ;
.
agift:National-security
  a skos:Concept ;
  dcterms:contributor "KOdea" ;
  dcterms:created "2016-07-06T03:44:59+00:00"^^xsd:dateTime ;
  dcterms:creator "superadmin" ;
  dcterms:modified "2016-09-12T06:58:42+00:00"^^xsd:dateTime ;
  skos:altLabel "Community protection"@en ;
  skos:altLabel "Counter terrorism"@en ;
  skos:altLabel "Homeland security"@en ;
  skos:altLabel "Internal security"@en ;
  skos:broader agift:SECURITY ;
  skos:definition "Developing policy and procedures to protect the Australian continent. Implementing strategies to identify and apprehend individuals who may pose a threat to national security. Reviewing the powers of the security and intelligence services."@en ;
  skos:narrower agift:Border-protection ;
  skos:prefLabel "National security"@en ;
  skos:related agift:Deportation ;
  skos:related agift:Detention-programs ;
.
agift:Native-title-claims
  a skos:Concept ;
  dcterms:contributor "KOdea" ;
  dcterms:created "2016-07-06T03:38:33+00:00"^^xsd:dateTime ;
  dcterms:creator "superadmin" ;
  dcterms:modified "2016-09-09T07:25:04+00:00"^^xsd:dateTime ;
  skos:altLabel "Aboriginal land rights"@en ;
  skos:altLabel "Application for Native Title"@en ;
  skos:altLabel "Indigenous land rights"@en ;
  skos:altLabel "Land claims"@en ;
  skos:altLabel "Land rights"@en ;
  skos:altLabel "Litigation processes"@en ;
  skos:broader agift:JUSTICE-ADMINISTRATION ;
  skos:definition "Administering procedures to assess Indigenous interest in or rights to the use of specified areas of land or water. Identifying traditional customs and connections with a particular region. Includes processing applications, providing advice and support for litigation."@en ;
  skos:narrower agift:Native-title-mediation-programs ;
  skos:narrower agift:Native-title-settlement-negotiations ;
  skos:prefLabel "Native title claims"@en ;
  skos:related agift:Indigenous-heritage-conservation ;
  skos:related agift:Indigenous-land-management ;
  skos:related agift:Land-councils ;
.
agift:Native-title-mediation-programs
  a skos:Concept ;
  dcterms:contributor "KOdea" ;
  dcterms:created "2016-07-06T04:56:42+00:00"^^xsd:dateTime ;
  dcterms:creator "superadmin" ;
  dcterms:modified "2016-09-09T07:25:47+00:00"^^xsd:dateTime ;
  skos:altLabel "Land claim mediation"@en ;
  skos:altLabel "Mediation programs"@en ;
  skos:altLabel "Native title mediation"@en ;
  skos:broader agift:Native-title-claims ;
  skos:definition "Providing arbitration services to parties involved in claims for Indigenous land rights. Acting as an intermediary in an effort to reconcile competing interests and bring about agreement. Includes facilitating access to these programs."@en ;
  skos:prefLabel "Native title mediation programs"@en ;
  skos:related agift:Dispute-mediation-programs ;
  skos:related agift:Native-title-settlement-negotiations ;
.
agift:Native-title-settlement-negotiations
  a skos:Concept ;
  dcterms:contributor "KOdea" ;
  dcterms:created "2016-07-06T04:56:51+00:00"^^xsd:dateTime ;
  dcterms:creator "superadmin" ;
  dcterms:modified "2016-09-09T07:25:47+00:00"^^xsd:dateTime ;
  skos:broader agift:Native-title-claims ;
  skos:definition "Establishing procedures for mutual discussions to resolve claims for Indigenous land rights. Attempting to reach a compromise in disputes, and agree on arrangements for shared land use. Includes management of compensation payments, where rights have been infringed."@en ;
  skos:prefLabel "Native title settlement negotiations"@en ;
  skos:related agift:Native-title-mediation-programs ;
.
agift:Natural-disasters
  a skos:Concept ;
  dcterms:contributor "KOdea" ;
  dcterms:created "2016-07-06T02:56:10+00:00"^^xsd:dateTime ;
  dcterms:creator "superadmin" ;
  dcterms:modified "2016-09-08T06:50:47+00:00"^^xsd:dateTime ;
  skos:altLabel "Acts of God"@en ;
  skos:altLabel "Disasters"@en ;
  skos:broader agift:COMMUNITY-SERVICES ;
  skos:definition "Managing programs to provide urgent assistance during emergencies caused by the elements - such as floods, earthquakes, cyclones, storms or major bushfires. Monitoring conditions to anticipate the likelihood and effects of natural disasters. Coordinating government and community-based services, and regulating the use of volunteers. Includes liaison with defence forces, where civil community assistance is provided."@en ;
  skos:narrower agift:Disaster-recovery ;
  skos:narrower agift:Disaster-relief ;
  skos:prefLabel "Natural disasters"@en ;
  skos:related agift:Ambulance-services ;
  skos:related agift:Atmospheric-sciences ;
  skos:related agift:Civil-community-assistance ;
  skos:related agift:Climate-information-services ;
  skos:related agift:Emergency-funding ;
  skos:related agift:Emergency-management ;
  skos:related agift:Emergency-services ;
  skos:related agift:Firefighting-services ;
  skos:related agift:Search-and-rescue ;
.
agift:Natural-heritage-protection
  a skos:Concept ;
  dcterms:contributor "KOdea" ;
  dcterms:created "2016-07-06T03:03:06+00:00"^^xsd:dateTime ;
  dcterms:creator "superadmin" ;
  dcterms:modified "2016-09-09T07:32:51+00:00"^^xsd:dateTime ;
  skos:altLabel "Maritime heritage"@en ;
  skos:altLabel "National Estate preservation"@en ;
  skos:broader agift:ENVIRONMENT ;
  skos:definition "Developing policy and programs to manage and conserve elements of the biological environment that have particular historic, scientific or social significance. Establishing standards for maintaining and preserving natural heritage areas, such as access and development restrictions, or regeneration requirements."@en ;
  skos:narrower agift:Feral-pest-control ;
  skos:narrower agift:National-park-management ;
  skos:narrower agift:Nature-reserve-management ;
  skos:narrower agift:Wilderness-area-management ;
  skos:narrower agift:Wildlife-sanctuary-management ;
  skos:prefLabel "Natural heritage protection"@en ;
  skos:related agift:Built-environment ;
  skos:related agift:Conservation-programs ;
  skos:related agift:Historic-relic-protection ;
  skos:related agift:Indigenous-heritage-conservation ;
.
agift:Naturalisation-assessment
  a skos:Concept ;
  dcterms:contributor "KOdea" ;
  dcterms:created "2016-07-06T04:49:53+00:00"^^xsd:dateTime ;
  dcterms:creator "superadmin" ;
  dcterms:modified "2016-08-26T07:13:04+00:00"^^xsd:dateTime ;
  skos:altLabel "Citizenship applications"@en ;
  skos:altLabel "Naturalisation"@en ;
  skos:broader agift:Citizenship ;
  skos:definition "Administering programs to evaluate applications for Australian citizenship. Managing procedures for lodging submissions. Conducting interviews and assessing applicants against standard criteria. Notifying applicants of the outcome of assessment."@en ;
  skos:prefLabel "Naturalisation assessment"@en ;
.
agift:Nature-reserve-management
  a skos:Concept ;
  dcterms:contributor "KOdea" ;
  dcterms:created "2016-07-06T04:34:20+00:00"^^xsd:dateTime ;
  dcterms:creator "superadmin" ;
  dcterms:modified "2016-09-13T06:32:51+00:00"^^xsd:dateTime ;
  skos:altLabel "Bush reserves"@en ;
  skos:altLabel "Marine reserves"@en ;
  skos:altLabel "Nature parks"@en ;
  skos:altLabel "Reserve management"@en ;
  skos:altLabel "Wetlands management"@en ;
  skos:broader agift:Natural-heritage-protection ;
  skos:definition "Administering designated native flora and fauna reserves, including nature parks, bush reserves and wetlands. Monitoring access restrictions and maintaining public amenities. Issuing permits for commercial or recreational activities. Assessing applications for development within nature reserves. Implementing regeneration or breeding programs for indigenous plants and animals."@en ;
  skos:prefLabel "Nature reserve management"@en ;
  skos:related agift:Feral-pest-control ;
  skos:related agift:Garden-management ;
  skos:related agift:National-park-management ;
  skos:related agift:Park-and-reserve-services ;
  skos:related agift:Recreational-park-management ;
  skos:related agift:Wilderness-area-management ;
  skos:related agift:Wildlife-sanctuary-management ;
.
agift:Navigation
  a skos:Concept ;
  dcterms:contributor "KOdea" ;
  dcterms:created "2016-07-06T03:39:28+00:00"^^xsd:dateTime ;
  dcterms:creator "superadmin" ;
  dcterms:modified "2016-09-09T07:31:38+00:00"^^xsd:dateTime ;
  skos:altLabel "Sea lane management"@en ;
  skos:altLabel "Sea lanes"@en ;
  skos:altLabel "Shipping channel management"@en ;
  skos:broader agift:MARITIME-SERVICES ;
  skos:definition "Developing policy to regulate the movement of ships and other commercial or private vessels. Managing shipping channels and monitoring the movement of ships at sea. Administering standards for safe and efficient navigation. Installing infrastructure to support maritime navigation."@en ;
  skos:narrower agift:Charting-sea-lanes ;
  skos:narrower agift:Light-station-maintenance ;
  skos:narrower agift:Navigation-systems-development ;
  skos:prefLabel "Navigation"@en ;
  skos:related agift:Port-regulation ;
.
agift:Navigation-systems-development
  a skos:Concept ;
  dcterms:contributor "KOdea" ;
  dcterms:created "2016-07-06T04:58:15+00:00"^^xsd:dateTime ;
  dcterms:creator "superadmin" ;
  dcterms:modified "2016-09-09T07:39:31+00:00"^^xsd:dateTime ;
  skos:broader agift:Navigation ;
  skos:definition "Conducting research into the application of specialist knowledge and equipment to support the plotting of courses at sea. Providing technical advice on the purchase of maritime navigational equipment and the development of global positioning networks. Includes designing, testing and overseeing the manufacture of new products."@en ;
  skos:prefLabel "Navigation systems development"@en ;
  skos:related agift:COMMUNICATIONS ;
  skos:related agift:Light-station-maintenance ;
  skos:related agift:Satellite-communication ;
  skos:related agift:Search-technology-development ;
  skos:related agift:Spatial-information-research ;
.
agift:Navy
  a skos:Concept ;
  dcterms:contributor "KOdea" ;
  dcterms:created "2016-07-06T04:08:50+00:00"^^xsd:dateTime ;
  dcterms:creator "superadmin" ;
  dcterms:modified "2016-09-09T07:42:14+00:00"^^xsd:dateTime ;
  skos:altLabel "Naval forces"@en ;
  skos:altLabel "RAN"@en ;
  skos:altLabel "Royal Australian Navy"@en ;
  skos:altLabel "Sailors"@en ;
  skos:broader agift:Australian-Defence-Forces ;
  skos:definition "Raising, equipping and maintaining the seagoing capability of Australia's defence forces. Administering Navy activities, implementing defence policy and coordinating joint defence forces operations. Includes on-the-job and basic training of new Navy recruits."@en ;
  skos:prefLabel "Navy"@en ;
  skos:related agift:MARITIME-SERVICES ;
  skos:related agift:Personnel-safety-standards ;
  skos:related agift:Reserves ;
  skos:related agift:Ship-personnel ;
.
agift:Notifiable-disease-management
  a skos:Concept ;
  dcterms:contributor "KOdea" ;
  dcterms:created "2016-07-06T04:48:25+00:00"^^xsd:dateTime ;
  dcterms:creator "superadmin" ;
  dcterms:modified "2016-09-09T06:22:19+00:00"^^xsd:dateTime ;
  skos:altLabel "Communicable diseases prevention"@en ;
  skos:altLabel "Contagious disease management"@en ;
  skos:altLabel "Disease reporting"@en ;
  skos:altLabel "Infectious disease management"@en ;
  skos:broader agift:Public-health-services ;
  skos:definition "Monitoring the incidence of communicable diseases and preventing large-scale outbreaks or epidemics. Compiling and managing data on the location and circumstances of infection. Developing reporting mechanisms to support the collection of data. Alerting authorities to significant occurrences or levels of contamination."@en ;
  skos:prefLabel "Notifiable disease management"@en ;
  skos:related agift:Epidemiology ;
  skos:related agift:Health-disaster-preparedness ;
  skos:related agift:Medical-quarantine-services ;
.
agift:Nuclear-safeguards
  a skos:Concept ;
  dcterms:contributor "KOdea" ;
  dcterms:created "2016-07-06T04:53:09+00:00"^^xsd:dateTime ;
  dcterms:creator "superadmin" ;
  dcterms:modified "2016-09-09T07:04:09+00:00"^^xsd:dateTime ;
  skos:altLabel "Nuclear safety"@en ;
  skos:broader agift:International-affairs ;
  skos:definition "Ensuring that nuclear material and associated equipment is fully accounted for and controlled. Developing and implementing security measures and precautions for the physical protection of nuclear items. Includes the operation of bilateral safeguard agreements."@en ;
  skos:prefLabel "Nuclear safeguards"@en ;
  skos:related agift:Disarmament-and-arms-control ;
  skos:related agift:Radiation-protection ;
.
agift:Nuclear-sciences
  a skos:Concept ;
  dcterms:contributor "KOdea" ;
  dcterms:created "2016-07-06T05:05:58+00:00"^^xsd:dateTime ;
  dcterms:creator "superadmin" ;
  dcterms:modified "2016-09-12T06:43:35+00:00"^^xsd:dateTime ;
  skos:altLabel "Atomic energy"@en ;
  skos:altLabel "Nuclear power"@en ;
  skos:broader agift:Physical-sciences ;
  skos:definition "Conducting research into the structure and nature of subatomic particles and related energy. Analysing changes in the behaviour and state of a nucleus in various conditions. Observing nuclear reactions to identify or develop products or processes for use in medical, industrial or defence applications, or to support other fields of scientific research. Determining the effects of nuclear weapons, radiation and fallout. Includes the management of reactors and other specialist equipment, and training programs for students and industry researchers."@en ;
  skos:prefLabel "Nuclear sciences"@en ;
  skos:related agift:Atomic-and-molecular-sciences ;
  skos:related agift:Defence-science-and-technology ;
  skos:related agift:Medical-radiation-services ;
.
agift:Occupational-health-and-safety
  a skos:Concept ;
  dcterms:contributor "KOdea" ;
  dcterms:created "2016-07-06T04:20:54+00:00"^^xsd:dateTime ;
  dcterms:creator "superadmin" ;
  dcterms:modified "2016-09-09T07:42:25+00:00"^^xsd:dateTime ;
  skos:altLabel "OH&S"@en ;
  skos:altLabel "Safety"@en ;
  skos:altLabel "Working conditions"@en ;
  skos:altLabel "Workplace health and safety"@en ;
  skos:altLabel "Workplace safety"@en ;
  skos:broader agift:Human-resources-development ;
  skos:definition "Administering programs to prevent death, injury or disease in the workplace. Implementing standards for occupational health and safety. Conducting research and collecting statistics. Monitoring workplace conditions and safety training programs"@en ;
  skos:prefLabel "Occupational health and safety"@en ;
  skos:related agift:Award-conditions ;
  skos:related agift:Cargo-control ;
  skos:related agift:Certified-employment-conditions ;
  skos:related agift:Health-hazard-prevention ;
  skos:related agift:Industrial-awards-and-conditions ;
  skos:related agift:Personnel-safety-standards ;
  skos:related agift:Workers-compensation-schemes ;
  skos:related agift:Workplace-agreement-processes ;
.
agift:Oceanography
  a skos:Concept ;
  dcterms:contributor "KOdea" ;
  dcterms:created "2016-07-06T05:05:16+00:00"^^xsd:dateTime ;
  dcterms:creator "superadmin" ;
  dcterms:modified "2016-09-12T06:36:33+00:00"^^xsd:dateTime ;
  skos:altLabel "El Nino effect"@en ;
  skos:altLabel "Marine science"@en ;
  skos:broader agift:Earth-sciences ;
  skos:definition "Conducting research into marine environments and the physical geography of seas. Studying interactions between oceans, continents, atmosphere and biosphere. Providing scientific advice on the sustainable use of coastal and ocean resources, and the impact of climate change. Analysing waves, currents, tides, ocean temperatures, salinity and acoustic properties. Includes oceanographic data collection, such as drilling and mapping of sea floor geology, and consultancy services in support of maritime activities."@en ;
  skos:prefLabel "Oceanography"@en ;
  skos:related agift:Biological-sciences ;
  skos:related agift:Marine-life-protection-programs ;
  skos:related agift:Oceans-governance ;
.
agift:Oceans-governance
  a skos:Concept ;
  dcterms:contributor "KOdea" ;
  dcterms:created "2016-07-06T03:03:13+00:00"^^xsd:dateTime ;
  dcterms:creator "superadmin" ;
  dcterms:modified "2016-09-12T06:34:30+00:00"^^xsd:dateTime ;
  skos:altLabel "Coastal engineering programs"@en ;
  skos:altLabel "Harbour protection programs"@en ;
  skos:broader agift:ENVIRONMENT ;
  skos:definition "Developing policy for the management and protection of marine environments. Planning for the sustainable development of ocean resources. Conducting negotiations across jurisdictions to ascertain authority over particular ocean regions."@en ;
  skos:prefLabel "Oceans governance"@en ;
  skos:related agift:Aquaculture-industry ;
  skos:related agift:Fisheries-industry ;
  skos:related agift:Harbour-management ;
  skos:related agift:Hydrology ;
  skos:related agift:Marina-management ;
  skos:related agift:Marine-and-rural-regulation ;
  skos:related agift:Marine-life-protection-programs ;
  skos:related agift:Oceanography ;
  skos:related agift:Port-regulation ;
  skos:related agift:Water-resources ;
  skos:related agift:Waterway-management ;
.
agift:Official-establishment-management
  a skos:Concept ;
  dcterms:contributor "KOdea" ;
  dcterms:created "2016-07-06T04:42:22+00:00"^^xsd:dateTime ;
  dcterms:creator "superadmin" ;
  dcterms:modified "2016-09-09T05:54:52+00:00"^^xsd:dateTime ;
  skos:altLabel "Government residences"@en ;
  skos:altLabel "Official residences"@en ;
  skos:broader agift:Official-protocol ;
  skos:definition "Administering the buildings and grounds of official residences of high-level government representatives. Overseeing maintenance and tenancy arrangements. Managing public visits to official residences. Includes liaison with occupants and official establishment committees, in accordance with official protocol."@en ;
  skos:prefLabel "Official establishment management"@en ;
  skos:related agift:Head-of-Government-protocol ;
  skos:related agift:Official-hospitality ;
  skos:related agift:Official-visits ;
.
agift:Official-hospitality
  a skos:Concept ;
  dcterms:contributor "KOdea" ;
  dcterms:created "2016-07-06T04:42:30+00:00"^^xsd:dateTime ;
  dcterms:creator "superadmin" ;
  dcterms:modified "2016-09-09T05:54:07+00:00"^^xsd:dateTime ;
  skos:altLabel "Government hospitality"@en ;
  skos:broader agift:Official-protocol ;
  skos:definition "Planning the reception and entertainment of high-level government representatives. Making arrangements to support official protocol, such as arranging gifts, researching customs and procedures. Organising accommodation, catering and decorations."@en ;
  skos:prefLabel "Official hospitality"@en ;
  skos:related agift:Ceremonial-events-and-representation ;
  skos:related agift:Head-of-Government-protocol ;
  skos:related agift:Official-establishment-management ;
  skos:related agift:Official-visits ;
.
agift:Official-protocol
  a skos:Concept ;
  dcterms:contributor "KOdea" ;
  dcterms:created "2016-07-06T03:06:16+00:00"^^xsd:dateTime ;
  dcterms:creator "superadmin" ;
  dcterms:modified "2016-09-09T05:51:18+00:00"^^xsd:dateTime ;
  skos:altLabel "Ceremonial protocol"@en ;
  skos:altLabel "Government protocol"@en ;
  skos:altLabel "International protocol"@en ;
  skos:broader agift:GOVERNANCE ;
  skos:definition "Developing policy and guidelines to support the activities of high-level government representatives in carrying out their official duties. Determining appropriate conventions, customs and arrangements required during formal procedures and functions, either in Australia or overseas. Includes research, advice and support services for occasions where official protocol is to be followed."@en ;
  skos:narrower agift:Ceremonial-events-and-representation ;
  skos:narrower agift:Head-of-Government-protocol ;
  skos:narrower agift:Official-establishment-management ;
  skos:narrower agift:Official-hospitality ;
  skos:narrower agift:Official-visits ;
  skos:prefLabel "Official protocol"@en ;
.
agift:Official-visits
  a skos:Concept ;
  dcterms:contributor "KOdea" ;
  dcterms:created "2016-07-06T04:42:37+00:00"^^xsd:dateTime ;
  dcterms:creator "superadmin" ;
  dcterms:modified "2016-09-09T05:54:52+00:00"^^xsd:dateTime ;
  skos:altLabel "Government visits"@en ;
  skos:altLabel "Royal visits"@en ;
  skos:broader agift:Official-protocol ;
  skos:definition "Planning visits for domestic government representatives, and making arrangements for visits by representatives of other governments. Developing programs and itineraries. Managing publicity. Organising accommodation, travel and security. Includes visits for business, cultural or social reasons."@en ;
  skos:prefLabel "Official visits"@en ;
  skos:related agift:Ceremonial-events-and-representation ;
  skos:related agift:Head-of-Government-protocol ;
  skos:related agift:Official-establishment-management ;
  skos:related agift:Official-hospitality ;
.
agift:Online-transaction-standards
  a skos:Concept ;
  dcterms:contributor "KOdea" ;
  dcterms:created "2016-07-06T03:57:09+00:00"^^xsd:dateTime ;
  dcterms:creator "superadmin" ;
  dcterms:modified "2016-09-05T07:35:59+00:00"^^xsd:dateTime ;
  skos:altLabel "Digital transactions standards"@en ;
  skos:altLabel "Electronic transactions standards"@en ;
  skos:broader agift:Electronic-commerce ;
  skos:definition "Establishing guidelines and models to facilitate the conduct of electronic commerce. Supporting the application of existing commercial legislation in an online environment. Providing advice on the implementation of standards and monitoring compliance."@en ;
  skos:prefLabel "Online transaction standards"@en ;
  skos:related agift:Data-management ;
  skos:related agift:Information-management-standards ;
  skos:related agift:Information-technology-standards ;
.
agift:Open-government
  a skos:Concept ;
  dcterms:contributor "KOdea" ;
  dcterms:created "2016-07-06T03:06:22+00:00"^^xsd:dateTime ;
  dcterms:creator "superadmin" ;
  dcterms:modified "2016-09-09T05:55:29+00:00"^^xsd:dateTime ;
  skos:broader agift:GOVERNANCE ;
  skos:definition "Facilitating citizen collaboration by developing services and programs based on open government principles. Encouraging public engagement in policy and service design and delivery."@en ;
  skos:prefLabel "Open government"@en ;
  skos:related agift:Freedom-of-information ;
  skos:related agift:Recordkeeping-standards ;
.
agift:Overseas-aid-programs
  a skos:Concept ;
  dcterms:contributor "KOdea" ;
  dcterms:created "2016-07-06T03:36:23+00:00"^^xsd:dateTime ;
  dcterms:creator "superadmin" ;
  dcterms:modified "2016-09-08T07:12:02+00:00"^^xsd:dateTime ;
  skos:altLabel "Aid development"@en ;
  skos:altLabel "Aid programs"@en ;
  skos:altLabel "International aid"@en ;
  skos:broader agift:INTERNATIONAL-RELATIONS ;
  skos:definition "Developing policy and schemes to assist developing countries to reduce poverty, promote sustainable economic growth and recover from conflict or disasters. Working in partnership with other governments, businesses, non-government organisations and international agencies. Fostering links between the Australian community and the people of developing countries. Includes contributions to multilateral development banks and direct assistance packages."@en ;
  skos:narrower agift:Development-assistance-programs ;
  skos:narrower agift:Overseas-student-scholarship-programs ;
  skos:prefLabel "Overseas aid programs"@en ;
  skos:related agift:School-education ;
.
agift:Overseas-promotion
  a skos:Concept ;
  dcterms:contributor "KOdea" ;
  dcterms:created "2016-07-06T03:36:30+00:00"^^xsd:dateTime ;
  dcterms:creator "superadmin" ;
  dcterms:modified "2016-09-13T06:56:45+00:00"^^xsd:dateTime ;
  skos:altLabel "Expos"@en ;
  skos:altLabel "Expositions"@en ;
  skos:altLabel "International cultural exchanges"@en ;
  skos:altLabel "International expositions"@en ;
  skos:broader agift:INTERNATIONAL-RELATIONS ;
  skos:definition "Undertaking liaison activities to raise Australia's international profile. Developing cultural exchange programs and advocating the benefits of international business. Establishing corporate networks and reciprocal visitor programs. Includes identifying and negotiating opportunities to promote Australia overseas, such as participating in international expositions, hosting major sporting events or cultural festivals."@en ;
  skos:prefLabel "Overseas promotion"@en ;
  skos:related agift:Cultural-festivals ;
  skos:related agift:Export-promotion ;
  skos:related agift:Games-promotion ;
  skos:related agift:Multicultural-festivals ;
  skos:related agift:Tourist-event-promotion ;
  skos:related agift:Trade-expositions ;
.
agift:Overseas-skills-recognition
  a skos:Concept ;
  dcterms:contributor "KOdea" ;
  dcterms:created "2016-07-06T03:00:31+00:00"^^xsd:dateTime ;
  dcterms:creator "superadmin" ;
  dcterms:modified "2016-09-09T06:13:49+00:00"^^xsd:dateTime ;
  skos:altLabel "Accreditation criteria"@en ;
  skos:altLabel "International qualifications"@en ;
  skos:altLabel "International skills recognition"@en ;
  skos:altLabel "Overseas qualifications"@en ;
  skos:broader agift:EDUCATION-AND-TRAINING ;
  skos:definition "Endorsing or accrediting educational qualifications obtained outside Australia. Recognising Australians who have studied overseas or migrants wishing to apply their qualifications in Australia. Includes processing applications, managing examinations and setting conditions on the right to apply qualifications in certain fields."@en ;
  skos:prefLabel "Overseas skills recognition"@en ;
  skos:related agift:Practitioner-registration ;
  skos:related agift:Professional-accreditation ;
.
agift:Overseas-student-scholarship-programs
  a skos:Concept ;
  dcterms:contributor "KOdea" ;
  dcterms:created "2016-07-06T04:53:54+00:00"^^xsd:dateTime ;
  dcterms:creator "superadmin" ;
  dcterms:modified "2016-09-09T07:08:50+00:00"^^xsd:dateTime ;
  skos:altLabel "International scholarship programs"@en ;
  skos:altLabel "Regional scholarship programs"@en ;
  skos:altLabel "Scholarship programs"@en ;
  skos:broader agift:Overseas-aid-programs ;
  skos:definition "Supporting access to higher education for students from developing countries and the Pacific region. Providing assistance to study at regional education institutions, or opportunities to attend Australian education institutions. Includes services and training to help scholarship students realise the full benefits of the program."@en ;
  skos:prefLabel "Overseas student scholarship programs"@en ;
  skos:related agift:Arts-education ;
  skos:related agift:Development-assistance-programs ;
  skos:related agift:EDUCATION-AND-TRAINING ;
  skos:related agift:Tertiary-education ;
.
agift:PRIMARY-INDUSTRIES
  skos:prefLabel "PRIMARY INDUSTRIES"@en ;
  owl:deprecated true ;
.
agift:PRIMARY-INDUSTRIES
  a skos:Concept ;
  dcterms:contributor "fionamcl" ;
  dcterms:created "2016-07-06T02:47:26+00:00"^^xsd:dateTime ;
  dcterms:creator "superadmin" ;
  dcterms:modified "2016-09-20T00:05:53+00:00"^^xsd:dateTime ;
  skos:altLabel "Agriculture"@en ;
  skos:altLabel "Industry"@en ;
  skos:altLabel "Marine industry"@en ;
  skos:altLabel "Rural industry"@en ;
  skos:definition "Developing policy to support and regulate rural and marine industries. Promoting strategies for efficient and sustainable operations. Administering programs to monitor current practices, to meet national and international standards. Includes liaison with industry bodies and across jurisdictions in relation to the needs of primary industries."@en ;
  skos:narrower agift:Chemical-and-pesticide-regulation ;
  skos:narrower agift:Marine-and-rural-regulation ;
  skos:narrower agift:Marine-and-rural-support ;
  skos:narrower agift:Quarantine ;
  skos:narrower agift:Rural-field-day-promotion ;
  skos:narrower agift:Rural-partnership-programs ;
  skos:prefLabel "PRIMARY INDUSTRIES"@en ;
  skos:related agift:BUSINESS-SUPPORT-AND-REGULATION ;
  skos:related agift:NATURAL-RESOURCES ;
  skos:related agift:SCIENCE ;
  skos:related agift:Waterway-management ;
  skos:topConceptOf agift:AGIFT ;
.
agift:Park-and-reserve-services
  a skos:Concept ;
  dcterms:contributor "KOdea" ;
  dcterms:created "2016-07-06T03:45:45+00:00"^^xsd:dateTime ;
  dcterms:creator "superadmin" ;
  dcterms:modified "2016-09-13T06:33:39+00:00"^^xsd:dateTime ;
  skos:altLabel "Cricket grounds"@en ;
  skos:altLabel "Football stadiums"@en ;
  skos:altLabel "Park access and permits"@en ;
  skos:altLabel "Reserve management"@en ;
  skos:altLabel "Sporting field management"@en ;
  skos:broader agift:SPORT-AND-RECREATION ;
  skos:definition "Administering areas of public land set aside for sport and recreational activities. Managing bookings, programs and payments. Controlling access and issuing permits for the use of parks and reserves. Supervising the allocation of sponsorships and corporate memberships. Ensuring the availability of staff such as referees or umpires."@en ;
  skos:prefLabel "Park and reserve services"@en ;
  skos:related agift:Garden-management ;
  skos:related agift:Indigenous-heritage-conservation ;
  skos:related agift:National-park-management ;
  skos:related agift:Nature-reserve-management ;
  skos:related agift:Recreational-park-management ;
  skos:related agift:Sporting-facilities-management ;
  skos:related agift:Sporting-grants-administration ;
.
agift:Parliamentary-chamber-support
  a skos:Concept ;
  dcterms:contributor "KOdea" ;
  dcterms:created "2016-07-06T03:06:30+00:00"^^xsd:dateTime ;
  dcterms:creator "superadmin" ;
  dcterms:modified "2016-09-09T05:57:33+00:00"^^xsd:dateTime ;
  skos:altLabel "Council chambers support"@en ;
  skos:altLabel "House of Representatives support"@en ;
  skos:altLabel "Joint Standing Committee support"@en ;
  skos:altLabel "Legislative Assembly support"@en ;
  skos:altLabel "Municipal council support"@en ;
  skos:altLabel "Parliamentary support services"@en ;
  skos:broader agift:GOVERNANCE ;
  skos:definition "Providing corporate assistance and security services to Houses of Parliament, assemblies or governing councils. Making arrangements for accommodation, equipment and catering. Overseeing building and maintenance requirements. Supervising broadcasts of parliamentary proceedings."@en ;
  skos:narrower agift:Hansard-services ;
  skos:narrower agift:Parliamentary-papers ;
  skos:narrower agift:Tabling-of-official-documents ;
  skos:prefLabel "Parliamentary chamber support"@en ;
  skos:related agift:Parliamentary-committee-and-member-support ;
  skos:related agift:Parliamentary-papers ;
.
agift:Parliamentary-committee-and-member-support
  a skos:Concept ;
  dcterms:contributor "KOdea" ;
  dcterms:created "2016-07-06T03:06:37+00:00"^^xsd:dateTime ;
  dcterms:creator "superadmin" ;
  dcterms:modified "2016-09-09T05:56:33+00:00"^^xsd:dateTime ;
  skos:altLabel "Lord Mayor"@en ;
  skos:altLabel "Mayor"@en ;
  skos:broader agift:GOVERNANCE ;
  skos:definition "Supplying administrative assistance to elected members, in all tiers of Australian government, to help them fulfil their duties. Managing secretariat support and secretarial staff. Providing access to reference and research services. Offering advice on procedures and the interpretation of standing orders."@en ;
  skos:prefLabel "Parliamentary committee and member support"@en ;
  skos:related agift:Hansard-services ;
  skos:related agift:Parliamentary-chamber-support ;
.
agift:Parliamentary-papers
  a skos:Concept ;
  dcterms:contributor "KOdea" ;
  dcterms:created "2016-07-06T04:43:06+00:00"^^xsd:dateTime ;
  dcterms:creator "superadmin" ;
  dcterms:modified "2016-09-09T05:57:33+00:00"^^xsd:dateTime ;
  skos:broader agift:Parliamentary-chamber-support ;
  skos:definition "Managing reports and other documents that have been officially tabled before parliament or an assembly. Organising the printing of presented papers, to support public scrutiny of government policy and parliamentary processes. Includes printing and gazetting of legislation passed through parliament."@en ;
  skos:prefLabel "Parliamentary papers"@en ;
  skos:related agift:Court-reporting ;
  skos:related agift:Draft-Bill-amendment-process ;
  skos:related agift:Legislative-drafting ;
  skos:related agift:Parliamentary-chamber-support ;
.
agift:Passenger-services
  a skos:Concept ;
  dcterms:contributor "KOdea" ;
  dcterms:created "2016-07-06T03:49:46+00:00"^^xsd:dateTime ;
  dcterms:creator "superadmin" ;
  dcterms:modified "2016-09-13T07:20:47+00:00"^^xsd:dateTime ;
  skos:broader agift:TRANSPORT ;
  skos:definition "Developing policy for the transportation of people by air, rail or road. Monitoring compliance with pricing regulations or the provision of appropriate facilities for passenger convenience. Includes services such as timetables, route maps or ticketing."@en ;
  skos:prefLabel "Passenger services"@en ;
  skos:related agift:Airport-services ;
  skos:related agift:Public-transport ;
  skos:related agift:Rail-transport ;
  skos:related agift:Road-transport-safety ;
  skos:related agift:School-transport-regulation ;
  skos:related agift:Sea-passengers ;
  skos:related agift:Transport-network-maintenance ;
.
agift:Passport-services
  a skos:Concept ;
  dcterms:contributor "KOdea" ;
  dcterms:created "2016-07-06T03:36:39+00:00"^^xsd:dateTime ;
  dcterms:creator "superadmin" ;
  dcterms:modified "2016-09-09T06:59:09+00:00"^^xsd:dateTime ;
  skos:altLabel "Passports"@en ;
  skos:broader agift:INTERNATIONAL-RELATIONS ;
  skos:definition "Issuing passports and travel documents to Australian citizens in Australia and overseas. Managing applications and renewals, providing advice and liaising with outlets that provide lodgement services."@en ;
  skos:prefLabel "Passport services"@en ;
  skos:related agift:Consular-services ;
  skos:related agift:Travel-authorisation ;
.
agift:Pastoral-industry
  a skos:Concept ;
  dcterms:contributor "KOdea" ;
  dcterms:created "2016-07-06T05:02:48+00:00"^^xsd:dateTime ;
  dcterms:creator "superadmin" ;
  dcterms:modified "2016-09-12T06:16:43+00:00"^^xsd:dateTime ;
  skos:altLabel "Dairy industry support"@en ;
  skos:altLabel "Game  animal  industry support"@en ;
  skos:altLabel "Livestock industry support"@en ;
  skos:altLabel "Wool industry support"@en ;
  skos:broader agift:Marine-and-rural-support ;
  skos:definition "Administering programs to support commercial game and livestock farming. Assisting industry growth and development. Encouraging businesses to adopt innovative practices, processes and products. Providing advice on production methods and business management to improve competitiveness."@en ;
  skos:prefLabel "Pastoral industry"@en ;
  skos:related agift:Agricultural-industry ;
  skos:related agift:Animal-and-veterinary-sciences ;
  skos:related agift:Horticultural-industry ;
.
agift:Patent-rights-management
  a skos:Concept ;
  dcterms:contributor "KOdea" ;
  dcterms:created "2016-07-06T05:13:41+00:00"^^xsd:dateTime ;
  dcterms:creator "superadmin" ;
  dcterms:modified "2016-09-13T07:05:56+00:00"^^xsd:dateTime ;
  skos:broader agift:Intellectual-property-management ;
  skos:definition "Conferring exclusive legal rights to the production or sale of an invention or an industrial or scientific process. Registering and granting patent rights and making patent specifications  available to the public."@en ;
  skos:prefLabel "Patent rights management"@en ;
  skos:related agift:Design-rights-management ;
  skos:related agift:Plant-breeders-rights-management ;
  skos:related agift:Trademark-registration ;
.
agift:Patient-care
  a skos:Concept ;
  dcterms:contributor "KOdea" ;
  dcterms:created "2016-07-06T04:46:15+00:00"^^xsd:dateTime ;
  dcterms:creator "superadmin" ;
  dcterms:modified "2016-09-09T06:15:25+00:00"^^xsd:dateTime ;
  skos:altLabel "Nursing"@en ;
  skos:altLabel "Outpatient services"@en ;
  skos:broader agift:Hospital-services ;
  skos:definition "Providing direct supervision and nursing for individuals under medical or surgical treatment. Implementing hospital policy and standards of best practice to ensure patients recover as fully and quickly as possible. Supplying food, amenities and recreation. Includes follow-up services after a patient has been released."@en ;
  skos:prefLabel "Patient care"@en ;
  skos:related agift:Independent-living-services ;
  skos:related agift:Residential-services ;
.
agift:Payments-management
  a skos:Concept ;
  dcterms:contributor "KOdea" ;
  dcterms:created "2016-07-06T04:36:09+00:00"^^xsd:dateTime ;
  dcterms:creator "superadmin" ;
  dcterms:modified "2016-08-22T05:58:23+00:00"^^xsd:dateTime ;
  skos:altLabel "Automatic teller machine (ATM)"@en ;
  skos:altLabel "Cheques"@en ;
  skos:altLabel "Credit cards"@en ;
  skos:altLabel "Debit cards"@en ;
  skos:altLabel "EFT/POS"@en ;
  skos:altLabel "Electronic Funds Transfer (EFT)"@en ;
  skos:altLabel "Real-time gross settlement (RTGS)"@en ;
  skos:broader agift:Financial-system-management ;
  skos:definition "Managing the transfer of funds between consumers, businesses and financial institutions. Monitoring the payment instruments (cash, cheque and electronic funds transfer) used by consumers and businesses to transact business, and the transfer of funds from accounts in one financial institution to another."@en ;
  skos:prefLabel "Payments management"@en ;
.
agift:Peacekeeping-forces
  a skos:Concept ;
  dcterms:contributor "KOdea" ;
  dcterms:created "2016-07-06T05:06:47+00:00"^^xsd:dateTime ;
  dcterms:creator "superadmin" ;
  dcterms:modified "2016-09-09T07:08:10+00:00"^^xsd:dateTime ;
  skos:broader agift:External-security ;
  skos:definition "Deploying defence units to stabilise unrest and restore order in a designated international arena. Participating in cooperative efforts to alleviate international conflict, establish and maintain peace."@en ;
  skos:prefLabel "Peacekeeping forces"@en ;
  skos:related agift:Defence-cooperation-programs ;
  skos:related agift:Development-assistance-programs ;
  skos:related agift:Disaster-support ;
  skos:related agift:Military-operations ;
  skos:related agift:Special-operations ;
  skos:related agift:Warfare ;
.
agift:Permanent-entry-arrangements
  a skos:Concept ;
  dcterms:contributor "KOdea" ;
  dcterms:created "2016-07-06T04:50:50+00:00"^^xsd:dateTime ;
  dcterms:creator "superadmin" ;
  dcterms:modified "2016-09-09T06:39:49+00:00"^^xsd:dateTime ;
  skos:altLabel "Migration applications"@en ;
  skos:altLabel "Permanent residence visas"@en ;
  skos:altLabel "Resident return visas"@en ;
  skos:altLabel "Skilled migrant program"@en ;
  skos:altLabel "Visa applications"@en ;
  skos:broader agift:Travel-authorisation ;
  skos:definition "Administering programs to ensure lawful entrance of foreign nationals or refugees intending to settle in Australia. Processing applications for visas or migration and providing advice to applicants. Includes family reunion and special eligibility streams."@en ;
  skos:prefLabel "Permanent entry arrangements"@en ;
  skos:related agift:Migrant-services ;
.
agift:Personnel-safety-standards
  a skos:Concept ;
  dcterms:contributor "KOdea" ;
  dcterms:created "2016-07-06T04:59:03+00:00"^^xsd:dateTime ;
  dcterms:creator "superadmin" ;
  dcterms:modified "2016-09-09T07:43:46+00:00"^^xsd:dateTime ;
  skos:altLabel "Crew safety standards"@en ;
  skos:altLabel "Ship operation standards"@en ;
  skos:broader agift:Ship-personnel ;
  skos:definition "Monitoring compliance with standards and guidelines for the operation of private or commercial marine vessels. Conducting safety training, competency checks and inspections to assess operational practices."@en ;
  skos:prefLabel "Personnel safety standards"@en ;
  skos:related agift:Navy ;
  skos:related agift:Occupational-health-and-safety ;
  skos:related agift:Sea-passengers ;
.
agift:Pharmaceutical-and-drug-support
  a skos:Concept ;
  dcterms:contributor "KOdea" ;
  dcterms:created "2016-07-06T04:46:24+00:00"^^xsd:dateTime ;
  dcterms:creator "superadmin" ;
  dcterms:modified "2016-08-23T06:37:59+00:00"^^xsd:dateTime ;
  skos:altLabel "Drug support services"@en ;
  skos:altLabel "Pharmaceutical information"@en ;
  skos:broader agift:Hospital-services ;
  skos:definition "Providing information about medical substances to hospitals and other health services. Administering drug management systems and offering advice on drug interactions for prescribers. Maintaining patient histories, including drug sensitivities and allergies."@en ;
  skos:prefLabel "Pharmaceutical and drug support"@en ;
.
agift:Physical-sciences
  a skos:Concept ;
  dcterms:contributor "KOdea" ;
  dcterms:created "2016-07-06T03:43:48+00:00"^^xsd:dateTime ;
  dcterms:creator "superadmin" ;
  dcterms:modified "2016-09-12T06:41:30+00:00"^^xsd:dateTime ;
  skos:altLabel "Chemical analysis"@en ;
  skos:altLabel "Chemistry"@en ;
  skos:altLabel "Physics"@en ;
  skos:broader agift:SCIENCE ;
  skos:definition "Conducting research into the properties of inanimate matter, substances and energy. Analysing and manipulating such material to identify the principles and processes that govern its behaviour. Includes the development of new methods to exploit physical substances or energy."@en ;
  skos:narrower agift:Astronomical-sciences ;
  skos:narrower agift:Atomic-and-molecular-sciences ;
  skos:narrower agift:Nuclear-sciences ;
  skos:prefLabel "Physical sciences"@en ;
  skos:related agift:Applied-sciences ;
  skos:related agift:Biological-sciences ;
.
agift:Physiology
  a skos:Concept ;
  dcterms:contributor "KOdea" ;
  dcterms:created "2016-07-06T05:04:37+00:00"^^xsd:dateTime ;
  dcterms:creator "superadmin" ;
  dcterms:modified "2016-09-12T06:33:33+00:00"^^xsd:dateTime ;
  skos:altLabel "Anatomy"@en ;
  skos:altLabel "Neurology"@en ;
  skos:broader agift:Biological-sciences ;
  skos:definition "Conducting research into biological functions and systems. Analysing the structure and anatomy of organisms. Investigating the internal processes of plants and animals at tissue- and organ-level. Determining how particular physiological attributes contribute to an organism's fitness and performance. Includes pharmacological and immunological studies to develop new drugs or vaccines."@en ;
  skos:prefLabel "Physiology"@en ;
  skos:related agift:Animal-and-veterinary-sciences ;
  skos:related agift:Medical-and-health-sciences ;
.
agift:Pilotage-management
  a skos:Concept ;
  dcterms:contributor "KOdea" ;
  dcterms:created "2016-07-06T03:39:35+00:00"^^xsd:dateTime ;
  dcterms:creator "superadmin" ;
  dcterms:modified "2016-08-29T06:47:00+00:00"^^xsd:dateTime ;
  skos:altLabel "Coastal pilotage"@en ;
  skos:altLabel "Marine pilotage"@en ;
  skos:altLabel "Vessel piloting"@en ;
  skos:broader agift:MARITIME-SERVICES ;
  skos:definition "Providing qualified operators to steer vessels into and out of ports. Monitoring pilotage procedures and clarifying the responsibilities of pilots and pilotage providers. Developing and administering standards for pilotage operations that support international requirements."@en ;
  skos:prefLabel "Pilotage management"@en ;
.
agift:Place-names
  a skos:Concept ;
  dcterms:contributor "KOdea" ;
  dcterms:created "2016-07-06T02:52:09+00:00"^^xsd:dateTime ;
  dcterms:creator "superadmin" ;
  dcterms:modified "2016-08-05T03:54:53+00:00"^^xsd:dateTime ;
  skos:altLabel "Geographic names"@en ;
  skos:broader agift:CIVIC-INFRASTRUCTURE ;
  skos:definition "Approving and registering the formal names of rivers, mountains, plains, towns, suburbs, reefs, shoals and undersea features."@en ;
  skos:prefLabel "Place names"@en ;
.
agift:Plant-breeders-rights-management
  a skos:Concept ;
  dcterms:contributor "KOdea" ;
  dcterms:created "2016-07-06T05:13:48+00:00"^^xsd:dateTime ;
  dcterms:creator "superadmin" ;
  dcterms:modified "2016-09-13T07:06:09+00:00"^^xsd:dateTime ;
  skos:broader agift:Intellectual-property-management ;
  skos:definition "Developing policy to protect the rights of plant  breeders developing new plant varieties."@en ;
  skos:prefLabel "Plant breeders' rights management"@en ;
  skos:related agift:Design-rights-management ;
  skos:related agift:Patent-rights-management ;
  skos:related agift:Trademark-registration ;
.
agift:Police-administration
  a skos:Concept ;
  dcterms:contributor "KOdea" ;
  dcterms:created "2016-07-06T05:08:08+00:00"^^xsd:dateTime ;
  dcterms:creator "superadmin" ;
  dcterms:modified "2016-08-30T07:24:04+00:00"^^xsd:dateTime ;
  skos:altLabel "Police stations"@en ;
  skos:broader agift:Law-enforcement ;
  skos:definition "Providing trained personnel to assist citizens who have been victims of crime, or in matters of law enforcement. Managing staff and facilities at police stations. Administering internal command, investigation and disciplinary procedures"@en ;
  skos:prefLabel "Police administration"@en ;
.
agift:Pollutant-prevention-programs
  a skos:Concept ;
  dcterms:contributor "KOdea" ;
  dcterms:created "2016-07-06T03:03:20+00:00"^^xsd:dateTime ;
  dcterms:creator "superadmin" ;
  dcterms:modified "2016-09-08T07:50:55+00:00"^^xsd:dateTime ;
  skos:altLabel "Noise pollution"@en ;
  skos:altLabel "Oil spill prevention programs"@en ;
  skos:altLabel "Smog prevention programs"@en ;
  skos:altLabel "Waste control programs"@en ;
  skos:broader agift:ENVIRONMENT ;
  skos:definition "Establishing standards and developing initiatives to reduce contamination of the air, water and land by emissions and waste. Developing strategies to counteract the effects of pollutants if accidents occur. Raising awareness and supporting community activities to change common practice. Promoting environmentally friendly alternatives."@en ;
  skos:prefLabel "Pollutant prevention programs"@en ;
  skos:related agift:Atmospheric-sciences ;
  skos:related agift:Pollution-emission-control ;
  skos:related agift:Waste-management ;
  skos:related agift:Waterway-management ;
.
agift:Pollution-emission-control
  a skos:Concept ;
  dcterms:contributor "KOdea" ;
  dcterms:created "2016-07-06T03:41:13+00:00"^^xsd:dateTime ;
  dcterms:creator "superadmin" ;
  dcterms:modified "2016-09-12T06:02:58+00:00"^^xsd:dateTime ;
  skos:altLabel "Effluent control"@en ;
  skos:altLabel "Emissions control"@en ;
  skos:altLabel "Pollution"@en ;
  skos:broader agift:NATURAL-RESOURCES ;
  skos:definition "Monitoring compliance with standards for the discharge of industrial contaminants and waste. Regulating industry practices through waste minimisation strategies and pollutant inventories. Includes assessment, inspections and providing emissions information to the community."@en ;
  skos:prefLabel "Pollution emission control"@en ;
  skos:related agift:Atmospheric-sciences ;
  skos:related agift:Pollutant-prevention-programs ;
  skos:related agift:Waste-management ;
  skos:related agift:Water-quality-monitoring ;
.
agift:Population-based-research
  a skos:Concept ;
  dcterms:contributor "KOdea" ;
  dcterms:created "2016-07-06T04:47:08+00:00"^^xsd:dateTime ;
  dcterms:creator "superadmin" ;
  dcterms:modified "2016-09-09T06:19:49+00:00"^^xsd:dateTime ;
  skos:altLabel "Drug support services"@en ;
  skos:broader agift:Medical-research ;
  skos:definition "Conducting clinical investigations of the health of particular groups of individuals. Evaluating the incidence of particular diseases within a geographical area or demographic category. Making recommendations to support public health policy development."@en ;
  skos:prefLabel "Population-based research"@en ;
  skos:related agift:Epidemiology ;
  skos:related agift:Medical-and-health-sciences ;
  skos:related agift:Statistical-collection ;
.
agift:Port-regulation
  a skos:Concept ;
  dcterms:contributor "KOdea" ;
  dcterms:created "2016-07-06T03:39:43+00:00"^^xsd:dateTime ;
  dcterms:creator "superadmin" ;
  dcterms:modified "2016-09-13T07:23:00+00:00"^^xsd:dateTime ;
  skos:altLabel "Ports"@en ;
  skos:altLabel "Seaport regulation"@en ;
  skos:altLabel "Shipping channel management"@en ;
  skos:altLabel "Wharf management"@en ;
  skos:broader agift:MARITIME-SERVICES ;
  skos:definition "Managing sea-based entry and exit points. Building and maintaining infrastructure to allow ships to load or unload passengers and cargo. Monitoring private terminal operators and regulating port activities to protect against environmental impacts. Assessing the integration of road, rail and air transport infrastructure with maritime services. Includes liaison to promote coordination and consistency among port authorities from different jurisdictions."@en ;
  skos:prefLabel "Port regulation"@en ;
  skos:related agift:Cargo-control ;
  skos:related agift:Charting-sea-lanes ;
  skos:related agift:Export-regulation ;
  skos:related agift:Harbour-management ;
  skos:related agift:Import-regulation ;
  skos:related agift:Marina-management ;
  skos:related agift:Navigation ;
  skos:related agift:Oceans-governance ;
  skos:related agift:Tariff-regulation ;
  skos:related agift:Transport-infrastructure-development ;
  skos:related agift:Waterway-management ;
.
agift:Postal-services
  a skos:Concept ;
  dcterms:contributor "KOdea" ;
  dcterms:created "2016-07-06T02:54:23+00:00"^^xsd:dateTime ;
  dcterms:creator "superadmin" ;
  dcterms:modified "2016-08-05T05:40:59+00:00"^^xsd:dateTime ;
  skos:altLabel "Australia Post"@en ;
  skos:altLabel "Mail services"@en ;
  skos:altLabel "Postage stamps"@en ;
  skos:broader agift:COMMUNICATIONS ;
  skos:definition "Developing policy and guidelines to support the collection and delivery of letters, parcels and other mail. Establishing standards for pricing and processing, such as ensuring dangerous goods are intercepted. Designing and issuing postage stamps."@en ;
  skos:narrower agift:Courier-services ;
  skos:narrower agift:Electronic-postal-services ;
  skos:narrower agift:Retail-postal-services ;
  skos:prefLabel "Postal services"@en ;
.
agift:Practitioner-discipline
  a skos:Concept ;
  dcterms:contributor "KOdea" ;
  dcterms:created "2016-07-06T04:45:42+00:00"^^xsd:dateTime ;
  dcterms:creator "superadmin" ;
  dcterms:modified "2016-09-09T06:14:22+00:00"^^xsd:dateTime ;
  skos:altLabel "Malpractice"@en ;
  skos:altLabel "Medical negligence"@en ;
  skos:broader agift:Health-protocol-administration ;
  skos:definition "Administering guidelines to assess the professional conduct of health care providers. Evaluating performance against established standards and codes of practice. Investigating complaints and initiating disciplinary proceedings or applying penalties when appropriate. Includes suspending or deregistering practitioners found in breach of regulations."@en ;
  skos:prefLabel "Practitioner discipline"@en ;
  skos:related agift:Practitioner-registration ;
.
agift:Practitioner-registration
  a skos:Concept ;
  dcterms:contributor "KOdea" ;
  dcterms:created "2016-07-06T04:45:48+00:00"^^xsd:dateTime ;
  dcterms:creator "superadmin" ;
  dcterms:modified "2016-09-09T06:14:22+00:00"^^xsd:dateTime ;
  skos:altLabel "Doctor registration"@en ;
  skos:altLabel "General practitioner registration"@en ;
  skos:altLabel "Health accreditation"@en ;
  skos:altLabel "Health practitioner registration"@en ;
  skos:broader agift:Health-protocol-administration ;
  skos:definition "Evaluating the qualifications of health care providers to determine their fitness for medical practice. Assessing applications and providing advice to unsuccessful applicants. Maintaining a register of approved applicants who may legally practice."@en ;
  skos:prefLabel "Practitioner registration"@en ;
  skos:related agift:Overseas-skills-recognition ;
  skos:related agift:Practitioner-discipline ;
.
agift:Preparation-of-legislative-regulations
  a skos:Concept ;
  dcterms:contributor "KOdea" ;
  dcterms:created "2016-07-06T04:41:45+00:00"^^xsd:dateTime ;
  dcterms:creator "superadmin" ;
  dcterms:modified "2016-08-22T06:59:20+00:00"^^xsd:dateTime ;
  skos:altLabel "Regulation development"@en ;
  skos:altLabel "Statutory rules"@en ;
  skos:broader agift:Legislative-drafting ;
  skos:definition "Drafting statutory rules to support the implementation of laws and parliamentary acts. Analysing government policy and existing legislation. Managing submission and approval processes, printing and gazetting."@en ;
  skos:prefLabel "Preparation of legislative regulations"@en ;
.
agift:Presentation-arrangements
  a skos:Concept ;
  dcterms:contributor "KOdea" ;
  dcterms:created "2016-07-06T04:50:02+00:00"^^xsd:dateTime ;
  dcterms:creator "superadmin" ;
  dcterms:modified "2016-09-09T05:40:34+00:00"^^xsd:dateTime ;
  skos:altLabel "Citizenship ceremonies"@en ;
  skos:altLabel "Naturalisation ceremonies"@en ;
  skos:broader agift:Citizenship ;
  skos:definition "Organising and conducting ceremonies to confer Australian citizenship. Preparing participants to take their citizenship pledge and arranging the presentation of certificates. Coordinating security, publicity and facilities. Includes affirmation ceremonies for existing Australian citizens."@en ;
  skos:prefLabel "Presentation arrangements"@en ;
  skos:related agift:Civic-celebrations ;
.
agift:Preservation-services
  skos:prefLabel "Preservation services"@en ;
  owl:deprecated true ;
.
agift:Preservation-services
  a skos:Concept ;
  dcterms:contributor "fionamcl" ;
  dcterms:created "2016-09-08T01:34:26+00:00"^^xsd:dateTime ;
  dcterms:creator "fionamcl" ;
  dcterms:modified "2016-11-28T22:47:59+00:00"^^xsd:dateTime ;
  skos:altLabel "Collection preservation"@en ;
  skos:altLabel "Conservation services"@en ;
  skos:altLabel "Restoration services"@en ;
  skos:broader agift:Collection-management ;
  skos:definition "Developing strategies to protect and conserve material in cultural collections. Applying treatments to prevent decomposition over time or through excessive handling. Includes repair of badly damaged items or transfer to stable media."@en ;
  skos:prefLabel "Preservation services"@en ;
  skos:related agift:Collection-storage ;
.
agift:Prices-surveillance
  a skos:Concept ;
  dcterms:contributor "KOdea" ;
  dcterms:created "2016-07-06T03:51:12+00:00"^^xsd:dateTime ;
  dcterms:creator "superadmin" ;
  dcterms:modified "2016-09-05T06:49:52+00:00"^^xsd:dateTime ;
  skos:altLabel "Price control"@en ;
  skos:altLabel "Price fixing"@en ;
  skos:altLabel "Price surveillance"@en ;
  skos:broader agift:Fair-trading-compliance ;
  skos:definition "Monitoring and regulating the charges for goods or services offered for sale. Evaluating proposed price increases, where an industry or organisation is under surveillance. Making recommendations on pricing practices."@en ;
  skos:prefLabel "Prices surveillance"@en ;
  skos:related agift:Energy-supply ;
  skos:related agift:Monetary-policy ;
.
agift:Primary-health-care
  a skos:Concept ;
  dcterms:contributor "KOdea" ;
  dcterms:created "2016-07-06T04:45:11+00:00"^^xsd:dateTime ;
  dcterms:creator "superadmin" ;
  dcterms:modified "2016-09-09T06:09:19+00:00"^^xsd:dateTime ;
  skos:altLabel "Community health centres"@en ;
  skos:altLabel "Community midwifery"@en ;
  skos:altLabel "Family planning"@en ;
  skos:altLabel "Immunisation programs"@en ;
  skos:altLabel "Maternal health services"@en ;
  skos:altLabel "Remote community health care"@en ;
  skos:altLabel "Vaccination programs"@en ;
  skos:broader agift:Community-health-services ;
  skos:definition "Administering programs that deliver essential health care services at the most local level. Ensuring all members of the community have access to basic methods of prevention and treatment for disease or injury. Monitoring the provision of primary health care services in remote or isolated areas."@en ;
  skos:prefLabel "Primary health care"@en ;
  skos:related agift:Adult-education-programs ;
  skos:related agift:Clinical-health-services ;
  skos:related agift:Health-promotion ;
  skos:related agift:Indigenous-health-services ;
  skos:related agift:School-education ;
.
agift:Privacy
  a skos:Concept ;
  dcterms:contributor "KOdea" ;
  dcterms:created "2016-07-06T03:38:40+00:00"^^xsd:dateTime ;
  dcterms:creator "superadmin" ;
  dcterms:modified "2016-09-09T07:26:52+00:00"^^xsd:dateTime ;
  skos:altLabel "Privacy Act"@en ;
  skos:altLabel "Privacy guideline monitoring"@en ;
  skos:altLabel "Privacy protection"@en ;
  skos:broader agift:JUSTICE-ADMINISTRATION ;
  skos:definition "Establishing privacy principles to ensure an individual's rights to the confidentiality of their personal information. Monitoring compliance with legislation and guidelines. Includes investigating breaches of privacy and evaluating new technology for potential risks to individual privacy."@en ;
  skos:prefLabel "Privacy"@en ;
  skos:related agift:Cybersafety ;
  skos:related agift:Freedom-of-information ;
  skos:related agift:Human-rights-obligations ;
  skos:related agift:Information-management-standards ;
  skos:related agift:Information-security ;
  skos:related agift:Recordkeeping-standards ;
.
agift:Probate-applications
  a skos:Concept ;
  dcterms:contributor "KOdea" ;
  dcterms:created "2016-07-06T04:56:23+00:00"^^xsd:dateTime ;
  dcterms:creator "superadmin" ;
  dcterms:modified "2016-08-29T06:20:46+00:00"^^xsd:dateTime ;
  skos:altLabel "Deceased estates"@en ;
  skos:altLabel "Will registration"@en ;
  skos:broader agift:Civil-law ;
  skos:definition "Managing the registration and validation of wills. Authorising a named executor to administer the estate of a deceased person. Includes procedures to handle contested probate requests."@en ;
  skos:prefLabel "Probate applications"@en ;
.
agift:Product-safety
  a skos:Concept ;
  dcterms:contributor "KOdea" ;
  dcterms:created "2016-07-06T03:51:19+00:00"^^xsd:dateTime ;
  dcterms:creator "superadmin" ;
  dcterms:modified "2016-08-04T06:37:38+00:00"^^xsd:dateTime ;
  skos:broader agift:Fair-trading-compliance ;
  skos:definition "Administering programs to ensure the quality of products offered for sale. Assessing statements made about the goods - such as origin, conditions of sale, warranties and guarantees. Evaluating product safety, banning goods or issuing product recalls. Imposing penalties as appropriate."@en ;
  skos:prefLabel "Product safety"@en ;
.
agift:Productivity
  a skos:Concept ;
  dcterms:contributor "KOdea" ;
  dcterms:created "2016-07-06T04:38:07+00:00"^^xsd:dateTime ;
  dcterms:creator "superadmin" ;
  dcterms:modified "2016-09-08T08:00:31+00:00"^^xsd:dateTime ;
  skos:broader agift:Resource-management ;
  skos:definition "Developing measures and programs to capture the ability of an economy to harness its physical and human resources to generate output and income."@en ;
  skos:prefLabel "Productivity"@en ;
  skos:related agift:Financial-system-management ;
  skos:related agift:Fiscal-policy ;
  skos:related agift:Monetary-policy ;
.
agift:Professional-accreditation
  a skos:Concept ;
  dcterms:contributor "KOdea" ;
  dcterms:created "2016-07-06T02:50:46+00:00"^^xsd:dateTime ;
  dcterms:creator "superadmin" ;
  dcterms:modified "2016-09-05T06:40:34+00:00"^^xsd:dateTime ;
  skos:altLabel "Accreditation criteria"@en ;
  skos:altLabel "Competency standards"@en ;
  skos:altLabel "Professional codes of practice"@en ;
  skos:altLabel "Qualified professionals"@en ;
  skos:broader agift:BUSINESS-SUPPORT-AND-REGULATION ;
  skos:definition "Administering programs to certify individuals as meeting official requirements to perform a skilled occupation. Includes processing applications, managing examinations and setting conditions on the right to apply qualifications in certain fields."@en ;
  skos:prefLabel "Professional accreditation"@en ;
  skos:related agift:Overseas-skills-recognition ;
.
agift:Prohibited-export-control
  a skos:Concept ;
  dcterms:contributor "KOdea" ;
  dcterms:created "2016-07-06T05:12:42+00:00"^^xsd:dateTime ;
  dcterms:creator "superadmin" ;
  dcterms:modified "2016-09-12T06:18:12+00:00"^^xsd:dateTime ;
  skos:broader agift:Export-regulation ;
  skos:definition "Regulating the international sale and movement out of Australia of restricted goods such as wildlife, heritage artefacts, weaponry, military equipment, nuclear material, chemicals and toxins, electronics, software and technology, currency, illicit drugs. Includes policy development, procedures for inspection and seizure, and liaison with other jurisdictions."@en ;
  skos:prefLabel "Prohibited export control"@en ;
  skos:related agift:Artefact-export-regulation ;
  skos:related agift:Quarantine ;
.
agift:Prohibited-import-control
  a skos:Concept ;
  dcterms:contributor "KOdea" ;
  dcterms:created "2016-07-06T05:13:09+00:00"^^xsd:dateTime ;
  dcterms:creator "superadmin" ;
  dcterms:modified "2016-09-13T07:03:34+00:00"^^xsd:dateTime ;
  skos:broader agift:Import-regulation ;
  skos:definition "Regulating the international purchase and movement into Australia of restricted goods such as medicines and illicit drugs, animals and animal-derived products, plants and plant-derived products, weaponry, military equipment, nuclear material, chemicals and toxins, heritage artefacts, motor vehicles, currency. Includes policy development, procedures for inspection and seizure, and liaison with other jurisdictions."@en ;
  skos:prefLabel "Prohibited import control"@en ;
  skos:related agift:Artefact-export-regulation ;
  skos:related agift:Border-protection ;
  skos:related agift:Quarantine ;
  skos:related agift:Tariff-regulation ;
.
agift:Prosecution-services
  a skos:Concept ;
  dcterms:contributor "KOdea" ;
  dcterms:created "2016-07-06T03:38:49+00:00"^^xsd:dateTime ;
  dcterms:creator "superadmin" ;
  dcterms:modified "2016-09-09T07:27:47+00:00"^^xsd:dateTime ;
  skos:altLabel "Public prosecutions"@en ;
  skos:broader agift:JUSTICE-ADMINISTRATION ;
  skos:definition "Bringing individuals or organisations to trial for criminal offences. Carrying on of legal proceedings against a party, in the interests of the public."@en ;
  skos:prefLabel "Prosecution services"@en ;
  skos:related agift:Corrective-services ;
  skos:related agift:Law-enforcement ;
  skos:related agift:Legal-aid-services ;
.
agift:Protective-services
  a skos:Concept ;
  dcterms:contributor "KOdea" ;
  dcterms:created "2016-07-06T05:08:14+00:00"^^xsd:dateTime ;
  dcterms:creator "superadmin" ;
  dcterms:modified "2016-09-12T06:58:12+00:00"^^xsd:dateTime ;
  skos:altLabel "Bodyguards"@en ;
  skos:altLabel "Diplomatic protection"@en ;
  skos:altLabel "Security guards"@en ;
  skos:broader agift:Law-enforcement ;
  skos:definition "Providing specialist security products and services to shield an individual from threat of attack. Managing physical security programs, designated persons protection, X-ray screening, bomb threat management and protective surveillance. Includes administration of security personnel through staff vetting and clearance procedures."@en ;
  skos:prefLabel "Protective services"@en ;
  skos:related agift:Intelligence ;
  skos:related agift:Intelligence-support ;
.
agift:Public-administration
  a skos:Concept ;
  dcterms:contributor "KOdea" ;
  dcterms:created "2016-07-06T03:06:47+00:00"^^xsd:dateTime ;
  dcterms:creator "superadmin" ;
  dcterms:modified "2016-09-09T05:58:43+00:00"^^xsd:dateTime ;
  skos:broader agift:GOVERNANCE ;
  skos:definition "Administering programs to implement the policies and programs of the executive and elected representatives. Review the performance of such programs. Developing policy and guidelines to improve public administration."@en ;
  skos:narrower agift:Corruption-prevention ;
  skos:narrower agift:Government-auditing ;
  skos:narrower agift:Integrity-compliance ;
  skos:narrower agift:Public-service ;
  skos:narrower agift:Territories-administration ;
  skos:narrower agift:Whistleblowing ;
  skos:prefLabel "Public administration"@en ;
  skos:related agift:Administrative-law ;
.
agift:Public-borrowing
  a skos:Concept ;
  dcterms:contributor "KOdea" ;
  dcterms:created "2016-07-06T04:36:29+00:00"^^xsd:dateTime ;
  dcterms:creator "superadmin" ;
  dcterms:modified "2016-09-08T07:58:42+00:00"^^xsd:dateTime ;
  skos:altLabel "Bonds"@en ;
  skos:altLabel "Government bonds"@en ;
  skos:altLabel "Government borrowing"@en ;
  skos:altLabel "Treasury bonds"@en ;
  skos:broader agift:Fiscal-policy ;
  skos:definition "Administering programs to raise funds to finance government expenditure, in accordance with fiscal policy. Includes the issue and sale of government bonds."@en ;
  skos:prefLabel "Public borrowing"@en ;
  skos:related agift:Public-debt ;
.
agift:Public-debt
  a skos:Concept ;
  dcterms:contributor "KOdea" ;
  dcterms:created "2016-07-06T04:36:38+00:00"^^xsd:dateTime ;
  dcterms:creator "superadmin" ;
  dcterms:modified "2016-09-08T07:59:44+00:00"^^xsd:dateTime ;
  skos:altLabel "Government debt management"@en ;
  skos:broader agift:Fiscal-policy ;
  skos:definition "Managing the repayment of public borrowings, including the redemption of government bonds. Minimising associated costs such as interest payments by coordinating payments with tax revenue flows."@en ;
  skos:prefLabel "Public debt"@en ;
  skos:related agift:Public-borrowing ;
.
agift:Public-expenditure
  a skos:Concept ;
  dcterms:contributor "KOdea" ;
  dcterms:created "2016-07-06T04:36:45+00:00"^^xsd:dateTime ;
  dcterms:creator "superadmin" ;
  dcterms:modified "2016-09-08T07:59:28+00:00"^^xsd:dateTime ;
  skos:altLabel "Government spending"@en ;
  skos:broader agift:Fiscal-policy ;
  skos:definition "Managing the disbursement of public money in accordance with fiscal policy. Monitoring revenue forecasts and projecting the costs of proposed programs or services. Determining the economic impact of government spending."@en ;
  skos:prefLabel "Public expenditure"@en ;
  skos:related agift:Financial-budgeting ;
.
agift:Public-fitness-promotion
  a skos:Concept ;
  dcterms:contributor "KOdea" ;
  dcterms:created "2016-07-06T05:09:06+00:00"^^xsd:dateTime ;
  dcterms:creator "superadmin" ;
  dcterms:modified "2016-09-13T06:29:53+00:00"^^xsd:dateTime ;
  skos:altLabel "Fitness promotion"@en ;
  skos:altLabel "National fitness campaigns"@en ;
  skos:broader agift:Community-recreational-programs ;
  skos:definition "Administering schemes to encourage physical activity across the community. Developing programs to raise awareness of the health benefits of fitness. Providing activities for target groups and supporting clubs and community groups that promote physical fitness."@en ;
  skos:prefLabel "Public fitness promotion"@en ;
  skos:related agift:Health-promotion ;
  skos:related agift:Sport-and-fitness-development ;
.
agift:Public-health-services
  a skos:Concept ;
  dcterms:contributor "KOdea" ;
  dcterms:created "2016-07-06T03:07:41+00:00"^^xsd:dateTime ;
  dcterms:creator "superadmin" ;
  dcterms:modified "2016-09-09T06:18:39+00:00"^^xsd:dateTime ;
  skos:altLabel "Public health"@en ;
  skos:broader agift:HEALTH-CARE ;
  skos:definition "Developing policy to protect the physical and mental wellbeing of all people at a broad level. Establishing programs to understand and control the determinants of disease, and reduce public exposure to risks encountered as part of lifestyle or the environment."@en ;
  skos:narrower agift:Blood-and-organ-donation-management ;
  skos:narrower agift:Epidemiology ;
  skos:narrower agift:Health-disaster-preparedness ;
  skos:narrower agift:Health-hazard-prevention ;
  skos:narrower agift:Medical-quarantine-services ;
  skos:narrower agift:Medical-radiation-services ;
  skos:narrower agift:Notifiable-disease-management ;
  skos:narrower agift:Radiation-protection ;
  skos:prefLabel "Public health services"@en ;
  skos:related agift:Community-health-services ;
.
agift:Public-housing
  a skos:Concept ;
  dcterms:contributor "KOdea" ;
  dcterms:created "2016-07-06T02:52:17+00:00"^^xsd:dateTime ;
  dcterms:creator "superadmin" ;
  dcterms:modified "2016-09-09T06:35:18+00:00"^^xsd:dateTime ;
  skos:altLabel "Commission housing"@en ;
  skos:altLabel "Government housing"@en ;
  skos:altLabel "Housing"@en ;
  skos:altLabel "Indigenous housing"@en ;
  skos:altLabel "Social housing"@en ;
  skos:broader agift:CIVIC-INFRASTRUCTURE ;
  skos:definition "Administering programs to supply low cost government-owned accommodation. Providing guidelines to direct the design of public housing. Evaluating the need for public housing and setting construction targets. Allocating appropriate funds to enable ongoing maintenance."@en ;
  skos:narrower agift:Community-housing ;
  skos:narrower agift:Public-housing-construction ;
  skos:narrower agift:Public-housing-design ;
  skos:narrower agift:Public-housing-maintenance ;
  skos:prefLabel "Public housing"@en ;
  skos:related agift:Accommodation-services ;
  skos:related agift:Crown-land-administration ;
  skos:related agift:Income-support-schemes ;
  skos:related agift:Migrant-accommodation-services ;
  skos:related agift:Public-housing-entitlements ;
.
agift:Public-housing-construction
  a skos:Concept ;
  dcterms:contributor "KOdea" ;
  dcterms:created "2016-07-06T03:54:24+00:00"^^xsd:dateTime ;
  dcterms:creator "superadmin" ;
  dcterms:modified "2016-09-05T07:02:44+00:00"^^xsd:dateTime ;
  skos:broader agift:Public-housing ;
  skos:definition "Building low cost government-owned accommodation.  Managing tenders and overseeing construction projects. Negotiating value for money on materials and services to support affordability.  Ensuring that public  housing construction meets government targets."@en ;
  skos:prefLabel "Public housing construction"@en ;
  skos:related agift:Architectural-services ;
.
agift:Public-housing-design
  a skos:Concept ;
  dcterms:contributor "KOdea" ;
  dcterms:created "2016-07-06T03:54:32+00:00"^^xsd:dateTime ;
  dcterms:creator "superadmin" ;
  dcterms:modified "2016-08-05T04:07:03+00:00"^^xsd:dateTime ;
  skos:broader agift:Public-housing ;
  skos:definition "Planning and drafting low cost government-owned accommodation. Implementing best practice design strategies to incorporate facilities for tenants with special needs. Ensuring that public housing design meets government guidelines."@en ;
  skos:prefLabel "Public housing design"@en ;
.
agift:Public-housing-entitlements
  a skos:Concept ;
  dcterms:contributor "KOdea" ;
  dcterms:created "2016-07-06T04:01:47+00:00"^^xsd:dateTime ;
  dcterms:creator "superadmin" ;
  dcterms:modified "2016-09-06T07:11:15+00:00"^^xsd:dateTime ;
  skos:broader agift:Accommodation-services ;
  skos:definition "Assessing eligibility for community accommodation, against established criteria. Allocating public housing to approved applicants. Providing advice to tenants about their rights and obligations, and options to purchase public housing. Includes entitlement review and complaint processes."@en ;
  skos:prefLabel "Public housing entitlements"@en ;
  skos:related agift:Financial-assistance ;
  skos:related agift:Public-housing ;
.
agift:Public-housing-maintenance
  a skos:Concept ;
  dcterms:contributor "KOdea" ;
  dcterms:created "2016-07-06T03:54:39+00:00"^^xsd:dateTime ;
  dcterms:creator "superadmin" ;
  dcterms:modified "2016-08-05T04:08:53+00:00"^^xsd:dateTime ;
  skos:altLabel "Maintenance"@en ;
  skos:broader agift:Public-housing ;
  skos:definition "Preserving and repairing low cost government-owned accommodation. Implementing programs of regular maintenance. Reporting on the condition of public housing and recommending upgrades or major renovation when necessary."@en ;
  skos:prefLabel "Public housing maintenance"@en ;
.
agift:Public-land-management
  a skos:Concept ;
  dcterms:contributor "KOdea" ;
  dcterms:created "2016-07-06T02:52:24+00:00"^^xsd:dateTime ;
  dcterms:creator "superadmin" ;
  dcterms:modified "2016-09-12T05:56:30+00:00"^^xsd:dateTime ;
  skos:altLabel "Property"@en ;
  skos:altLabel "Street light maintenance"@en ;
  skos:altLabel "Street tree management"@en ;
  skos:altLabel "Urban land management"@en ;
  skos:altLabel "Urban tree management"@en ;
  skos:broader agift:CIVIC-INFRASTRUCTURE ;
  skos:definition "Controlling and maintaining buildings or areas of land set aside for community use. Providing guidelines to direct the use of public land. Allocating appropriate funds to enable ongoing maintenance. Evaluating the need for public land and providing advice for planning purposes."@en ;
  skos:narrower agift:Burial-ground-management ;
  skos:narrower agift:Cultural-centre-management ;
  skos:narrower agift:Garden-management ;
  skos:narrower agift:Memorial-maintenance ;
  skos:narrower agift:Recreational-park-management ;
  skos:narrower agift:Sporting-facilities-management ;
  skos:prefLabel "Public land management"@en ;
  skos:related agift:Crown-land-administration ;
.
agift:Public-service
  a skos:Concept ;
  dcterms:contributor "KOdea" ;
  dcterms:created "2016-07-06T04:43:54+00:00"^^xsd:dateTime ;
  dcterms:creator "superadmin" ;
  dcterms:modified "2016-09-09T06:01:04+00:00"^^xsd:dateTime ;
  skos:broader agift:Public-administration ;
  skos:definition "Implementing the policies of the executive and elected representatives. Providing services to the community in accordance with agreed performance standards."@en ;
  skos:prefLabel "Public service"@en ;
  skos:related agift:EMPLOYMENT ;
.
agift:Public-transport
  a skos:Concept ;
  dcterms:contributor "KOdea" ;
  dcterms:created "2016-07-06T03:49:55+00:00"^^xsd:dateTime ;
  dcterms:creator "superadmin" ;
  dcterms:modified "2016-09-13T07:13:51+00:00"^^xsd:dateTime ;
  skos:broader agift:TRANSPORT ;
  skos:definition "Developing and maintaining a system of vehicles such as buses and trains that operates at regular times on fixed routes and are used by the public."@en ;
  skos:narrower agift:Transport-accessibility ;
  skos:prefLabel "Public transport"@en ;
  skos:related agift:Passenger-services ;
  skos:related agift:Transport-access-schemes ;
  skos:related agift:Transport-network-maintenance ;
.
agift:Publicity-programs
  skos:prefLabel "Publicity programs"@en ;
  owl:deprecated true ;
.
agift:Publicity-programs
  a skos:Concept ;
  dcterms:contributor "fionamcl" ;
  dcterms:created "2016-09-08T01:41:31+00:00"^^xsd:dateTime ;
  dcterms:creator "fionamcl" ;
  dcterms:modified "2016-11-28T22:48:25+00:00"^^xsd:dateTime ;
  skos:altLabel "Marketing campaigns"@en ;
  skos:broader agift:Collection-promotion ;
  skos:definition "Planning and implementing campaigns to promote cultural institutions and their collections. Developing media releases, advertising material and catalogues for exhibitions. Organising tours, visits and speaking engagements."@en ;
  skos:prefLabel "Publicity programs"@en ;
  skos:related agift:Exhibition-programs ;
  skos:related agift:Government-media ;
  skos:related agift:Publishing ;
.
agift:Publishing
  a skos:Concept ;
  dcterms:contributor "KOdea" ;
  dcterms:created "2016-07-06T02:54:34+00:00"^^xsd:dateTime ;
  dcterms:creator "superadmin" ;
  dcterms:modified "2016-09-13T06:54:14+00:00"^^xsd:dateTime ;
  skos:altLabel "Publications"@en ;
  skos:broader agift:COMMUNICATIONS ;
  skos:definition "Developing policy to support the compilation and distribution of government information via print or electronic media. Managing applications to use material under government copyright. Includes editing and publishing material in printed formats."@en ;
  skos:narrower agift:Electronic-publishing ;
  skos:narrower agift:Publishing-standards ;
  skos:narrower agift:Website-development ;
  skos:prefLabel "Publishing"@en ;
  skos:related agift:Advertising-campaigns ;
  skos:related agift:Collection-promotion ;
  skos:related agift:Copyright-regulation ;
  skos:related agift:Government-media ;
  skos:related agift:Information-dissemination ;
  skos:related agift:Publicity-programs ;
.
agift:Publishing-standards
  a skos:Concept ;
  dcterms:contributor "KOdea" ;
  dcterms:created "2016-07-06T03:59:28+00:00"^^xsd:dateTime ;
  dcterms:creator "superadmin" ;
  dcterms:modified "2016-09-05T07:46:02+00:00"^^xsd:dateTime ;
  skos:broader agift:Publishing ;
  skos:prefLabel "Publishing standards"@en ;
  skos:related agift:Censorship-standards ;
.
agift:Quarantine
  a skos:Concept ;
  dcterms:contributor "KOdea" ;
  dcterms:created "2016-07-06T03:42:08+00:00"^^xsd:dateTime ;
  dcterms:creator "superadmin" ;
  dcterms:modified "2016-09-13T07:07:55+00:00"^^xsd:dateTime ;
  skos:altLabel "Animal quarantine"@en ;
  skos:altLabel "Isolation facilities"@en ;
  skos:broader agift:PRIMARY-INDUSTRIES ;
  skos:definition "Developing strategies to protect the health of Australia's plant and animal populations from risks associated with exotic pests and disease. Conducting inspections at borders, ports, airports and other entry or exit points. Managing isolation and disinfection facilities. Applying penalties for breaches of regulations."@en ;
  skos:prefLabel "Quarantine"@en ;
  skos:related agift:Interstate-trade-agreements ;
  skos:related agift:Medical-quarantine-services ;
  skos:related agift:Prohibited-export-control ;
  skos:related agift:Prohibited-import-control ;
.
agift:Radiation-protection
  a skos:Concept ;
  dcterms:contributor "KOdea" ;
  dcterms:created "2016-07-06T04:48:34+00:00"^^xsd:dateTime ;
  dcterms:creator "superadmin" ;
  dcterms:modified "2016-09-09T06:23:38+00:00"^^xsd:dateTime ;
  skos:broader agift:Public-health-services ;
  skos:definition "Regulating the safe use of radioactive substances. Developing legislation and standards for keeping and using radioactive substances. Includes the sale, transfer, storage, possession, transport, installation, maintenance and remediation of regulated material."@en ;
  skos:prefLabel "Radiation protection"@en ;
  skos:related agift:Medical-radiation-services ;
  skos:related agift:Nuclear-safeguards ;
.
agift:Radio-broadcasting
  a skos:Concept ;
  dcterms:contributor "KOdea" ;
  dcterms:created "2016-07-06T03:56:36+00:00"^^xsd:dateTime ;
  dcterms:creator "superadmin" ;
  dcterms:modified "2016-09-05T07:26:03+00:00"^^xsd:dateTime ;
  skos:altLabel "Broadcasting licenses"@en ;
  skos:altLabel "Commercial radio"@en ;
  skos:altLabel "Wireless broadcasting"@en ;
  skos:broader agift:Broadcasting ;
  skos:definition "Supporting industries that transmit content as electromagnetic waves sent through the air to a receiver. Managing publicly owned radio stations and issuing commercial broadcasting licenses. Developing strategies to promote Australian radio programming. Providing radio broadcasting services locally, nationally and internationally. Negotiating retransmission arrangements."@en ;
  skos:prefLabel "Radio broadcasting"@en ;
  skos:related agift:Broadcasting-standards ;
  skos:related agift:Radio-communication ;
.
agift:Radio-communication
  a skos:Concept ;
  dcterms:contributor "KOdea" ;
  dcterms:created "2016-07-06T02:54:41+00:00"^^xsd:dateTime ;
  dcterms:creator "superadmin" ;
  dcterms:modified "2016-09-05T07:48:17+00:00"^^xsd:dateTime ;
  skos:altLabel "Radio communications"@en ;
  skos:broader agift:COMMUNICATIONS ;
  skos:definition "Developing policy to support and regulate the operation of wireless communications infrastructure. Maintaining a regulatory framework for the radio communications industry. Supporting market entry, enabling firms to acquire spectrum to introduce new technologies. Includes liaison across jurisdictions on radio communications issues."@en ;
  skos:narrower agift:Apparatus-licensing ;
  skos:narrower agift:Spectrum-management ;
  skos:prefLabel "Radio communication"@en ;
  skos:related agift:Mobile-telephone-services ;
  skos:related agift:Radio-broadcasting ;
.
agift:Rail-harmonisation-standards
  a skos:Concept ;
  dcterms:contributor "KOdea" ;
  dcterms:created "2016-07-06T05:15:14+00:00"^^xsd:dateTime ;
  dcterms:creator "superadmin" ;
  dcterms:modified "2016-09-02T06:00:45+00:00"^^xsd:dateTime ;
  skos:altLabel "Locomotive standards"@en ;
  skos:altLabel "Railway gauge standards"@en ;
  skos:broader agift:Rail-transport ;
  skos:definition "Developing a consistent approach to technical and operational railway practices across jurisdictions. Includes standards relating to locomotives, track gauge, signalling, control systems and emissions."@en ;
  skos:prefLabel "Rail harmonisation standards"@en ;
.
agift:Rail-land-acquisition-regulation
  a skos:Concept ;
  dcterms:contributor "KOdea" ;
  dcterms:created "2016-07-06T05:15:22+00:00"^^xsd:dateTime ;
  dcterms:creator "superadmin" ;
  dcterms:modified "2016-09-02T06:01:13+00:00"^^xsd:dateTime ;
  skos:broader agift:Rail-transport ;
  skos:definition "Developing policy and procedures for the purchase or possession of property to accommodate railway infrastructure. Regulating proposals and payments for compensation in relation to acquired land."@en ;
  skos:prefLabel "Rail land acquisition regulation"@en ;
.
agift:Rail-transport
  a skos:Concept ;
  dcterms:contributor "KOdea" ;
  dcterms:created "2016-07-06T03:50:03+00:00"^^xsd:dateTime ;
  dcterms:creator "superadmin" ;
  dcterms:modified "2016-09-13T07:14:40+00:00"^^xsd:dateTime ;
  skos:altLabel "Railways"@en ;
  skos:altLabel "Train travel"@en ;
  skos:broader agift:TRANSPORT ;
  skos:definition "Regulating the railway industry and developing policy relating to all aspects of the rail network system. Administering rail transport standards, security and services and licensing of rail transport operators. Includes liaison to promote coordination and consistency among rail authorities from different jurisdictions."@en ;
  skos:narrower agift:Rail-harmonisation-standards ;
  skos:narrower agift:Rail-land-acquisition-regulation ;
  skos:narrower agift:Rail-transport-safety ;
  skos:narrower agift:Railway-maintenance ;
  skos:narrower agift:Rolling-stock-regulation ;
  skos:prefLabel "Rail transport"@en ;
  skos:related agift:Freight-movement-regulation ;
  skos:related agift:Passenger-services ;
.
agift:Rail-transport-safety
  a skos:Concept ;
  dcterms:contributor "KOdea" ;
  dcterms:created "2016-07-06T05:15:29+00:00"^^xsd:dateTime ;
  dcterms:creator "superadmin" ;
  dcterms:modified "2016-09-13T07:15:50+00:00"^^xsd:dateTime ;
  skos:altLabel "Accident investigation"@en ;
  skos:altLabel "Safety investigation"@en ;
  skos:broader agift:Rail-transport ;
  skos:definition "Regulating all railway activities to improve security, reducing the risk of accidents or emergencies and investigating accidents and incidents. Monitoring compliance with rail safety standards, signalling procedures and other regulations. Includes training and advice, consultation and inspection services and cooperation on railway safety issues across jurisdictions."@en ;
  skos:prefLabel "Rail transport safety"@en ;
  skos:related agift:Railway-maintenance ;
  skos:related agift:Rolling-stock-regulation ;
.
agift:Railway-maintenance
  a skos:Concept ;
  dcterms:contributor "KOdea" ;
  dcterms:created "2016-07-06T05:15:36+00:00"^^xsd:dateTime ;
  dcterms:creator "superadmin" ;
  dcterms:modified "2016-09-13T07:23:54+00:00"^^xsd:dateTime ;
  skos:altLabel "Railway crossings"@en ;
  skos:altLabel "Railway lines"@en ;
  skos:altLabel "Railway stations"@en ;
  skos:altLabel "Railway tracks"@en ;
  skos:altLabel "Train tracks"@en ;
  skos:altLabel "Tram lines"@en ;
  skos:broader agift:Rail-transport ;
  skos:definition "Managing and preserving railway tracks and associated infrastructure. Ensuring that railway stations, crossings, signals, bridges and tunnels meet operating standards. Includes inspections, assessments and ongoing repair work."@en ;
  skos:prefLabel "Railway maintenance"@en ;
  skos:related agift:Rail-transport-safety ;
  skos:related agift:Transport-infrastructure-development ;
  skos:related agift:Transport-network-maintenance ;
.
agift:Recordkeeping-standards
  a skos:Concept ;
  dcterms:contributor "KOdea" ;
  dcterms:created "2016-07-06T04:55:01+00:00"^^xsd:dateTime ;
  dcterms:creator "superadmin" ;
  dcterms:modified "2016-09-12T06:50:43+00:00"^^xsd:dateTime ;
  skos:altLabel "Archives"@en ;
  skos:altLabel "Records management"@en ;
  skos:broader agift:Administrative-law ;
  skos:definition "Regulating the creation, capture, management and disposal of government records. Monitoring compliance to ensure appropriate availability of authentic evidence of government or business activities."@en ;
  skos:prefLabel "Recordkeeping standards"@en ;
  skos:related agift:Business-process-auditing ;
  skos:related agift:Freedom-of-information ;
  skos:related agift:Information-management-standards ;
  skos:related agift:Information-security ;
  skos:related agift:Open-government ;
  skos:related agift:Privacy ;
.
agift:Recreational-park-management
  a skos:Concept ;
  dcterms:contributor "KOdea" ;
  dcterms:created "2016-07-06T03:55:29+00:00"^^xsd:dateTime ;
  dcterms:creator "superadmin" ;
  dcterms:modified "2016-09-05T07:13:39+00:00"^^xsd:dateTime ;
  skos:altLabel "Park management"@en ;
  skos:altLabel "Playground management"@en ;
  skos:altLabel "Public leisure areas"@en ;
  skos:broader agift:Public-land-management ;
  skos:definition "Administering public leisure areas and playgrounds. Managing site layout and landscaping. Ensuring facilities are kept clean and maintained. Monitoring rights of access and opening hours."@en ;
  skos:prefLabel "Recreational park management"@en ;
  skos:related agift:Garden-management ;
  skos:related agift:National-park-management ;
  skos:related agift:Nature-reserve-management ;
  skos:related agift:Park-and-reserve-services ;
  skos:related agift:Sporting-facilities-management ;
.
agift:Recruitment-programs
  a skos:Concept ;
  dcterms:contributor "KOdea" ;
  dcterms:created "2016-07-06T04:21:05+00:00"^^xsd:dateTime ;
  dcterms:creator "superadmin" ;
  dcterms:modified "2016-09-08T07:22:49+00:00"^^xsd:dateTime ;
  skos:broader agift:Human-resources-development ;
  skos:definition "Managing activities to engage staff and promote employment with the organisation. Developing selection documentation, conducting interviews and appointing new employees. Establishing procedures for advertising public sector vacancies or managing recruitment exercises in accordance with government policies."@en ;
  skos:prefLabel "Recruitment programs"@en ;
  skos:related agift:Defence-force-careers ;
  skos:related agift:Government-media ;
  skos:related agift:Vocational-education ;
.
agift:Reference-services
  skos:prefLabel "Reference services"@en ;
  owl:deprecated true ;
.
agift:Reference-services
  a skos:Concept ;
  dcterms:contributor "fionamcl" ;
  dcterms:created "2016-09-08T01:29:24+00:00"^^xsd:dateTime ;
  dcterms:creator "fionamcl" ;
  dcterms:modified "2016-11-28T22:47:00+00:00"^^xsd:dateTime ;
  skos:altLabel "Access services"@en ;
  skos:altLabel "Client services"@en ;
  skos:altLabel "Information services"@en ;
  skos:altLabel "Reader services"@en ;
  skos:broader agift:Collection-access ;
  skos:definition "Providing personal or online assistance to help clients locate and use items held in cultural collections. Explaining access provisions and restrictions, and the procedures to view material. Includes research and referral services, mobile or special services for target community groups."@en ;
  skos:prefLabel "Reference services"@en ;
  skos:related agift:Collection-access ;
  skos:related agift:Finding-aids-development ;
.
agift:Refuge-support
  a skos:Concept ;
  dcterms:contributor "KOdea" ;
  dcterms:created "2016-07-06T04:01:53+00:00"^^xsd:dateTime ;
  dcterms:creator "superadmin" ;
  dcterms:modified "2016-09-06T07:12:18+00:00"^^xsd:dateTime ;
  skos:broader agift:Accommodation-services ;
  skos:definition "Managing sheltered accommodation to provide assistance to members of the community at risk. Includes funding and services to support private facilities or refuges operated by non-government organisations"@en ;
  skos:prefLabel "Refuge support"@en ;
  skos:related agift:Residential-services ;
.
agift:Refugee-services
  a skos:Concept ;
  dcterms:contributor "KOdea" ;
  dcterms:created "2016-07-06T03:34:11+00:00"^^xsd:dateTime ;
  dcterms:creator "superadmin" ;
  dcterms:modified "2016-09-09T07:23:04+00:00"^^xsd:dateTime ;
  skos:altLabel "Asylum seekers"@en ;
  skos:altLabel "Exiles"@en ;
  skos:broader agift:IMMIGRATION ;
  skos:definition "Providing assistance to asylum seekers and victims of human rights violations. Assessing applications for refugee status. Arranging health checks, counselling, community support and special services as required. Includes liaison with community groups and across jurisdictions to ensure appropriate support."@en ;
  skos:prefLabel "Refugee services"@en ;
  skos:related agift:Deportation ;
  skos:related agift:Detention-programs ;
  skos:related agift:Human-rights-obligations ;
  skos:related agift:Migrant-services ;
  skos:related agift:Migrant-settlement-programs ;
.
agift:Regional-development
  a skos:Concept ;
  dcterms:contributor "KOdea" ;
  dcterms:created "2016-07-06T02:52:34+00:00"^^xsd:dateTime ;
  dcterms:creator "superadmin" ;
  dcterms:modified "2016-09-06T07:52:47+00:00"^^xsd:dateTime ;
  skos:altLabel "Territories"@en ;
  skos:broader agift:CIVIC-INFRASTRUCTURE ;
  skos:definition "Managing infrastructure projects to support multiple districts, such as building schools or hospitals. Extending facilities beyond urban boundaries to supply services to remote or rural areas. Installing equipment to enable communications."@en ;
  skos:prefLabel "Regional development"@en ;
  skos:related agift:Infrastructure-planning ;
  skos:related agift:Integrated-services-planning ;
  skos:related agift:Rural-community-development ;
  skos:related agift:Transport-infrastructure-development ;
.
agift:Remuneration-review
  a skos:Concept ;
  dcterms:contributor "KOdea" ;
  dcterms:created "2016-07-06T04:21:55+00:00"^^xsd:dateTime ;
  dcterms:creator "superadmin" ;
  dcterms:modified "2016-08-19T06:58:00+00:00"^^xsd:dateTime ;
  skos:altLabel "Statutory appointees"@en ;
  skos:broader agift:Industrial-awards-and-conditions ;
  skos:definition "Monitoring the salary levels and employment conditions of specified public sector and statutory appointees. Evaluating remuneration against market rates for equivalent positions. Making recommendations for the review of salary, allowances, leave or entitlements."@en ;
  skos:prefLabel "Remuneration review"@en ;
.
agift:Renewable-energy-development
  a skos:Concept ;
  dcterms:contributor "fionamcl" ;
  dcterms:created "2016-07-06T05:00:03+00:00"^^xsd:dateTime ;
  dcterms:creator "superadmin" ;
  dcterms:modified "2016-09-20T00:07:49+00:00"^^xsd:dateTime ;
  skos:altLabel "Alternative energy"@en ;
  skos:altLabel "Clean energy"@en ;
  skos:altLabel "Geothermal energy"@en ;
  skos:altLabel "Hydroelectric power"@en ;
  skos:altLabel "Hydroelectricity"@en ;
  skos:altLabel "Solar energy"@en ;
  skos:altLabel "Tidal energy"@en ;
  skos:altLabel "Wind farms"@en ;
  skos:broader agift:Energy-resources ;
  skos:definition "Promoting the development and use of renewable energy resources. Licensing infrastructure and operational activities. Supporting industry partnerships and collaboration between research institutions. Providing assistance to commercialise research and development in renewable energy technologies."@en ;
  skos:prefLabel "Renewable energy development"@en ;
  skos:related agift:SCIENCE ;
  skos:related agift:Water-usage-management ;
.
agift:Rescue-coordination
  a skos:Concept ;
  dcterms:contributor "KOdea" ;
  dcterms:created "2016-07-06T04:58:32+00:00"^^xsd:dateTime ;
  dcterms:creator "superadmin" ;
  dcterms:modified "2016-09-09T07:38:43+00:00"^^xsd:dateTime ;
  skos:broader agift:Search-and-rescue ;
  skos:definition "Directing and controlling operations to locate individuals, vessels or aircraft lost at sea and return them to safety. Providing specially equipped vehicles and trained personnel. Includes liaison with community-based services, or across jurisdictions."@en ;
  skos:prefLabel "Rescue coordination"@en ;
  skos:related agift:Emergency-services ;
  skos:related agift:Firefighting-services ;
.
agift:Reserves
  a skos:Concept ;
  dcterms:contributor "KOdea" ;
  dcterms:created "2016-07-06T04:08:57+00:00"^^xsd:dateTime ;
  dcterms:creator "superadmin" ;
  dcterms:modified "2016-09-08T07:09:12+00:00"^^xsd:dateTime ;
  skos:broader agift:Australian-Defence-Forces ;
  skos:definition "Managing Australia's part-time defence units. Developing policy and programs for recruitment, training and deployment of Army, Navy or Air Force Reserves. Coordinating activities to provide support to permanent forces during peacetime and conflict."@en ;
  skos:prefLabel "Reserves"@en ;
  skos:related agift:Air-Force ;
  skos:related agift:Army ;
  skos:related agift:Army-reserve-training ;
  skos:related agift:Military-education-and-training ;
  skos:related agift:Navy ;
.
agift:Residential-services
  a skos:Concept ;
  dcterms:contributor "KOdea" ;
  dcterms:created "2016-07-06T04:49:25+00:00"^^xsd:dateTime ;
  dcterms:creator "superadmin" ;
  dcterms:modified "2016-09-09T06:28:25+00:00"^^xsd:dateTime ;
  skos:altLabel "Aged care facilities"@en ;
  skos:altLabel "Asylums"@en ;
  skos:altLabel "Disability care facilities"@en ;
  skos:altLabel "Homes"@en ;
  skos:altLabel "Hospices"@en ;
  skos:altLabel "Hostels"@en ;
  skos:altLabel "Nursing homes"@en ;
  skos:altLabel "Old people's homes"@en ;
  skos:altLabel "Retirement villages"@en ;
  skos:broader agift:Special-needs-services ;
  skos:definition "Administering programs that provide care and accommodation for aged or disabled persons, or those suffering from disease or mental illness. Providing trained personnel to attend residents. Managing staff and facilities. Monitoring the activities of private residential care providers."@en ;
  skos:prefLabel "Residential services"@en ;
  skos:related agift:Accommodation-services ;
  skos:related agift:Aged-care-services ;
  skos:related agift:Counselling-services ;
  skos:related agift:Independent-living-services ;
  skos:related agift:Mental-health-services ;
  skos:related agift:Patient-care ;
  skos:related agift:Refuge-support ;
.
agift:Resource-management
  a skos:Concept ;
  dcterms:contributor "KOdea" ;
  dcterms:created "2016-07-06T03:04:53+00:00"^^xsd:dateTime ;
  dcterms:creator "superadmin" ;
  dcterms:modified "2016-09-05T06:28:05+00:00"^^xsd:dateTime ;
  skos:broader agift:FINANCE-MANAGEMENT ;
  skos:definition "Developing policy for the management of financial and other government assets. Providing advice on legislative responsibilities and reporting requirements. Supporting accountable use and management of government resources."@en ;
  skos:narrower agift:Contract-management ;
  skos:narrower agift:Financial-administration ;
  skos:narrower agift:Financial-budgeting ;
  skos:narrower agift:Productivity ;
  skos:prefLabel "Resource management"@en ;
  skos:related agift:Government-procurement-regulation ;
.
agift:Retail-postal-services
  a skos:Concept ;
  dcterms:contributor "KOdea" ;
  dcterms:created "2016-07-06T03:58:59+00:00"^^xsd:dateTime ;
  dcterms:creator "superadmin" ;
  dcterms:modified "2016-08-05T05:45:55+00:00"^^xsd:dateTime ;
  skos:altLabel "General post offices"@en ;
  skos:altLabel "Post offices"@en ;
  skos:broader agift:Postal-services ;
  skos:definition "Administering general services to collect and deliver letters, parcels and other mail. Coordinating routes and schedules for postal delivery. Managing post offices and other retail outlets providing mail products and services."@en ;
  skos:prefLabel "Retail postal services"@en ;
.
agift:Retirement-income
  a skos:Concept ;
  dcterms:contributor "KOdea" ;
  dcterms:created "2016-07-06T03:05:00+00:00"^^xsd:dateTime ;
  dcterms:creator "superadmin" ;
  dcterms:modified "2016-09-05T06:36:36+00:00"^^xsd:dateTime ;
  skos:altLabel "Part-pension retirees"@en ;
  skos:altLabel "Retirees"@en ;
  skos:altLabel "Self-funded retirees"@en ;
  skos:broader agift:FINANCE-MANAGEMENT ;
  skos:definition "Formulating policy to safeguard the savings of individuals who have left the workforce. Setting criteria to evaluate a retiree's assets, for tax or benefit purposes. Developing standards for the operation of superannuation funds. Implementing mechanisms to support retirement saving by individuals."@en ;
  skos:narrower agift:Asset-assessment ;
  skos:narrower agift:Retirement-saving ;
  skos:narrower agift:Superannuation-regulation ;
  skos:prefLabel "Retirement income"@en ;
  skos:related agift:Financial-institutions-regulation ;
  skos:related agift:Insurance-regulation ;
.
agift:Retirement-saving
  a skos:Concept ;
  dcterms:contributor "KOdea" ;
  dcterms:created "2016-07-06T04:38:38+00:00"^^xsd:dateTime ;
  dcterms:creator "superadmin" ;
  dcterms:modified "2016-09-08T08:04:39+00:00"^^xsd:dateTime ;
  skos:altLabel "Savings bonus"@en ;
  skos:altLabel "Superannuation guarantee"@en ;
  skos:broader agift:Retirement-income ;
  skos:definition "Encouraging individuals to set aside funds to support themselves after they leave the work force. Administering programs to support and regulate retirement saving. Developing incentives for the ongoing management of retirement savings. Includes advice to employers, employees and self-employed individuals."@en ;
  skos:prefLabel "Retirement saving"@en ;
  skos:related agift:Superannuation-regulation ;
.
agift:Revenue-raising
  a skos:Concept ;
  dcterms:contributor "KOdea" ;
  dcterms:created "2016-07-06T04:39:15+00:00"^^xsd:dateTime ;
  dcterms:creator "superadmin" ;
  dcterms:modified "2016-09-08T08:08:39+00:00"^^xsd:dateTime ;
  skos:altLabel "BAS"@en ;
  skos:altLabel "Business Activity Statements"@en ;
  skos:altLabel "Departure tax"@en ;
  skos:altLabel "Excise"@en ;
  skos:altLabel "Fines"@en ;
  skos:altLabel "PAYG instalments"@en ;
  skos:altLabel "Pay As You Go taxation"@en ;
  skos:altLabel "Payments to government"@en ;
  skos:altLabel "Stamp Duty"@en ;
  skos:altLabel "Tolls"@en ;
  skos:altLabel "Withholding schemes"@en ;
  skos:broader agift:Taxation ;
  skos:definition "Developing mechanisms to support the collection of taxes from individuals and organisations. Includes deductions at point of sale, services for making payments or having sums withheld from earnings."@en ;
  skos:prefLabel "Revenue raising"@en ;
  skos:related agift:Local-laws-and-ordinances ;
  skos:related agift:Taxation-compliance ;
.
agift:Road-safety-awareness
  a skos:Concept ;
  dcterms:contributor "KOdea" ;
  dcterms:created "2016-07-06T04:13:35+00:00"^^xsd:dateTime ;
  dcterms:creator "superadmin" ;
  dcterms:modified "2016-09-13T07:20:03+00:00"^^xsd:dateTime ;
  skos:altLabel "Driver training"@en ;
  skos:altLabel "Traffic training school"@en ;
  skos:broader agift:Community-education ;
  skos:definition "Administering training designed to educate the community about the importance of road safety. Includes traffic training centres, driving instruction, school visits and campaigns to illustrate the consequences of dangerous behavior."@en ;
  skos:prefLabel "Road safety awareness"@en ;
  skos:related agift:Driving-licences-administration ;
  skos:related agift:Law-enforcement ;
  skos:related agift:Road-transport-safety ;
  skos:related agift:School-transport-regulation ;
.
agift:Road-surface-maintenance
  a skos:Concept ;
  dcterms:contributor "KOdea" ;
  dcterms:created "2016-07-06T05:16:11+00:00"^^xsd:dateTime ;
  dcterms:creator "superadmin" ;
  dcterms:modified "2016-09-13T07:24:15+00:00"^^xsd:dateTime ;
  skos:altLabel "Roads"@en ;
  skos:broader agift:Road-transport ;
  skos:definition "Managing and preserving road surfaces and associated infrastructure. Ensuring traffic lights, road markings and signage meet legislative requirements. Includes inspections, assessments and ongoing repair work."@en ;
  skos:prefLabel "Road surface maintenance"@en ;
  skos:related agift:Road-traffic-regulation ;
  skos:related agift:Transport-infrastructure-development ;
  skos:related agift:Transport-network-maintenance ;
.
agift:Road-traffic-regulation
  a skos:Concept ;
  dcterms:contributor "KOdea" ;
  dcterms:created "2016-07-06T05:16:17+00:00"^^xsd:dateTime ;
  dcterms:creator "superadmin" ;
  dcterms:modified "2016-09-13T07:19:30+00:00"^^xsd:dateTime ;
  skos:broader agift:Road-transport ;
  skos:definition "Developing and implementing regulations for all road users - such as motor vehicle drivers, cyclists and pedestrians. Determining appropriate speed limits, signage and road markings, identifying the need for traffic lights, facilities for parking, pedestrians and cyclists. Includes developing and maintaining the traffic code for interaction and behaviour of all road users."@en ;
  skos:prefLabel "Road traffic regulation"@en ;
  skos:related agift:Driving-licences-administration ;
  skos:related agift:Road-surface-maintenance ;
  skos:related agift:Road-transport-safety ;
  skos:related agift:Vehicle-registration ;
  skos:related agift:Vehicle-standards ;
.
agift:Road-transport
  a skos:Concept ;
  dcterms:contributor "superadmin" ;
  dcterms:created "2016-07-06T03:50:23+00:00"^^xsd:dateTime ;
  dcterms:creator "superadmin" ;
  dcterms:modified "2016-07-07T00:45:21+00:00"^^xsd:dateTime ;
  skos:broader agift:TRANSPORT ;
  skos:definition "Developing policy relating to all aspects of private or commercial road usage. Administering road transport standards, security and services. Includes liaison across jurisdictions to provide uniform road regulations and enforcement practices."@en ;
  skos:narrower agift:Driving-licences-administration ;
  skos:narrower agift:Road-surface-maintenance ;
  skos:narrower agift:Road-traffic-regulation ;
  skos:narrower agift:Road-transport-safety ;
  skos:narrower agift:Vehicle-registration ;
  skos:narrower agift:Vehicle-standards ;
  skos:prefLabel "Road transport"@en ;
.
agift:Road-transport-safety
  a skos:Concept ;
  dcterms:contributor "KOdea" ;
  dcterms:created "2016-07-06T05:16:24+00:00"^^xsd:dateTime ;
  dcterms:creator "superadmin" ;
  dcterms:modified "2016-09-13T07:21:12+00:00"^^xsd:dateTime ;
  skos:altLabel "Accident investigation"@en ;
  skos:altLabel "Road rules"@en ;
  skos:altLabel "Road safety"@en ;
  skos:altLabel "Safety investigation"@en ;
  skos:broader agift:Road-transport ;
  skos:definition "Regulating all road-use activities to improve security and reduce the risk of accidents or emergencies. Investigating accidents and incidents. Monitoring compliance with safety standards in the road transport industry. Developing standards for driver fitness, such as limits for alcohol consumption or driving hours. Encouraging the use of helmets or pedestrian crossings. Promoting road safety through programs targeting driver health and on-road behaviour. Includes training and advice, consultation and inspection services and cooperation across jurisdictions on road safety issues."@en ;
  skos:prefLabel "Road transport safety"@en ;
  skos:related agift:Driving-licences-administration ;
  skos:related agift:Freight-movement-regulation ;
  skos:related agift:Law-enforcement ;
  skos:related agift:Passenger-services ;
  skos:related agift:Road-safety-awareness ;
  skos:related agift:Road-traffic-regulation ;
  skos:related agift:Vehicle-standards ;
.
agift:Rolling-stock-regulation
  a skos:Concept ;
  dcterms:contributor "KOdea" ;
  dcterms:created "2016-07-06T05:15:43+00:00"^^xsd:dateTime ;
  dcterms:creator "superadmin" ;
  dcterms:modified "2016-09-13T07:15:50+00:00"^^xsd:dateTime ;
  skos:altLabel "Coupling standards"@en ;
  skos:altLabel "Engine drivers"@en ;
  skos:altLabel "Locomotives"@en ;
  skos:altLabel "Rail motors"@en ;
  skos:altLabel "Train drivers"@en ;
  skos:altLabel "Trains"@en ;
  skos:altLabel "Trams"@en ;
  skos:broader agift:Rail-transport ;
  skos:definition "Developing policy to support the design, construction, maintenance and operation of any vehicle operating on a railway track - such as locomotives, carriages, rail cars, rail motors, light rail vehicles, trains, trams or wagons. Ensuring rolling stock conform to operational standards. Conducting inspections, testing and licensing. Includes certification of engine drivers, railway engineers and other personnel engaged in the use or maintenance of rolling stock."@en ;
  skos:prefLabel "Rolling stock regulation"@en ;
  skos:related agift:Rail-transport-safety ;
.
agift:Rural-community-development
  a skos:Concept ;
  dcterms:contributor "KOdea" ;
  dcterms:created "2016-07-06T02:56:20+00:00"^^xsd:dateTime ;
  dcterms:creator "superadmin" ;
  dcterms:modified "2016-09-06T07:53:32+00:00"^^xsd:dateTime ;
  skos:altLabel "Community development"@en ;
  skos:broader agift:COMMUNITY-SERVICES ;
  skos:definition "Supporting outback and country communities through targeted services and programs to develop self-reliance. Establishing social networks and activities. Providing funding and support for community-based or volunteer organisations. Includes activities to improve rural access to government services and liaising with local business to support community projects."@en ;
  skos:prefLabel "Rural community development"@en ;
  skos:related agift:Community-support ;
  skos:related agift:Indigenous-welfare-programs ;
  skos:related agift:Regional-development ;
  skos:related agift:Rural-partnership-programs ;
.
agift:Rural-field-day-promotion
  a skos:Concept ;
  dcterms:contributor "KOdea" ;
  dcterms:created "2016-07-06T03:42:14+00:00"^^xsd:dateTime ;
  dcterms:creator "superadmin" ;
  dcterms:modified "2016-08-30T06:14:15+00:00"^^xsd:dateTime ;
  skos:altLabel "Agricultural shows"@en ;
  skos:broader agift:PRIMARY-INDUSTRIES ;
  skos:definition "Developing programs to support shows, exhibitions and conferences to encourage agricultural innovation. Includes financial assistance and advice on planning and marketing strategies."@en ;
  skos:prefLabel "Rural field day promotion"@en ;
.
agift:Rural-partnership-programs
  a skos:Concept ;
  dcterms:contributor "KOdea" ;
  dcterms:created "2016-07-06T03:42:24+00:00"^^xsd:dateTime ;
  dcterms:creator "superadmin" ;
  dcterms:modified "2016-09-12T06:19:21+00:00"^^xsd:dateTime ;
  skos:altLabel "Agricultural Development Partnership Program"@en ;
  skos:broader agift:PRIMARY-INDUSTRIES ;
  skos:definition "Initiating cooperative projects to support change in the operation of primary industries and agricultural business ventures. Developing strategies to help rural enterprises and communities adjust to changing commercial conditions, to improve profitability and competitiveness. Providing advice, training and project funding assistance."@en ;
  skos:prefLabel "Rural partnership programs"@en ;
  skos:related agift:Marine-and-rural-support ;
  skos:related agift:Rural-community-development ;
.
agift:SCIENCE
  a skos:Concept ;
  dcterms:contributor "fionamcl" ;
  dcterms:created "2016-07-06T02:47:36+00:00"^^xsd:dateTime ;
  dcterms:creator "superadmin" ;
  dcterms:modified "2016-09-20T00:08:41+00:00"^^xsd:dateTime ;
  skos:altLabel "Research"@en ;
  skos:definition "Developing policy and standards to support research and systematic studies. Administering scientific bodies and monitoring industry research and development programs. Providing funding and implementing promotional strategies. Includes research into living things and their environments, natural laws and the application of knowledge to practical problems."@en ;
  skos:narrower agift:Agricultural-sciences ;
  skos:narrower agift:Animal-and-veterinary-sciences ;
  skos:narrower agift:Applied-sciences ;
  skos:narrower agift:Biological-sciences ;
  skos:narrower agift:Earth-sciences ;
  skos:narrower agift:Ethical-compliance ;
  skos:narrower agift:Mathematical-sciences ;
  skos:narrower agift:Medical-and-health-sciences ;
  skos:narrower agift:Physical-sciences ;
  skos:narrower agift:Spatial-information-research ;
  skos:prefLabel "SCIENCE"@en ;
  skos:related agift:Energy-resources ;
  skos:related agift:NATURAL-RESOURCES ;
  skos:related agift:PRIMARY-INDUSTRIES ;
  skos:related agift:Renewable-energy-development ;
  skos:topConceptOf agift:AGIFT ;
.
agift:SECURITY
  a skos:Concept ;
  dcterms:contributor "KOdea" ;
  dcterms:created "2016-07-06T02:47:46+00:00"^^xsd:dateTime ;
  dcterms:creator "superadmin" ;
  dcterms:modified "2016-09-09T07:11:28+00:00"^^xsd:dateTime ;
  skos:definition "Maintaining the safety of Australia at all levels of society. Developing policy and programs to guard against internal or external threats to peace and stability. Providing funding for law enforcement, community protection and corrective services. Coordinating intelligence gathering and international security activities."@en ;
  skos:narrower agift:Corrective-services ;
  skos:narrower agift:External-security ;
  skos:narrower agift:Information-security ;
  skos:narrower agift:Intelligence ;
  skos:narrower agift:Law-enforcement ;
  skos:narrower agift:National-security ;
  skos:prefLabel "SECURITY"@en ;
  skos:related agift:DEFENCE ;
  skos:related agift:JUSTICE-ADMINISTRATION ;
  skos:topConceptOf agift:AGIFT ;
.
agift:SPORT-AND-RECREATION
  a skos:Concept ;
  dcterms:contributor "superadmin" ;
  dcterms:created "2016-07-06T02:47:54+00:00"^^xsd:dateTime ;
  dcterms:creator "superadmin" ;
  dcterms:modified "2016-07-07T00:35:33+00:00"^^xsd:dateTime ;
  skos:definition "Developing policy and programs to encourage community participation in organised games or leisure activities. Implementing promotional strategies, providing funding and administering regulatory bodies."@en ;
  skos:narrower agift:Caravan-and-camping-services ;
  skos:narrower agift:Community-recreational-programs ;
  skos:narrower agift:Gaming-industry-regulation ;
  skos:narrower agift:Park-and-reserve-services ;
  skos:narrower agift:Sport-and-fitness-development ;
  skos:narrower agift:Sports-drugs-monitoring ;
  skos:prefLabel "SPORT AND RECREATION"@en ;
  skos:topConceptOf agift:AGIFT ;
.
agift:STATISTICAL-SERVICES
  a skos:Concept ;
  dcterms:contributor "KOdea" ;
  dcterms:created "2016-07-06T02:48:03+00:00"^^xsd:dateTime ;
  dcterms:creator "superadmin" ;
  dcterms:modified "2016-09-12T06:39:00+00:00"^^xsd:dateTime ;
  skos:altLabel "Statistics"@en ;
  skos:definition "Providing a high quality, objective and responsive statistical service to assist and encourage informed decision making, research and discussion within governments and the community."@en ;
  skos:narrower agift:Statistical-collection ;
  skos:narrower agift:Statistical-design ;
  skos:narrower agift:Statistical-standards ;
  skos:narrower agift:Statistics-dissemination ;
  skos:prefLabel "STATISTICAL SERVICES"@en ;
  skos:related agift:Mathematical-sciences ;
  skos:topConceptOf agift:AGIFT ;
.
agift:Satellite-communication
  a skos:Concept ;
  dcterms:contributor "KOdea" ;
  dcterms:created "2016-07-06T02:54:48+00:00"^^xsd:dateTime ;
  dcterms:creator "superadmin" ;
  dcterms:modified "2016-09-05T07:52:58+00:00"^^xsd:dateTime ;
  skos:altLabel "Satellites"@en ;
  skos:broader agift:COMMUNICATIONS ;
  skos:definition "Developing policy to support and regulate industries that relay radio and television signals via equipment located in space. Managing government-owned satellite equipment. Providing advice on the introduction of new technology and the effects of government policy on the satellite communication industry. Includes liaison with international bodies on shared access to satellite equipment."@en ;
  skos:prefLabel "Satellite communication"@en ;
  skos:related agift:Astronomical-sciences ;
  skos:related agift:Navigation-systems-development ;
  skos:related agift:Search-technology-development ;
  skos:related agift:Spatial-information-research ;
.
agift:School-education
  a skos:Concept ;
  dcterms:contributor "KOdea" ;
  dcterms:created "2016-07-06T03:00:50+00:00"^^xsd:dateTime ;
  dcterms:creator "superadmin" ;
  dcterms:modified "2016-09-09T06:09:50+00:00"^^xsd:dateTime ;
  skos:altLabel "Health education"@en ;
  skos:altLabel "Primary schools"@en ;
  skos:altLabel "Private school regulation"@en ;
  skos:altLabel "Secondary schools"@en ;
  skos:altLabel "Sex education"@en ;
  skos:altLabel "State schools"@en ;
  skos:broader agift:EDUCATION-AND-TRAINING ;
  skos:definition "Administering programs that offer instruction to children, to impart knowledge and develop skills. Providing public school education for children in Years 1 to 12. Monitoring and regulating non-government schools. Managing school facilities. Implementing standards and guidelines to support teachers. Includes the provision of scholarships and study grants."@en ;
  skos:narrower agift:Discipline-programs ;
  skos:narrower agift:School-transport-regulation ;
  skos:narrower agift:Special-needs-programs ;
  skos:prefLabel "School education"@en ;
  skos:related agift:Arts-education ;
  skos:related agift:Curriculum-development ;
  skos:related agift:Early-childhood-education ;
  skos:related agift:Health-promotion ;
  skos:related agift:Overseas-aid-programs ;
  skos:related agift:Primary-health-care ;
.
agift:School-transport-regulation
  a skos:Concept ;
  dcterms:contributor "KOdea" ;
  dcterms:created "2016-07-06T04:14:22+00:00"^^xsd:dateTime ;
  dcterms:creator "superadmin" ;
  dcterms:modified "2016-09-08T07:13:56+00:00"^^xsd:dateTime ;
  skos:altLabel "School bus services"@en ;
  skos:broader agift:School-education ;
  skos:definition "Designing services to help children travel to and from school. Developing standards and guidelines to assist bus drivers or children with special needs. Identifying requirements for bus stops, cycle routes, footpaths, crossings and low speed limits. Liaising with government and non-government organisations to implement and regulate school transport services."@en ;
  skos:prefLabel "School transport regulation"@en ;
  skos:related agift:Passenger-services ;
  skos:related agift:Road-safety-awareness ;
  skos:related agift:Transport-access-schemes ;
  skos:related agift:Transport-network-maintenance ;
.
agift:Sea-passengers
  a skos:Concept ;
  dcterms:contributor "KOdea" ;
  dcterms:created "2016-07-06T03:39:50+00:00"^^xsd:dateTime ;
  dcterms:creator "superadmin" ;
  dcterms:modified "2016-09-09T07:43:46+00:00"^^xsd:dateTime ;
  skos:broader agift:MARITIME-SERVICES ;
  skos:definition "Developing policy for the transportation of people by sea. Monitoring compliance with pricing regulations or the provision of appropriate facilities for passenger convenience. Includes services such as timetables, route maps or ticketing."@en ;
  skos:prefLabel "Sea passengers"@en ;
  skos:related agift:Passenger-services ;
  skos:related agift:Personnel-safety-standards ;
  skos:related agift:Ship-personnel ;
.
agift:Search-and-rescue
  a skos:Concept ;
  dcterms:contributor "KOdea" ;
  dcterms:created "2016-07-06T03:39:57+00:00"^^xsd:dateTime ;
  dcterms:creator "superadmin" ;
  dcterms:modified "2016-09-09T07:38:03+00:00"^^xsd:dateTime ;
  skos:altLabel "Coastguard"@en ;
  skos:broader agift:MARITIME-SERVICES ;
  skos:definition "Developing policy and providing resources to ensure the safety of individuals, vessels or aircraft that become lost at sea. Managing reporting systems. Monitoring compliance with equipment standards and response requirements. Includes support for community-based services and regulating the use of volunteers and coordinating maritime emergency services."@en ;
  skos:narrower agift:Rescue-coordination ;
  skos:narrower agift:Search-technology-development ;
  skos:prefLabel "Search and rescue"@en ;
  skos:related agift:Civil-community-assistance ;
  skos:related agift:Emergency-management ;
  skos:related agift:Firefighting-services ;
  skos:related agift:Natural-disasters ;
.
agift:Search-technology-development
  a skos:Concept ;
  dcterms:contributor "KOdea" ;
  dcterms:created "2016-07-06T04:58:42+00:00"^^xsd:dateTime ;
  dcterms:creator "superadmin" ;
  dcterms:modified "2016-09-12T06:46:38+00:00"^^xsd:dateTime ;
  skos:broader agift:Search-and-rescue ;
  skos:definition "Conducting research into the application of specialist knowledge and equipment to assist marine rescue operations. Developing communications systems to help locate individuals, vessels or aircraft lost at sea. Providing technical advice on the purchase of search equipment. Includes designing, testing and overseeing the manufacture of new products."@en ;
  skos:prefLabel "Search technology development"@en ;
  skos:related agift:COMMUNICATIONS ;
  skos:related agift:Navigation-systems-development ;
  skos:related agift:Satellite-communication ;
  skos:related agift:Spatial-information-research ;
.
agift:Seaworthiness
  a skos:Concept ;
  dcterms:contributor "KOdea" ;
  dcterms:created "2016-07-06T04:59:17+00:00"^^xsd:dateTime ;
  dcterms:creator "superadmin" ;
  dcterms:modified "2016-08-29T06:57:27+00:00"^^xsd:dateTime ;
  skos:altLabel "Unseaworthiness"@en ;
  skos:broader agift:Ship-safety ;
  skos:definition "Certifying private or commercial marine vessels as fit for use at sea. Assessing applications to ensure compliance with standards and inspection requirements. Providing training and advice on safety requirements."@en ;
  skos:prefLabel "Seaworthiness"@en ;
.
agift:Seismology
  a skos:Concept ;
  dcterms:contributor "KOdea" ;
  dcterms:created "2016-07-06T05:05:23+00:00"^^xsd:dateTime ;
  dcterms:creator "superadmin" ;
  dcterms:modified "2016-09-12T06:36:05+00:00"^^xsd:dateTime ;
  skos:altLabel "Earthquake studies"@en ;
  skos:altLabel "Seismography"@en ;
  skos:broader agift:Earth-sciences ;
  skos:definition "Conducting research into earthquakes. Monitoring and recording seismic surface waves, quarry blasts and mining activities, and data mapping of tectonic plate structures. Providing scientific advice on hazard management. Includes asset vulnerability assessment and emergency simulation and training, to deal with seismic events and their effects."@en ;
  skos:prefLabel "Seismology"@en ;
  skos:related agift:Mineral-exploration ;
.
agift:Ship-commissioning
  a skos:Concept ;
  dcterms:contributor "KOdea" ;
  dcterms:created "2016-07-06T04:59:25+00:00"^^xsd:dateTime ;
  dcterms:creator "superadmin" ;
  dcterms:modified "2016-08-29T06:58:33+00:00"^^xsd:dateTime ;
  skos:altLabel "Decommissioning"@en ;
  skos:altLabel "Shipbuilding"@en ;
  skos:broader agift:Ship-safety ;
  skos:definition "Transferring commercial and private marine vessels into or out of active service. Includes ship building activities and supply of captain and crew."@en ;
  skos:prefLabel "Ship commissioning"@en ;
.
agift:Ship-inspection
  a skos:Concept ;
  dcterms:contributor "KOdea" ;
  dcterms:created "2016-07-06T04:59:32+00:00"^^xsd:dateTime ;
  dcterms:creator "superadmin" ;
  dcterms:modified "2016-08-29T06:59:03+00:00"^^xsd:dateTime ;
  skos:broader agift:Ship-safety ;
  skos:definition "Monitoring compliance with standards and guidelines for the design, construction and maintenance of private or commercial marine vessels. Conducting inspections of structural integrity, safety equipment or emissions. Examining foreign flagships in Australian ports to monitor compliance with international regulations."@en ;
  skos:prefLabel "Ship inspection"@en ;
.
agift:Ship-personnel
  a skos:Concept ;
  dcterms:contributor "KOdea" ;
  dcterms:created "2016-07-06T03:40:04+00:00"^^xsd:dateTime ;
  dcterms:creator "superadmin" ;
  dcterms:modified "2016-09-09T07:41:24+00:00"^^xsd:dateTime ;
  skos:altLabel "Crew"@en ;
  skos:altLabel "Maritime personnel"@en ;
  skos:altLabel "Ship captains"@en ;
  skos:broader agift:MARITIME-SERVICES ;
  skos:definition "Regulating the operation of private or commercial marine vessels to improve security and reduce the risk of accidents or emergencies. Developing standards and guidelines for operational practices and crew competencies. Includes cooperation on maritime personnel safety across jurisdictions."@en ;
  skos:narrower agift:Personnel-safety-standards ;
  skos:prefLabel "Ship personnel"@en ;
  skos:related agift:Navy ;
  skos:related agift:Sea-passengers ;
  skos:related agift:Ship-safety ;
.
agift:Ship-safety
  a skos:Concept ;
  dcterms:contributor "KOdea" ;
  dcterms:created "2016-07-06T03:40:12+00:00"^^xsd:dateTime ;
  dcterms:creator "superadmin" ;
  dcterms:modified "2016-09-09T07:41:24+00:00"^^xsd:dateTime ;
  skos:altLabel "Accident investigation"@en ;
  skos:altLabel "Boat safety"@en ;
  skos:altLabel "Marine safety"@en ;
  skos:altLabel "Safety investigation"@en ;
  skos:altLabel "Sea safety"@en ;
  skos:altLabel "Shipbuilding standards"@en ;
  skos:broader agift:MARITIME-SERVICES ;
  skos:definition "Regulating the design, construction and maintenance of private or commercial marine vessels. Developing standards and guidelines for safety equipment, seaworthiness, noise or emissions. Investigating the circumstances and causes of marine accidents. Promoting safety awareness across the maritime industry."@en ;
  skos:narrower agift:Seaworthiness ;
  skos:narrower agift:Ship-commissioning ;
  skos:narrower agift:Ship-inspection ;
  skos:prefLabel "Ship safety"@en ;
  skos:related agift:Ship-personnel ;
.
agift:Silvicultural-industry
  a skos:Concept ;
  dcterms:contributor "KOdea" ;
  dcterms:created "2016-07-06T05:02:56+00:00"^^xsd:dateTime ;
  dcterms:creator "superadmin" ;
  dcterms:modified "2016-09-12T06:17:12+00:00"^^xsd:dateTime ;
  skos:altLabel "Forest support"@en ;
  skos:altLabel "National Forestry Inventory"@en ;
  skos:altLabel "Plantation management support"@en ;
  skos:broader agift:Marine-and-rural-support ;
  skos:definition "Administering programs to support commercial cultivation of forests. Assisting industry growth and development. Encouraging businesses to adopt innovative practices, processes and products. Providing advice on growing or harvesting methods and business management to improve competitiveness."@en ;
  skos:prefLabel "Silvicultural industry"@en ;
  skos:related agift:Agricultural-sciences ;
  skos:related agift:Forestry-industry ;
.
agift:Small-business-advocacy
  a skos:Concept ;
  dcterms:contributor "KOdea" ;
  dcterms:created "2016-07-06T03:52:30+00:00"^^xsd:dateTime ;
  dcterms:creator "superadmin" ;
  dcterms:modified "2016-09-05T06:31:19+00:00"^^xsd:dateTime ;
  skos:broader agift:Small-business-services ;
  skos:definition "Administering programs to support the interests of commercial enterprises of limited size or capital. Promoting the establishment of small businesses. Providing advice on the impact of government policy on small business. Includes liaison with industry groups and small business representatives."@en ;
  skos:prefLabel "Small business advocacy"@en ;
  skos:related agift:Industry-assistance-schemes ;
  skos:related agift:Marine-and-rural-support ;
  skos:related agift:Vocational-education ;
.
agift:Small-business-development
  a skos:Concept ;
  dcterms:contributor "KOdea" ;
  dcterms:created "2016-07-06T03:52:38+00:00"^^xsd:dateTime ;
  dcterms:creator "superadmin" ;
  dcterms:modified "2016-09-05T06:33:20+00:00"^^xsd:dateTime ;
  skos:broader agift:Small-business-services ;
  skos:definition "Administering programs to encourage the growth of commercial enterprises of limited size or capital. Identifying markets or investment opportunities for small business. Developing quality assurance systems and reporting requirements appropriate to the scale of operations. Allocating grants or incentives for new initiatives."@en ;
  skos:prefLabel "Small business development"@en ;
  skos:related agift:Industry-development ;
.
agift:Small-business-services
  a skos:Concept ;
  dcterms:contributor "KOdea" ;
  dcterms:created "2016-07-06T02:50:53+00:00"^^xsd:dateTime ;
  dcterms:creator "superadmin" ;
  dcterms:modified "2016-09-05T06:29:25+00:00"^^xsd:dateTime ;
  skos:broader agift:BUSINESS-SUPPORT-AND-REGULATION ;
  skos:definition "Developing policy and programs to assist commercial enterprises of limited size or capital. Providing advisory services to support the start-up and ongoing operation of small businesses. Encouraging the adoption of innovative practices, processes and products. Includes the establishment of communication networks or resource centres."@en ;
  skos:narrower agift:Small-business-advocacy ;
  skos:narrower agift:Small-business-development ;
  skos:prefLabel "Small business services"@en ;
.
agift:Social-club-support
  a skos:Concept ;
  dcterms:contributor "fionamcl" ;
  dcterms:created "2016-07-06T05:09:13+00:00"^^xsd:dateTime ;
  dcterms:creator "superadmin" ;
  dcterms:modified "2016-09-08T01:49:23+00:00"^^xsd:dateTime ;
  skos:altLabel "Non-profit organisations support"@en ;
  skos:broader agift:Community-recreational-programs ;
  skos:definition "Providing financial assistance and services for community-based and non-profit organisations that promote friendship and recreation. Raising awareness of local groups though sponsorship, advertising and facilitating links between organisations."@en ;
  skos:prefLabel "Social club support"@en ;
  skos:related agift:Multicultural-services ;
.
agift:Social-justice-and-equity
  a skos:Concept ;
  dcterms:contributor "KOdea" ;
  dcterms:created "2016-07-06T02:56:29+00:00"^^xsd:dateTime ;
  dcterms:creator "superadmin" ;
  dcterms:modified "2016-09-08T07:25:24+00:00"^^xsd:dateTime ;
  skos:altLabel "Affirmative action"@en ;
  skos:altLabel "Age discrimination"@en ;
  skos:altLabel "Anti-discrimination programs"@en ;
  skos:altLabel "Anti-discrimination"@en ;
  skos:altLabel "Community access programs"@en ;
  skos:altLabel "Cultural diversity programs"@en ;
  skos:altLabel "Disability rights"@en ;
  skos:altLabel "Discrimination"@en ;
  skos:altLabel "Equal opportunity programs"@en ;
  skos:altLabel "Equity programs"@en ;
  skos:altLabel "Gender discrimination"@en ;
  skos:altLabel "Inclusion"@en ;
  skos:altLabel "Racial discrimination"@en ;
  skos:altLabel "Religious discrimination"@en ;
  skos:altLabel "Sex discrimination"@en ;
  skos:altLabel "Status of women"@en ;
  skos:altLabel "Welfare complaint services"@en ;
  skos:broader agift:COMMUNITY-SERVICES ;
  skos:definition "Developing policy to support the fair treatment of all people, regardless of gender, race, colour, ethnicity, age, marital or parental status, sexual preference, disability or religious belief. Ensuring that government services are implemented with fairness and sensitivity to community needs. Reviewing services and making recommendations to improve access. Promoting equal opportunity and anti-discrimination principles. Includes liaison with target groups to evaluate the effectiveness of equity programs."@en ;
  skos:prefLabel "Social justice and equity"@en ;
  skos:related agift:Community-support ;
  skos:related agift:Indigenous-advocacy ;
  skos:related agift:Workplace-discrimination-monitoring ;
  skos:related agift:Workplace-equity-and-justice-programs ;
.
agift:Social-media
  a skos:Concept ;
  dcterms:contributor "KOdea" ;
  dcterms:created "2016-07-06T03:58:27+00:00"^^xsd:dateTime ;
  dcterms:creator "superadmin" ;
  dcterms:modified "2016-09-05T07:39:17+00:00"^^xsd:dateTime ;
  skos:broader agift:Internet ;
  skos:definition "Developing policy and programs to enable governments to  consult widely with citizens via social media platforms"@en ;
  skos:prefLabel "Social media"@en ;
  skos:related agift:Community-engagement ;
  skos:related agift:Government-media ;
.
agift:Social-research
  a skos:Concept ;
  dcterms:contributor "KOdea" ;
  dcterms:created "2016-07-06T02:56:37+00:00"^^xsd:dateTime ;
  dcterms:creator "superadmin" ;
  dcterms:modified "2016-08-09T07:56:05+00:00"^^xsd:dateTime ;
  skos:altLabel "Family research"@en ;
  skos:broader agift:COMMUNITY-SERVICES ;
  skos:definition "Developing research programs to examine Australians' attitudes, beliefs, trends, stratifications and rules."@en ;
  skos:prefLabel "Social research"@en ;
.
agift:Soil-preservation-programs
  a skos:Concept ;
  dcterms:contributor "KOdea" ;
  dcterms:created "2016-07-06T04:33:28+00:00"^^xsd:dateTime ;
  dcterms:creator "superadmin" ;
  dcterms:modified "2016-09-12T06:20:08+00:00"^^xsd:dateTime ;
  skos:altLabel "Beach stabilisation programs"@en ;
  skos:altLabel "Erosion prevention programs"@en ;
  skos:altLabel "Sustainable agriculture"@en ;
  skos:broader agift:Conservation-programs ;
  skos:definition "Managing programs to prevent or repair damage to the ground or earth. Restoring specific areas to their native state or preventing further degradation. Conducting activities to counteract soil erosion or chemical contamination. Includes funding for joint projects with local business or community groups."@en ;
  skos:prefLabel "Soil preservation programs"@en ;
  skos:related agift:Agricultural-sciences ;
  skos:related agift:Chemical-and-pesticide-regulation ;
  skos:related agift:Land-rehabilitation-programs ;
  skos:related agift:Waterway-management ;
.
agift:Spatial-information-research
  a skos:Concept ;
  dcterms:contributor "KOdea" ;
  dcterms:created "2016-07-06T03:43:56+00:00"^^xsd:dateTime ;
  dcterms:creator "superadmin" ;
  dcterms:modified "2016-09-12T06:46:38+00:00"^^xsd:dateTime ;
  skos:altLabel "Geographical Information Systems"@en ;
  skos:altLabel "Global positioning systems"@en ;
  skos:broader agift:SCIENCE ;
  skos:definition "Investigating practical applications for geographical data. Providing advice on the development of standards, protocols and specifications for spatial information systems. Includes developing integrated access to information via the Internet, mobile information systems and global positioning systems (GPS)."@en ;
  skos:prefLabel "Spatial information research"@en ;
  skos:related agift:Applied-sciences ;
  skos:related agift:CIVIC-INFRASTRUCTURE ;
  skos:related agift:COMMUNICATIONS ;
  skos:related agift:Charting-sea-lanes ;
  skos:related agift:Community-based-corrections ;
  skos:related agift:Defence-science-and-technology ;
  skos:related agift:Navigation-systems-development ;
  skos:related agift:Satellite-communication ;
  skos:related agift:Search-technology-development ;
.
agift:Special-needs-programs
  a skos:Concept ;
  dcterms:contributor "KOdea" ;
  dcterms:created "2016-07-06T04:14:34+00:00"^^xsd:dateTime ;
  dcterms:creator "superadmin" ;
  dcterms:modified "2016-09-09T06:03:19+00:00"^^xsd:dateTime ;
  skos:altLabel "Extension education programs"@en ;
  skos:altLabel "Remedial education programs"@en ;
  skos:altLabel "Tutoring"@en ;
  skos:broader agift:School-education ;
  skos:definition "Administering learning and community support programs for primary and secondary students in target groups. Providing remedial education to assist those in difficulty, and extension programs for the gifted. Includes children with physical or intellectual disabilities, those with English as a second language, migrant or Indigenous children."@en ;
  skos:prefLabel "Special needs programs"@en ;
  skos:related agift:Adult-migrant-education ;
.
agift:Special-needs-services
  a skos:Concept ;
  dcterms:contributor "KOdea" ;
  dcterms:created "2016-07-06T03:07:50+00:00"^^xsd:dateTime ;
  dcterms:creator "superadmin" ;
  dcterms:modified "2016-09-09T06:24:59+00:00"^^xsd:dateTime ;
  skos:altLabel "Adolescent health services"@en ;
  skos:altLabel "Brain injury support services"@en ;
  skos:altLabel "Cancer support services"@en ;
  skos:altLabel "Child and adolescent health services"@en ;
  skos:altLabel "Disability services"@en ;
  skos:altLabel "Hearing services"@en ;
  skos:altLabel "Infant health services"@en ;
  skos:altLabel "Migrant health services"@en ;
  skos:altLabel "Occupational therapy"@en ;
  skos:altLabel "Physiotherapy"@en ;
  skos:altLabel "Rehabilitation services"@en ;
  skos:altLabel "Sexual assault victims support"@en ;
  skos:altLabel "Speech pathology"@en ;
  skos:altLabel "Support groups"@en ;
  skos:altLabel "Women's health services"@en ;
  skos:altLabel "Youth health services"@en ;
  skos:broader agift:HEALTH-CARE ;
  skos:definition "Developing policy to support the physical and mental wellbeing of people with particular requirements. Establishing health care programs to assist target groups. Includes advisory and support services for individuals with a particular medical condition."@en ;
  skos:narrower agift:Dental-health-services ;
  skos:narrower agift:Independent-living-services ;
  skos:narrower agift:Mental-health-services ;
  skos:narrower agift:Residential-services ;
  skos:prefLabel "Special needs services"@en ;
  skos:related agift:Aged-care-services ;
  skos:related agift:Clinical-health-services ;
  skos:related agift:Community-health-services ;
  skos:related agift:Counselling-services ;
  skos:related agift:Indigenous-health-services ;
  skos:related agift:Veterans-health-services ;
.
agift:Special-operations
  a skos:Concept ;
  dcterms:contributor "KOdea" ;
  dcterms:created "2016-07-06T04:12:21+00:00"^^xsd:dateTime ;
  dcterms:creator "superadmin" ;
  dcterms:modified "2016-09-08T07:00:44+00:00"^^xsd:dateTime ;
  skos:altLabel "Unconventional warfare"@en ;
  skos:broader agift:Military-operations ;
  skos:definition "Developing unique approaches to achieve specific military objectives. Deploying small units of highly trained combat personnel, in response to extraordinary circumstances or where specialist skills and equipment are required. Includes training provided to foreign local forces, when military aid is given to other countries."@en ;
  skos:prefLabel "Special operations"@en ;
  skos:related agift:Australian-theatre-of-war ;
  skos:related agift:Emergency-management ;
  skos:related agift:Intelligence-support ;
  skos:related agift:Military-law ;
  skos:related agift:Peacekeeping-forces ;
  skos:related agift:Warfare ;
.
agift:Spectrum-management
  a skos:Concept ;
  dcterms:contributor "KOdea" ;
  dcterms:created "2016-07-06T04:00:02+00:00"^^xsd:dateTime ;
  dcterms:creator "superadmin" ;
  dcterms:modified "2016-08-05T05:53:32+00:00"^^xsd:dateTime ;
  skos:altLabel "Bandwidth licensing"@en ;
  skos:altLabel "Radio bandwidth licensing"@en ;
  skos:broader agift:Radio-communication ;
  skos:definition "Administering the allocation and use of radio spectrum or 'space'. Assessing compliance with government regulations. Processing licence applications for bandwidth and radiofrequency. Monitoring signals allocation to reduce interference and developing long-term spectrum plans with defence, scientific, aircraft and maritime industries."@en ;
  skos:prefLabel "Spectrum management"@en ;
.
agift:Sport-and-fitness-development
  a skos:Concept ;
  dcterms:contributor "KOdea" ;
  dcterms:created "2016-07-06T03:45:52+00:00"^^xsd:dateTime ;
  dcterms:creator "superadmin" ;
  dcterms:modified "2016-09-13T06:52:05+00:00"^^xsd:dateTime ;
  skos:broader agift:SPORT-AND-RECREATION ;
  skos:definition "Developing policy and programs to support the growth of competitive sports and associated industries. Encouraging increased participation and funding for sports and fitness programs. Providing training institutions and facilities for elite athletes."@en ;
  skos:narrower agift:Athlete-scholarship-programs ;
  skos:narrower agift:Fundraising-and-donation-schemes ;
  skos:narrower agift:Games-administration ;
  skos:narrower agift:Games-promotion ;
  skos:narrower agift:Sporting-grants-administration ;
  skos:prefLabel "Sport and fitness development"@en ;
  skos:related agift:Business-association ;
  skos:related agift:Games-administration ;
  skos:related agift:Public-fitness-promotion ;
.
agift:Sporting-facilities-management
  a skos:Concept ;
  dcterms:contributor "KOdea" ;
  dcterms:created "2016-07-06T03:55:39+00:00"^^xsd:dateTime ;
  dcterms:creator "superadmin" ;
  dcterms:modified "2016-09-05T07:14:21+00:00"^^xsd:dateTime ;
  skos:altLabel "Oval maintenance"@en ;
  skos:altLabel "Playing fields"@en ;
  skos:altLabel "Public swimming pool maintenance"@en ;
  skos:altLabel "Skate parks"@en ;
  skos:altLabel "Swimming pools"@en ;
  skos:broader agift:Public-land-management ;
  skos:definition "Overseeing the care and preparation of land set aside for sporting grounds and amenities. Ensuring facilities are kept clean and maintained. Includes field or court markings, turf or pitch quality, spectator seating, and swimming pools."@en ;
  skos:prefLabel "Sporting facilities management"@en ;
  skos:related agift:Park-and-reserve-services ;
  skos:related agift:Recreational-park-management ;
  skos:related agift:Sporting-grants-administration ;
.
agift:Sporting-grants-administration
  a skos:Concept ;
  dcterms:contributor "KOdea" ;
  dcterms:created "2016-07-06T05:10:16+00:00"^^xsd:dateTime ;
  dcterms:creator "superadmin" ;
  dcterms:modified "2016-09-13T06:37:15+00:00"^^xsd:dateTime ;
  skos:broader agift:Sport-and-fitness-development ;
  skos:definition "Providing financial assistance to help build and develop sporting facilities. Identifying groups that may have less access to opportunities in sport. Allocating funds to support the training and development of athletes, coaches, officials and sports administrators."@en ;
  skos:prefLabel "Sporting grants administration"@en ;
  skos:related agift:Athlete-scholarship-programs ;
  skos:related agift:Park-and-reserve-services ;
  skos:related agift:Sporting-facilities-management ;
.
agift:Sports-drugs-monitoring
  a skos:Concept ;
  dcterms:contributor "KOdea" ;
  dcterms:created "2016-07-06T03:46:00+00:00"^^xsd:dateTime ;
  dcterms:creator "superadmin" ;
  dcterms:modified "2016-09-01T07:28:57+00:00"^^xsd:dateTime ;
  skos:altLabel "Drugs"@en ;
  skos:altLabel "Performance-enhancing drugs"@en ;
  skos:broader agift:SPORT-AND-RECREATION ;
  skos:definition "Developing policy to reduce the supply and use of banned or performance-enhancing substances. Preparing criteria to determine whether a substance is illegal and applying penalties for athletes found in breach of policy. Establishing measures to improve accountability in the prescription of sports drugs. Providing funding for research into doping detection tests. Collaborating with scientists and sporting bodies to share information and research."@en ;
  skos:narrower agift:Doping-detection-research ;
  skos:prefLabel "Sports drugs monitoring"@en ;
.
agift:Statistical-collection
  a skos:Concept ;
  dcterms:contributor "KOdea" ;
  dcterms:created "2016-07-06T03:46:24+00:00"^^xsd:dateTime ;
  dcterms:creator "superadmin" ;
  dcterms:modified "2016-09-13T06:48:50+00:00"^^xsd:dateTime ;
  skos:altLabel "Census"@en ;
  skos:altLabel "Demographic surveys"@en ;
  skos:altLabel "Household census"@en ;
  skos:altLabel "Population census"@en ;
  skos:altLabel "Statistical analysis"@en ;
  skos:broader agift:STATISTICAL-SERVICES ;
  skos:definition "Collecting statistics from official providers in Australia and as well as using administrative data to generate statistics. Analysing this collected data to identify trends and other significant information about social or economic activities."@en ;
  skos:prefLabel "Statistical collection"@en ;
  skos:related agift:Population-based-research ;
  skos:related agift:Statistical-design ;
  skos:related agift:Statistical-standards ;
  skos:related agift:Statistics-dissemination ;
.
agift:Statistical-design
  a skos:Concept ;
  dcterms:contributor "KOdea" ;
  dcterms:created "2016-07-06T03:46:32+00:00"^^xsd:dateTime ;
  dcterms:creator "superadmin" ;
  dcterms:modified "2016-09-13T06:47:09+00:00"^^xsd:dateTime ;
  skos:broader agift:STATISTICAL-SERVICES ;
  skos:definition "Designing statistical outputs, concepts, methodologies, metadata, and collection instruments ."@en ;
  skos:prefLabel "Statistical design"@en ;
  skos:related agift:Statistical-collection ;
  skos:related agift:Statistical-standards ;
  skos:related agift:Statistics-dissemination ;
.
agift:Statistical-standards
  a skos:Concept ;
  dcterms:contributor "KOdea" ;
  dcterms:created "2016-07-06T03:46:39+00:00"^^xsd:dateTime ;
  dcterms:creator "superadmin" ;
  dcterms:modified "2016-09-13T06:48:17+00:00"^^xsd:dateTime ;
  skos:broader agift:STATISTICAL-SERVICES ;
  skos:definition "Supporting and providing standards for numerical facts issued to the Australian community to ensure the information is coherent, comprehensible and consistent. Representing Australia on international standards bodies (such as the System of National Accounts and the International Monetary Fund's Balance of Payments Manual), advising official bodies within Australia about existing statistical standards and consulting on the development of new standards."@en ;
  skos:prefLabel "Statistical standards"@en ;
  skos:related agift:Statistical-collection ;
  skos:related agift:Statistical-design ;
  skos:related agift:Statistics-dissemination ;
.
agift:Statistics-dissemination
  a skos:Concept ;
  dcterms:contributor "KOdea" ;
  dcterms:created "2016-07-06T03:46:47+00:00"^^xsd:dateTime ;
  dcterms:creator "superadmin" ;
  dcterms:modified "2016-09-13T06:48:50+00:00"^^xsd:dateTime ;
  skos:broader agift:STATISTICAL-SERVICES ;
  skos:definition "Disseminating statistical information for use by a broad cross-section of the community, businesses, the research sector, the media, government departments and agencies, other governments and international agencies. Statistical categories may focus on environmental matters, government activities, population, economic or social matters."@en ;
  skos:prefLabel "Statistics dissemination"@en ;
  skos:related agift:Statistical-collection ;
  skos:related agift:Statistical-design ;
  skos:related agift:Statistical-standards ;
.
agift:Stock-market-regulation
  a skos:Concept ;
  dcterms:contributor "KOdea" ;
  dcterms:created "2016-07-06T02:51:02+00:00"^^xsd:dateTime ;
  dcterms:creator "superadmin" ;
  dcterms:modified "2016-08-04T07:13:51+00:00"^^xsd:dateTime ;
  skos:altLabel "Capital stock regulation"@en ;
  skos:altLabel "Company shares"@en ;
  skos:altLabel "Securities exchange"@en ;
  skos:altLabel "Shares regulation"@en ;
  skos:altLabel "Stock exchange"@en ;
  skos:broader agift:BUSINESS-SUPPORT-AND-REGULATION ;
  skos:definition "Developing policy to control the buying, selling and trading of shares and securities. Monitoring the activities of stock exchanges and stockbrokers. Issuing licenses, investigating suspected breaches of regulations and applying penalties when appropriate."@en ;
  skos:prefLabel "Stock market regulation"@en ;
.
agift:Strategic-decisions
  a skos:Concept ;
  dcterms:contributor "KOdea" ;
  dcterms:created "2016-07-06T04:10:29+00:00"^^xsd:dateTime ;
  dcterms:creator "superadmin" ;
  dcterms:modified "2016-09-08T06:43:10+00:00"^^xsd:dateTime ;
  skos:broader agift:Defence-strategic-policy ;
  skos:definition "Determining a course of action in relation to the deployment of Australia's defence capability. Reaching a conclusion to direct the conduct of military operations. Resolving a dilemma or choosing from a range of options, to realise defence strategic policy."@en ;
  skos:prefLabel "Strategic decisions"@en ;
  skos:related agift:Military-advisors ;
  skos:related agift:Military-operations ;
  skos:related agift:Strategic-planning ;
.
agift:Strategic-planning
  a skos:Concept ;
  dcterms:contributor "KOdea" ;
  dcterms:created "2016-07-06T04:10:36+00:00"^^xsd:dateTime ;
  dcterms:creator "superadmin" ;
  dcterms:modified "2016-09-08T06:43:56+00:00"^^xsd:dateTime ;
  skos:broader agift:Defence-strategic-policy ;
  skos:definition "Assessing military and diplomatic advice. Evaluating circumstances and the relative merits of various recommendations regarding deployment of defence resources or the conduct of military operations. Preparing materials to support decision making to realise defence strategic policy."@en ;
  skos:prefLabel "Strategic planning"@en ;
  skos:related agift:Defence-strategic-development ;
  skos:related agift:Military-advisors ;
  skos:related agift:Strategic-decisions ;
.
agift:Superannuation-regulation
  a skos:Concept ;
  dcterms:contributor "KOdea" ;
  dcterms:created "2016-07-06T04:38:48+00:00"^^xsd:dateTime ;
  dcterms:creator "superadmin" ;
  dcterms:modified "2016-09-08T08:05:19+00:00"^^xsd:dateTime ;
  skos:altLabel "Superannuation industry supervision"@en ;
  skos:broader agift:Retirement-income ;
  skos:definition "Certifying trust funds as superannuation funds, allowing them to accept superannuation contributions and receive concessional tax treatment. Assessing applications against set criteria. Monitoring activities to ensure compliance with superannuation regulations."@en ;
  skos:prefLabel "Superannuation regulation"@en ;
  skos:related agift:Financial-investment ;
  skos:related agift:Investment-scheme-regulation ;
  skos:related agift:Retirement-saving ;
.
agift:TOURISM
  a skos:Concept ;
  dcterms:contributor "KOdea" ;
  dcterms:created "2016-07-06T02:48:14+00:00"^^xsd:dateTime ;
  dcterms:creator "superadmin" ;
  dcterms:modified "2016-09-01T07:32:11+00:00"^^xsd:dateTime ;
  skos:altLabel "Tourism awards"@en ;
  skos:definition "Developing policy and programs to encourage recreational visitors to a region. Supporting and regulating the tourism industry. Implementing long-term strategies for tourism development and coordinating across jurisdictions on large-scale projects. Providing funding for promotional campaigns."@en ;
  skos:narrower agift:Tourism-industry-development ;
  skos:narrower agift:Tourist-event-promotion ;
  skos:narrower agift:Travel-missions ;
  skos:prefLabel "TOURISM"@en ;
  skos:topConceptOf agift:AGIFT ;
.
agift:TRADE
  a skos:Concept ;
  dcterms:contributor "KOdea" ;
  dcterms:created "2016-07-06T02:48:21+00:00"^^xsd:dateTime ;
  dcterms:creator "superadmin" ;
  dcterms:modified "2016-09-13T06:55:40+00:00"^^xsd:dateTime ;
  skos:altLabel "Balance of payments"@en ;
  skos:definition "Developing policy to regulate the purchase, sale or exchange of commodities. Monitoring the balance of trade, industry protection and subsidy schemes. Includes foreign and domestic activities, and liaison across jurisdictions to support trade agreement negotiations."@en ;
  skos:narrower agift:Export-regulation ;
  skos:narrower agift:Import-regulation ;
  skos:narrower agift:Intellectual-property-management ;
  skos:narrower agift:International-trade-agreements ;
  skos:narrower agift:Interstate-trade-agreements ;
  skos:narrower agift:Trade-development-programs ;
  skos:narrower agift:Trade-expositions ;
  skos:narrower agift:Trade-measurement-compliance ;
  skos:prefLabel "TRADE"@en ;
  skos:related agift:BUSINESS-SUPPORT-AND-REGULATION ;
  skos:topConceptOf agift:AGIFT ;
.
agift:TRANSPORT
  a skos:Concept ;
  dcterms:contributor "KOdea" ;
  dcterms:created "2016-07-06T02:48:28+00:00"^^xsd:dateTime ;
  dcterms:creator "superadmin" ;
  dcterms:modified "2016-09-09T07:28:38+00:00"^^xsd:dateTime ;
  skos:altLabel "Aerospace"@en ;
  skos:altLabel "Airlines"@en ;
  skos:altLabel "Airspace"@en ;
  skos:altLabel "Aviation"@en ;
  skos:definition "Developing policy to regulate road, rail and air transportation systems. Planning and managing schemes for the movement of people or freight. Monitoring the safety of vehicles and their operators. Providing resources for the development of transport infrastructure."@en ;
  skos:narrower agift:Air-transport ;
  skos:narrower agift:Freight-movement-regulation ;
  skos:narrower agift:Passenger-services ;
  skos:narrower agift:Public-transport ;
  skos:narrower agift:Rail-transport ;
  skos:narrower agift:Road-transport ;
  skos:narrower agift:Transport-infrastructure-development ;
  skos:prefLabel "TRANSPORT"@en ;
  skos:related agift:MARITIME-SERVICES ;
  skos:topConceptOf agift:AGIFT ;
.
agift:Tabling-of-official-documents
  a skos:Concept ;
  dcterms:contributor "KOdea" ;
  dcterms:created "2016-07-06T04:43:15+00:00"^^xsd:dateTime ;
  dcterms:creator "superadmin" ;
  dcterms:modified "2016-09-09T05:49:06+00:00"^^xsd:dateTime ;
  skos:broader agift:Parliamentary-chamber-support ;
  skos:definition "Submitting reports and other official documents to parliament or an assembly for discussion. Tabled documents allow review and scrutiny of government policy and through tabling become public documents. Includes programming documents and other procedures associated with their official tabling."@en ;
  skos:prefLabel "Tabling of official documents"@en ;
  skos:related agift:Draft-Bill-amendment-process ;
  skos:related agift:Legislative-drafting ;
.
agift:Tariff-regulation
  a skos:Concept ;
  dcterms:contributor "KOdea" ;
  dcterms:created "2016-07-06T05:13:18+00:00"^^xsd:dateTime ;
  dcterms:creator "superadmin" ;
  dcterms:modified "2016-09-13T07:03:34+00:00"^^xsd:dateTime ;
  skos:altLabel "Duties"@en ;
  skos:altLabel "Industry protection"@en ;
  skos:altLabel "Tariffs"@en ;
  skos:broader agift:Import-regulation ;
  skos:definition "Setting and collecting taxes or duties on imported goods and resources. Developing policy to control the imposition of charges, and procedures to process tariff payments."@en ;
  skos:prefLabel "Tariff regulation"@en ;
  skos:related agift:Port-regulation ;
  skos:related agift:Prohibited-import-control ;
  skos:related agift:Taxation ;
.
agift:Taxation
  a skos:Concept ;
  dcterms:contributor "KOdea" ;
  dcterms:created "2016-07-06T03:05:08+00:00"^^xsd:dateTime ;
  dcterms:creator "superadmin" ;
  dcterms:modified "2016-09-08T08:06:29+00:00"^^xsd:dateTime ;
  skos:altLabel "GST"@en ;
  skos:altLabel "Goods and Services Tax"@en ;
  skos:altLabel "Levies"@en ;
  skos:altLabel "Payroll tax"@en ;
  skos:broader agift:FINANCE-MANAGEMENT ;
  skos:definition "Developing policy to support the collection of taxes and levies from business and the community. Assessing and reviewing the operation of the tax system. Providing taxation advice to individuals and organisations."@en ;
  skos:hiddenLabel "Tax exemptions"@en ;
  skos:narrower agift:Income-assessment ;
  skos:narrower agift:Revenue-raising ;
  skos:narrower agift:Taxation-compliance ;
  skos:prefLabel "Taxation"@en ;
  skos:related agift:Financial-assistance ;
  skos:related agift:Local-laws-and-ordinances ;
  skos:related agift:Tariff-regulation ;
.
agift:Taxation-compliance
  a skos:Concept ;
  dcterms:contributor "KOdea" ;
  dcterms:created "2016-07-06T04:39:22+00:00"^^xsd:dateTime ;
  dcterms:creator "superadmin" ;
  dcterms:modified "2016-09-08T08:08:39+00:00"^^xsd:dateTime ;
  skos:altLabel "Child support payments"@en ;
  skos:altLabel "HECS payments"@en ;
  skos:altLabel "Higher Education Contribution Scheme payments"@en ;
  skos:altLabel "Tax avoidance"@en ;
  skos:broader agift:Taxation ;
  skos:definition "Monitoring the documentation submitted by individuals and organisations to ensure it is completed according to taxation laws. Investigating suspected tax avoidance and applying penalties where appropriate. Determining amounts of outstanding tax and implementing recovery procedures. Includes managing payments made by individuals through withholding schemes."@en ;
  skos:prefLabel "Taxation compliance"@en ;
  skos:related agift:Benefits ;
  skos:related agift:Child-and-youth-support ;
  skos:related agift:Child-care-services ;
  skos:related agift:Financial-assistance ;
  skos:related agift:Income-assessment ;
  skos:related agift:Income-support-schemes ;
  skos:related agift:Revenue-raising ;
  skos:related agift:Tertiary-education ;
.
agift:Telecommunications
  a skos:Concept ;
  dcterms:contributor "KOdea" ;
  dcterms:created "2016-07-06T02:54:55+00:00"^^xsd:dateTime ;
  dcterms:creator "superadmin" ;
  dcterms:modified "2016-08-05T05:55:46+00:00"^^xsd:dateTime ;
  skos:altLabel "Broadband networks"@en ;
  skos:altLabel "Telephones"@en ;
  skos:broader agift:COMMUNICATIONS ;
  skos:definition "Developing policy to support and regulate industries that transmit signals along a wire or cable to a receiver. Providing advice on the introduction of new technology and the effects of government policy on the telecommunications industry. Includes consultation with peak industry bodies."@en ;
  skos:narrower agift:Carriage-service-providers ;
  skos:narrower agift:Carrier-licensing ;
  skos:narrower agift:Communications-infrastructure ;
  skos:narrower agift:Equipment-licensing ;
  skos:narrower agift:Mobile-telephone-services ;
  skos:narrower agift:Telephone-services ;
  skos:prefLabel "Telecommunications"@en ;
.
agift:Telephone-services
  a skos:Concept ;
  dcterms:contributor "KOdea" ;
  dcterms:created "2016-07-06T04:01:00+00:00"^^xsd:dateTime ;
  dcterms:creator "superadmin" ;
  dcterms:modified "2016-09-05T07:56:06+00:00"^^xsd:dateTime ;
  skos:altLabel "Phone services"@en ;
  skos:broader agift:Telecommunications ;
  skos:definition "Monitoring the activities of suppliers of fixed-line telecommunications services. Ensuring compliance with pricing guidelines, standards of service and maintenance requirements. Managing and maintaining government-owned telecommunications equipment. Setting minimum standards for community access to telephone services."@en ;
  skos:prefLabel "Telephone services"@en ;
  skos:related agift:Mobile-telephone-services ;
.
agift:Television-broadcasting
  a skos:Concept ;
  dcterms:contributor "KOdea" ;
  dcterms:created "2016-07-06T03:56:45+00:00"^^xsd:dateTime ;
  dcterms:creator "superadmin" ;
  dcterms:modified "2016-09-05T07:26:46+00:00"^^xsd:dateTime ;
  skos:altLabel "Broadcasting licenses"@en ;
  skos:altLabel "Commercial television"@en ;
  skos:broader agift:Broadcasting ;
  skos:definition "Supporting industries that transmit content as transient images accompanied by a sound signal. Managing publicly owned television stations and issuing commercial broadcasting licenses. Developing strategies to promote Australian television programming. Providing television broadcasting services locally, nationally and internationally. Negotiating retransmission arrangements."@en ;
  skos:prefLabel "Television broadcasting"@en ;
  skos:related agift:Broadcasting-standards ;
.
agift:Temporary-entry-arrangements
  a skos:Concept ;
  dcterms:contributor "KOdea" ;
  dcterms:created "2016-07-06T04:50:57+00:00"^^xsd:dateTime ;
  dcterms:creator "superadmin" ;
  dcterms:modified "2016-08-26T07:28:34+00:00"^^xsd:dateTime ;
  skos:altLabel "Business visas"@en ;
  skos:altLabel "Cultural stay visas"@en ;
  skos:altLabel "Holiday visas"@en ;
  skos:altLabel "Short stay visas"@en ;
  skos:altLabel "Student entry visas"@en ;
  skos:altLabel "Temporary residence visas"@en ;
  skos:altLabel "Transit visas"@en ;
  skos:altLabel "Visa applications"@en ;
  skos:altLabel "Visitor visas"@en ;
  skos:altLabel "Work permits"@en ;
  skos:altLabel "Work visas"@en ;
  skos:broader agift:Travel-authorisation ;
  skos:definition "Administering programs to ensure lawful entrance of foreign nationals intending to visit Australia for a limited time. Processing applications for visas and providing advice to applicants. Includes visitors entering the country for business or cultural purposes."@en ;
  skos:prefLabel "Temporary entry arrangements"@en ;
.
agift:Termination-processes
  a skos:Concept ;
  dcterms:contributor "KOdea" ;
  dcterms:created "2016-07-06T04:21:11+00:00"^^xsd:dateTime ;
  dcterms:creator "superadmin" ;
  dcterms:modified "2016-09-08T07:24:30+00:00"^^xsd:dateTime ;
  skos:altLabel "Disciplinary proceedings"@en ;
  skos:altLabel "Personnel termination processes"@en ;
  skos:altLabel "Redundancy"@en ;
  skos:altLabel "Retirement"@en ;
  skos:altLabel "Retrenchment"@en ;
  skos:altLabel "Severance"@en ;
  skos:altLabel "Staff separations"@en ;
  skos:altLabel "Staff transfers"@en ;
  skos:broader agift:Human-resources-development ;
  skos:definition "Managing activities associated with staff separation from the organisation. Issuing warnings and initiating disciplinary proceedings for unacceptable conduct. Arranging exit interviews. Providing access to counselling and advice for retirement or redundancy. Establishing procedures for public sector separations or transfers in accordance with government policy."@en ;
  skos:prefLabel "Termination processes"@en ;
  skos:related agift:Military-employment-services ;
.
agift:Territories-administration
  a skos:Concept ;
  dcterms:contributor "KOdea" ;
  dcterms:created "2016-07-06T04:44:01+00:00"^^xsd:dateTime ;
  dcterms:creator "superadmin" ;
  dcterms:modified "2016-08-22T07:17:22+00:00"^^xsd:dateTime ;
  skos:broader agift:Public-administration ;
  skos:definition "Developing policy and administering programs for Australia's self governing and non self-governing territories. Includes providing services in non self-governing territories. Includes policy advice and administration of Commonwealth functions in the national capital."@en ;
  skos:prefLabel "Territories administration"@en ;
.
agift:Tertiary-education
  a skos:Concept ;
  dcterms:contributor "KOdea" ;
  dcterms:created "2016-07-06T03:00:59+00:00"^^xsd:dateTime ;
  dcterms:creator "superadmin" ;
  dcterms:modified "2016-09-08T07:16:02+00:00"^^xsd:dateTime ;
  skos:altLabel "Colleges of advanced education"@en ;
  skos:altLabel "Higher education"@en ;
  skos:altLabel "Institutes of technology"@en ;
  skos:altLabel "Teachers colleges"@en ;
  skos:altLabel "Tertiary institutions"@en ;
  skos:altLabel "Universities"@en ;
  skos:broader agift:EDUCATION-AND-TRAINING ;
  skos:definition "Administering programs that offer instruction beyond secondary school education, to impart knowledge and develop skills. Developing and implementing entry requirements. Managing tertiary education institutions and facilities. Implementing standards and guidelines to support lecturers. Includes the provision of scholarships and study grants."@en ;
  skos:prefLabel "Tertiary education"@en ;
  skos:related agift:Arts-education ;
  skos:related agift:Curriculum-development ;
  skos:related agift:Overseas-student-scholarship-programs ;
  skos:related agift:Taxation-compliance ;
.
agift:Tourism-industry-development
  a skos:Concept ;
  dcterms:contributor "KOdea" ;
  dcterms:created "2016-07-06T03:47:16+00:00"^^xsd:dateTime ;
  dcterms:creator "superadmin" ;
  dcterms:modified "2016-09-13T06:52:29+00:00"^^xsd:dateTime ;
  skos:broader agift:TOURISM ;
  skos:definition "Supporting the growth of businesses that provide travel products and other services to visitors. Identifying the potential of new and emerging markets. Providing grants and sponsorship. Encouraging partnerships and coordinating initiatives to optimise tourism employment and create a favourable environment for investment. Includes recognising excellence in the Australian tourism industry through the presentation of awards."@en ;
  skos:prefLabel "Tourism industry development"@en ;
  skos:related agift:Caravan-and-camping-services ;
  skos:related agift:Tourist-event-promotion ;
  skos:related agift:Trade-expositions ;
.
agift:Tourist-event-promotion
  a skos:Concept ;
  dcterms:contributor "KOdea" ;
  dcterms:created "2016-07-06T03:47:23+00:00"^^xsd:dateTime ;
  dcterms:creator "superadmin" ;
  dcterms:modified "2016-09-13T06:52:47+00:00"^^xsd:dateTime ;
  skos:altLabel "Exhibition marketing"@en ;
  skos:altLabel "Exhibition promotion"@en ;
  skos:altLabel "Trade fair promotion"@en ;
  skos:broader agift:TOURISM ;
  skos:definition "Developing special activities to draw visitors to a region. Marketing and promoting events and attractions as catalysts for tourism growth. Managing publicity to increase awareness of tourism initiatives, exhibitions and trade fairs. Includes the promotion of overseas tourist events."@en ;
  skos:narrower agift:Advertising-campaigns ;
  skos:prefLabel "Tourist event promotion"@en ;
  skos:related agift:Games-promotion ;
  skos:related agift:Overseas-promotion ;
  skos:related agift:Tourism-industry-development ;
  skos:related agift:Trade-expositions ;
.
agift:Town-planning
  a skos:Concept ;
  dcterms:contributor "KOdea" ;
  dcterms:created "2016-07-06T03:53:41+00:00"^^xsd:dateTime ;
  dcterms:creator "superadmin" ;
  dcterms:modified "2016-09-12T05:57:38+00:00"^^xsd:dateTime ;
  skos:broader agift:Civic-management ;
  skos:definition "Establishing a framework of objectives and strategies for controlled urban development. Initiating projects to meet current and future needs for infrastructure and facilities. Providing guidelines to assist applicants for building approval."@en ;
  skos:prefLabel "Town planning"@en ;
  skos:related agift:Building-approval-services ;
  skos:related agift:Housing-industry-policy ;
  skos:related agift:Infrastructure-planning ;
  skos:related agift:Integrated-services-planning ;
  skos:related agift:Land-use-zoning ;
.
agift:Trade-development-programs
  a skos:Concept ;
  dcterms:contributor "KOdea" ;
  dcterms:created "2016-07-06T03:48:45+00:00"^^xsd:dateTime ;
  dcterms:creator "superadmin" ;
  dcterms:modified "2016-09-13T07:08:24+00:00"^^xsd:dateTime ;
  skos:broader agift:TRADE ;
  skos:definition "Implementing schemes to assist local businesses to compete in regional or international markets and win overseas or interstate contracts. Includes programs to attract investment to Australia, liaison with other governments and industry partners, providing practical assistance such as identifying foreign investment partners and administering grants."@en ;
  skos:prefLabel "Trade development programs"@en ;
  skos:related agift:Arts-development ;
  skos:related agift:Development-assistance-programs ;
.
agift:Trade-expositions
  a skos:Concept ;
  dcterms:contributor "KOdea" ;
  dcterms:created "2016-07-06T03:48:56+00:00"^^xsd:dateTime ;
  dcterms:creator "superadmin" ;
  dcterms:modified "2016-09-13T06:56:56+00:00"^^xsd:dateTime ;
  skos:altLabel "Expositions"@en ;
  skos:altLabel "Trade fairs"@en ;
  skos:broader agift:TRADE ;
  skos:definition "Organising national and international events to promote trade and maximise marketing opportunities. Participating in trade fairs and developing exhibits. Includes activities to raise business profiles in a specific industry, or across a range of sectors."@en ;
  skos:prefLabel "Trade expositions"@en ;
  skos:related agift:Export-promotion ;
  skos:related agift:Overseas-promotion ;
  skos:related agift:Tourism-industry-development ;
  skos:related agift:Tourist-event-promotion ;
.
agift:Trade-measurement-compliance
  a skos:Concept ;
  dcterms:contributor "KOdea" ;
  dcterms:created "2016-07-06T03:49:08+00:00"^^xsd:dateTime ;
  dcterms:creator "superadmin" ;
  dcterms:modified "2016-09-12T06:27:03+00:00"^^xsd:dateTime ;
  skos:broader agift:TRADE ;
  skos:definition "Administering national trade measurement compliance and enforcement with trade measurement legislation."@en ;
  skos:prefLabel "Trade measurement compliance"@en ;
  skos:related agift:Weights-and-measures-standards ;
.
agift:Trade-practices-compliance
  a skos:Concept ;
  dcterms:contributor "KOdea" ;
  dcterms:created "2016-07-06T03:51:28+00:00"^^xsd:dateTime ;
  dcterms:creator "superadmin" ;
  dcterms:modified "2016-08-04T06:38:42+00:00"^^xsd:dateTime ;
  skos:altLabel "Trade practices"@en ;
  skos:broader agift:Fair-trading-compliance ;
  skos:definition "Administering programs to ensure that individuals and businesses comply with competition, fair-trading and consumer protection laws. Investigating misleading or deceptive action in commercial transactions. Imposing penalties when appropriate."@en ;
  skos:prefLabel "Trade practices compliance"@en ;
.
agift:Trademark-registration
  a skos:Concept ;
  dcterms:contributor "KOdea" ;
  dcterms:created "2016-07-06T05:13:56+00:00"^^xsd:dateTime ;
  dcterms:creator "superadmin" ;
  dcterms:modified "2016-09-13T07:06:37+00:00"^^xsd:dateTime ;
  skos:altLabel "Brand names"@en ;
  skos:altLabel "Logo registration"@en ;
  skos:broader agift:Intellectual-property-management ;
  skos:definition "Conferring legal ownership over signs or symbols used to distinguish the goods and services associated with a business entity or product. Including processing and approving trademark applications, liaising with trademark owners, granting registrations for trademarks and issuing decisions on disputes over the registration or refusal of  trademark rights."@en ;
  skos:prefLabel "Trademark registration"@en ;
  skos:related agift:Copyright-regulation ;
  skos:related agift:Design-rights-management ;
  skos:related agift:Patent-rights-management ;
  skos:related agift:Plant-breeders-rights-management ;
.
agift:Trainee-programs
  a skos:Concept ;
  dcterms:contributor "KOdea" ;
  dcterms:created "2016-07-06T04:15:23+00:00"^^xsd:dateTime ;
  dcterms:creator "superadmin" ;
  dcterms:modified "2016-09-08T07:17:59+00:00"^^xsd:dateTime ;
  skos:altLabel "Graduate programs"@en ;
  skos:altLabel "Hospitality training"@en ;
  skos:altLabel "Office traineeships"@en ;
  skos:altLabel "Service industry training"@en ;
  skos:altLabel "Tourism training"@en ;
  skos:altLabel "Traineeships"@en ;
  skos:broader agift:Vocational-education ;
  skos:definition "Administering industry-based training schemes where students learn on-the-job - such as general office traineeships, graduate or cadet programs and service industry training in tourism or hospitality. Monitoring compliance with standards and guidelines."@en ;
  skos:prefLabel "Trainee programs"@en ;
  skos:related agift:Apprenticeship-programs ;
.
agift:Transport-access-schemes
  a skos:Concept ;
  dcterms:contributor "KOdea" ;
  dcterms:created "2016-07-06T02:56:46+00:00"^^xsd:dateTime ;
  dcterms:creator "superadmin" ;
  dcterms:modified "2016-09-06T07:56:22+00:00"^^xsd:dateTime ;
  skos:altLabel "Community transport"@en ;
  skos:altLabel "Transport concessions"@en ;
  skos:altLabel "Travel concession schemes"@en ;
  skos:broader agift:COMMUNITY-SERVICES ;
  skos:definition "Managing programs to ensure public transport facilities are readily available to all sectors of the community. Formulating policy to support the provision of transport services to those in need. Developing strategies to assist specific community groups and establishing eligibility criteria for concessions. Includes liaison with areas responsible for public transport construction, to determine short-term and long-term community transport needs."@en ;
  skos:prefLabel "Transport access schemes"@en ;
  skos:related agift:Financial-assistance ;
  skos:related agift:Public-transport ;
  skos:related agift:School-transport-regulation ;
  skos:related agift:Transport-accessibility ;
  skos:related agift:Transport-network-maintenance ;
.
agift:Transport-accessibility
  a skos:Concept ;
  dcterms:contributor "KOdea" ;
  dcterms:created "2016-07-06T05:14:58+00:00"^^xsd:dateTime ;
  dcterms:creator "superadmin" ;
  dcterms:modified "2016-09-06T07:56:22+00:00"^^xsd:dateTime ;
  skos:altLabel "Disabled transport"@en ;
  skos:broader agift:Public-transport ;
  skos:definition "Developing standards and policies to make public transport accessible to people with disabilities."@en ;
  skos:prefLabel "Transport accessibility"@en ;
  skos:related agift:Transport-access-schemes ;
.
agift:Transport-infrastructure-development
  a skos:Concept ;
  dcterms:contributor "KOdea" ;
  dcterms:created "2016-07-06T03:50:31+00:00"^^xsd:dateTime ;
  dcterms:creator "superadmin" ;
  dcterms:modified "2016-09-13T07:24:15+00:00"^^xsd:dateTime ;
  skos:altLabel "Road building"@en ;
  skos:altLabel "Road construction"@en ;
  skos:broader agift:TRANSPORT ;
  skos:definition "Designing systems for the movement of people or goods. Installing facilities to support a network of air, rail and road transport services. Assessing existing infrastructure and planning for future requirements. Includes developing transport corridors, links to airport and rail terminals, and collaborating across jurisdictions on infrastructure development."@en ;
  skos:prefLabel "Transport infrastructure development"@en ;
  skos:related agift:Airport-services ;
  skos:related agift:Engineering-services ;
  skos:related agift:Port-regulation ;
  skos:related agift:Railway-maintenance ;
  skos:related agift:Regional-development ;
  skos:related agift:Road-surface-maintenance ;
  skos:related agift:Transport-network-maintenance ;
.
agift:Transport-network-maintenance
  a skos:Concept ;
  dcterms:contributor "KOdea" ;
  dcterms:created "2016-07-06T02:52:48+00:00"^^xsd:dateTime ;
  dcterms:creator "superadmin" ;
  dcterms:modified "2016-09-13T07:11:52+00:00"^^xsd:dateTime ;
  skos:altLabel "Bus services"@en ;
  skos:altLabel "Cycle path maintenance"@en ;
  skos:altLabel "Footpath maintenance"@en ;
  skos:altLabel "Train services"@en ;
  skos:altLabel "Tram services"@en ;
  skos:broader agift:CIVIC-INFRASTRUCTURE ;
  skos:definition "Managing public transport networks at a local level. Developing interconnecting services for road, rail and air transport. Maintaining public car parks, bus shelters, train stations, footpaths and cycle ways."@en ;
  skos:prefLabel "Transport network maintenance"@en ;
  skos:related agift:Integrated-services-planning ;
  skos:related agift:Passenger-services ;
  skos:related agift:Public-transport ;
  skos:related agift:Railway-maintenance ;
  skos:related agift:Road-surface-maintenance ;
  skos:related agift:School-transport-regulation ;
  skos:related agift:Transport-access-schemes ;
  skos:related agift:Transport-infrastructure-development ;
.
agift:Travel-authorisation
  a skos:Concept ;
  dcterms:contributor "KOdea" ;
  dcterms:created "2016-07-06T03:34:20+00:00"^^xsd:dateTime ;
  dcterms:creator "superadmin" ;
  dcterms:modified "2016-09-28T07:01:59+00:00"^^xsd:dateTime ;
  skos:altLabel "Arrivals"@en ;
  skos:altLabel "Passenger entry control"@en ;
  skos:altLabel "Passport control"@en ;
  skos:broader agift:IMMIGRATION ;
  skos:definition "Developing policy to regulate the entry and presence of non-citizens or foreign nationals in Australia. Establishing eligibility criteria, visa classes and entry conditions. Providing on-arrival immigration clearance through the passenger entry control system."@en ;
  skos:narrower agift:Permanent-entry-arrangements ;
  skos:narrower agift:Temporary-entry-arrangements ;
  skos:prefLabel "Travel authorisation"@en ;
  skos:related agift:Border-protection ;
  skos:related agift:Citizenship ;
  skos:related agift:Passport-services ;
.
agift:Travel-missions
  a skos:Concept ;
  dcterms:contributor "superadmin" ;
  dcterms:created "2016-07-06T03:47:42+00:00"^^xsd:dateTime ;
  dcterms:creator "superadmin" ;
  dcterms:modified "2016-07-07T00:39:36+00:00"^^xsd:dateTime ;
  skos:broader agift:TOURISM ;
  skos:definition "Marketing activities carried out overseas for the promotion of Australia or specific regions as a travel and tourism destination. Organising meetings between members of the Australian tourism industry, travel agents and overseas tour operators. Includes familiarisation tours in Australia for international travel agents, tour operators and members of the travel press."@en ;
  skos:prefLabel "Travel missions"@en ;
.
agift:Treaty-administration
  a skos:Concept ;
  dcterms:contributor "KOdea" ;
  dcterms:created "2016-07-06T04:53:27+00:00"^^xsd:dateTime ;
  dcterms:creator "superadmin" ;
  dcterms:modified "2016-09-13T07:07:10+00:00"^^xsd:dateTime ;
  skos:altLabel "Treaty negotiations"@en ;
  skos:broader agift:International-treaties ;
  skos:definition "Implementing the terms and conditions of formal agreements made between Australia and one or more other countries. Monitoring compliance with provisions and obligations .Assessing  the ongoing benefits of treaty participation."@en ;
  skos:prefLabel "Treaty administration"@en ;
  skos:related agift:Disarmament-and-arms-control ;
  skos:related agift:Human-rights-obligations ;
  skos:related agift:International-trade-agreements ;
  skos:related agift:Military-law ;
.
agift:Vehicle-registration
  a skos:Concept ;
  dcterms:contributor "KOdea" ;
  dcterms:created "2016-07-06T05:16:34+00:00"^^xsd:dateTime ;
  dcterms:creator "superadmin" ;
  dcterms:modified "2016-09-13T07:21:37+00:00"^^xsd:dateTime ;
  skos:altLabel "Car registration"@en ;
  skos:altLabel "Licence plates"@en ;
  skos:altLabel "Motor vehicle national certification"@en ;
  skos:altLabel "Registration"@en ;
  skos:broader agift:Road-transport ;
  skos:definition "Administering arrangements to uniquely identify motor vehicles. Issuing certificates of ownership and maintaining records to allocate responsibility for individual motor vehicles. Includes processing applications, renewals, transfer, suspension and cancellation of vehicle registrations."@en ;
  skos:prefLabel "Vehicle registration"@en ;
  skos:related agift:Road-traffic-regulation ;
  skos:related agift:Vehicle-standards ;
.
agift:Vehicle-standards
  a skos:Concept ;
  dcterms:contributor "KOdea" ;
  dcterms:created "2016-07-06T05:16:41+00:00"^^xsd:dateTime ;
  dcterms:creator "superadmin" ;
  dcterms:modified "2016-09-13T07:22:04+00:00"^^xsd:dateTime ;
  skos:altLabel "Roadworthy certificates"@en ;
  skos:altLabel "Vehicle regulation"@en ;
  skos:broader agift:Road-transport ;
  skos:definition "Regulating the design, construction, maintenance and operation of any machine intended for use on public roads. Setting standards for vehicle safety, configuration, noise and emissions. Monitoring conformance through inspections and testing. Issuing or declining certificates of roadworthiness to support the process of vehicle registration."@en ;
  skos:prefLabel "Vehicle standards"@en ;
  skos:related agift:Driving-licences-administration ;
  skos:related agift:Road-traffic-regulation ;
  skos:related agift:Road-transport-safety ;
  skos:related agift:Vehicle-registration ;
.
agift:Veterans-entitlements
  a skos:Concept ;
  dcterms:contributor "KOdea" ;
  dcterms:created "2016-07-06T04:02:51+00:00"^^xsd:dateTime ;
  dcterms:creator "superadmin" ;
  dcterms:modified "2016-09-09T06:28:48+00:00"^^xsd:dateTime ;
  skos:altLabel "Veteran"@en ;
  skos:altLabel "War pensions"@en ;
  skos:broader agift:Community-support ;
  skos:definition "Managing social support services to returned defence service personnel and their families. Providing advice on rights to financial or other assistance, such as residential care or medical services. Includes funding and support for community-based or volunteer programs providing veterans' services."@en ;
  skos:prefLabel "Veterans' entitlements"@en ;
  skos:related agift:Aged-care-services ;
  skos:related agift:Benefits ;
  skos:related agift:Defence-community-programs ;
  skos:related agift:Financial-assistance ;
  skos:related agift:Income-support-schemes ;
  skos:related agift:Veterans-health-services ;
.
agift:Veterans-health-services
  a skos:Concept ;
  dcterms:contributor "KOdea" ;
  dcterms:created "2016-07-06T03:07:56+00:00"^^xsd:dateTime ;
  dcterms:creator "superadmin" ;
  dcterms:modified "2016-09-09T06:28:48+00:00"^^xsd:dateTime ;
  skos:altLabel "Returned services health programs"@en ;
  skos:broader agift:HEALTH-CARE ;
  skos:definition "Developing policy to support the physical and mental wellbeing of returned defence service personnel and their families. Managing health care programs that address the specific needs of veterans. Establishing eligibility criteria for access to health services."@en ;
  skos:prefLabel "Veterans' health services"@en ;
  skos:related agift:Special-needs-services ;
  skos:related agift:Veterans-entitlements ;
.
agift:Viticultural-industry
  a skos:Concept ;
  dcterms:contributor "KOdea" ;
  dcterms:created "2016-07-06T05:03:06+00:00"^^xsd:dateTime ;
  dcterms:creator "superadmin" ;
  dcterms:modified "2016-09-12T06:17:46+00:00"^^xsd:dateTime ;
  skos:altLabel "Grape growing industry"@en ;
  skos:altLabel "Viticulture"@en ;
  skos:altLabel "Wine industry support"@en ;
  skos:altLabel "Wine making industry"@en ;
  skos:broader agift:Marine-and-rural-support ;
  skos:definition "Administering programs to support commercial grape growing and wine production. Assisting industry growth and development. Encouraging businesses to adopt innovative practices, processes and products. Providing advice on cultivation methods and business management to improve competitiveness."@en ;
  skos:prefLabel "Viticultural industry"@en ;
  skos:related agift:Agricultural-industry ;
  skos:related agift:Agricultural-sciences ;
  skos:related agift:Horticultural-industry ;
.
agift:Vocational-education
  a skos:Concept ;
  dcterms:contributor "KOdea" ;
  dcterms:created "2016-07-06T03:01:11+00:00"^^xsd:dateTime ;
  dcterms:creator "superadmin" ;
  dcterms:modified "2016-09-08T07:31:56+00:00"^^xsd:dateTime ;
  skos:altLabel "Business schools"@en ;
  skos:altLabel "Competency standards"@en ;
  skos:altLabel "Professional education"@en ;
  skos:altLabel "Technical and further education"@en ;
  skos:broader agift:EDUCATION-AND-TRAINING ;
  skos:definition "Developing and promoting programs that offer training and further education for work-related disciplines. Setting standards and guidelines to support the operation of vocational education programs. Initiating joint ventures with industry, schools and tertiary institutions to make use of facilities. Includes the provision of scholarships and study grants."@en ;
  skos:narrower agift:Apprenticeship-programs ;
  skos:narrower agift:Hospital-teaching-programs ;
  skos:narrower agift:Industry-collaboration ;
  skos:narrower agift:Trainee-programs ;
  skos:narrower agift:Workplace-training ;
  skos:prefLabel "Vocational education"@en ;
  skos:related agift:Community-based-corrections ;
  skos:related agift:EMPLOYMENT ;
  skos:related agift:Employment-services-marketing ;
  skos:related agift:Job-placement-programs ;
  skos:related agift:Military-education-and-training ;
  skos:related agift:Recruitment-programs ;
  skos:related agift:Small-business-advocacy ;
.
agift:Volunteer-support-programs
  a skos:Concept ;
  dcterms:contributor "KOdea" ;
  dcterms:created "2016-07-06T05:09:23+00:00"^^xsd:dateTime ;
  dcterms:creator "superadmin" ;
  dcterms:modified "2016-09-13T06:39:55+00:00"^^xsd:dateTime ;
  skos:broader agift:Community-recreational-programs ;
  skos:definition "Providing financial assistance and services for groups and individuals who offer their time and labour to the community free of charge. Raising awareness of volunteer programs groups though sponsorship, advertising and facilitating links between organisations. Includes organising large volunteer groups for major sporting events."@en ;
  skos:prefLabel "Volunteer support programs"@en ;
  skos:related agift:Games-administration ;
.
agift:Warfare
  a skos:Concept ;
  dcterms:contributor "KOdea" ;
  dcterms:created "2016-07-06T04:12:28+00:00"^^xsd:dateTime ;
  dcterms:creator "superadmin" ;
  dcterms:modified "2016-09-12T06:07:35+00:00"^^xsd:dateTime ;
  skos:altLabel "Armed combat"@en ;
  skos:altLabel "Battlefront operations"@en ;
  skos:altLabel "Conflicts"@en ;
  skos:altLabel "Military action"@en ;
  skos:altLabel "Military engagement"@en ;
  skos:altLabel "War"@en ;
  skos:broader agift:Military-operations ;
  skos:definition "Entering into armed combat with opposing defence forces. Conducting military, naval or air attacks against designated targets. Performing offensive or defensive operations on the battlefield to win campaigns."@en ;
  skos:prefLabel "Warfare"@en ;
  skos:related agift:Australian-theatre-of-war ;
  skos:related agift:Chemical-and-pesticide-regulation ;
  skos:related agift:Peacekeeping-forces ;
  skos:related agift:Special-operations ;
.
agift:Waste-management
  a skos:Concept ;
  dcterms:contributor "KOdea" ;
  dcterms:created "2016-07-06T02:52:57+00:00"^^xsd:dateTime ;
  dcterms:creator "superadmin" ;
  dcterms:modified "2016-09-05T07:20:56+00:00"^^xsd:dateTime ;
  skos:altLabel "Garbage collection"@en ;
  skos:altLabel "Graffiti removal"@en ;
  skos:altLabel "Hazardous materials management"@en ;
  skos:altLabel "Hazardous waste management"@en ;
  skos:altLabel "Landfill sites"@en ;
  skos:altLabel "Needle disposal"@en ;
  skos:altLabel "Public toilets"@en ;
  skos:altLabel "Recycling"@en ;
  skos:altLabel "Refuse management"@en ;
  skos:altLabel "Rubbish collection"@en ;
  skos:altLabel "Sewerage"@en ;
  skos:altLabel "Waste disposal"@en ;
  skos:altLabel "Wheelie bins"@en ;
  skos:broader agift:CIVIC-INFRASTRUCTURE ;
  skos:definition "Providing services to collect and dispose of garbage. Operating waste management centres, landfill sites, recycling depots and sewerage facilities. Developing and promoting strategies for consumer waste minimisation. Providing services for graffiti removal and street cleaning."@en ;
  skos:prefLabel "Waste management"@en ;
  skos:related agift:Pollutant-prevention-programs ;
  skos:related agift:Pollution-emission-control ;
.
agift:Water-conservation-plans
  a skos:Concept ;
  dcterms:contributor "KOdea" ;
  dcterms:created "2016-07-06T05:01:01+00:00"^^xsd:dateTime ;
  dcterms:creator "superadmin" ;
  dcterms:modified "2016-09-12T06:02:30+00:00"^^xsd:dateTime ;
  skos:broader agift:Water-resources ;
  skos:definition "Developing strategies to prevent the loss or waste of water resources. Monitoring dam and reservoir levels, rainfall and projected water usage figures. Recommending water restrictions and other measures to ensure water supplies continue to meet user needs over time. Conducting consultation exercises and education programs to raise community awareness of water conservation issues."@en ;
  skos:prefLabel "Water conservation plans"@en ;
  skos:related agift:ENVIRONMENT ;
.
agift:Water-quality-monitoring
  a skos:Concept ;
  dcterms:contributor "KOdea" ;
  dcterms:created "2016-07-06T05:01:08+00:00"^^xsd:dateTime ;
  dcterms:creator "superadmin" ;
  dcterms:modified "2016-09-12T06:02:58+00:00"^^xsd:dateTime ;
  skos:broader agift:Water-resources ;
  skos:definition "Administering programs to assess the characteristics of water resources, to determine their fitness for purpose. Analysing water samples for the presence of contaminants or minerals to ensure it is potable. Includes testing for salinity, bacteria, pesticides and other pollutants."@en ;
  skos:prefLabel "Water quality monitoring"@en ;
  skos:related agift:Pollution-emission-control ;
.
agift:Water-resources
  a skos:Concept ;
  dcterms:contributor "KOdea" ;
  dcterms:created "2016-07-06T03:41:20+00:00"^^xsd:dateTime ;
  dcterms:creator "superadmin" ;
  dcterms:modified "2016-09-12T06:01:59+00:00"^^xsd:dateTime ;
  skos:altLabel "Water supplies"@en ;
  skos:altLabel "Water supply"@en ;
  skos:broader agift:NATURAL-RESOURCES ;
  skos:definition "Developing policy and administering legislation relating to waterways and water resources. Supporting industry partnerships and cooperative approaches to the management and use of water. Regulating the exploitation of water resources to ensure sustainable quality and availability for household, industrial and agricultural use."@en ;
  skos:narrower agift:Water-conservation-plans ;
  skos:narrower agift:Water-quality-monitoring ;
  skos:narrower agift:Water-usage-management ;
  skos:narrower agift:Waterway-management ;
  skos:prefLabel "Water resources"@en ;
  skos:related agift:Energy-supply ;
  skos:related agift:Hydrology ;
  skos:related agift:Oceans-governance ;
.
agift:Water-usage-management
  a skos:Concept ;
  dcterms:contributor "KOdea" ;
  dcterms:created "2016-07-06T05:01:15+00:00"^^xsd:dateTime ;
  dcterms:creator "superadmin" ;
  dcterms:modified "2016-09-12T05:54:23+00:00"^^xsd:dateTime ;
  skos:altLabel "Water services"@en ;
  skos:altLabel "Water supply"@en ;
  skos:broader agift:Water-resources ;
  skos:definition "Monitoring water consumption and implementing schemes to regulate water usage. Implementing water conservation recommendations, such as water restrictions. Administering water rights and evaluating compliance with the terms of waterway agreements. Assessing agricultural and industrial water usage practices. Issuing permits for the use of bore water."@en ;
  skos:prefLabel "Water usage management"@en ;
  skos:related agift:Renewable-energy-development ;
.
agift:Waterway-management
  a skos:Concept ;
  dcterms:contributor "KOdea" ;
  dcterms:created "2016-07-06T05:01:21+00:00"^^xsd:dateTime ;
  dcterms:creator "superadmin" ;
  dcterms:modified "2016-09-12T06:05:01+00:00"^^xsd:dateTime ;
  skos:altLabel "Floodplain management"@en ;
  skos:broader agift:Water-resources ;
  skos:definition "Monitoring river flows and catchment areas. Implementing strategies for salinity management and river care programs. Evaluating the effects of land use and climate on waterways. Developing agreements for the equitable use of water resources from river systems that may cross jurisdictional boundaries."@en ;
  skos:prefLabel "Waterway management"@en ;
  skos:related agift:Conservation-programs ;
  skos:related agift:ENVIRONMENT ;
  skos:related agift:Harbour-management ;
  skos:related agift:Marina-management ;
  skos:related agift:Oceans-governance ;
  skos:related agift:PRIMARY-INDUSTRIES ;
  skos:related agift:Pollutant-prevention-programs ;
  skos:related agift:Port-regulation ;
  skos:related agift:Soil-preservation-programs ;
.
agift:Website-development
  a skos:Concept ;
  dcterms:contributor "KOdea" ;
  dcterms:created "2016-07-06T03:59:35+00:00"^^xsd:dateTime ;
  dcterms:creator "superadmin" ;
  dcterms:modified "2016-09-05T07:46:47+00:00"^^xsd:dateTime ;
  skos:broader agift:Publishing ;
  skos:definition "Designing and maintaining online information and services. Managing the supporting software to make electronic publications and transactions available via internal or external networks. Planning the layout of web pages and marking up content."@en ;
  skos:prefLabel "Website development"@en ;
  skos:related agift:Electronic-publishing ;
  skos:related agift:Information-dissemination ;
.
agift:Weights-and-measures-standards
  a skos:Concept ;
  dcterms:contributor "KOdea" ;
  dcterms:created "2016-07-06T05:03:39+00:00"^^xsd:dateTime ;
  dcterms:creator "superadmin" ;
  dcterms:modified "2016-09-12T06:27:03+00:00"^^xsd:dateTime ;
  skos:altLabel "Industrial measurement"@en ;
  skos:altLabel "Measurement standards"@en ;
  skos:broader agift:Applied-sciences ;
  skos:definition "Conducting research into methods of ascertaining dimensions, extent, size or amounts. Setting and maintaining standards consistent with international conventions for units, values and industrial measurements. Includes testing and calibration of measuring equipment, training and consultancy in measurement science."@en ;
  skos:prefLabel "Weights and measures standards"@en ;
  skos:related agift:Trade-measurement-compliance ;
.
agift:Whistleblowing
  a skos:Concept ;
  dcterms:contributor "KOdea" ;
  dcterms:created "2016-07-06T04:44:08+00:00"^^xsd:dateTime ;
  dcterms:creator "superadmin" ;
  dcterms:modified "2016-09-09T06:01:47+00:00"^^xsd:dateTime ;
  skos:altLabel "Protected disclosure"@en ;
  skos:altLabel "Public interest disclosure"@en ;
  skos:broader agift:Public-administration ;
  skos:definition "Disclosure  of illegal, immoral or illegitimate practices under the control of their employer by government employees (former or current ) to persons or organisations that may be able to effect action such as  watchdog  bodies,  the media or the public."@en ;
  skos:prefLabel "Whistleblowing"@en ;
  skos:related agift:Corruption-prevention ;
  skos:related agift:Government-auditing ;
  skos:related agift:Integrity-compliance ;
.
agift:Wilderness-area-management
  a skos:Concept ;
  dcterms:contributor "KOdea" ;
  dcterms:created "2016-07-06T04:34:28+00:00"^^xsd:dateTime ;
  dcterms:creator "superadmin" ;
  dcterms:modified "2016-09-08T07:48:16+00:00"^^xsd:dateTime ;
  skos:altLabel "Bushland management"@en ;
  skos:broader agift:Natural-heritage-protection ;
  skos:definition "Administering designated wilderness areas, where the ecology is undisturbed. Monitoring access restrictions. Issuing permits for commercial or recreational activities. Providing advice on developments that might encroach on wilderness areas."@en ;
  skos:prefLabel "Wilderness area management"@en ;
  skos:related agift:Endangered-species-protection ;
  skos:related agift:Feral-pest-control ;
  skos:related agift:Garden-management ;
  skos:related agift:Indigenous-heritage-conservation ;
  skos:related agift:National-park-management ;
  skos:related agift:Nature-reserve-management ;
  skos:related agift:Wildlife-sanctuary-management ;
.
agift:Wildlife-sanctuary-management
  a skos:Concept ;
  dcterms:contributor "KOdea" ;
  dcterms:created "2016-07-06T04:34:37+00:00"^^xsd:dateTime ;
  dcterms:creator "superadmin" ;
  dcterms:modified "2016-09-08T07:48:54+00:00"^^xsd:dateTime ;
  skos:altLabel "Wildlife park management"@en ;
  skos:altLabel "Zoo management"@en ;
  skos:broader agift:Natural-heritage-protection ;
  skos:definition "Administering sheltered facilities where animals live in conditions that resemble their natural habitat. Building special amenities, or allocating space from wilderness areas or nature reserves. Supporting protection programs for endangered species and services to rehabilitate injured wildlife. Monitoring the activities of privately run sanctuaries and zoos."@en ;
  skos:prefLabel "Wildlife sanctuary management"@en ;
  skos:related agift:Endangered-species-protection ;
  skos:related agift:National-park-management ;
  skos:related agift:Nature-reserve-management ;
  skos:related agift:Wilderness-area-management ;
.
agift:Workers-compensation-schemes
  a skos:Concept ;
  dcterms:contributor "KOdea" ;
  dcterms:created "2016-07-06T04:21:17+00:00"^^xsd:dateTime ;
  dcterms:creator "superadmin" ;
  dcterms:modified "2016-09-09T06:11:32+00:00"^^xsd:dateTime ;
  skos:altLabel "Asbestos related compensation claims"@en ;
  skos:altLabel "Compensation schemes"@en ;
  skos:altLabel "Employment insurance schemes"@en ;
  skos:altLabel "Work cover"@en ;
  skos:broader agift:Human-resources-development ;
  skos:definition "Administering workplace insurance programs. Granting financial compensation for death, injury or disease incurred in the course of employment activities. Providing access to rehabilitation services. Monitoring compliance with government policy on workers compensation schemes. Includes liaison across jurisdictions to promote a consistent benefits structure."@en ;
  skos:prefLabel "Workers compensation schemes"@en ;
  skos:related agift:Health-insurance-schemes ;
  skos:related agift:Insurance-regulation ;
  skos:related agift:Occupational-health-and-safety ;
.
agift:Workplace-agreement-processes
  a skos:Concept ;
  dcterms:contributor "KOdea" ;
  dcterms:created "2016-07-06T03:02:07+00:00"^^xsd:dateTime ;
  dcterms:creator "superadmin" ;
  dcterms:modified "2016-09-08T07:33:59+00:00"^^xsd:dateTime ;
  skos:altLabel "Arbitration"@en ;
  skos:altLabel "Australian Workplace Agreements"@en ;
  skos:altLabel "Certified agreements"@en ;
  skos:altLabel "Enterprise codes of practice"@en ;
  skos:altLabel "Enterprise employment conditions"@en ;
  skos:altLabel "Working conditions"@en ;
  skos:broader agift:EMPLOYMENT ;
  skos:definition "Regulating the conduct of employer and employees across a particular organisation, or between an employer and an individual employee. Certifying agreements with regard to rates of pay and working conditions. Developing policy to support the establishment and use of workplace agreements. Includes enterprise codes of practice."@en ;
  skos:narrower agift:Agreement-bargaining-processes ;
  skos:narrower agift:Agreement-dispute-mediation ;
  skos:narrower agift:Certified-employment-conditions ;
  skos:narrower agift:Employment-advocacy-services ;
  skos:prefLabel "Workplace agreement processes"@en ;
  skos:related agift:Industrial-awards-and-conditions ;
  skos:related agift:Military-education-and-training ;
  skos:related agift:Occupational-health-and-safety ;
.
agift:Workplace-discrimination-monitoring
  a skos:Concept ;
  dcterms:contributor "KOdea" ;
  dcterms:created "2016-07-06T04:21:23+00:00"^^xsd:dateTime ;
  dcterms:creator "superadmin" ;
  dcterms:modified "2016-09-08T07:26:00+00:00"^^xsd:dateTime ;
  skos:altLabel "Defence families"@en ;
  skos:broader agift:Human-resources-development ;
  skos:prefLabel "Workplace discrimination monitoring"@en ;
  skos:related agift:Defence-force-careers ;
  skos:related agift:Social-justice-and-equity ;
  skos:related agift:Workplace-equity-and-justice-programs ;
.
agift:Workplace-equity-and-justice-programs
  a skos:Concept ;
  dcterms:contributor "KOdea" ;
  dcterms:created "2016-07-06T04:21:31+00:00"^^xsd:dateTime ;
  dcterms:creator "superadmin" ;
  dcterms:modified "2016-09-09T07:19:30+00:00"^^xsd:dateTime ;
  skos:altLabel "Dispute resolution services"@en ;
  skos:altLabel "Diversity programs"@en ;
  skos:altLabel "Equal employment opportunity"@en ;
  skos:altLabel "Harassment"@en ;
  skos:altLabel "Workplace dispute mediation"@en ;
  skos:altLabel "Workplace diversity"@en ;
  skos:altLabel "Workplace harassment"@en ;
  skos:altLabel "Workplace justice services"@en ;
  skos:broader agift:Human-resources-development ;
  skos:definition "Administering programs that support workplace diversity in accordance with human resources policy. Ensuring all people have equal access to employment opportunities and conditions, regardless of gender, race, colour, ethnicity, age, marital or parental status, sexual preference, disability or religious belief. Mediating disputes and managing resolution processes. Discouraging offensive behaviour, intimidation or harassment through training and information programs"@en ;
  skos:prefLabel "Workplace equity and justice programs"@en ;
  skos:related agift:Agreement-dispute-mediation ;
  skos:related agift:Dispute-mediation-programs ;
  skos:related agift:Military-employment-services ;
  skos:related agift:Social-justice-and-equity ;
  skos:related agift:Workplace-discrimination-monitoring ;
.
agift:Workplace-training
  a skos:Concept ;
  dcterms:contributor "KOdea" ;
  dcterms:created "2016-07-06T04:15:30+00:00"^^xsd:dateTime ;
  dcterms:creator "superadmin" ;
  dcterms:modified "2016-09-08T07:20:29+00:00"^^xsd:dateTime ;
  skos:altLabel "Career development training"@en ;
  skos:altLabel "Personal development training"@en ;
  skos:altLabel "Professional development training"@en ;
  skos:altLabel "Trade union training"@en ;
  skos:broader agift:Vocational-education ;
  skos:definition "Administering programs of training that provide learning and development opportunities for personnel already employed in an organisation. Includes courses to improve computer literacy, learn job-specific skills, personal or career development programs and training to maintain or upgrade professional qualifications."@en ;
  skos:prefLabel "Workplace training"@en ;
  skos:related agift:Human-resources-development ;
  skos:related agift:Military-education-and-training ;
.
agift:World-heritage-listings
  a skos:Concept ;
  dcterms:contributor "KOdea" ;
  dcterms:created "2016-07-06T03:03:28+00:00"^^xsd:dateTime ;
  dcterms:creator "superadmin" ;
  dcterms:modified "2016-08-22T05:30:56+00:00"^^xsd:dateTime ;
  skos:altLabel "Heritage listings"@en ;
  skos:broader agift:ENVIRONMENT ;
  skos:definition "Developing policy to support the maintenance of items or areas registered by UNESCO in accordance with the World Heritage Convention for protection and conservation. Assessing natural, Indigenous and historic sites in Australia for possible inclusion on international heritage lists. Includes liaison with international bodies and community groups to manage the listing process."@en ;
  skos:prefLabel "World heritage listings"@en ;
.